@prefix agrovoc: <http://aims.fao.org/aos/agrovoc/> .
@prefix ccat: <http://data.ga-group.nl/comcat/> .
@prefix dbr: <http://dbpedia.org/resource/> .
@prefix dct: <http://purl.org/dc/terms/> .
@prefix eurovoc: <http://eurovoc.europa.eu/> .
@prefix msa: <http://academic.microsoft.com/v2/detail/> .
@prefix owl: <http://www.w3.org/2002/07/owl#> .
@prefix rdf: <http://www.w3.org/1999/02/22-rdf-syntax-ns#> .
@prefix rdfs: <http://www.w3.org/2000/01/rdf-schema#> .
@prefix skos: <http://www.w3.org/2004/02/skos/core#> .
@prefix sm: <http://www.omg.org/techprocess/ab/SpecificationMetadata/> .
@prefix stw: <http://zbw.eu/stw/descriptor/> .
@prefix vann: <http://purl.org/vocab/vann/> .
@prefix wd: <http://www.wikidata.org/entity/> .
@prefix xsd: <http://www.w3.org/2001/XMLSchema#> .

ccat:
	a	skos:ConceptScheme ;
	dct:abstract	"""A taxonomy concerned with the collection of traded commodities for use by the global financial community. Taxons are assigned a numeric code across up to four tiers of hierarchy: the class of commodity, the category within the class, and the kind of commodity within the category, possibly extended with the sub-kind.

The list of traded commodities, be it standard listed products or products traded OTC, is constantly monitored for the purpose of regular revisions to the standard."""@en ;
	dct:creator	<https://orcid.org/0000-0002-7352-2825> ;
	dct:format	"text/turtle"^^xsd:string ;
	dct:issued	"2022-06-28T02:25:19Z"^^xsd:dateTime ;
	dct:license	<https://creativecommons.org/licenses/by/4.0/> ;
	dct:modified	"2022-06-18T12:43:00Z"^^xsd:dateTime ;
	dct:title	"comcat" ;
	skos:definition	"A commodity is an economic good or service that has full or substantial fungibility, i.e the market treats instances of the good as equivalent or nearly so with no regard to who produced them."@en ;
	skos:note	"This taxonomy (broadly) follows industry's vocabularies, such as FAO's agrovoc, various tariff systems, or the STW thesaurus. It is made by market participants who needed  a single fine-grained classification system instead of choosing between several domain-specific ones or a single coarse one."@en ;
	skos:prefLabel	"Taxonomy for traded commodities"@en ;
	sm:copyright	"Copyright (c) 2022 GA Financial Solutions GmbH" ;
	sm:fileAbbreviation	"comcat" ;
	sm:filename	"comcat.skos.ttl" ;
	vann:preferredNamespacePrefix	"ccat"^^xsd:string ;
	vann:preferredNamespaceUri	"http://data.ga-group.nl/comcat/" .

ccat:10
	a	skos:Concept ;
	skos:definition	"Hard commodities, or hards, are commodities that, generally, are mined, rather than grown."@en ;
	skos:inScheme	ccat: ;
	skos:notation	"10" ;
	skos:prefLabel	"Hards"@en ;
	skos:topConceptOf	ccat: .

ccat:1010
	a	skos:Concept ;
	skos:broader	ccat:10 ;
	skos:closeMatch	stw:18996-5 , wd:Q1239166 ;
	skos:definition	"Commodities that deal specifically with the trade and supply of energy."@en ;
	skos:inScheme	ccat: ;
	skos:notation	"1010" ;
	skos:prefLabel	"Energy"@en .

ccat:101010
	a	skos:Concept ;
	skos:broader	ccat:1010 ;
	skos:definition	"Products associated with the extraction and processing of crude oil."@en ;
	skos:inScheme	ccat: ;
	skos:notation	"101010" ;
	skos:prefLabel	"Crude Products"@en .

ccat:10101010
	a	skos:Concept ;
	skos:broader	ccat:101010 ;
	skos:definition	"Raw, unprocessed blend of various petroleum products. Highly volatile components are traded as Natural Gas (101020)."@en ;
	skos:exactMatch	agrovoc:c_5747 , eurovoc:2366 , stw:14197-6 , wd:Q22656 ;
	skos:inScheme	ccat: ;
	skos:notation	"10101010" ;
	skos:prefLabel	"Crude Oil"@en .

ccat:10101015
	a	skos:Concept ;
	skos:broader	ccat:101010 ;
	skos:definition	"Product that tracks the variance or volatility of crude oil."@en ;
	skos:inScheme	ccat: ;
	skos:notation	"10101015" ;
	skos:prefLabel	"Crude Variance"@en .

ccat:10101050
	a	skos:Concept ;
	skos:broader	ccat:101010 ;
	skos:definition	"Booked pipeline capacity for the purpose of oil transfers."@en ;
	skos:inScheme	ccat: ;
	skos:notation	"10101050" ;
	skos:prefLabel	"Crude Transfer"@en .

ccat:10101070
	a	skos:Concept ;
	skos:broader	ccat:101010 ;
	skos:definition	"Booked storage capacity for the purpose of deferring transfer or refining."@en ;
	skos:inScheme	ccat: ;
	skos:notation	"10101070" ;
	skos:prefLabel	"Crude Storage"@en .

ccat:10101080
	a	skos:Concept ;
	skos:broader	ccat:101010 ;
	skos:definition	"Premium of one oil over another due to chemical composition, freight or storage costs."@en ;
	skos:inScheme	ccat: ;
	skos:notation	"10101080" ;
	skos:prefLabel	"Crude Premium"@en .

ccat:10101085
	a	skos:Concept ;
	skos:broader	ccat:101010 ;
	skos:definition	"Premium of a component extracted from a crude oil over the crude oil itself. Also includes combinations of components, e.g. the 3-2-1 crack spread."@en ;
	skos:exactMatch	wd:Q5180334 ;
	skos:inScheme	ccat: ;
	skos:notation	"10101085" ;
	skos:prefLabel	"Crack Spread"@en .

ccat:101020
	a	skos:Concept ;
	skos:broader	ccat:1010 ;
	skos:definition	"Naturally occurring hydrocarbon gas mixture of higher alkanes (methane, ethane, propane, others), sometimes a small percentage of carbon dioxide, nitrogen, hydrogen sulfide, or helium."@en ;
	skos:exactMatch	agrovoc:c_5087 , eurovoc:1141 , stw:14196-1 , wd:Q40858 ;
	skos:inScheme	ccat: ;
	skos:notation	"101020" ;
	skos:prefLabel	"Natural Gas"@en .

ccat:10102010
	a	skos:Concept ;
	skos:broader	ccat:101020 ;
	skos:definition	"Processed natural gas, or gas from petro-chemical processes, that is close to pure methane or pure ethane."@en ;
	skos:inScheme	ccat: ;
	skos:notation	"10102010" ;
	skos:prefLabel	"Purified Natural Gas"@en .

ccat:10102015
	a	skos:Concept ;
	skos:broader	ccat:101020 ;
	skos:definition	"Product that tracks the variance or volatility of natural gas."@en ;
	skos:inScheme	ccat: ;
	skos:notation	"10102015" ;
	skos:prefLabel	"Natural Gas Variance"@en .

ccat:10102020
	a	skos:Concept ;
	skos:altLabel	"LNG"@en ;
	skos:broader	ccat:101020 ;
	skos:definition	"Natural gas or purified natural gas that has been cooled down to liquid form for ease and safety of non-pressurized storage or transfer."@en ;
	skos:exactMatch	stw:18236-2 , wd:Q358333 ;
	skos:inScheme	ccat: ;
	skos:notation	"10102020" ;
	skos:prefLabel	"Liquefied Natural Gas"@en .

ccat:10102030
	a	skos:Concept ;
	skos:altLabel	"LPG"@en ;
	skos:broader	ccat:101020 ;
	skos:definition	"Flammable hydrocarbon gases used as fuel in heating appliances, cooking equipment, and vehicles. Either propane or butane or a mixture of roughly equal amounts thereof. Pentane, propylene, butylenes and various other hydrocarbons are usually also present in small concentrations. Standardised in EN 589."@en ;
	skos:exactMatch	wd:Q351609 ;
	skos:inScheme	ccat: ;
	skos:notation	"10102030" ;
	skos:prefLabel	"Liquefied Petroleum Gas"@en .

ccat:10102040
	a	skos:Concept ;
	skos:altLabel	"Condy"@en ;
	skos:broader	ccat:101020 ;
	skos:definition	"Low-density mixture of hydrocarbons present in raw natural gas cooled down below the hydrocarbon dew point."@en ;
	skos:inScheme	ccat: ;
	skos:notation	"10102040" ;
	skos:prefLabel	"Natural Gas Condensate"@en .

ccat:10102050
	a	skos:Concept ;
	skos:broader	ccat:101020 ;
	skos:definition	"Baseload of gas delivered uniformly over a specified period of time (Time of delivery, TOD) through one or more designated hubs."@en ;
	skos:inScheme	ccat: ;
	skos:notation	"10102050" ;
	skos:prefLabel	"Gas Baseload"@en .

ccat:10102055
	a	skos:Concept ;
	skos:broader	ccat:101020 ;
	skos:definition	"Booked capacity for the purpose of gas transfers."@en ;
	skos:inScheme	ccat: ;
	skos:notation	"10102055" ;
	skos:prefLabel	"Pipeline capacity"@en .

ccat:10102080
	a	skos:Concept ;
	skos:broader	ccat:101020 ;
	skos:definition	"Premium of one gas over another due to chemical composition, freight or storage costs."@en ;
	skos:inScheme	ccat: ;
	skos:notation	"10102080" ;
	skos:prefLabel	"Gas Premium"@en ;
	skos:scopeNote	"This category is also used on spreads between hubs (delivery points)."@en .

ccat:10102085
	a	skos:Concept ;
	skos:broader	ccat:101020 ;
	skos:definition	"Premium of gas (possibly including emission rights) used to produce power over baseload electricity."@en ;
	skos:inScheme	ccat: ;
	skos:notation	"10102085" ;
	skos:prefLabel	"Spark Spread"@en .

ccat:101030
	a	skos:Concept ;
	skos:broader	ccat:1010 ;
	skos:definition	"Petrochemicals derived from crude oil when processed in oil refineries. This explicitly excludes chemical compounds produced in biochemical or (non-petro) industrial processes, e.g. ethanol from fermentation, or methanol from catalytic gas synthesis."@en ;
	skos:exactMatch	eurovoc:2772 , wd:Q1059843 ;
	skos:inScheme	ccat: ;
	skos:notation	"101030" ;
	skos:prefLabel	"Refined Products"@en ;
	skos:related	wd:Q3444730 .

ccat:10103010
	a	skos:Concept ;
	skos:broader	ccat:101030 ;
	skos:definition	"Fuel oil that is primarily used for heating. Chemically very similar to diesel (gasoil, the motor fuel) which is why imarkers, e.g. Yellow 124 in the EU, might have been added."@en ;
	skos:exactMatch	wd:Q912452 ;
	skos:inScheme	ccat: ;
	skos:narrowMatch	stw:14215-2 ;
	skos:notation	"10103010" ;
	skos:prefLabel	"Heating Oil"@en .

ccat:10103020
	a	skos:Concept ;
	skos:altLabel	"Petrol"@en ;
	skos:broader	ccat:101030 ;
	skos:definition	"Petroleum-derived flammable liquid used primarily as a motor fuel, obtained by the fractional distillation of petroleum, enhanced with a variety of additives."@en ;
	skos:exactMatch	agrovoc:c_5746 , eurovoc:3771 , stw:14212-1 , wd:Q39558 ;
	skos:inScheme	ccat: ;
	skos:notation	"10103020" ;
	skos:note	"On average, a 160-liter (42-U.S.-gallon) barrel of crude oil can yield up to about 72 liters (19 U.S. gallons) of gasoline, depending on the crude oil assay and on what other refined products are also extracted.  Additives improve chemical stability and performance characteristics, control corrosiveness, and provide fuel system cleaning. Gasoline may contain oxygen-containing chemicals such as ethanol, MTBE, or ETBE to improve combustion."@en ;
	skos:prefLabel	"Gasoline"@en .

ccat:10103030
	a	skos:Concept ;
	skos:altLabel	"Jet Fuel"@en , "Paraffin"@en ;
	skos:broader	ccat:101030 ;
	skos:definition	"Combustible hydrocarbon liquid widely used widely used as aviation fuel."@en ;
	skos:exactMatch	wd:Q76904 ;
	skos:inScheme	ccat: ;
	skos:notation	"10103030" ;
	skos:prefLabel	"Kerosene"@en .

ccat:10103040
	a	skos:Concept ;
	skos:altLabel	"Gas Oil"@en , "Petrodiesel"@en ;
	skos:broader	ccat:101030 ;
	skos:definition	"Any liquid fuel specifically designed for use in diesel engines"@en ;
	skos:exactMatch	eurovoc:3772 , stw:14214-4 , wd:Q38423 ;
	skos:inScheme	ccat: ;
	skos:notation	"10103040" ;
	skos:prefLabel	"Diesel"@en ;
	skos:scopeNote	"Standardised in EN 590 (EU)"@en .

ccat:10103050
	a	skos:Concept ;
	skos:altLabel	"Bunker"@en , "Fuel Oil"@en , "HFO"@en , "HSFO"@en , "NSFO"@en ;
	skos:broader	ccat:101030 ;
	skos:definition	"Any type of fuel oil used aboard water vessels. Usually bunker B or bunker C, also known as No. 5 or No. 6 respectively."@en ;
	skos:inScheme	ccat: ;
	skos:notation	"10103050" ;
	skos:prefLabel	"Marine Fuel"@en .

ccat:10103060
	a	skos:Concept ;
	skos:broader	ccat:101030 ;
	skos:definition	"Flammable liquid hydrocarbon mixture produced from natural gas condensates, petroleum distillates, and the distillation of coal tar and peat."@en ;
	skos:inScheme	ccat: ;
	skos:notation	"10103060" ;
	skos:note	"In different industries and regions naphtha may also be crude oil or refined products such as kerosene. It is also known as Shellite in Australia."@en ;
	skos:prefLabel	"Naphtha"@en .

ccat:10103080
	a	skos:Concept ;
	skos:broader	ccat:101030 ;
	skos:definition	"Spread between different refined products that determines the premium of one oil over the other due to chemical composition, freight or storage costs."@en ;
	skos:inScheme	ccat: ;
	skos:notation	"10103080" ;
	skos:prefLabel	"Visco Spread"@en .

ccat:10103090
	a	skos:Concept ;
	skos:broader	ccat:101030 ;
	skos:definition	"Any other petrochemicals."@en ;
	skos:inScheme	ccat: ;
	skos:notation	"10103090" ;
	skos:prefLabel	"Other Refined Products"@en .

ccat:101040
	a	skos:Concept ;
	skos:broader	ccat:1010 ;
	skos:definition	"Combustible black or brownish-black sedimentary rock, formed as rock strata called coal seams."@en ;
	skos:exactMatch	agrovoc:c_1693 , eurovoc:5386 , stw:14200-1 , wd:Q24489 ;
	skos:inScheme	ccat: ;
	skos:notation	"101040" ;
	skos:prefLabel	"Coal"@en .

ccat:10104010
	a	skos:Concept ;
	skos:altLabel	"Hard Coal"@en ;
	skos:broader	ccat:101040 ;
	skos:definition	"Coal variety with the highest carbon content and the highest energy density."@en ;
	skos:exactMatch	wd:Q182458 ;
	skos:inScheme	ccat: ;
	skos:notation	"10104010" ;
	skos:prefLabel	"Anthracite"@en .

ccat:10104020
	a	skos:Concept ;
	skos:altLabel	"Black Coal"@en , "Thermal Coal"@en ;
	skos:broader	ccat:101040 ;
	skos:definition	"Coal with bitumen or asphalt, second highest ranking coal. Widely used as a thermal coal."@en ;
	skos:exactMatch	wd:Q732607 ;
	skos:inScheme	ccat: ;
	skos:notation	"10104020" ;
	skos:prefLabel	"Bituminous Coal"@en .

ccat:10104025
	a	skos:Concept ;
	skos:broader	ccat:101040 ;
	skos:definition	"Lower grade of coal with 35%-45% carbon. Widely used as a thermal coal."@en ;
	skos:exactMatch	wd:Q790674 ;
	skos:inScheme	ccat: ;
	skos:notation	"10104025" ;
	skos:prefLabel	"Sub-Bituminous Coal"@en ;
	skos:scopeNote	"The properties of this type are between those of lignite, the lowest grade of coal, and those of bituminous coal, the second-highest grade of coal. Sub-bituminous coal is primarily used as a fuel for steam-electric power generation."@en .

ccat:10104030
	a	skos:Concept ;
	skos:altLabel	"Brown Coal"@en ;
	skos:broader	ccat:101040 ;
	skos:definition	"Soft coal with a relatively low heat content, used almost exclusively as a fuel for steam-electric power generation."@en ;
	skos:exactMatch	agrovoc:c_32489 , eurovoc:1656 , stw:14194-5 , wd:Q156267 ;
	skos:inScheme	ccat: ;
	skos:notation	"10104030" ;
	skos:prefLabel	"Lignite"@en .

ccat:10104040
	a	skos:Concept ;
	skos:broader	ccat:101040 ;
	skos:definition	"Made from thermal coal or oil in the absence of air, a process known as coking. May also be formed naturally by geologic processes."@en ;
	skos:exactMatch	wd:Q192795 ;
	skos:inScheme	ccat: ;
	skos:notation	"10104040" ;
	skos:prefLabel	"Coke"@en .

ccat:101050
	a	skos:Concept ;
	skos:broader	ccat:1010 ;
	skos:definition	"Energy derived from electric potential energy or kinetic energy, supplied by the combination of electric current and electric potential that is delivered by an electrical circuit"@en ;
	skos:exactMatch	eurovoc:747 , stw:14174-4 , wd:Q206799 ;
	skos:inScheme	ccat: ;
	skos:notation	"101050" ;
	skos:prefLabel	"Electricity"@en .

ccat:10105010
	a	skos:Concept ;
	skos:broader	ccat:101050 ;
	skos:definition	"The minimum level of demand on an electrical grid over a span of time, met by unvarying power plants, dispatchable generation, or by a collection of smaller intermittent energy sources."@en ;
	skos:exactMatch	wd:Q360897 ;
	skos:inScheme	ccat: ;
	skos:notation	"10105010" ;
	skos:prefLabel	"Base Load"@en .

ccat:10105020
	a	skos:Concept ;
	skos:broader	ccat:101050 ;
	skos:definition	"Period in the load profile where demand is significantly higher than minimum supply level. Fluctuations may occur from hour to hour. Met by intermittent energy sources."@en ;
	skos:exactMatch	wd:Q3393666 ;
	skos:inScheme	ccat: ;
	skos:notation	"10105020" ;
	skos:prefLabel	"Peak Load"@en .

ccat:10105030
	a	skos:Concept ;
	skos:broader	ccat:101050 ;
	skos:definition	"Period in the load profile that shows nearly no peaks, typically the night, met by unvarying power plants."@en ;
	skos:inScheme	ccat: ;
	skos:notation	"10105030" ;
	skos:prefLabel	"Off-peak"@en .

ccat:10105040
	a	skos:Concept ;
	skos:broader	ccat:101050 ;
	skos:definition	"Upwards or downwards flank between off-peak and on-peak demand covered by special load following plants."@en ;
	skos:inScheme	ccat: ;
	skos:notation	"10105040" ;
	skos:prefLabel	"Shoulder"@en .

ccat:10105050
	a	skos:Concept ;
	skos:broader	ccat:101050 ;
	skos:definition	"Entitles the holder to receive compensation when the spot price (possibly including transmission charges) goes below/above a strike price."@en ;
	skos:inScheme	ccat: ;
	skos:notation	"10105050" ;
	skos:prefLabel	"Floor/Cap"@en .

ccat:10105080
	a	skos:Concept ;
	skos:broader	ccat:101050 ;
	skos:definition	"Entitles the holder to receive compensation for congestion charges across an energy path."@en ;
	skos:inScheme	ccat: ;
	skos:notation	"10105080" ;
	skos:prefLabel	"Transmission Rights"@en ;
	skos:scopeNote	"This category is also used on spreads between hubs (delivery points) provided the legs' delivery times (peak/off-peak), or profiles (base/peak), or power sources (hydro/spark) are identical."@en .

ccat:1020
	a	skos:Concept ;
	skos:broader	ccat:10 ;
	skos:definition	"Rare, naturally occurring metallic chemical element of high economic value. Chemically, less reactive than most elements."@en ;
	skos:exactMatch	eurovoc:1886 , stw:14296-4 , wd:Q271449 ;
	skos:inScheme	ccat: ;
	skos:notation	"1020" ;
	skos:prefLabel	"Precious Metal"@en .

ccat:102010
	a	skos:Concept ;
	skos:broader	ccat:1020 ;
	skos:definition	"Bright, slightly reddish yellow, dense, soft, malleable, and ductile metal. One of the least reactive chemical elements. Solid under standard conditions."@en ;
	skos:exactMatch	agrovoc:c_33067 , eurovoc:2156 , stw:14298-0 , wd:Q897 ;
	skos:inScheme	ccat: ;
	skos:notation	"102010" ;
	skos:note	"As of 2017, the world's largest gold producer by far was China with 440 tonnes per year."@en ;
	skos:prefLabel	"Gold"@en .

ccat:102015
	a	skos:Concept ;
	dct:isReplacedBy	ccat:102085 ;
	skos:broader	ccat:1020 ;
	skos:definition	"Product that tracks the variance or volatility of spot gold."@en ;
	skos:inScheme	ccat: ;
	skos:notation	"102015" ;
	skos:prefLabel	"Gold Variance"@en .

ccat:102020
	a	skos:Concept ;
	skos:broader	ccat:1020 ;
	skos:definition	"Soft, white, lustrous transition metal, exhibits the highest electrical conductivity, thermal conductivity, and reflectivity of any metal. Solid under standard conditions."@en ;
	skos:exactMatch	agrovoc:c_7068 , eurovoc:2514 , stw:14308-2 , wd:Q1090 ;
	skos:inScheme	ccat: ;
	skos:notation	"102020" ;
	skos:prefLabel	"Silver"@en .

ccat:102025
	a	skos:Concept ;
	dct:isReplacedBy	ccat:102085 ;
	skos:broader	ccat:1020 ;
	skos:definition	"Product that tracks the variance or volatility of spot silver."@en ;
	skos:inScheme	ccat: ;
	skos:notation	"102025" ;
	skos:prefLabel	"Silver Variance"@en .

ccat:102030
	a	skos:Concept ;
	skos:broader	ccat:1020 ;
	skos:definition	"Dense, malleable, ductile, highly unreactive, precious, silverish-white transition metal."@en ;
	skos:exactMatch	agrovoc:c_33116 , eurovoc:2424 , stw:14306-6 , wd:Q880 ;
	skos:inScheme	ccat: ;
	skos:notation	"102030" ;
	skos:note	"Used in catalytic converters, laboratory equipment, electrical contacts and electrodes, platinum resistance thermometers, dentistry equipment, and jewelry. Being a heavy metal, it leads to health problems upon exposure to its salts; but due to its corrosion resistance, metallic platinum has not been linked to adverse health effects. Compounds containing platinum, such as cisplatin, oxaliplatin and carboplatin, are applied in chemotherapy against certain types of cancer."@en ;
	skos:prefLabel	"Platinum"@en .

ccat:102040
	a	skos:Concept ;
	skos:broader	ccat:1020 ;
	skos:definition	"Rare and lustrous silvery-white metal with the lowest melting point and is the least density of platinum group elements."@en ;
	skos:exactMatch	agrovoc:c_549615fb , wd:Q1089 ;
	skos:inScheme	ccat: ;
	skos:notation	"102040" ;
	skos:note	"Used in catalytic converters, electronics, dentistry, medicine, hydrogen purification, chemical applications, groundwater treatment, and jewelry. Key component of fuel cells, which react hydrogen with oxygen to produce electricity, heat, and water."@en ;
	skos:prefLabel	"Palladium"@en .

ccat:102050
	a	skos:Concept ;
	skos:broader	ccat:1020 ;
	skos:definition	"Very rare, very hard, very dense, brittle, silvery-white transition metal."@en ;
	skos:exactMatch	agrovoc:c_c2041bc1 , wd:Q877 ;
	skos:inScheme	ccat: ;
	skos:notation	"102050" ;
	skos:note	"Second-densest metal (after osmium). One of the rarest elements in Earth's crust, with annual production and consumption of only three tonnes. Iridium metal is employed when high corrosion resistance at high temperatures is needed, as in high-performance spark plugs, crucibles for recrystallization of semiconductors at high temperatures, and electrodes for the production of chlorine in the chloralkali process. Iridium radioisotopes are used in some radioisotope thermoelectric generators."@en ;
	skos:prefLabel	"Iridium"@en .

ccat:102060
	a	skos:Concept ;
	skos:broader	ccat:1020 ;
	skos:definition	"Ultra-rare, silvery-white, hard, corrosion-resistant, and chemically inert transition metal."@en ;
	skos:exactMatch	agrovoc:c_ea2af13b , wd:Q1087 ;
	skos:inScheme	ccat: ;
	skos:notation	"102060" ;
	skos:note	"Found in platinum or nickel ores together with the other members of the platinum group metals. Used as catalyst in three-way catalytic converters in automobiles. Because rhodium metal is inert against corrosion and most aggressive chemicals, and because of its rarity, rhodium is usually alloyed with platinum or palladium and applied in high-temperature and corrosion-resistive coatings. White gold is often plated with a thin rhodium layer to improve its appearance while sterling silver is often rhodium-plated for tarnish resistance. Rhodium is sometimes used to cure silicones; a two-part silicone in which one part containing a silicon hydride and the other containing a vinyl-terminated silicone are mixed. One of these liquids contains a rhodium complex. Rhodium detectors are used in nuclear reactors to measure the neutron flux level. Other uses of rhodium include asymmetric hydrogenation used to form drug precursors and the processes for the production of acetic acid."@en ;
	skos:prefLabel	"Rhodium"@en .

ccat:102070
	a	skos:Concept ;
	skos:broader	ccat:1020 ;
	skos:definition	"Rare transition metal belonging to the platinum group, inert to most other chemicals."@en ;
	skos:exactMatch	agrovoc:c_87cd9fbc , wd:Q1086 ;
	skos:inScheme	ccat: ;
	skos:notation	"102070" ;
	skos:note	"Annual production in 2017 was 35.5 tonnes. Used in wear-resistant electrical contacts and thick-film resistors, as the capping layer for extreme ultraviolet photomasks. Ruthenium is generally found in ores with the other platinum group metals in the Ural Mountains and in North and South America. Small but commercially important quantities are also found in pentlandite extracted from Sudbury, Ontario and in pyroxenite deposits in South Africa."@en ;
	skos:prefLabel	"Ruthenium"@en .

ccat:102075
	a	skos:Concept ;
	skos:broader	ccat:1020 ;
	skos:definition	"Hard, brittle, bluish-white transition metal in the platinum group."@en ;
	skos:exactMatch	agrovoc:c_9d49077b ;
	skos:inScheme	ccat: ;
	skos:notation	"102075" ;
	skos:note	"Found as a trace element in alloys, mostly in platinum ores. Osmium is the densest naturally occurring element. Used in fountain pen nib tipping, electrical contacts, and in other applications that require extreme durability and hardness. Osmium is among the rarest elements in the Earth's crust, making up only 50 parts per trillion (ppt)."@en ;
	skos:prefLabel	"Osmium"@en .

ccat:102080
	a	skos:Concept ;
	skos:broader	ccat:1020 ;
	skos:definition	"Precious metals expressed in terms of other precious metals, e.g. XAUXAG, XAUXPT, etc."@en ;
	skos:inScheme	ccat: ;
	skos:notation	"102080" ;
	skos:note	"ISO officially assigned currency codes to gold, silver, platinum, and palladium (XAU, XAG, XPT, XPL), by extension unofficial codes for other precious metals are XRH, XIR, XOS, XRU."@en ;
	skos:prefLabel	"Precious Metal Cross"@en .

ccat:102085
	a	skos:Concept ;
	skos:broader	ccat:1020 ;
	skos:definition	"Product that tracks the variance or volatility of precious metal."@en ;
	skos:inScheme	ccat: ;
	skos:notation	"102085" ;
	skos:prefLabel	"Precious Metal Variance"@en .

ccat:1030
	a	skos:Concept ;
	skos:altLabel	"Non-ferrous Metal"@en ;
	skos:broader	ccat:10 ;
	skos:closeMatch	wd:Q428855 , wd:Q5679431 ;
	skos:definition	"Common and inexpensive non-ferrous metals, as opposed to precious metals."@en ;
	skos:inScheme	ccat: ;
	skos:notation	"1030" ;
	skos:prefLabel	"Base Metal"@en .

ccat:103010
	a	skos:Concept ;
	skos:broader	ccat:1030 ;
	skos:definition	"Soft, malleable, and ductile metal with very high thermal and electrical conductivity."@en ;
	skos:exactMatch	agrovoc:c_1868 , stw:14299-5 , wd:Q753 ;
	skos:inScheme	ccat: ;
	skos:notation	"103010" ;
	skos:note	"A freshly exposed surface of pure copper has a pinkish-orange color. Copper is used as a conductor of heat and electricity, as a building material, and as a constituent of various metal alloys, such as sterling silver used in jewelry, cupronickel used to make marine hardware and coins, and constantan used in strain gauges and thermocouples for temperature measurement."@en ;
	skos:prefLabel	"Copper"@en .

ccat:103013
	a	skos:Concept ;
	skos:broader	ccat:1030 ;
	skos:definition	"Alloy of copper and zinc."@en ;
	skos:inScheme	ccat: ;
	skos:notation	"103013" ;
	skos:prefLabel	"Brass"@en .

ccat:103015
	a	skos:Concept ;
	skos:broader	ccat:1030 ;
	skos:definition	"Alloy of copper and tin."@en ;
	skos:inScheme	ccat: ;
	skos:notation	"103015" ;
	skos:prefLabel	"Bronze"@en .

ccat:103020
	a	skos:Concept ;
	skos:broader	ccat:1030 ;
	skos:definition	"Silvery-white, soft, non-magnetic and ductile metal in the boron group."@en ;
	skos:exactMatch	agrovoc:c_317 , eurovoc:1446 , msa:513153333 , stw:14293-3 , wd:Q663 ;
	skos:inScheme	ccat: ;
	skos:notation	"103020" ;
	skos:note	"Aluminium is remarkable for its low density and its ability to resist corrosion through the phenomenon of passivation. Aluminium and its alloys are vital to the aerospace industry and important in transportation and building industries, such as building facades and window frames. The oxides and sulfates are the most useful compounds of aluminium. Despite its prevalence in the environment, no living organism is known to use aluminium salts metabolically, but aluminium is well tolerated by plants and animals. Because of these salts' abundance, the potential for a biological role for them is of continuing interest, and studies continue."@en ;
	skos:prefLabel	"Aluminium"@en .

ccat:103025
	a	skos:Concept ;
	skos:altLabel	"NASAAC"@en ;
	skos:broader	ccat:1030 ;
	skos:definition	"Aluminium alloy conforming to the LME NA380.1 specification which is a modification of The Aluminium Association Inc. A380.1 specification (1989).  The alloy has a composition of 8.50%-9.50% Si, 3.00%-3.50% Cu, 0.80%-1.00% Fe, a maximum of 3.00% Zn, a maximum of 1.80% sludge (Fe + 2Mn + 3Cr), a maximum of 0.50% Ni, a maximum of 0.45% Mn, a maximum of 0.10% Mg, Sn, Pb, Ti, and Cr each."@en ;
	skos:inScheme	ccat: ;
	skos:notation	"103025" ;
	skos:prefLabel	"North American Special Aluminum Alloy"@en .

ccat:103030
	a	skos:Concept ;
	skos:broader	ccat:1030 ;
	skos:definition	"Slightly brittle metal at room temperature, blue-silvery appearance when oxidation is removed."@en ;
	skos:exactMatch	agrovoc:c_8517 , eurovoc:4783 , stw:14309-0 , wd:Q758 ;
	skos:inScheme	ccat: ;
	skos:notation	"103030" ;
	skos:prefLabel	"Zinc"@en .

ccat:103040
	a	skos:Concept ;
	skos:broader	ccat:1030 ;
	skos:definition	"Silvery-white, hard, ductile, lustrous transition metal with a slight golden tinge."@en ;
	skos:exactMatch	agrovoc:c_5172 , eurovoc:2056 , stw:14305-1 , wd:Q744 ;
	skos:inScheme	ccat: ;
	skos:notation	"103040" ;
	skos:note	"Nickel is one of four elements (the others are iron, cobalt, and gadolinium) that are ferromagnetic at approximately room temperature. About 68% of world production is used in stainless steel. A further 10% is used for nickel-based and copper-based alloys, 7% for alloy steels, 3% in foundries, 9% in plating and 4% in other applications, including the fast-growing battery sector, including those in electric vehicles (EVs). As a compound, nickel has a number of niche chemical manufacturing uses, such as a catalyst for hydrogenation, cathodes for batteries, pigments and metal surface treatments. Nickel is an essential nutrient for some microorganisms and plants that have enzymes with nickel as an active site."@en ;
	skos:prefLabel	"Nickel"@en .

ccat:103050
	a	skos:Concept ;
	skos:broader	ccat:1030 ;
	skos:definition	"Silvery metal that characteristically has a faint yellow hue, soft enough to be cut without much force"@en ;
	skos:exactMatch	agrovoc:c_7782 , eurovoc:879 , stw:14310-1 , wd:Q1096 ;
	skos:inScheme	ccat: ;
	skos:notation	"103050" ;
	skos:note	"Obtained chiefly from the mineral cassiterite, which contains stannic oxide, SnO2. Tin shows a chemical similarity to both of its neighbors in group 14, germanium and lead, and has two main oxidation states, +2 and the slightly more stable +4. Tin is the 49th most abundant element on Earth and has, with 10 stable isotopes, the largest number of stable isotopes in the periodic table, thanks to its magic number of protons. It has two main allotropes: at room temperature, the stable allotrope is beta-tin, a silvery-white, malleable metal, but at low temperatures, it transforms into the less dense grey alpha-tin, which has the diamond cubic structure. Metallic tin does not easily oxidize in air. Tin is used in many alloys, most notably tin / lead soft solders, which are typically 60% or more tin, and in the manufacture of transparent, electrically conducting films of indium tin oxide in optoelectronic applications. Another large application for tin is corrosion-resistant tin plating of steel. Because of the low toxicity of inorganic tin, tin-plated steel is widely used for food packaging as tin cans. However, some organotin compounds can be almost as toxic as cyanide."@en ;
	skos:prefLabel	"Tin"@en .

ccat:103060
	a	skos:Concept ;
	skos:broader	ccat:1030 ;
	skos:definition	"Heavy, soft, malleable, and relatively unreactive post-transition metal with a relatively low melting point, silvery with a hint of blue when freshly cut, tarnishes to a dull grey when exposed to air."@en ;
	skos:exactMatch	agrovoc:c_4235 , eurovoc:2428 , msa:2909791279 , stw:14294-1 , wd:Q708 ;
	skos:inScheme	ccat: ;
	skos:notation	"103060" ;
	skos:note	"""Lead's weak metallic character is illustrated by its amphoteric nature; lead and lead oxides react with acids and bases, and it tends to form covalent bonds. Compounds of lead are usually found in the +2 oxidation state rather than the +4 state common with lighter members of the carbon group. Exceptions are mostly limited to organolead compounds. Like the lighter members of the group, lead tends to bond with itself; it can form chains and polyhedral structures.

Lead's high density, low melting point, ductility and relative inertness to oxidation make it useful. These properties, combined with its relative abundance and low cost, resulted in its extensive use in construction, plumbing, batteries, bullets and shot, weights, solders, pewters, fusible alloys, white paints, leaded gasoline, and radiation shielding."""@en ;
	skos:prefLabel	"Lead"@en .

ccat:103070
	a	skos:Concept ;
	skos:broader	ccat:1030 ;
	skos:definition	"Traded almost exclusively as titanium dioxide. Lustrous transition metal with a silver colour, low density, and high strength, resistant to corrosion in sea water, aqua regia, and chlorine."@en ;
	skos:exactMatch	agrovoc:c_32704 , eurovoc:4462 , msa:506065880 , stw:18240-4 , wd:Q716 ;
	skos:inScheme	ccat: ;
	skos:notation	"103070" ;
	skos:note	"""Occurs within a number of mineral deposits, principally rutile and ilmenite, which are widely distributed in the Earth's crust and lithosphere; it is found in almost all living things, as well as bodies of water, rocks, and soils. The metal is extracted from its principal mineral ores by the Kroll and Hunter processes. The most common compound, titanium dioxide, is a popular photocatalyst and is used in the manufacture of white pigments. Other compounds include titanium tetrachloride (TiCl4), a component of smoke screens and catalysts; and titanium trichloride (TiCl3), which is used as a catalyst in the production of polypropylene.

Titanium can be alloyed with iron, aluminium, vanadium, and molybdenum, among other elements, to produce strong, lightweight alloys for aerospace (jet engines, missiles, and spacecraft), military, industrial processes (chemicals and petrochemicals, desalination plants, pulp, and paper), automotive, agriculture (farming), medical prostheses, orthopedic implants, dental and endodontic instruments and files, dental implants, sporting goods, jewelry, mobile phones, and other applications.

The two most useful properties of the metal are corrosion resistance and strength-to-density ratio, the highest of any metallic element. In its unalloyed condition, titanium is as strong as some steels, but less dense."""@en ;
	skos:prefLabel	"Titanium"@en .

ccat:1035
	a	skos:Concept ;
	skos:broader	ccat:10 ;
	skos:definition	"Iron and iron-related metals, or alloys that contain iron or iron-related metals, such as steel or pig iron."@en ;
	skos:exactMatch	wd:Q2380954 ;
	skos:inScheme	ccat: ;
	skos:notation	"1035" ;
	skos:prefLabel	"Ferrous Metal"@en .

ccat:103510
	a	skos:Concept ;
	skos:broader	ccat:1035 ;
	skos:definition	"Obtained by smelting iron ore in a blast furnace as intermediate product in the production of steel."@en ;
	skos:exactMatch	agrovoc:c_3950 , eurovoc:981 , stw:14281-3 , wd:Q901785 ;
	skos:inScheme	ccat: ;
	skos:notation	"103510" ;
	skos:prefLabel	"Pig Iron"@en .

ccat:103520
	a	skos:Concept ;
	skos:broader	ccat:1035 ;
	skos:definition	"Alloy of iron with typically a few percent of carbon to improve its strength and fracture resistance, or 11% of chromium to produce corrosion and oxidation resistant stainless steel."@en ;
	skos:exactMatch	agrovoc:c_7384 , eurovoc:5065 , stw:14285-2 , wd:Q11427 ;
	skos:inScheme	ccat: ;
	skos:notation	"103520" ;
	skos:note	"Because of its high tensile strength and low cost, steel is used in buildings, infrastructure, tools, ships, trains, cars, machines, electrical appliances, and weapons. Iron is the base metal of steel and it can take on two crystalline forms (allotropic forms): body centred cubic and face-centred cubic. These forms depend on temperature. In the body-centred cubic arrangement, there is an iron atom in the centre and eight atoms at the vertices of each cubic unit cell; in the face-centred cubic, there is one atom at the centre of each of the six faces of the cubic unit cell and eight atoms at its vertices. It is the interaction of the allotropes of iron with the alloying elements, primarily carbon, that gives steel and cast iron their range of unique properties."@en ;
	skos:prefLabel	"Steel"@en .

ccat:103530
	a	skos:Concept ;
	skos:broader	ccat:1035 ;
	skos:definition	"Rocks and minerals from which metallic iron can be economically extracted. The ores are usually rich in iron oxides and vary in colour from dark grey, bright yellow, or deep purple to rusty red. The iron is usually found in the form of magnetite (Fe3O4, 72.4% Fe), hematite (Fe2O3, 69.9% Fe), goethite (FeO(OH), 62.9% Fe), limonite (FeO(OH)\u00B7n(H2O), 55% Fe) or siderite (FeCO3, 48.2% Fe)."@en ;
	skos:exactMatch	eurovoc:1933 , stw:14195-3 , wd:Q191552 ;
	skos:inScheme	ccat: ;
	skos:notation	"103530" ;
	skos:note	"Ores containing very high quantities of hematite or magnetite (greater than about 60% iron) are known as \"natural ore\" or \"direct shipping ore\", meaning they can be fed directly into iron-making blast furnaces. Iron ore is the raw material used to make pig iron, which is one of the main raw materials to make steel---98% of the mined iron ore is used to make steel. In 2011 the Financial Times has speculated that iron ore is \"more integral to the global economy than any other commodity, except perhaps oil."@en ;
	skos:prefLabel	"Iron Ore"@en .

ccat:103535
	a	skos:Concept ;
	skos:broader	ccat:1035 ;
	skos:definition	"Iron and steel scrap from automobiles, trains, ships, bridges, buildings, railway rails and fasteners, or farming equipment."@en ;
	skos:inScheme	ccat: ;
	skos:notation	"103535" ;
	skos:note	"Ferrous scrap is the most recycled material in the world. The U.S. Geological Survey estimates that 65 million metric tons of iron and steel scrap was processed around the world in 2016.  Ferrous scrap comes from many consumer products like automobiles or household appliances, or from industrial structures and equipment such as buildings, railroads, trains, bridges, ships, and farming equipment."@en ;
	skos:prefLabel	"Ferrous Scrap"@en .

ccat:103540
	a	skos:Concept ;
	skos:broader	ccat:1035 ;
	skos:definition	"Sedimentary rock with a relatively high aluminium content. The world's main source of aluminium and gallium. Used as flux in blast furnaces for smelting."@en ;
	skos:exactMatch	eurovoc:3755 , stw:14190-6 , wd:Q102078 ;
	skos:inScheme	ccat: ;
	skos:notation	"103540" ;
	skos:prefLabel	"Bauxite"@en .

ccat:103550
	a	skos:Concept ;
	skos:broader	ccat:1035 ;
	skos:definition	"Hard, brittle, silvery transition metal, often found in minerals in combination with iron. Alloys are used in stainless steels. It improves strength, workability, and resistance to wear."@en ;
	skos:exactMatch	agrovoc:c_4570 , eurovoc:1779 , stw:14301-2 , wd:Q731 ;
	skos:inScheme	ccat: ;
	skos:notation	"103550" ;
	skos:note	"Manganese oxide is used as an oxidising agent; as a rubber additive; and in glass making, fertilisers, and ceramics. Manganese sulfate can be used as a fungicide."@en ;
	skos:prefLabel	"Manganese"@en .

ccat:103560
	a	skos:Concept ;
	skos:broader	ccat:1035 ;
	skos:closeMatch	wd:Q1053 ;
	skos:definition	"Silvery metal with a grey cast."@en ;
	skos:inScheme	ccat: ;
	skos:notation	"103560" ;
	skos:note	"Molybdenum does not occur naturally as a free metal on Earth; it is found only in various oxidation states in minerals. As free element molybdenum has the sixth-highest melting point of any element. It readily forms hard, stable carbides in alloys, and for this reason most of world production of the element (about 80%) is used in steel alloys, including high-strength alloys and superalloys."@en ;
	skos:prefLabel	"Molybdenum"@en .

ccat:103570
	a	skos:Concept ;
	skos:broader	ccat:1035 ;
	skos:closeMatch	wd:Q725 ;
	skos:definition	"Main additive in stainless steel adding anti-corrosive properties."@en ;
	skos:inScheme	ccat: ;
	skos:notation	"103570" ;
	skos:note	"Chromium is also highly valued as a metal that is able to be highly polished while resisting tarnishing. Polished chromium reflects almost 70% of the visible spectrum, with almost 90% of infrared light being reflected."@en ;
	skos:prefLabel	"Chromium"@en .

ccat:1040
	a	skos:Concept ;
	skos:broader	ccat:10 ;
	skos:definition	"Metals that are not abundant and mostly extracted as a by-product."@en ;
	skos:inScheme	ccat: ;
	skos:notation	"1040" ;
	skos:prefLabel	"Rare Metal"@en .

ccat:104010
	a	skos:Concept ;
	skos:broader	ccat:1040 ;
	skos:closeMatch	agrovoc:c_8084 , eurovoc:4617 , stw:14222-5 , wd:Q1098 ;
	skos:definition	"Uranium oxide or Uranium fluoride, extracted from uranium-bearing minerals such as uraninite."@en ;
	skos:inScheme	ccat: ;
	skos:notation	"104010" ;
	skos:note	"Uranium-235 is the only naturally occurring fissile isotope, which makes it widely used in nuclear power plants and nuclear weapons. However, because of the tiny amounts found in nature, uranium needs to undergo enrichment so that enough uranium-235 is present. Uranium-238 is fissionable by fast neutrons, and is fertile, meaning it can be transmuted to fissile plutonium-239 in a nuclear reactor. Another fissile isotope, uranium-233, can be produced from natural thorium and is studied for future industrial use in nuclear technology. Depleted uranium (238U) is used in kinetic energy penetrators and armor plating. Uranium is used as a colorant in uranium glass, producing lemon yellow to green colors. Uranium glass fluoresces green in ultraviolet light. It was also used for tinting and shading in early photography."@en ;
	skos:prefLabel	"Uranium"@en .

ccat:104020
	a	skos:Concept ;
	skos:broader	ccat:1040 ;
	skos:closeMatch	agrovoc:c_1702 , eurovoc:6018 , wd:Q740 ;
	skos:definition	"Cobalt 99.8%, cobalt standard grade, cobalt alloy grade, cobalt hydroxide 0%, cobalt sulfate 20.5%, or cobalt tetroxide 72.6%."@en ;
	skos:inScheme	ccat: ;
	skos:notation	"104020" ;
	skos:note	"Cobalt is primarily used in lithium-ion batteries, and in the manufacture of magnetic, wear-resistant and high-strength alloys. The compounds cobalt silicate and cobalt(II) aluminate (CoAl2O4, cobalt blue) give a distinctive deep blue color to glass, ceramics, inks, paints and varnishes. Cobalt occurs naturally as only one stable isotope, cobalt-59. Cobalt-60 is a commercially important radioisotope, used as a radioactive tracer and for the production of high-energy gamma rays."@en ;
	skos:prefLabel	"Cobalt"@en .

ccat:104030
	a	skos:Concept ;
	skos:broader	ccat:1040 ;
	skos:closeMatch	agrovoc:c_4386 , wd:Q568 ;
	skos:definition	"Lithium carbonate 99%, or Lithium hydroxide monohydrate 56.5%."@en ;
	skos:inScheme	ccat: ;
	skos:notation	"104030" ;
	skos:note	"Lithium and its compounds have several industrial applications, including heat-resistant glass and ceramics, lithium grease lubricants, flux additives for iron, steel and aluminium production, lithium batteries, and lithium-ion batteries. These uses consume more than three-quarters of lithium production."@en ;
	skos:prefLabel	"Lithium"@en .

ccat:104040
	a	skos:Concept ;
	skos:broader	ccat:1040 ;
	skos:closeMatch	wd:Q942 ;
	skos:definition	"Bismuth 99.99% extracted from ores containing bismuth oxide or sulfide"@en ;
	skos:exactMatch	agrovoc:c_938 , eurovoc:4990 ;
	skos:inScheme	ccat: ;
	skos:notation	"104040" ;
	skos:note	"It is a brittle metal with a silvery white color when freshly produced, but surface oxidation can give it an iridescent tinge in numerous colours. Bismuth is the most naturally diamagnetic element, and has one of the lowest values of thermal conductivity among metals."@en ;
	skos:prefLabel	"Bismuth"@en .

ccat:20
	a	skos:Concept ;
	skos:definition	"Soft commodities, or softs, are commodities that, generally, are grown, rather than mined.  Furthermore, softs in this concept scheme are primarily for consumption, i.e. distinct from Materials."@en ;
	skos:inScheme	ccat: ;
	skos:notation	"20" ;
	skos:prefLabel	"Softs"@en ;
	skos:topConceptOf	ccat: .

ccat:2010
	a	skos:Concept ;
	skos:broader	ccat:20 ;
	skos:definition	"Any grass cultivated for the edible components of its grain. Cereal grain crops are grown in greater quantities and provide more food energy worldwide than any other type of crop and are therefore staple crops. Edible grains from other plant families, such as buckwheat, quinoa and chia, are referred to as pseudocereals."@en ;
	skos:exactMatch	agrovoc:c_1474 , eurovoc:536 , wd:Q12117 ;
	skos:inScheme	ccat: ;
	skos:notation	"2010" ;
	skos:prefLabel	"Cereals"@en .

ccat:201010
	a	skos:Concept ;
	skos:altLabel	"Corn"@en ;
	skos:broader	ccat:2010 ;
	skos:closeMatch	wd:Q25618328 ;
	skos:definition	"Cereal grain with a leafy stalk that produces pollen inflorescences and separate ovuliferous inflorescences called ears that yield kernels or seeds, which are fruits."@en ;
	skos:exactMatch	agrovoc:c_12332 , stw:14093-4 , wd:Q11575 ;
	skos:inScheme	ccat: ;
	skos:notation	"201010" ;
	skos:note	"Maize has become a staple food in many parts of the world, with the total production of maize surpassing that of wheat or rice. In addition to being consumed directly by humans (often in the form of masa), maize is also used for corn ethanol, animal feed and other maize products, such as corn starch and corn syrup."@en ;
	skos:prefLabel	"Maize"@en .

ccat:201020
	a	skos:Concept ;
	skos:broader	ccat:2010 ;
	skos:closeMatch	wd:Q5090 ;
	skos:definition	"Seed of the grass species Oryza glaberrima (African rice) or Oryza sativa (Asian rice)."@en ;
	skos:exactMatch	agrovoc:c_6599 , stw:14095-0 , wd:Q5090 ;
	skos:inScheme	ccat: ;
	skos:notation	"201020" ;
	skos:note	"As a cereal grain, it is the most widely consumed staple food for a large part of the world's human population, especially in Asia and Africa. It is the agricultural commodity with the third-highest worldwide production (rice, 741.5 million tonnes in 2014), after sugarcane (1.9 billion tonnes) and maize (1.0 billion tonnes)."@en ;
	skos:prefLabel	"Rice"@en .

ccat:201030
	a	skos:Concept ;
	skos:broader	ccat:2010 ;
	skos:closeMatch	wd:Q15645384 ;
	skos:definition	"Cereal grain in the genus Triticum; the most widely grown is common wheat (T. aestivum)."@en ;
	skos:exactMatch	agrovoc:c_8373 , stw:14098-1 , wd:Q15645384 ;
	skos:inScheme	ccat: ;
	skos:notation	"201030" ;
	skos:prefLabel	"Wheat"@en .

ccat:201035
	a	skos:Concept ;
	skos:altLabel	"Pasta Wheat"@en ;
	skos:broader	ccat:2010 ;
	skos:definition	"Tetraploid species of wheat, second most cultivated species of wheat after common wheat, predominant wheat of the Middle East."@en ;
	skos:exactMatch	agrovoc:c_11456 , wd:Q618324 ;
	skos:inScheme	ccat: ;
	skos:notation	"201035" ;
	skos:note	"Durum in Latin means \"hard\", and the species is the hardest of all wheats. This refers to the resistance of the grain to milling, in particular of the starchy endosperm, implying dough made from its flour is weak or \"soft\". This makes durum favorable for semolina and pasta and less practical for flour, which requires more work than with hexaploid wheats like common bread wheats. Despite its high protein content, durum is not a strong wheat in the sense of giving strength to dough through the formation of a gluten network. Durum contains 27% extractable wet gluten, about 3% higher than in common wheat (T. aestivum L.)."@en ;
	skos:prefLabel	"Durum"@en .

ccat:201040
	a	skos:Concept ;
	skos:broader	ccat:2010 ;
	skos:definition	"Major cereal grain grown in temperate climates globally; Hordeum vulgare, a member of the grass family."@en ;
	skos:exactMatch	agrovoc:c_823 , stw:14087-6 , wd:Q61665121 ;
	skos:inScheme	ccat: ;
	skos:notation	"201040" ;
	skos:note	"Barley has been used as animal fodder, as a source of fermentable material for beer and certain distilled beverages, and as a component of various health foods. It is used in soups and stews, and in barley bread of various cultures. Barley grains are commonly made into malt in a traditional and ancient method of preparation. In 2017, barley was ranked fourth among grains in quantity produced (149 million tonnes) behind maize, rice and wheat."@en ;
	skos:prefLabel	"Barley"@en .

ccat:201050
	a	skos:Concept ;
	skos:broader	ccat:2010 ;
	skos:definition	"Cereal grain in the Avena genus (Avena sativa)."@en ;
	skos:exactMatch	agrovoc:c_5287 , stw:14090-3 , wd:Q24265484 ;
	skos:inScheme	ccat: ;
	skos:notation	"201050" ;
	skos:note	"While oats are suitable for human consumption as oatmeal and oat milk, one of the most common uses is as livestock feed. Oats are associated with lower blood cholesterol when consumed regularly."@en ;
	skos:prefLabel	"Oats"@en .

ccat:201060
	a	skos:Concept ;
	skos:broader	ccat:2010 ;
	skos:definition	"Grain of an annual cereal, some cultivars are perennial, in the Sorghum genus ranging from 2 to 4 mm in diameter."@en ;
	skos:exactMatch	agrovoc:c_7247 , wd:Q332062 ;
	skos:inScheme	ccat: ;
	skos:notation	"201060" ;
	skos:note	"""Primarily grown for forage, syrup production, and ethanol. The leading producers of S. bicolor in 2011 were Nigeria (12.6%), India (11.2%), Mexico (11.2%), and the United States (10.0%). Sorghum grows in a wide range of temperatures, high altitudes, and toxic soils, and can recover growth after some drought. It has five features that make it one of the most drought-resistant crops:

- It has a very large root-to-leaf surface area ratio.
- In times of drought, it rolls its leaves to lessen water loss by transpiration.
- If drought continues, it goes into dormancy rather than dying.
- Its leaves are protected by a waxy cuticle.
- It uses C4 carbon fixation thus using only a third the amount of water that C3 plants require."""@en ;
	skos:prefLabel	"Sorghum"@en .

ccat:201065
	a	skos:Concept ;
	skos:altLabel	"Bajra"@en , "Kambu"@en , "Sajjey"@en ;
	skos:broader	ccat:2010 ;
	skos:definition	"Grain of Pennisetum glaucum, ovoid, of 3-4 mm length, nearly white, pale yellow, brown, grey, slate blue or purple."@en ;
	skos:exactMatch	agrovoc:c_e4e17d1b , wd:Q104037539 ;
	skos:inScheme	ccat: ;
	skos:notation	"201065" ;
	skos:note	"Pearl millet is well adapted to growing areas characterized by drought, low soil fertility, and high temperature. It performs well in soils with high salinity or low pH. Because of its tolerance to difficult growing conditions, it can be grown in areas where other cereal crops, such as maize or wheat, would not survive. Pearl millet is a summer annual crop well-suited for double cropping and rotations."@en ;
	skos:prefLabel	"Pearl Millet"@en .

ccat:201070
	a	skos:Concept ;
	skos:broader	ccat:2010 ;
	skos:definition	"Grain of the cereal of the Triticeae tribe in the Secale genus."@en ;
	skos:exactMatch	agrovoc:c_14010 , eurovoc:4059 , stw:14096-5 , wd:Q12099 ;
	skos:inScheme	ccat: ;
	skos:notation	"201070" ;
	skos:note	"Rye grain is used for flour, bread, beer, crispbread, some whiskeys, some vodkas, and animal fodder. It can also be eaten whole, either as boiled rye berries or by being rolled, similar to rolled oats."@en ;
	skos:prefLabel	"Rye"@en .

ccat:201075
	a	skos:Concept ;
	skos:broader	ccat:2010 ;
	skos:definition	"Hybrid of wheat (female) and rye (male)."@en ;
	skos:exactMatch	agrovoc:c_33914 , wd:Q380329 ;
	skos:inScheme	ccat: ;
	skos:notation	"201075" ;
	skos:note	"""Almost always a second-generation hybrid, i.e., a cross between two kinds of primary (first-cross) triticales. As a rule, triticale combines the yield potential and grain quality of wheat with the disease and environmental tolerance (including soil conditions) of rye. Only recently has it been developed into a commercially viable crop. Grown mostly for forage or fodder, although some triticale-based foods can be purchased at health food stores and can be found in some breakfast cereals.

The primary producers of triticale are Poland, Germany, Belarus, France and Russia. In 2014, according to the Food and Agriculture Organization (FAO), 17.1 million tons were harvested in 37 countries across the world.

The triticale hybrids are all amphidiploid, which means the plant is diploid for two genomes derived from different species. In other words, triticale is an allotetraploid. In earlier years, most work was done on octoploid triticale. Different ploidy levels have been created and evaluated over time. The tetraploids showed little promise, but hexaploid triticale was successful enough to find commercial application.

The International Maize and Wheat Improvement Center triticale improvement program was intended to improve food production and nutrition in developing countries. Triticale was thought to have potential in the production of bread and other food products, such as cookies, pasta, pizza dough and breakfast cereals. The protein content is higher than that of wheat, although the glutenin fraction is less. The grain has also been stated to have higher levels of lysine than wheat. Acceptance would require the milling industry to adapt to triticale, as the milling techniques employed for wheat are unsuited to triticale. Past research indicated that triticale could be used as a feed grain and, particularly, later research found that its starch is readily digested. As a feed grain, triticale is already well established and of high economic importance. It has received attention as a potential energy crop, and research is currently being conducted on the use of the crop's biomass in bioethanol production."""@en ;
	skos:prefLabel	"Triticale"@en .

ccat:201080
	a	skos:Concept ;
	skos:broader	ccat:2010 ;
	skos:definition	"Intercommodity spread between grains, or grains and oilseeds."@en ;
	skos:inScheme	ccat: ;
	skos:notation	"201080" ;
	skos:prefLabel	"Grain Inter Spread"@en .

ccat:201090
	a	skos:Concept ;
	skos:broader	ccat:2010 ;
	skos:closeMatch	agrovoc:c_6301 , wd:Q2643145 ;
	skos:definition	"Cereals and grains of minor economic importance."@en ;
	skos:inScheme	ccat: ;
	skos:notation	"201090" ;
	skos:prefLabel	"Other Cereals and Pseudocereals"@en .

ccat:20109010
	a	skos:Concept ;
	skos:broader	ccat:201090 ;
	skos:definition	"Grain-like seeds of a pseudocereal in the genus Fagopyrum."@en ;
	skos:exactMatch	agrovoc:c_9471 , eurovoc:3898 , wd:Q132734 ;
	skos:inScheme	ccat: ;
	skos:notation	"20109010" ;
	skos:note	"Buckwheat is referred to as a pseudocereal because its seeds' culinary use is the same as cereals', owing to their composition of complex carbohydrates."@en ;
	skos:prefLabel	"Buckwheat"@en .

ccat:20109020
	a	skos:Concept ;
	skos:broader	ccat:201090 ;
	skos:definition	"Seeds of a flowering plant in the amaranth family."@en ;
	skos:exactMatch	agrovoc:c_13716 , wd:Q139925 ;
	skos:inScheme	ccat: ;
	skos:notation	"20109020" ;
	skos:note	"""The seeds are rich in protein, dietary fiber, B vitamins, and dietary minerals in amounts greater than in many grains. Quinoa is not a grass, but rather a pseudocereal botanically related to spinach and amaranth (Amaranthus spp.), and originated in the Andean region of northwestern South America. It was first used to feed livestock 5.2-7.0 thousand years ago, and for human consumption-4 thousand years ago in the Lake Titicaca basin of Peru and Bolivia.

Today, almost all production in the Andean region is done by small farms and associations. Its cultivation has spread to more than 70 countries, including Kenya, India, the United States, and several European countries. As a result of increased popularity and consumption in North America, Europe, and Australasia, quinoa crop prices tripled between 2006 and 2014."""@en ;
	skos:prefLabel	"Quinoa"@en .

ccat:2020
	a	skos:Concept ;
	skos:broader	ccat:20 ;
	skos:definition	"Plants that are grown primarily for their oil. The oil may be used for cooking, as food additives, or processed into oleochemicals, e.g. as a substitute for petroleum-based fuels. Some may be also used for cosmetics, medical purposes, wood finishing, oil painting and other industrial purposes."@en ;
	skos:inScheme	ccat: ;
	skos:notation	"2020" ;
	skos:prefLabel	"Oil-Bearing Crops"@en .

ccat:202010
	a	skos:Concept ;
	skos:broader	ccat:2020 ;
	skos:definition	"Beans of Glycine max, a species of legume native to East Asia."@en ;
	skos:exactMatch	agrovoc:c_14477 , stw:14081-4 , wd:Q61503220 ;
	skos:inScheme	ccat: ;
	skos:notation	"202010" ;
	skos:note	"""Traditional unfermented food uses of soybeans include soy milk, from which tofu and tofu skin are made. Fermented soy foods include soy sauce, fermented bean paste, natto, and tempeh. Fat-free (defatted) soybean meal is a significant and cheap source of protein for animal feeds and many packaged meals. For example, soybean products, such as textured vegetable protein (TVP), are ingredients in many meat and dairy substitutes.

Soy beans contain significant amounts of phytic acid, dietary minerals and B vitamins. Soy vegetable oil, used in food and industrial applications, is another product of processing the soybean crop. Soybean is the most important protein source for feed farm animals (that in turn yields animal protein for human consumption)."""@en ;
	skos:prefLabel	"Soybeans"@en .

ccat:202020
	a	skos:Concept ;
	skos:altLabel	"Canola"@en ;
	skos:broader	ccat:2020 ;
	skos:definition	"Seed of rapeseed (Brassica napus subsp. napus), a bright-yellow flowering member of the family Brassicaceae (mustard or cabbage family)"@en ;
	skos:exactMatch	agrovoc:c_25499 , eurovoc:6042 , stw:14078-0 , wd:Q177932 ;
	skos:inScheme	ccat: ;
	skos:notation	"202020" ;
	skos:note	"The seed naturally contains appreciable amounts of toxic erucic acid. Canola are a group of rapeseed cultivars which were bred to have very low levels of erucic acid and are especially prized for use for human and animal food. Rapeseed is the third-largest source of vegetable oil and second-largest source of protein meal in the world."@en ;
	skos:prefLabel	"Rapeseed"@en .

ccat:202030
	a	skos:Concept ;
	skos:broader	ccat:2020 ;
	skos:closeMatch	agrovoc:c_2509 , agrovoc:c_5330 , wd:Q165403 ;
	skos:definition	"Fruit of oil palms in the Elaeis genus"@en ;
	skos:inScheme	ccat: ;
	skos:notation	"202030" ;
	skos:note	"""The species is also now naturalised in Madagascar, Sri Lanka, Malaysia, Indonesia, Central America, Cambodia, the West Indies, and several islands in the Indian and Pacific Oceans. The closely related American oil palm Elaeis oleifera and a more distantly related palm, Attalea maripa, are also used to produce palm oil.

Oil palms can produce much more oil per unit of land area than most other oil-producing plants (about nine time more than soy, and 4.5 times more than rapeseed)."""@en ;
	skos:prefLabel	"Oil Palm Fruit"@en .

ccat:202035
	a	skos:Concept ;
	skos:broader	ccat:2020 ;
	skos:definition	"Drupe of the trees in the Cocos genus."@en ;
	skos:exactMatch	agrovoc:c_25470 , stw:14066-0 , wd:Q3342808 ;
	skos:inScheme	ccat: ;
	skos:notation	"202035" ;
	skos:note	"Trees grow up to 30 m (100 ft) tall and can yield up to 75 fruits per year, though fewer than 30 is more typical. Plants are intolerant of cold weather and prefer copious precipitation, as well as full sunlight. Many insect pests and diseases affect the species and are a nuisance for commercial production. About 75% of the world's supply of coconuts is produced by Indonesia, the Philippines, and India combined."@en ;
	skos:prefLabel	"Coconuts"@en .

ccat:202040
	a	skos:Concept ;
	skos:broader	ccat:2020 ;
	skos:definition	"Seed of the cotton plant. This includes seeds with the attached lint."@en ;
	skos:exactMatch	agrovoc:c_25473 , wd:Q17104079 ;
	skos:inScheme	ccat: ;
	skos:notation	"202040" ;
	skos:prefLabel	"Cottonseed"@en .

ccat:202050
	a	skos:Concept ;
	skos:broader	ccat:2020 ;
	skos:definition	"Seed of the plant Arachis hypogaea"@en ;
	skos:exactMatch	agrovoc:c_11368 , stw:14056-3 , wd:Q37383 ;
	skos:inScheme	ccat: ;
	skos:notation	"202050" ;
	skos:note	"Widely grown in the tropics and subtropics, being important to both small and large commercial producers. In botany, it is classified as both a grain legume and, due to its high oil content, an oil crop."@en ;
	skos:prefLabel	"Groundnuts"@en .

ccat:202080
	a	skos:Concept ;
	skos:broader	ccat:2020 ;
	skos:definition	"Intercommodity spread between two oilseeds."@en ;
	skos:inScheme	ccat: ;
	skos:notation	"202080" ;
	skos:prefLabel	"Oilseed Inter Spread"@en .

ccat:202085
	a	skos:Concept ;
	skos:broader	ccat:2020 ;
	skos:definition	"Spread between an oilseed and its oil or meal/cake."@en ;
	skos:inScheme	ccat: ;
	skos:notation	"202085" ;
	skos:prefLabel	"Crush Spread"@en .

ccat:202090
	a	skos:Concept ;
	skos:broader	ccat:2020 ;
	skos:definition	"Members of a large clade (monophyletic group) of flowering plants making up more than a quarter of all angiosperms with their about 70,000 species."@en ;
	skos:inScheme	ccat: ;
	skos:notation	"202090" ;
	skos:prefLabel	"Other Rosid Seeds"@en .

ccat:20209010
	a	skos:Concept ;
	skos:altLabel	"Egusi"@en ;
	skos:broader	ccat:202090 ;
	skos:closeMatch	agrovoc:c_12487 ;
	skos:definition	"Seed of certain cucurbitaceous plants (squash, melon, gourd)."@en ;
	skos:exactMatch	wd:Q10771593 ;
	skos:inScheme	ccat: ;
	skos:notation	"20209010" ;
	skos:note	"""Authorities disagree whether the word is used more properly for the seeds of the colocynth, those of a particular large-seeded variety of the watermelon, or generically for those of any cucurbitaceous plant. The characteristics and uses of all these seeds are broadly similar. Major egusi-growing nations include Mali, Burkina Faso, Togo, Ghana, Cote d'Ivoire, Benin, Nigeria, and Cameroon.

Species from which egusi is derived include Cucumeropsis mannii and Citrullus lanatus."""@en ;
	skos:prefLabel	"Melonseed"@en .

ccat:20209020
	a	skos:Concept ;
	skos:broader	ccat:202090 ;
	skos:definition	"Seed of a species of perennial flowering plant in the spurge family, Euphorbiaceae."@en ;
	skos:exactMatch	agrovoc:c_18705 , eurovoc:3724 , wd:Q64597240 ;
	skos:inScheme	ccat: ;
	skos:notation	"20209020" ;
	skos:note	"""Castor is indigenous to the southeastern Mediterranean Basin, Eastern Africa, and India, but is widespread throughout tropical regions (and widely grown elsewhere as an ornamental plant).

Castor seed is the source of castor oil, which has a wide variety of uses. The seeds contain between 40% and 60% oil that is rich in triglycerides, mainly ricinolein. The seed also contains ricin, a water-soluble toxin, which is also present in lower concentrations throughout the plant."""@en ;
	skos:prefLabel	"Castor Beans"@en .

ccat:20209030
	a	skos:Concept ;
	skos:broader	ccat:202090 ;
	skos:closeMatch	wd:Q2699247 ;
	skos:definition	"Fruit of Vernicia fordii, usually known as the tung tree, a species of Vernicia in the spurge family."@en ;
	skos:inScheme	ccat: ;
	skos:notation	"20209030" ;
	skos:note	"""The tree is native to southern China, Burma, and northern Vietnam. It is a hard, woody pear-shaped berry 4 to 6 cm long and 3 to 5 cm in diameter, containing four or five large, oily seeds. The tung nut is green initially, becoming dull brown when it is ripe in autumn. Tung oil, or China wood oil, is extracted from the nut.

Global production of the fruit rose from just over 100,000 tonnes in 1970 to almost 200,000 tonnes by 1980. Fruit yields are typically in the range of 4.5 to 5 tonnes per hectare. A number of cultivars have been selected for increased yield and small tree size, including 'Folsom', 'Cahl', 'Isabel', 'La Crosser', and 'Lampton'."""@en ;
	skos:prefLabel	"Tung Nuts"@en .

ccat:20209040
	a	skos:Concept ;
	skos:broader	ccat:202090 ;
	skos:definition	"Small round seeds of various mustard plants, e.g. black mustard (Brassica nigra), brown Indian mustard (B. juncea), or white/yellow mustard (B. hirta/Sinapis alba)."@en ;
	skos:exactMatch	agrovoc:c_fd07a050 , wd:Q1937700 ;
	skos:inScheme	ccat: ;
	skos:notation	"20209040" ;
	skos:note	"""Mustard seeds are a rich source of oil and protein. The seed has oil as high as 46-48%, and whole seed meal has 43.6% protein. Grinding and mixing the seeds with water, vinegar or other liquids creates the yellow condiment known as prepared mustard."""@en ;
	skos:prefLabel	"Mustard Seed"@en .

ccat:20209050
	a	skos:Concept ;
	skos:broader	ccat:202090 ;
	skos:definition	"Seeds of Triadica sebifera as well as Triadica cochinchinensis."@en ;
	skos:exactMatch	wd:Q113005689 ;
	skos:inScheme	ccat: ;
	skos:notation	"20209050" ;
	skos:note	"""Tallowtree is native to eastern China and Taiwan. It is commonly called Chinese tallow, Chinese tallowtree, Florida aspen, chicken tree, gray popcorn tree, or candleberry tree.

It is relevant to biodiesel production because it is the third most productive vegetable oil producing crop in the world, after algae and oil palm. The leaves are used as herbal medicine to treat boils."""@en ;
	skos:prefLabel	"Tallowtree Seeds"@en .

ccat:20209060
	a	skos:Concept ;
	skos:broader	ccat:202090 ;
	skos:definition	"Seed of the flax plant."@en ;
	skos:exactMatch	agrovoc:c_12192 , wd:Q911332 ;
	skos:inScheme	ccat: ;
	skos:notation	"20209060" ;
	skos:note	"""Depending on the sort they are brown or yellow in colour, taste nutty and contain about 40% oil."""@en ;
	skos:prefLabel	"Linseed"@en .

ccat:20209065
	a	skos:Concept ;
	skos:broader	ccat:202090 ;
	skos:definition	"Seed of Cannabis sativa."@en ;
	skos:exactMatch	wd:Q113005802 ;
	skos:inScheme	ccat: ;
	skos:notation	"20209065" ;
	skos:prefLabel	"Hempseed"@en .

ccat:20209070
	a	skos:Concept ;
	skos:broader	ccat:202095 ;
	skos:definition	"Fruit of Ceiba pentandra, a tropical tree of the order Malvales and the family Malvaceae."@en ;
	skos:inScheme	ccat: ;
	skos:notation	"20209070" ;
	skos:note	"""The tree is native to Mexico, Central America and the Caribbean, northern South America, and (as the variety Ceiba pentandra var guineensis) West Africa. A somewhat smaller variety was introduced to South and Southeast Asia, where it is cultivated.

The fruit is famous for its cottonlike seed fibre, known as Java cotton. Its seeds are used to press a vegetable oil. The oil has a yellow colour and a pleasant, mild odour and taste, resembling cottonseed oil. It becomes rancid quickly when exposed to air. Kapok oil is produced in India, Indonesia and Malaysia. The oil has some potential as a biofuel and in paint preparation."""@en ;
	skos:prefLabel	"Kapok Fruit"@en .

ccat:202095
	a	skos:Concept ;
	skos:broader	ccat:2020 ;
	skos:definition	"Members of the largest group of flowering plant with more than 80,000 species, about a third of the total flowering plant species."@en ;
	skos:inScheme	ccat: ;
	skos:notation	"202095" ;
	skos:prefLabel	"Other Asterid Seeds"@en .

ccat:20209510
	a	skos:Concept ;
	skos:broader	ccat:202095 ;
	skos:definition	"Fruit of the sunflower (Helianthus annuus). There are three types of commonly used sunflower seeds: linoleic (most common), high oleic, and sunflower oil seeds."@en ;
	skos:exactMatch	agrovoc:c_25507 , wd:Q1076906 ;
	skos:inScheme	ccat: ;
	skos:notation	"20209510" ;
	skos:note	"""For commercial purposes, sunflower seeds are usually classified by the pattern on their husks. If the husk is solid black, the seeds are called black oil sunflower seeds. The crops may be referred to as oilseed sunflower crops. Striped sunflower seeds are primarily eaten as a snack food; as a result, they may be called confectionery sunflower seeds.

The term \"sunflower seed\" is actually a misnomer when applied to the seed in its pericarp (hull). Botanically speaking, it is a cypsela. When dehulled, the edible remainder is called the sunflower kernel or heart."""@en ;
	skos:prefLabel	"Sunflower Seed"@en .

ccat:20209520
	a	skos:Concept ;
	skos:broader	ccat:202095 ;
	skos:definition	"Fruit of the olive tree, Olea europaea, an evergreen tree or shrub native to Mediterranean Europe, Asia, and Africa."@en ;
	skos:exactMatch	agrovoc:c_12926 , wd:Q1621080 ;
	skos:inScheme	ccat: ;
	skos:notation	"20209520" ;
	skos:note	"""The species is cultivated in all the countries of the Mediterranean, as well as South America, South Africa, China, Australia, New Zealand, Mexico, and the United States. Olea europaea is the type species for the genus Olea."""@en ;
	skos:prefLabel	"Olives"@en .

ccat:20209530
	a	skos:Concept ;
	skos:broader	ccat:202095 ;
	skos:definition	"Safflower seed is the seed of Carthamus tinctorius, a highly branched, herbaceous, thistle-like annual plant in the family Asteraceae."@en ;
	skos:exactMatch	agrovoc:c_25503 , wd:Q104413623 ;
	skos:inScheme	ccat: ;
	skos:notation	"20209530" ;
	skos:note	"""In 2020, global production of safflower seeds was 653,030 tonnes, led by Kazakhstan with 35% of the world total. Other significant producers were Russia and Mexico, with 28% of world production combined."""@en ;
	skos:prefLabel	"Safflower Seed"@en .

ccat:20209535
	a	skos:Concept ;
	skos:broader	ccat:202095 ;
	skos:definition	"Seed of Sesamum indicum."@en ;
	skos:exactMatch	agrovoc:c_14216 , wd:Q12000036 ;
	skos:inScheme	ccat: ;
	skos:notation	"20209535" ;
	skos:note	"""In 2020, world production of sesame seeds was 7 million metric tons (6,900,000 long tons; 7,700,000 short tons), led by Sudan, Myanmar, and Tanzania. The white and other lighter-coloured sesame seeds are common in Europe, the Americas, West Asia, and the Indian subcontinent. The black and darker-coloured sesame seeds are mostly produced in China and Southeast Asia. In the United States most sesame is raised by farmers under contract to Sesaco, which also supplies proprietary seed.

Japan is the world's largest sesame importer. China is the second-largest importer of sesame, mostly oil-grade. China exports lower-priced food-grade sesame seeds, particularly to Southeast Asia. Other major importers are United States, Canada, Netherlands, Turkey, and France."""@en ;
	skos:prefLabel	"Sesame Seed"@en .

ccat:20209540
	a	skos:Concept ;
	skos:altLabel	"Shea Nuts"@en ;
	skos:broader	ccat:202095 ;
	skos:definition	"Seed of Butyrospermum parkii."@en ;
	skos:exactMatch	agrovoc:c_25505 , wd:Q104212650 ;
	skos:inScheme	ccat: ;
	skos:notation	"20209540" ;
	skos:note	"""The tree that can get up to 300 years old. After 20 years it blooms for the first time and carries fruits, after 50 years it will carry an anual yield of about 20 kg of fruits.

Farming and processing the fruit is traditionally done by hand. The falling shea fruits are collected from the savanna ground. They are then separated from the pulp, cleaned, and left out in the sun to dry. After a few days the nuts are cracked open, and the kernels are removed and dried bagain before the fat extraction can begin."""@en ;
	skos:prefLabel	"Karite Nuts"@en .

ccat:202099
	a	skos:Concept ;
	skos:broader	ccat:2020 ;
	skos:definition	"Any other oil seeds"@en ;
	skos:inScheme	ccat: ;
	skos:notation	"202099" ;
	skos:prefLabel	"Other Oilseeds"@en .

ccat:20209910
	a	skos:Concept ;
	skos:broader	ccat:202099 ;
	skos:definition	"Seed obtained from the opium poppy (Papaver somniferum)."@en ;
	skos:exactMatch	agrovoc:c_25498 , wd:Q2007388 ;
	skos:inScheme	ccat: ;
	skos:notation	"20209910" ;
	skos:prefLabel	"Poppy Seed"@en .

ccat:20209920
	a	skos:Concept ;
	skos:altLabel	"Goat Nut"@en ;
	skos:broader	ccat:202099 ;
	skos:closeMatch	wd:Q267749 ;
	skos:definition	"Seed of Simmondsia chinensis."@en ;
	skos:exactMatch	agrovoc:c_11913 ;
	skos:inScheme	ccat: ;
	skos:notation	"20209920" ;
	skos:note	"""The shrub is native to the Southwestern United States. Jojoba is normally harvested by hand because seeds do not all mature in the same time. Yield is around 3.5 t/ha depending on the age of the plantation."""@en ;
	skos:prefLabel	"Jojoba"@en .

ccat:2025
	a	skos:Concept ;
	skos:broader	ccat:20 ;
	skos:definition	"Vegetal oils and fats are extractions from the seed or other parts of fruits. They are mixtures of triglycerides, usually liquid at room temperature, and usually edible."@en ;
	skos:exactMatch	agrovoc:c_8170 , wd:Q4739805 ;
	skos:inScheme	ccat: ;
	skos:notation	"2025" ;
	skos:prefLabel	"Vegetal Oils and Fats"@en .

ccat:202510
	a	skos:Concept ;
	skos:broader	ccat:2025 ;
	skos:definition	"Vegetal oil extracted from the seeds of the soybean (Glycine max)."@en ;
	skos:exactMatch	agrovoc:c_16508 , wd:Q926892 ;
	skos:inScheme	ccat: ;
	skos:notation	"202510" ;
	skos:prefLabel	"Oil of Soybeans"@en .

ccat:202520
	a	skos:Concept ;
	skos:broader	ccat:2025 ;
	skos:definition	"Vegetal oil derived from a variety of rapeseed."@en ;
	skos:exactMatch	agrovoc:c_24939 ;
	skos:inScheme	ccat: ;
	skos:narrowMatch	wd:Q697248 , wd:Q98841400 ;
	skos:notation	"202520" ;
	skos:note	"The oil's specific gravity varies between 0.9/12 and 0.920. The cake left after extraction of the oil is a valuable feed ingredient for pigs."@en ;
	skos:prefLabel	"Oil of Rapeseed"@en .

ccat:202530
	a	skos:Concept ;
	skos:altLabel	"CPO"@en , "Crude Palm Oil"@en ;
	skos:broader	ccat:2025 ;
	skos:definition	"Vegetal oil derived from the mesocarp (reddish pulp) of the fruit of the oil palms."@en ;
	skos:exactMatch	agrovoc:c_5514 , stw:18077-3 , wd:Q231458 ;
	skos:inScheme	ccat: ;
	skos:notation	"202530" ;
	skos:prefLabel	"Oil of Palm"@en .

ccat:202531
	a	skos:Concept ;
	skos:broader	ccat:2025 ;
	skos:definition	"Crude palm oil that has undergone some or all processes of refinement (neutralisation, bleaching, dewaxing, deodourising, fractionation, degumming). The PORAM standard specifies qualities and properties."@en ;
	skos:inScheme	ccat: ;
	skos:notation	"202531" ;
	skos:prefLabel	"Processed Oil of Palm"@en .

ccat:20253110
	a	skos:Concept ;
	skos:broader	ccat:202531 ;
	skos:definition	"Liquid fraction of crude palm oil that is then bleached, degummed, and deodourised."@en ;
	skos:inScheme	ccat: ;
	skos:notation	"20253110" ;
	skos:prefLabel	"RBD Palm Olein"@en .

ccat:20253120
	a	skos:Concept ;
	skos:broader	ccat:202531 ;
	skos:definition	"Solid fraction of palm oil that is produced by partial crystallisation at controlled temperature."@en ;
	skos:inScheme	ccat: ;
	skos:notation	"20253120" ;
	skos:prefLabel	"Palm Stearin"@en .

ccat:20253130
	a	skos:Concept ;
	skos:broader	ccat:202531 ;
	skos:definition	"By-product of neutralising crude palm oil."@en ;
	skos:inScheme	ccat: ;
	skos:notation	"20253130" ;
	skos:prefLabel	"Palm Acid Oil"@en .

ccat:20253135
	a	skos:Concept ;
	skos:altLabel	"PFAD"@en ;
	skos:broader	ccat:202531 ;
	skos:definition	"Fatty acids removed from CPO during RBD production."@en ;
	skos:inScheme	ccat: ;
	skos:notation	"20253135" ;
	skos:prefLabel	"Palm Fatty Acid Distillate"@en .

ccat:202532
	a	skos:Concept ;
	skos:altLabel	"CPKO"@en ;
	skos:broader	ccat:2025 ;
	skos:definition	"Oil derived from the kernel of the fruit of oil palms."@en ;
	skos:exactMatch	agrovoc:c_5515 , wd:Q1960534 ;
	skos:inScheme	ccat: ;
	skos:notation	"202532" ;
	skos:prefLabel	"Oil of Palm Kernel"@en .

ccat:202533
	a	skos:Concept ;
	skos:broader	ccat:2025 ;
	skos:definition	"Crude palm kernel oil that has undergone some or all processes of refinement (neutralisation, bleaching, dewaxing, deodourising, fractionation, degumming). The PORAM standard specifies qualities and properties."@en ;
	skos:inScheme	ccat: ;
	skos:notation	"202533" ;
	skos:prefLabel	"Processed Oil of Palm Kernel"@en .

ccat:20253310
	a	skos:Concept ;
	skos:altLabel	"RBDPKO"@en ;
	skos:broader	ccat:202531 ;
	skos:definition	"Liquid fraction of crude palm kernel oil that is then bleached, degummed, and deodourised."@en ;
	skos:inScheme	ccat: ;
	skos:notation	"20253310" ;
	skos:prefLabel	"RBD Palm Kernel Oil"@en .

ccat:20253320
	a	skos:Concept ;
	skos:broader	ccat:202531 ;
	skos:definition	"Solid fraction of palm kernel oil that is produced by partial crystallisation at controlled temperature."@en ;
	skos:inScheme	ccat: ;
	skos:notation	"20253320" ;
	skos:prefLabel	"Palm Kernel Stearin"@en .

ccat:20253330
	a	skos:Concept ;
	skos:broader	ccat:202531 ;
	skos:definition	"By-product of neutralising crude palm kernel oil."@en ;
	skos:inScheme	ccat: ;
	skos:notation	"20253330" ;
	skos:prefLabel	"Palm Kernel Acid Oil"@en .

ccat:20253335
	a	skos:Concept ;
	skos:altLabel	"PKFAD"@en ;
	skos:broader	ccat:202531 ;
	skos:definition	"Fatty acids removed from CPKO during RBDPKO production."@en ;
	skos:inScheme	ccat: ;
	skos:notation	"20253335" ;
	skos:prefLabel	"Palm Kernel Fatty Acid Distillate"@en .

ccat:202535
	a	skos:Concept ;
	skos:altLabel	"Oil of Copra"@en ;
	skos:broader	ccat:2025 ;
	skos:closeMatch	<https://www.trade-tariff.service.gov.uk/commodities/1513110000> , <https://www.trade-tariff.service.gov.uk/commodities/1513190000> ;
	skos:definition	"Oil extracted from the kernel or meat of mature coconuts."@en ;
	skos:exactMatch	agrovoc:c_1714 , wd:Q216235 ;
	skos:inScheme	ccat: ;
	skos:notation	"202535" ;
	skos:prefLabel	"Oil of Coconuts"@en .

ccat:202540
	a	skos:Concept ;
	skos:broader	ccat:2025 ;
	skos:definition	"Oil from the seeds of cotton plants of various species, mainly Gossypium hirsutum and Gossypium herbaceum."@en ;
	skos:exactMatch	agrovoc:c_25474 , wd:Q811663 ;
	skos:inScheme	ccat: ;
	skos:notation	"202540" ;
	skos:prefLabel	"Oil of Cottonseed"@en .

ccat:202550
	a	skos:Concept ;
	skos:broader	ccat:2025 ;
	skos:definition	"Vegetal oil derived from groundnuts."@en ;
	skos:exactMatch	agrovoc:c_25477 , eurovoc:1263 , wd:Q265878 ;
	skos:inScheme	ccat: ;
	skos:notation	"202550" ;
	skos:prefLabel	"Oil of Groundnuts"@en .

ccat:202590
	a	skos:Concept ;
	skos:broader	ccat:2025 ;
	skos:definition	"Oil of oil seeds of the rosid clade"@en ;
	skos:inScheme	ccat: ;
	skos:notation	"202590" ;
	skos:prefLabel	"Other Rosid Oils"@en .

ccat:20259010
	a	skos:Concept ;
	skos:altLabel	"Ootanga Oil"@en ;
	skos:broader	ccat:202590 ;
	skos:closeMatch	wd:Q3819066 ;
	skos:definition	"Oil extracted by pressing the seeds of the Citrullus lanatus (watermelon)."@en ;
	skos:exactMatch	agrovoc:c_66bba3ad ;
	skos:inScheme	ccat: ;
	skos:notation	"20259010" ;
	skos:prefLabel	"Melon Seed Oil"@en .

ccat:20259020
	a	skos:Concept ;
	skos:broader	ccat:202590 ;
	skos:definition	"Vegetal oil pressed from castor beans."@en ;
	skos:exactMatch	agrovoc:c_25466 , wd:Q337492 ;
	skos:inScheme	ccat: ;
	skos:notation	"20259020" ;
	skos:note	"""Castor oil and its derivatives are used in the manufacturing of soaps, lubricants, hydraulic and brake fluids, paints, dyes, coatings, inks, cold-resistant plastics, waxes and polishes, nylon, and perfumes."""@en ;
	skos:prefLabel	"Oil of Castor Beans"@en .

ccat:20259025
	a	skos:Concept ;
	skos:broader	ccat:202590 ;
	skos:definition	"Oil made from castor oil by hydrogenation. The process saturates the alkenes, giving a waxy lubricant."@en ;
	skos:inScheme	ccat: ;
	skos:notation	"20259025" ;
	skos:prefLabel	"Hydrogenated Castor Oil"@en .

ccat:20259030
	a	skos:Concept ;
	skos:altLabel	"China wood oil"@en ;
	skos:broader	ccat:202590 ;
	skos:definition	"Oil obtained by pressing the seed from the nut of the tung tree (Vernicia fordii)."@en ;
	skos:exactMatch	agrovoc:c_8005 , wd:Q2094522 ;
	skos:inScheme	ccat: ;
	skos:notation	"20259030" ;
	skos:note	"""Tung oil hardens upon exposure to air (through polymerization), and the resulting coating is transparent and has a deep, almost wet look. Used mostly for finishing and protecting wood, after numerous coats, the finish can even look plastic-like. Related drying oils include linseed, safflower, poppy, and soybean oils."""@en ;
	skos:prefLabel	"Oil of Tung Nuts"@en .

ccat:20259040
	a	skos:Concept ;
	skos:broader	ccat:202590 ;
	skos:definition	"Oil pressed from mustard seeds. Sale is restricted in some countries due to high levels of erucic acid."@en ;
	skos:exactMatch	agrovoc:c_36137 , wd:Q910958 ;
	skos:inScheme	ccat: ;
	skos:notation	"20259040" ;
	skos:note	"""Oil makes up about 30% of the mustard seeds. It can be produced from black mustard (Brassica nigra), brown Indian mustard (B. juncea), and white mustard (B. hirta).

Mustard oil has about 60% monounsaturated fatty acids (42% erucic acid and 12% oleic acid); it has about 21% polyunsaturated fats (6% the omega-3 alpha-linolenic acid and 15% the omega-6 linoleic acid), and it has about 12% saturated fats."""@en ;
	skos:prefLabel	"Oil of Mustard Seed"@en .

ccat:20259050
	a	skos:Concept ;
	skos:altLabel	"Chinese Vegetable Tallow"@en ;
	skos:broader	ccat:202590 ;
	skos:definition	"Fatty substance extracted from the coat of the seeds of Triadica sebifera (Chinese tallow tree) or Triadica cochinchinensis (Mountain tallow tree)."@en ;
	skos:exactMatch	wd:Q102347788 ;
	skos:inScheme	ccat: ;
	skos:notation	"20259050" ;
	skos:note	"""Stillingia tallow is essentially a mixture of triglycerides (esters of glycerol and fatty acids). The main triglycerides are glicerotriyl tripalmitate (5-30%) and 2-oleate,1,3-dipalmitate (~70%)."""@en ;
	skos:prefLabel	"Stillingia Tallow"@en .

ccat:20259052
	a	skos:Concept ;
	skos:broader	ccat:202590 ;
	skos:definition	"Oil extracted (by solvents) from the seeds of plants of the Triadica genus such as Triadica sebifera (Chinese tallow tree) and Triadica cochinchinensis (Mountain tallow tree)."@en ;
	skos:exactMatch	wd:Q3142827 ;
	skos:inScheme	ccat: ;
	skos:notation	"20259052" ;
	skos:note	"""It is a drying oil used in paints and varnishes, and it is believed to be toxic in China. Stillingia oil is different from stillingia tallow, a fatty substance that surround the seeds in the fruit, which is removed before extracting the oil.

Stillingia oil has a typical drying time of 4-6 hours. The seeds produce 20-30% w/w of tallow fat and 10-17% w/w of stillingia oil. It has iodine number 127, a saponification value of 206, and a thiocyanogen value of 100.7."""@en ;
	skos:prefLabel	"Stillingia Oil"@en .

ccat:20259060
	a	skos:Concept ;
	skos:broader	ccat:202590 ;
	skos:definition	"Oil obtained from the dried, ripened seeds of the flax plant (Linum usitatissimum) by pressing, sometimes followed by solvent extraction."@en ;
	skos:exactMatch	agrovoc:c_4353 , wd:Q818405 ;
	skos:inScheme	ccat: ;
	skos:notation	"20259060" ;
	skos:prefLabel	"Oil of Linseed"@en .

ccat:20259065
	a	skos:Concept ;
	skos:broader	ccat:202590 ;
	skos:definition	"Oil obtained by pressing hemp seeds."@en ;
	skos:exactMatch	wd:Q1575477 ;
	skos:inScheme	ccat: ;
	skos:notation	"20259065" ;
	skos:note	"""The oil has a 3:1 ratio of omega-6 to omega-3 essential fatty acids. It may also be used as a feedstock for the large-scale production of biodiesel.

About 49% of the weight of hempseed is an edible oil that contains 76% as polyunsaturated fat, including omega-6 fatty acids such as linoleic acid (LA, 54%) and gamma-linolenic acid (GLA, 3%), and omega-3 fatty acids such as alpha-linolenic acid (ALA, 17%) and stearidonic acid (2%). Both LA and ALA are essential fatty acids. In addition, hempseed oil contains 5% to 11% monounsaturated fat and 5% to 7% saturated fat. In common with other oils and fats, hemp seed oil provides 9 kcal/g."""@en ;
	skos:prefLabel	"Oil of Hempseed"@en .

ccat:20259070
	a	skos:Concept ;
	skos:broader	ccat:202595 ;
	skos:definition	"Vegetal oil extracted from kapok seeds by pressing."@en ;
	skos:inScheme	ccat: ;
	skos:notation	"20259070" ;
	skos:prefLabel	"Oil of Kapok"@en .

ccat:202595
	a	skos:Concept ;
	skos:broader	ccat:2025 ;
	skos:definition	"Oil of oil seeds of the asterid clade."@en ;
	skos:inScheme	ccat: ;
	skos:notation	"202595" ;
	skos:prefLabel	"Other Asterid Oils"@en .

ccat:20259510
	a	skos:Concept ;
	skos:broader	ccat:202595 ;
	skos:definition	"Oil pressed from the seeds of sunflower (Helianthus annuus)."@en ;
	skos:exactMatch	agrovoc:c_25506 , wd:Q94787 ;
	skos:inScheme	ccat: ;
	skos:notation	"20259510" ;
	skos:note	"""Sunflower oil is primarily composed of linoleic acid, a polyunsaturated fat, and oleic acid, a monounsaturated fat. Through selective breeding and manufacturing processes, oils of differing proportions of the fatty acids are produced. The expressed oil has a neutral taste profile. The oil contains a large amount of vitamin E.

As of 2017, genome analysis and development of hybrid sunflowers to increase oil production are under development to meet greater consumer demand for sunflower oil and its commercial varieties.

Ukraine and Russia together accounted for 53% of the world's production of sunflower oil in 2018."""@en ;
	skos:prefLabel	"Oil of Sunflower"@en .

ccat:20259520
	a	skos:Concept ;
	skos:broader	ccat:202595 ;
	skos:definition	"Oil obtained from olives (the fruit of Olea europaea; family Oleaceae) produced by pressing whole olives."@en ;
	skos:exactMatch	agrovoc:c_25491 , eurovoc:1264 , stw:14960-4 , wd:Q93165 ;
	skos:inScheme	ccat: ;
	skos:notation	"20259520" ;
	skos:note	"""The top five producers of olive oil by volume are Spain, Italy, Tunisia, Greece and Turkey. Per capita consumption is highest in Greece, followed by Italy and Spain.

The composition of olive oil varies with the cultivar, altitude, time of harvest and extraction process. It consists mainly of oleic acid (up to 83%), with smaller amounts of other fatty acids including linoleic acid (up to 21%) and palmitic acid (up to 20%). Extra virgin olive oil is required to have no more than 0.8% free acidity and is considered to have favorable flavor characteristics."""@en ;
	skos:prefLabel	"Virgin Oil of Olives"@en .

ccat:20259525
	a	skos:Concept ;
	skos:broader	ccat:202595 ;
	skos:definition	"Oil made from the olive cake left after the virgin pressing."@en ;
	skos:inScheme	ccat: ;
	skos:notation	"20259525" ;
	skos:prefLabel	"Oil of Olive Cake"@en .

ccat:20259530
	a	skos:Concept ;
	skos:broader	ccat:202595 ;
	skos:definition	"Oil made from the achenes of safflower by either cold pressing the seeds (for a cooking oil) or hot pressing the seeds yields (for an industrial oil)."@en ;
	skos:exactMatch	agrovoc:c_25502 , wd:Q441113 ;
	skos:inScheme	ccat: ;
	skos:notation	"20259530" ;
	skos:prefLabel	"Oil of Safflower Seed"@en .

ccat:20259535
	a	skos:Concept ;
	skos:broader	ccat:202595 ;
	skos:definition	"Oil derived from sesame seeds."@en ;
	skos:exactMatch	agrovoc:c_25504 ;
	skos:inScheme	ccat: ;
	skos:notation	"20259535" ;
	skos:note	"""Industrial uses include solvents in injected drugs, as a carrier oil in cosmetics, or as a coating for stored grains to prevent weevil attacks."""@en ;
	skos:prefLabel	"Oil of Sesame Seed"@en .

ccat:20259540
	a	skos:Concept ;
	skos:altLabel	"Shea Butter"@en ;
	skos:broader	ccat:202595 ;
	skos:definition	"Fat extracted from the nut of the African shea tree (Vitellaria paradoxa)."@en ;
	skos:exactMatch	agrovoc:c_37951 ;
	skos:inScheme	ccat: ;
	skos:notation	"20259540" ;
	skos:note	"""The primary export market for shea butter is in the chocolate and confectionery industry. However, shea is also used as a cooking fat, food accompaniment and skin-care product in West Africa."""@en ;
	skos:prefLabel	"Butter of Karite Nuts"@en .

ccat:20259550
	a	skos:Concept ;
	skos:broader	ccat:202595 ;
	skos:definition	"Oil extracted from the leaves of the Mentha plant."@en ;
	skos:inScheme	ccat: ;
	skos:notation	"20259550" ;
	skos:prefLabel	"Oil of Mentha"@en .

ccat:202599
	a	skos:Concept ;
	skos:broader	ccat:2025 ;
	skos:definition	"Any other vegetal oils."@en ;
	skos:inScheme	ccat: ;
	skos:notation	"202599" ;
	skos:prefLabel	"Other Vegetal Oils"@en .

ccat:20259910
	a	skos:Concept ;
	skos:broader	ccat:202599 ;
	skos:definition	"Oil extracted from poppy seeds (specifically seeds of Papaver somniferum, the opium poppy)."@en ;
	skos:exactMatch	agrovoc:c_d5fc3c98 , wd:Q1757003 ;
	skos:inScheme	ccat: ;
	skos:notation	"20259910" ;
	skos:note	"""Poppy seeds yield 45-50% oil. Compared to other vegetable oils, poppyseed oil has a moderate amount of phytosterols: higher than soybean oil and peanut oil, lower than safflower oil, sesame oil, wheat germ oil, corn oil, and rice bran oil. It has little or no odor and a pleasant taste, and it is less likely than some other oils to become rancid."""@en ;
	skos:prefLabel	"Oil of Poppy Seed"@en .

ccat:20259920
	a	skos:Concept ;
	skos:broader	ccat:202599 ;
	skos:definition	"Oil extracted from Jojoba seeds."@en ;
	skos:inScheme	ccat: ;
	skos:notation	"20259920" ;
	skos:prefLabel	"Jojoba Oil"@en .

ccat:20259980
	a	skos:Concept ;
	skos:broader	ccat:202599 ;
	skos:definition	"Oil extracted from the hard outer brown layer of rice called chaff (rice husk)."@en ;
	skos:inScheme	ccat: ;
	skos:notation	"20259980" ;
	skos:prefLabel	"Oil of Rice Bran"@en .

ccat:20259981
	a	skos:Concept ;
	skos:altLabel	"Corn Oil"@en ;
	skos:broader	ccat:202599 ;
	skos:definition	"Oil extracted from the germ of maize."@en ;
	skos:inScheme	ccat: ;
	skos:notation	"20259981" ;
	skos:prefLabel	"Oil of Maize"@en .

ccat:2026
	a	skos:Concept ;
	skos:broader	ccat:20 ;
	skos:definition	"Vegetal cakes are made of the residue left after oil extraction. Meal is produced when the cakes are treated hydrothermally."@en ;
	skos:inScheme	ccat: ;
	skos:notation	"2026" ;
	skos:prefLabel	"Vegetal Cakes and Meals"@en .

ccat:202610
	a	skos:Concept ;
	skos:broader	ccat:2026 ;
	skos:definition	"Residue of soybean oil extraction."@en ;
	skos:exactMatch	agrovoc:c_16043 , wd:Q364900 ;
	skos:inScheme	ccat: ;
	skos:notation	"202610" ;
	skos:note	"""Typically 1 bushel (i.e. 60 lbs. or 27.2 kg) of soybeans yields 48 lbs. (21.8 kg) of soybean meal. Some, but not all, soybean meal is produced from the residue left after oil extraction. Removal of the oil, which is used mostly in food, but also for industrial oils, soaps and biodiesel, involves crushing and either pressing or solvent extraction. Some, but not all, soybean meal contains ground soybean hulls. Soybean meal is heat-treated during production, to denature the trypsin inhibitors of soybeans, which would otherwise interfere with protein digestion."""@en ;
	skos:prefLabel	"Cake and Meal of Soybeans"@en .

ccat:202620
	a	skos:Concept ;
	skos:broader	ccat:2026 ;
	skos:definition	"Residue of rapeseed oil extraction."@en ;
	skos:exactMatch	agrovoc:c_16027 , wd:Q113010548 ;
	skos:inScheme	ccat: ;
	skos:notation	"202620" ;
	skos:prefLabel	"Cake and Meal of Rapeseed"@en .

ccat:202630
	a	skos:Concept ;
	skos:broader	ccat:2026 ;
	skos:definition	"Residue of palm oil extraction."@en ;
	skos:inScheme	ccat: ;
	skos:notation	"202630" ;
	skos:prefLabel	"Palm Cake and Palm Meal"@en .

ccat:202632
	a	skos:Concept ;
	skos:altLabel	"PKC"@en , "PKM"@en ;
	skos:broader	ccat:2026 ;
	skos:definition	"Main by-product of the palm kernel oil extraction."@en ;
	skos:exactMatch	agrovoc:c_36344 , wd:Q110583134 ;
	skos:inScheme	ccat: ;
	skos:notation	"202632" ;
	skos:note	""" It is a highly fibrous and medium grade protein feed, hence most suited to ruminant or rabbit feeding (Pickard, 2005). Palm kernel resulting from mechanical extraction contains 5-12% oil and solvent-extracted palm kernel meal contains 0.5-3% oil (Chin, 2001)."""@en ;
	skos:prefLabel	"Cake and Meal of Palm Kernel"@en .

ccat:202640
	a	skos:Concept ;
	skos:broader	ccat:2026 ;
	skos:definition	"Residue of cottonseed after oil extraction."@en ;
	skos:exactMatch	agrovoc:c_35678 , wd:Q5175773 ;
	skos:inScheme	ccat: ;
	skos:notation	"202640" ;
	skos:prefLabel	"Cake and Meal of Cottonseed"@en .

ccat:202690
	a	skos:Concept ;
	skos:broader	ccat:2026 ;
	skos:definition	"Cake and meals of oil seeds of the rosid clade"@en ;
	skos:inScheme	ccat: ;
	skos:notation	"202690" ;
	skos:prefLabel	"Other Cake and Meal of Rosids"@en .

ccat:20269040
	a	skos:Concept ;
	skos:broader	ccat:202690 ;
	skos:definition	"Residue of mustard seeds after oil extraction."@en ;
	skos:inScheme	ccat: ;
	skos:notation	"20269040" ;
	skos:prefLabel	"Cake and Meal of Mustard Seed"@en .

ccat:2030
	a	skos:Concept ;
	skos:broader	ccat:20 ;
	skos:definition	"Crops that yield sweet-tasting soluble carbohydrates or substances that when added to food or drink impart the flavour of sweetness."@en ;
	skos:inScheme	ccat: ;
	skos:notation	"2030" ;
	skos:note	"""There are two major sugar crops: sugar beets and sugar cane. However, sugar and syrups are also produced from the sap of certain species of maple trees, from sweet sorghum when cultivated explicitly for making syrup and from sugar palm. Sugar beets that are cultivated solely as a fodder crop and red or garden beets that are classified as vegetable crops are excluded from the FAO list of sugar crops.

Sugar cane is a perennial grass (replanted at intervals using pieces of the cane stalks) that is cultivated mainly in the tropics. Sugar beet is an annual crop that is propagated by the seeds of the flowers. It is cultivated in cooler climates than sugar cane, mainly above the 35th parallel of the Northern Hemisphere.

Both sugar beets and sugar cane have a high water content, accounting for about 75 percent of the total weight of the plants. The sugar content of sugar cane ranges from 10 to 15 percent of the total weight, while that of sugar beets is between 13 and 18 percent. The protein and fat content of both beets and cane is almost nil.

Production data on sugar beets and sugar cane relate to the harvested crop, free of soil, plant tops and leaves.

FAO lists three primary sugar crops.

Under the name SWEETENERS, FAO includes products used for sweetening that are derived from sugar crops, cereals, fruits or milk, or that are produced by insects. This category includes a wide variety of monosaccharides (glucose and fructose) and disaccharides (sucrose and saccharose). They exist either in a crystallized state as sugar, or in thick liquid form as syrups.

The traditional sources of sugar are sugar cane and sugar beets. But in recent years, ever larger quantities of cereals (mainly maize) have been used to produce sweeteners derived from starch.

OTHER DERIVED PRODUCTS. In addition to sugar, molasses is also obtained with various degrees of sugar content. The by-product obtained from the extraction of sugar is called bagasse in the case of sugar cane, and beet pulp in the case of sugar beets."""@en ;
	skos:prefLabel	"Sugar Crops and Vegetal Sweeteners"@en .

ccat:203010
	a	skos:Concept ;
	skos:broader	ccat:2030 ;
	skos:definition	"Uncut and unshredded sugar canes suitable for milling."@en ;
	skos:exactMatch	agrovoc:c_7501 , wd:Q36940 ;
	skos:inScheme	ccat: ;
	skos:notation	"203010" ;
	skos:prefLabel	"Sugar Cane"@en .

ccat:20301010
	a	skos:Concept ;
	skos:broader	ccat:203010 ;
	skos:definition	"A non-refined, crystallized material derived from the juices of sugar-cane stalk and consisting either wholly or essentially of sucrose."@en ;
	skos:exactMatch	agrovoc:c_16477 , wd:Q487233 ;
	skos:inScheme	ccat: ;
	skos:notation	"20301010" ;
	skos:prefLabel	"Cane Sugar"@en .

ccat:203020
	a	skos:Concept ;
	skos:broader	ccat:2030 ;
	skos:definition	"Unsliced, unwashed sugar beets suitable for diffusion."@en ;
	skos:exactMatch	agrovoc:c_7499 , wd:Q151964 ;
	skos:inScheme	ccat: ;
	skos:notation	"203020" ;
	skos:prefLabel	"Sugar Beet"@en .

ccat:20302010
	a	skos:Concept ;
	skos:broader	ccat:203020 ;
	skos:definition	"A non-refined, crystallized material derived from the juices extracted from the root of the sugar beet and consisting either wholly or essentially of sucrose."@en ;
	skos:exactMatch	agrovoc:c_16474 , wd:Q9197055 ;
	skos:inScheme	ccat: ;
	skos:notation	"20302010" ;
	skos:prefLabel	"Beet Sugar"@en .

ccat:203030
	a	skos:Concept ;
	skos:broader	ccat:2030 ;
	skos:definition	"Includes minor sugar crops of local importance. In the case of saps, production is to be expressed in liquid equivalent."@en ;
	skos:inScheme	ccat: ;
	skos:notation	"203030" ;
	skos:prefLabel	"Other Sugar Crops"@en .

ccat:203040
	a	skos:Concept ;
	skos:broader	ccat:20301010 , ccat:20302010 ;
	skos:definition	"Sugar derived from sugar cane through traditional methods without centrifugation."@en ;
	skos:inScheme	ccat: ;
	skos:notation	"203040" ;
	skos:prefLabel	"Non-Centrifugal Sugar"@en .

ccat:203050
	a	skos:Concept ;
	skos:broader	ccat:20301010 , ccat:20302010 ;
	skos:definition	"Cane sugar or beet sugar processed by centrifuges.  Processed further it is called Refined Sugar."@en ;
	skos:inScheme	ccat: ;
	skos:notation	"203050" ;
	skos:prefLabel	"Raw Centrifugal Sugar"@en .

ccat:20305010
	a	skos:Concept ;
	skos:broader	ccat:203050 ;
	skos:definition	"Centrifugal sugar where molasses have been removed, 99.7% or higher purity."@en ;
	skos:inScheme	ccat: ;
	skos:notation	"20305010" ;
	skos:prefLabel	"Refined Sugar"@en .

ccat:20305020
	a	skos:Concept ;
	skos:broader	ccat:203050 ;
	skos:definition	"Residual molasses after refining sugar cane or beets."@en ;
	skos:inScheme	ccat: ;
	skos:notation	"20305020" ;
	skos:note	"""A by-product of the extraction or refining of beet or cane sugar or of the production of fructose from maize. Used for feed, food, industrial alcohol, alcoholic beverages and ethanol."""@en ;
	skos:prefLabel	"Molasses"@en .

ccat:203060
	a	skos:Concept ;
	skos:broader	ccat:2030 ;
	skos:definition	"Natural sweetener and sugar substitute derived from the leaves of the plant species Stevia rebaudiana."@en ;
	skos:inScheme	ccat: ;
	skos:notation	"203060" ;
	skos:prefLabel	"Stevia"@en .

ccat:2035
	a	skos:Concept ;
	skos:broader	ccat:20 ;
	skos:definition	"Most generally, polysaccharides of vegetal origin. Specifically starches from seeds, roots and tubers, or gums in the woody elements of plants or in seed coatings."@en ;
	skos:inScheme	ccat: ;
	skos:notation	"2035" ;
	skos:prefLabel	"Starches, Gums, and Polysaccharides"@en .

ccat:203510
	a	skos:Concept ;
	skos:altLabel	"Cornflour"@en ;
	skos:broader	ccat:2035 ;
	skos:definition	"Starch from the endosperm of maize kernels."@en ;
	skos:inScheme	ccat: ;
	skos:notation	"203510" ;
	skos:prefLabel	"Corn Starch"@en .

ccat:203520
	a	skos:Concept ;
	skos:broader	ccat:2035 ;
	skos:definition	"Starch extracted from crushed potatoes."@en ;
	skos:inScheme	ccat: ;
	skos:notation	"203520" ;
	skos:prefLabel	"Potatoe Starch"@en .

ccat:203530
	a	skos:Concept ;
	skos:broader	ccat:2035 ;
	skos:definition	"Germinated cereal grain that has been dried (a process known as \"malting\")."@en ;
	skos:inScheme	ccat: ;
	skos:notation	"203530" ;
	skos:prefLabel	"Malt"@en .

ccat:203540
	a	skos:Concept ;
	skos:broader	ccat:2035 ;
	skos:definition	"Starch extracted from the roots of the cassava plant (manioc)."@en ;
	skos:inScheme	ccat: ;
	skos:notation	"203540" ;
	skos:prefLabel	"Tapioca"@en .

ccat:203550
	a	skos:Concept ;
	skos:broader	ccat:2035 ;
	skos:definition	"Seed of Guar (Cyamopsis tetragonoloba), an annual legume."@en ;
	skos:exactMatch	wd:Q264770 ;
	skos:inScheme	ccat: ;
	skos:notation	"203550" ;
	skos:note	"""Guar has many functions for human and animal nutrition, but the gelling agent in its seeds (guar gum) is the most important use. Demand is rising due to the use of guar gum in hydraulic fracturing (oil shale gas). About 80% of world production occurs in India, but due to strong demand, the plant is being introduced elsewhere."""@en ;
	skos:prefLabel	"Guar Beans"@en .

ccat:203555
	a	skos:Concept ;
	skos:broader	ccat:2035 ;
	skos:definition	"Galactomannan polysaccharide extracted from guar beans by mechanically dehusking, hydrating, and milling."@en ;
	skos:inScheme	ccat: ;
	skos:notation	"203555" ;
	skos:prefLabel	"Guar Gum"@en .

ccat:203557
	a	skos:Concept ;
	skos:broader	ccat:2035 ;
	skos:definition	"Residue of Guar gum extraction from the Guar bean."@en ;
	skos:inScheme	ccat: ;
	skos:notation	"203557" ;
	skos:prefLabel	"Guar Meal"@en .

ccat:203560
	a	skos:Concept ;
	skos:broader	ccat:2035 ;
	skos:definition	"Dried exudate from the trunks and branches of Acacia senegal or Vachellia (Acacia) seyal in the family Fabaceae (Leguminosae)."@en ;
	skos:inScheme	ccat: ;
	skos:notation	"203560" ;
	skos:prefLabel	"Arabic Gum"@en .

ccat:2040
	a	skos:Concept ;
	skos:broader	ccat:20 ;
	skos:closeMatch	agrovoc:c_6651 , agrovoc:c_7998 ;
	skos:definition	"Parts of the plants whose main economic value is in their anchorage or storage organs, roots or tubers, respectively."@en ;
	skos:inScheme	ccat: ;
	skos:notation	"2040" ;
	skos:prefLabel	"Roots and Tubers"@en .

ccat:204010
	a	skos:Concept ;
	skos:broader	ccat:2040 ;
	skos:definition	"Starchy tuber of the plant Solanum tuberosum."@en ;
	skos:exactMatch	agrovoc:c_13551 , stw:14092-6 ;
	skos:inScheme	ccat: ;
	skos:notation	"204010" ;
	skos:note	"""The importance of the potato as a food source and culinary ingredient varies by region and is still changing. It remains an essential crop in Europe, especially Northern and Eastern Europe, where per capita production is still the highest in the world, while the most rapid expansion in production over the past few decades has occurred in southern and eastern Asia, with China and India leading the world in overall production as of 2018."""@en ;
	skos:prefLabel	"Potatoes"@en .

ccat:204015
	a	skos:Concept ;
	skos:broader	ccat:2040 ;
	skos:definition	"Starchy tubers or Ipomoea batatas from the bindweed or morning glory family, Convolvulaceae."@en ;
	skos:exactMatch	agrovoc:c_14729 ;
	skos:inScheme	ccat: ;
	skos:notation	"204015" ;
	skos:prefLabel	"Sweet Potatoes"@en .

ccat:204020
	a	skos:Concept ;
	skos:broader	ccat:2040 ;
	skos:definition	"Starchy tubers of plant species in the genus Dioscorea that form edible tubers."@en ;
	skos:inScheme	ccat: ;
	skos:notation	"204020" ;
	skos:prefLabel	"Yams"@en .

ccat:204030
	a	skos:Concept ;
	skos:altLabel	"Manioc"@en ;
	skos:broader	ccat:2040 ;
	skos:definition	"""Starchy tubers of Manihot esculenta."""@en ;
	skos:inScheme	ccat: ;
	skos:notation	"204030" ;
	skos:prefLabel	"Cassava"@en .

ccat:204040
	a	skos:Concept ;
	skos:broader	ccat:2040 ;
	skos:definition	"Starchy corms of Colocasia esculenta."@en ;
	skos:inScheme	ccat: ;
	skos:notation	"204040" ;
	skos:prefLabel	"Taro"@en .

ccat:204045
	a	skos:Concept ;
	skos:broader	ccat:2040 ;
	skos:definition	"Starchy corms of several plant species in the genus Xanthosoma."@en ;
	skos:inScheme	ccat: ;
	skos:notation	"204045" ;
	skos:note	"""The genus is native to tropical America but widely cultivated and naturalized in other tropical regions."""@en ;
	skos:prefLabel	"Yautia"@en .

ccat:204050
	a	skos:Concept ;
	skos:broader	ccat:2040 ;
	skos:definition	"Roots of Cichorium intybus."@en ;
	skos:inScheme	ccat: ;
	skos:notation	"204050" ;
	skos:prefLabel	"Chicory Roots"@en .

ccat:204090
	a	skos:Concept ;
	skos:broader	ccat:2040 ;
	skos:definition	"Any other roots or tubers."@en ;
	skos:inScheme	ccat: ;
	skos:notation	"204090" ;
	skos:prefLabel	"Other Roots or Tubers"@en .

ccat:2045
	a	skos:Concept ;
	skos:broader	ccat:20 ;
	skos:definition	"Fruits or seeds of plants in the family Fabaceae (or Leguminosae). Either fresh (legumes) or dried (pulses)."@en ;
	skos:exactMatch	agrovoc:c_4255 ;
	skos:inScheme	ccat: ;
	skos:notation	"2045" ;
	skos:prefLabel	"Legumes and Pulses"@en .

ccat:204510
	a	skos:Concept ;
	skos:altLabel	"Bengal Gram"@en , "Chana"@en ;
	skos:broader	ccat:2045 ;
	skos:definition	"Seed of annual legume Cicer arietinum."@en ;
	skos:exactMatch	agrovoc:c_9785 ;
	skos:inScheme	ccat: ;
	skos:notation	"204510" ;
	skos:prefLabel	"Chickpeas"@en .

ccat:204520
	a	skos:Concept ;
	skos:altLabel	"Azuki Beans"@en , "Red Beans"@en , "Red Mung Beans"@en ;
	skos:broader	ccat:2045 ;
	skos:definition	"Seed of Vigna angularis."@en ;
	skos:exactMatch	agrovoc:c_8632 , wd:Q380279 ;
	skos:inScheme	ccat: ;
	skos:notation	"204520" ;
	skos:prefLabel	"Adzuki Beans"@en .

ccat:204525
	a	skos:Concept ;
	skos:altLabel	"Green Gram"@en ;
	skos:broader	ccat:2045 ;
	skos:definition	"Seed of Vigna radiata."@en ;
	skos:inScheme	ccat: ;
	skos:notation	"204525" ;
	skos:prefLabel	"Mung Beans"@en .

ccat:204527
	a	skos:Concept ;
	skos:altLabel	"Black Gram"@en ;
	skos:broader	ccat:2045 ;
	skos:definition	"Seed of Vigna mungo."@en ;
	skos:inScheme	ccat: ;
	skos:notation	"204527" ;
	skos:prefLabel	"Urad"@en .

ccat:204530
	a	skos:Concept ;
	skos:broader	ccat:2045 ;
	skos:definition	"Seed of Lathyrus oleraceus"@en ;
	skos:inScheme	ccat: ;
	skos:notation	"204530" ;
	skos:prefLabel	"Peas"@en .

ccat:2050
	a	skos:Concept ;
	skos:broader	ccat:20 ;
	skos:definition	"The ripened reproductive body of a seed plant "@en ;
	skos:exactMatch	agrovoc:c_3131 , stw:14110-2 ;
	skos:inScheme	ccat: ;
	skos:notation	"2050" ;
	skos:prefLabel	"Fruits"@en .

ccat:205010
	a	skos:Concept ;
	skos:broader	ccat:2050 ;
	skos:definition	"Fruit of various citrus species in the family Rutaceae."@en ;
	skos:exactMatch	agrovoc:c_1641 , stw:14119-5 , wd:Q2574750 ;
	skos:inScheme	ccat: ;
	skos:notation	"205010" ;
	skos:note	"""The fruit of the orange tree can be eaten fresh, or processed for its juice or fragrant peel. As of 2012, sweet oranges accounted for approximately 70% of citrus production.

In 2017, 73 million tonnes of oranges were grown worldwide, with Brazil producing 24% of the world total, followed by China and India."""@en ;
	skos:prefLabel	"Citrus Fruits"@en .

ccat:20501010
	a	skos:Concept ;
	skos:broader	ccat:205010 ;
	skos:definition	"Fruit of Citrus x sinensis."@en ;
	skos:exactMatch	agrovoc:c_7550 , wd:Q13191 ;
	skos:inScheme	ccat: ;
	skos:notation	"20501010" ;
	skos:prefLabel	"Sweet Oranges"@en .

ccat:20501020
	a	skos:Concept ;
	skos:broader	ccat:205010 ;
	skos:definition	"Fruit of Citrus tangerina, Citrus reticulata, Citrus x clementina, or Citrus unshiu."@en ;
	skos:inScheme	ccat: ;
	skos:notation	"20501020" ;
	skos:prefLabel	"Tangerines and Mandarines and Clementines and Satsumas"@en .

ccat:20501030
	a	skos:Concept ;
	skos:broader	ccat:205010 ;
	skos:definition	"Fruit of Citrus limon."@en ;
	skos:exactMatch	agrovoc:c_4259 ;
	skos:inScheme	ccat: ;
	skos:notation	"20501030" ;
	skos:prefLabel	"Lemons"@en .

ccat:20501035
	a	skos:Concept ;
	skos:broader	ccat:205010 ;
	skos:definition	"Fruit of the hybrids produced from citrons (Citrus medica), mandarin oranges (Citrus reticulata), or pomeloes (Citrus maxima) and the lime varieties (Citrus hystrix var. micrantha)."@en ;
	skos:exactMatch	agrovoc:c_4341 ;
	skos:inScheme	ccat: ;
	skos:notation	"20501035" ;
	skos:prefLabel	"Limes"@en .

ccat:20501040
	a	skos:Concept ;
	skos:broader	ccat:205010 ;
	skos:definition	"Fruit of Citrus x paradisi."@en ;
	skos:exactMatch	agrovoc:c_3358 ;
	skos:inScheme	ccat: ;
	skos:notation	"20501040" ;
	skos:note	"""In 2019, world production of grapefruits (combined with pomelos) was 9.3 million tonnes, of which 53% was in China. Other significant producers include Vietnam, United States and Mexico."""@en ;
	skos:prefLabel	"Grapefruit"@en .

ccat:20501045
	a	skos:Concept ;
	skos:broader	ccat:205010 ;
	skos:definition	"Fruit of Citrus maxima."@en ;
	skos:exactMatch	agrovoc:c_6367 ;
	skos:inScheme	ccat: ;
	skos:notation	"20501045" ;
	skos:prefLabel	"Pomelo"@en .

ccat:20501090
	a	skos:Concept ;
	skos:broader	ccat:205010 ;
	skos:definition	"Any other fruit of plants in the Citrus genus."@en ;
	skos:inScheme	ccat: ;
	skos:notation	"20501090" ;
	skos:prefLabel	"Other Citrus Fruit"@en .

ccat:205020
	a	skos:Concept ;
	skos:broader	ccat:2050 ;
	skos:definition	"Fruit produced by flowering plants in the subtribe Malinae of the family Rosaceae."@en ;
	skos:exactMatch	agrovoc:c_25497 , wd:Q41274 ;
	skos:inScheme	ccat: ;
	skos:notation	"205020" ;
	skos:prefLabel	"Pome Fruits"@en .

ccat:20502010
	a	skos:Concept ;
	skos:broader	ccat:205020 ;
	skos:definition	"Fruit of Malus domestica."@en ;
	skos:exactMatch	agrovoc:c_541 , stw:19014-1 , wd:Q89 ;
	skos:inScheme	ccat: ;
	skos:notation	"20502010" ;
	skos:note	"""Worldwide production of apples in 2018 was 86 million tonnes, with China accounting for nearly half of the total."""@en ;
	skos:prefLabel	"Apples"@en .

ccat:20502020
	a	skos:Concept ;
	skos:broader	ccat:205020 ;
	skos:definition	"Fruit of trees in the genus Pyrus, in particular Pyrus communis, Pyrus x bretschneideri, and Pyrus pyrifolia."@en ;
	skos:inScheme	ccat: ;
	skos:notation	"20502020" ;
	skos:prefLabel	"Pears"@en .

ccat:20502030
	a	skos:Concept ;
	skos:broader	ccat:205020 ;
	skos:definition	"Fruit of Cydonia oblonga."@en ;
	skos:inScheme	ccat: ;
	skos:notation	"20502030" ;
	skos:prefLabel	"Quinces"@en .

ccat:20502090
	a	skos:Concept ;
	skos:broader	ccat:205020 ;
	skos:definition	"Any other fruit of plants in the subtribe Malinae."@en ;
	skos:inScheme	ccat: ;
	skos:notation	"20502090" ;
	skos:prefLabel	"Other Pome Fruits"@en .

ccat:205030
	a	skos:Concept ;
	skos:altLabel	"Drupe"@en ;
	skos:broader	ccat:2050 ;
	skos:definition	"Fruits of the botanical family Rosaceae that contain a single hard seed, called a stone, pit, or pip."@en ;
	skos:exactMatch	agrovoc:c_25461 , eurovoc:1117 , wd:Q14712 ;
	skos:inScheme	ccat: ;
	skos:notation	"205030" ;
	skos:prefLabel	"Stone Fruit"@en .

ccat:20503010
	a	skos:Concept ;
	skos:broader	ccat:205030 ;
	skos:definition	"Fruit of many plants of the genus Prunus different from apricots, e.g. Prunus avium (sweet cherry) or Prunus cerasus (sour cherries)."@en ;
	skos:inScheme	ccat: ;
	skos:notation	"20503010" ;
	skos:prefLabel	"Cherries"@en .

ccat:20503020
	a	skos:Concept ;
	skos:broader	ccat:205030 ;
	skos:definition	"Fruit of several species in the genus Prunus different from cherries, e.g. Prunus armeniaca, Prunus brigantina, etc."@en ;
	skos:inScheme	ccat: ;
	skos:notation	"20503020" ;
	skos:prefLabel	"Apricots"@en .

ccat:20503030
	a	skos:Concept ;
	skos:broader	ccat:205030 ;
	skos:definition	"Fruit of Prunus persica."@en ;
	skos:inScheme	ccat: ;
	skos:notation	"20503030" ;
	skos:note	"""Peaches and nectarines are the same species, though they are regarded commercially as different fruits. The skin of nectarines lacks the fuzz (fruit-skin trichomes) that peach skin has; a mutation in a single gene (MYB25) is thought to be responsible for the difference between the two."""@en ;
	skos:prefLabel	"Peaches and Nectarines"@en .

ccat:20503040
	a	skos:Concept ;
	skos:broader	ccat:205030 ;
	skos:definition	"Fruit of some species in Prunus subg. Prunus, e.g. Prunus domestica."@en ;
	skos:inScheme	ccat: ;
	skos:notation	"20503040" ;
	skos:prefLabel	"Plums"@en .

ccat:20503090
	a	skos:Concept ;
	skos:broader	ccat:205030 ;
	skos:definition	"Any other drupes."@en ;
	skos:inScheme	ccat: ;
	skos:notation	"20503090" ;
	skos:prefLabel	"Other Drupes"@en .

ccat:205040
	a	skos:Concept ;
	skos:broader	ccat:2050 ;
	skos:definition	"Fruit with fleshy pericarp, containing one or many seeds."@en ;
	skos:exactMatch	wd:Q13184 ;
	skos:inScheme	ccat: ;
	skos:notation	"205040" ;
	skos:prefLabel	"Berries"@en .

ccat:20504010
	a	skos:Concept ;
	skos:broader	ccat:205040 ;
	skos:definition	"Fruit of Fragaria x ananassa."@en ;
	skos:inScheme	ccat: ;
	skos:notation	"20504010" ;
	skos:note	"""In 2020, world production of strawberries was 8.9 million tonnes, led by China with 38% of the total, and the United States and Egypt as other significant producers.

Due the relatively fragile nature of the strawberry, approximately 35 percent of the $2.2 billion United States crop was spoiled in 2020. This led to an Idaho company planning to launch gene-edited strawberries in the near future in an effort to make them more durable and hardier. In the U.S. it costs growers around $35,000 per acre to plant and $35,000 per acre to harvest strawberries now, and more durable berries might reduce the rate of spoilage."""@en ;
	skos:prefLabel	"Strawberries"@en .

ccat:20504020
	a	skos:Concept ;
	skos:broader	ccat:205040 ;
	skos:definition	"Fruit of many plant species in the genus Rubus, most of which in the subgenus Idaeobatus."@en ;
	skos:inScheme	ccat: ;
	skos:notation	"20504020" ;
	skos:note	"""In 2020, world production of raspberries was 895,771 tonnes, led by Russia with 20% of the world total. Other major producers were Mexico, Poland, Serbia, and the United States."""@en ;
	skos:prefLabel	"Raspberries"@en .

ccat:20504030
	a	skos:Concept ;
	skos:broader	ccat:205040 ;
	skos:definition	"Fruit of many species of Ribes that are not currants, e.g. Ribes uva-crispa."@en ;
	skos:inScheme	ccat: ;
	skos:notation	"20504030" ;
	skos:prefLabel	"Gooseberries"@en .

ccat:20504040
	a	skos:Concept ;
	skos:broader	ccat:205040 ;
	skos:definition	"Fruit of many species of Ribes that are not gooseberries, e.g. Ribes nigrum, Ribes rubrum."@en ;
	skos:inScheme	ccat: ;
	skos:notation	"20504040" ;
	skos:prefLabel	"Currants"@en .

ccat:20504050
	a	skos:Concept ;
	skos:broader	ccat:205040 ;
	skos:definition	"Fruit of species in the section Cyanococcus within the genus Vaccinium, e.g. Vaccinium caesariense."@en ;
	skos:inScheme	ccat: ;
	skos:notation	"20504050" ;
	skos:prefLabel	"Blueberries"@en .

ccat:20504060
	a	skos:Concept ;
	skos:broader	ccat:205040 ;
	skos:definition	"Fruit of species in the subgenus Oxycoccus of the genus Vaccinium, e.g. Vaccinium oxycoccos."@en ;
	skos:inScheme	ccat: ;
	skos:notation	"20504060" ;
	skos:prefLabel	"Cranberries"@en .

ccat:20504090
	a	skos:Concept ;
	skos:broader	ccat:205040 ;
	skos:definition	"Fruit of any other shrubs and bushes whose fruits are berries, excluding those that are classified as tropical fruits."@en ;
	skos:inScheme	ccat: ;
	skos:notation	"20504090" ;
	skos:prefLabel	"Other Berries"@en .

ccat:205050
	a	skos:Concept ;
	skos:broader	ccat:2050 ;
	skos:definition	"Tropical fruit is any fruit produced by a tree native to the tropics. The tropics are generally defined as the region of the globe between the Tropic of Cancer and the Tropic of Capricorn."@en ;
	skos:exactMatch	agrovoc:c_7974 , stw:14117-2 , wd:Q844144 ;
	skos:inScheme	ccat: ;
	skos:notation	"205050" ;
	skos:prefLabel	"Tropical Fruits"@en .

ccat:20505010
	a	skos:Concept ;
	skos:broader	ccat:205050 ;
	skos:definition	"Fruit of many cultivars in the genus Musa."@en ;
	skos:inScheme	ccat: ;
	skos:notation	"20505010" ;
	skos:prefLabel	"Bananas and Plantains"@en ;
	skos:scopeNote	"Plantains are more starchy and less sweet; they are eaten cooked rather than raw; they have thicker skin, which may be green, yellow or black; and they can be used at any stage of ripeness."@en .

ccat:20505020
	a	skos:Concept ;
	skos:altLabel	"Chinese gooseberry"@en ;
	skos:broader	ccat:205050 ;
	skos:definition	"Fruit of several species of woody vines in the genus Actinidia."@en ;
	skos:inScheme	ccat: ;
	skos:notation	"20505020" ;
	skos:prefLabel	"Kiwi Fruit"@en .

ccat:20505030
	a	skos:Concept ;
	skos:broader	ccat:205050 ;
	skos:definition	"Fruit of Mangifera indica."@en ;
	skos:inScheme	ccat: ;
	skos:notation	"20505030" ;
	skos:prefLabel	"Mangoes"@en .

ccat:20505040
	a	skos:Concept ;
	skos:broader	ccat:205050 ;
	skos:definition	"Fruit of Ziziphus jujuba."@en ;
	skos:exactMatch	wd:Q3093648 ;
	skos:inScheme	ccat: ;
	skos:notation	"20505040" ;
	skos:prefLabel	"Jujube"@en .

ccat:20505050
	a	skos:Concept ;
	skos:broader	ccat:205050 ;
	skos:definition	"Fruit of Persea americana."@en ;
	skos:inScheme	ccat: ;
	skos:notation	"20505050" ;
	skos:prefLabel	"Avocados"@en .

ccat:20505060
	a	skos:Concept ;
	skos:broader	ccat:205050 ;
	skos:definition	"Fruit of the date palm (Phoenix dactylifera)."@en ;
	skos:inScheme	ccat: ;
	skos:notation	"20505060" ;
	skos:prefLabel	"Dates"@en .

ccat:20505065
	a	skos:Concept ;
	skos:broader	ccat:205050 ;
	skos:definition	"Fruit of Ficus carica."@en ;
	skos:exactMatch	agrovoc:c_10840 ;
	skos:inScheme	ccat: ;
	skos:notation	"20505065" ;
	skos:prefLabel	"Figs"@en .

ccat:20505068
	a	skos:Concept ;
	skos:broader	ccat:205050 ;
	skos:definition	"Fruit of Artocarpus heterophyllus."@en ;
	skos:exactMatch	agrovoc:c_10840 ;
	skos:inScheme	ccat: ;
	skos:notation	"20505068" ;
	skos:prefLabel	"Jackfruit"@en .

ccat:20505070
	a	skos:Concept ;
	skos:broader	ccat:205050 ;
	skos:definition	"Fruit of Carica papaya."@en ;
	skos:inScheme	ccat: ;
	skos:notation	"20505070" ;
	skos:prefLabel	"Papayas"@en .

ccat:20505080
	a	skos:Concept ;
	skos:broader	ccat:205050 ;
	skos:definition	"Fruit of Ananas comosus."@en ;
	skos:inScheme	ccat: ;
	skos:notation	"20505080" ;
	skos:prefLabel	"Pineapples"@en .

ccat:20505090
	a	skos:Concept ;
	skos:broader	ccat:205050 ;
	skos:definition	"Any other tropical fruits."@en ;
	skos:inScheme	ccat: ;
	skos:notation	"20505090" ;
	skos:prefLabel	"Other Tropical Fruit"@en .

ccat:205090
	a	skos:Concept ;
	skos:broader	ccat:2050 ;
	skos:definition	"Any other fruits."@en ;
	skos:inScheme	ccat: ;
	skos:notation	"205090" ;
	skos:prefLabel	"Other Fresh Fruit"@en .

ccat:2055
	a	skos:Concept ;
	skos:broader	ccat:20 ;
	skos:definition	"Juice is a drink made by extracting or pressing the natural liquid contained in fruit. Fruit syrups (or fruit molasses) are concentrated fruit juices."@en ;
	skos:inScheme	ccat: ;
	skos:notation	"2055" ;
	skos:prefLabel	"Fruit Juices and Fruit Syrups"@en .

ccat:205510
	a	skos:Concept ;
	skos:broader	ccat:2055 ;
	skos:definition	"Juices and syrups made by pressing citrus fruits."@en ;
	skos:inScheme	ccat: ;
	skos:notation	"205510" ;
	skos:prefLabel	"Juices and Syrups from Citrus Fruits"@en .

ccat:20551010
	a	skos:Concept ;
	skos:broader	ccat:205510 ;
	skos:definition	"U.S. Grade A frozen concentrate of sweet oranges with a Brix value of at least 62.5 degrees."@en ;
	skos:inScheme	ccat: ;
	skos:notation	"20551010" ;
	skos:prefLabel	"Frozen Orange Juice"@en .

ccat:205520
	a	skos:Concept ;
	skos:broader	ccat:2055 ;
	skos:definition	"Juices and syrups made by pressing pome fruits."@en ;
	skos:inScheme	ccat: ;
	skos:notation	"205520" ;
	skos:prefLabel	"Juices and Syrups from Pome Fruits"@en .

ccat:20552010
	a	skos:Concept ;
	skos:broader	ccat:205520 ;
	skos:definition	"Concentrate of pressed apples."@en ;
	skos:inScheme	ccat: ;
	skos:notation	"20552010" ;
	skos:prefLabel	"Apple Juice Concentrate"@en .

ccat:2060
	a	skos:Concept ;
	skos:broader	ccat:20 ;
	skos:definition	"Seed, fruit, root, bark, salt, or other plant substance primarily used for flavouring or colouring food."@en ;
	skos:exactMatch	agrovoc:c_15685 , stw:14060-5 , wd:Q42527 ;
	skos:inScheme	ccat: ;
	skos:notation	"2060" ;
	skos:prefLabel	"Spices"@en ;
	skos:scopeNote	"Spices are distinguished from herbs, which are the leaves, flowers, or stems of plants used for flavouring or as a garnish. Spices are sometimes used in medicine, religious rituals, cosmetics or perfume production."@en .

ccat:206010
	a	skos:Concept ;
	skos:broader	ccat:2060 ;
	skos:definition	"Spice made from the seeds of several plants in the genera Elettaria and Amomum in the family Zingiberaceae."@en ;
	skos:exactMatch	agrovoc:c_9620 ;
	skos:inScheme	ccat: ;
	skos:notation	"206010" ;
	skos:note	"""Cardamom is the world's third-most expensive spice, surpassed in price per weight only by saffron and vanilla."""@en ;
	skos:prefLabel	"Cardamom"@en .

ccat:206020
	a	skos:Concept ;
	skos:broader	ccat:2060 ;
	skos:definition	"Spice obtained from the inner bark of several tree species from the genus Cinnamomum."@en ;
	skos:inScheme	ccat: ;
	skos:notation	"206020" ;
	skos:note	"""In 2018, Indonesia and China produced 70% of the world's supply of cinnamon, Indonesia producing nearly 40% and China 30%."""@en ;
	skos:prefLabel	"Cinnamon"@en ;
	skos:scopeNote	"Cinnamon is the name for several species of trees and the commercial spice products that some of them produce. All are members of the genus Cinnamomum in the family Lauraceae. Only a few Cinnamomum species are grown commercially for spice. Cinnamomum verum is sometimes considered to be \"true cinnamon\", but most cinnamon in international commerce is derived from the related species Cinnamomum cassia, also referred to as \"cassia\"."@en .

ccat:206030
	a	skos:Concept ;
	skos:broader	ccat:2060 ;
	skos:definition	"Seed or ground spice of several species of the genus Myristica."@en ;
	skos:exactMatch	agrovoc:c_23169 , wd:Q83165 ;
	skos:inScheme	ccat: ;
	skos:notation	"206030" ;
	skos:note	"""Indonesia is the main producers of nutmeg and mace."""@en ;
	skos:prefLabel	"Nutmeg"@en .

ccat:206035
	a	skos:Concept ;
	skos:broader	ccat:2060 ;
	skos:definition	"Spice made from the reddish seed covering (aril) of the nutmeg seed."@en ;
	skos:exactMatch	agrovoc:c_25484 , wd:Q1882876 ;
	skos:inScheme	ccat: ;
	skos:notation	"206035" ;
	skos:prefLabel	"Mace"@en .

ccat:206040
	a	skos:Concept ;
	skos:broader	ccat:2060 ;
	skos:definition	"Rhizome of Ginger (Zingiber officinale)."@en ;
	skos:inScheme	ccat: ;
	skos:notation	"206040" ;
	skos:note	"""India holds the seventh position in ginger export worldwide, however is the largest producer of ginger in the world. Regions in southwest and Northeast India are most suitable for ginger production due to their warm and humid climate, average rainfall and land space."""@en ;
	skos:prefLabel	"Ginger"@en .

ccat:206045
	a	skos:Concept ;
	skos:altLabel	"Curcuma"@en ;
	skos:broader	ccat:2060 ;
	skos:closeMatch	wd:Q42562 ;
	skos:definition	"Rhizome of Curcuma longa of the ginger family, Zingiberaceae."@en ;
	skos:exactMatch	agrovoc:c_15048 , wd:Q20730193 ;
	skos:inScheme	ccat: ;
	skos:notation	"206045" ;
	skos:prefLabel	"Turmeric"@en .

ccat:206050
	a	skos:Concept ;
	skos:altLabel	"Jeera"@en ;
	skos:broader	ccat:2060 ;
	skos:definition	"Dried seed of Cumin (Cuminum cyminum), a flowering plant in the family Apiaceae."@en ;
	skos:exactMatch	agrovoc:c_10205 , wd:Q57328174 ;
	skos:inScheme	ccat: ;
	skos:notation	"206050" ;
	skos:prefLabel	"Cumin"@en .

ccat:206055
	a	skos:Concept ;
	skos:broader	ccat:2065 ;
	skos:definition	"Dried seeds of Coriandrum sativum in the family Apiaceae."@en ;
	skos:exactMatch	agrovoc:c_10097 , wd:Q41611 ;
	skos:inScheme	ccat: ;
	skos:notation	"206055" ;
	skos:prefLabel	"Coriander"@en ;
	skos:scopeNote	"The fresh leaves and the roots are used in cooking as well. This concept only refers to the dried seeds."@en .

ccat:206060
	a	skos:Concept ;
	skos:broader	ccat:2060 ;
	skos:definition	"Spice derived from the seed pods of orchids of the genus Vanilla, primarily obtained from flat-leaved vanilla (V. planifolia)."@en ;
	skos:exactMatch	agrovoc:c_15126 , wd:Q13241 ;
	skos:inScheme	ccat: ;
	skos:notation	"206060" ;
	skos:note	"""Three major species of vanilla currently are grown globally, all of which derive from a species originally found in Mesoamerica, including parts of modern-day Mexico. They are V. planifolia (syn. V. fragrans), grown on Madagascar, Runion, and other tropical areas along the Indian Ocean; V. tahitensis, grown in the South Pacific; and V. pompona, found in the West Indies, Central America, and South America.

The majority of the world's vanilla is the V. planifolia species, more commonly known as Bourbon vanilla (after the former name of Runion, e Bourbon) or Madagascar vanilla, which is produced in Madagascar and neighbouring islands in the southwestern Indian Ocean, and in Indonesia. Madagascar's and Indonesia's cultivations produce two-thirds of the world's supply of vanilla.

Vanilla is the second-most expensive spice after saffron because growing the vanilla seed pods is labor-intensive. Nevertheless, vanilla is widely used in both commercial and domestic baking, perfume manufacture, and aromatherapy."""@en ;
	skos:prefLabel	"Vanilla"@en .

ccat:206070
	a	skos:Concept ;
	skos:broader	ccat:2060 ;
	skos:definition	"Dried drupe of Black pepper (Piper nigrum) in the family Piperaceae."@en ;
	skos:exactMatch	agrovoc:c_25495 , wd:Q3143131 ;
	skos:inScheme	ccat: ;
	skos:notation	"206070" ;
	skos:note	"""Black pepper is native to present-day South India, and is extensively cultivated there and elsewhere in tropical regions. Producing 24% of the world total in 2019, Vietnam is the largest exporter of pepper.

Black pepper is the world's most traded spice, and is one of the most common spices added to cuisines around the world."""@en ;
	skos:prefLabel	"Pepper"@en .

ccat:206075
	a	skos:Concept ;
	skos:altLabel	"Allspice"@en ;
	skos:broader	ccat:2060 ;
	skos:definition	"Dried unripe berry of Pimenta dioica."@en ;
	skos:exactMatch	agrovoc:c_19193 , wd:Q1963621 ;
	skos:inScheme	ccat: ;
	skos:notation	"206075" ;
	skos:note	"""Midcanopy trees are native to the Greater Antilles, southern Mexico, and Central America, now cultivated in many warm parts of the world."""@en ;
	skos:prefLabel	"Pimento"@en .

ccat:206080
	a	skos:Concept ;
	skos:altLabel	"Chili"@en ;
	skos:broader	ccat:2060 ;
	skos:definition	"Spicy fruit of plants in the genus Capsicum."@en ;
	skos:inScheme	ccat: ;
	skos:notation	"206080" ;
	skos:prefLabel	"Chilli"@en .

ccat:206090
	a	skos:Concept ;
	skos:broader	ccat:2060 ;
	skos:definition	"Any other spices."@en ;
	skos:inScheme	ccat: ;
	skos:notation	"206090" ;
	skos:prefLabel	"Other Spices"@en .

ccat:2065
	a	skos:Concept ;
	skos:broader	ccat:20 ;
	skos:closeMatch	agrovoc:c_27977 ;
	skos:definition	"Leaves, flowers, or stems of plants used for flavouring or as a garnish."@en ;
	skos:exactMatch	wd:Q207123 ;
	skos:inScheme	ccat: ;
	skos:notation	"2065" ;
	skos:prefLabel	"Herbs"@en ;
	skos:scopeNote	"Herbs are distinguished from spices, which are the seed, fruit, root, bark, salt, or other plant substance primarily used for flavouring or colouring food."@en .

ccat:2070
	a	skos:Concept ;
	skos:broader	ccat:20 ;
	skos:definition	"Plants or plant parts that, if activated, e.g. by heating, infusion, etc., stimulate the central nervous system."@en ;
	skos:inScheme	ccat: ;
	skos:notation	"2070" ;
	skos:prefLabel	"Stimulant Crops"@en .

ccat:207010
	a	skos:Concept ;
	skos:broader	ccat:2070 ;
	skos:definition	"Stone inside the cherry of the Coffea plant."@en ;
	skos:exactMatch	agrovoc:c_28379 ;
	skos:inScheme	ccat: ;
	skos:notation	"207010" ;
	skos:note	"""The two most economically important varieties of coffee plant are the Arabica and the Robusta; ~60% of the coffee produced worldwide is Arabica and ~40% is Robusta. Arabica beans consist of 0.8-1.4% caffeine and Robusta beans consist of 1.7-4% caffeine. As coffee is one of the world's most widely consumed beverages, coffee beans are a major cash crop and an important export product, accounting for over 50% of some developing nations' foreign exchange earnings."""@en ;
	skos:prefLabel	"Green Coffee"@en .

ccat:207020
	a	skos:Concept ;
	skos:broader	ccat:2070 ;
	skos:definition	"Seeds from the pod of the cacao tree (Theobroma cacao)."@en ;
	skos:exactMatch	agrovoc:c_1711 ;
	skos:inScheme	ccat: ;
	skos:notation	"207020" ;
	skos:prefLabel	"Cocoa Beans"@en .

ccat:207025
	a	skos:Concept ;
	skos:broader	ccat:2070 ;
	skos:definition	"Seeds from the pod of the carob shrub (Ceratonia siliqua)."@en ;
	skos:inScheme	ccat: ;
	skos:notation	"207025" ;
	skos:prefLabel	"Carobs"@en .

ccat:207030
	a	skos:Concept ;
	skos:broader	ccat:2070 ;
	skos:definition	"Cured or fresh leaves of Camellia sinensis, or rarely Camellia taliensis."@en ;
	skos:inScheme	ccat: ;
	skos:notation	"207030" ;
	skos:prefLabel	"Tea"@en .

ccat:207035
	a	skos:Concept ;
	skos:broader	ccat:2070 ;
	skos:definition	"Dried or fresh leaves of the Yerba mate (Ilex paraguariensis)."@en ;
	skos:inScheme	ccat: ;
	skos:notation	"207035" ;
	skos:prefLabel	"Mate"@en .

ccat:207039
	a	skos:Concept ;
	skos:broader	ccat:2070 ;
	skos:definition	"Other leaves or plant parts that are consumed by infusion."@en ;
	skos:inScheme	ccat: ;
	skos:notation	"207039" ;
	skos:prefLabel	"Other Tea"@en .

ccat:207040
	a	skos:Concept ;
	skos:broader	ccat:2070 ;
	skos:definition	"Cured or fresh leaves of several plants in the genus Nicotiana."@en ;
	skos:inScheme	ccat: ;
	skos:notation	"207040" ;
	skos:prefLabel	"Tobacco Leaves"@en .

ccat:207050
	a	skos:Concept ;
	skos:broader	ccat:2070 ;
	skos:definition	"Wet or dried seed cones (strobiles) of the hop plant (Humulus lupulus)."@en ;
	skos:inScheme	ccat: ;
	skos:notation	"207050" ;
	skos:prefLabel	"Hops"@en .

ccat:207090
	a	skos:Concept ;
	skos:broader	ccat:2070 ;
	skos:definition	"Any other plant or plant parts with stimulatory effects."@en ;
	skos:inScheme	ccat: ;
	skos:notation	"207090" ;
	skos:prefLabel	"Other Stimulant Crops"@en .

ccat:2510
	a	skos:Concept ;
	skos:broader	ccat:20 ;
	skos:definition	"Domesticated animals raised in an agricultural setting to produce commodities such as food, fibre, and labour."@en ;
	skos:exactMatch	agrovoc:c_4397 , stw:14145-4 , wd:Q103459 ;
	skos:inScheme	ccat: ;
	skos:notation	"2510" ;
	skos:prefLabel	"Livestock"@en .

ccat:251010
	a	skos:Concept ;
	skos:broader	ccat:2510 ;
	skos:definition	"Large domesticated ungulates in the species Bos taurus."@en ;
	skos:exactMatch	agrovoc:c_1391 , eurovoc:5034 , stw:14142-3 , wd:Q830 ;
	skos:inScheme	ccat: ;
	skos:notation	"251010" ;
	skos:prefLabel	"Cattle"@en .

ccat:251015
	a	skos:Concept ;
	skos:broader	ccat:2510 ;
	skos:definition	"Domesticated animal in the species Bubalus bualis."@en ;
	skos:exactMatch	agrovoc:c_25410 ;
	skos:inScheme	ccat: ;
	skos:notation	"251015" ;
	skos:note	"""Around 26 million water buffaloes are slaughtered each year for meat worldwide. They contribute 72 million tonnes of milk and three million tonnes of meat annually to world food, much of it in areas that are prone to nutritional imbalances. In India, river buffaloes are kept mainly for milk production and for transport, whereas swamp buffaloes are kept mainly for work and a small amount of milk."""@en ;
	skos:prefLabel	"Buffaloes"@en .

ccat:251020
	a	skos:Concept ;
	skos:broader	ccat:2510 ;
	skos:definition	"Domesticated animal in the species Ovis aries."@en ;
	skos:exactMatch	agrovoc:c_7030 , eurovoc:2211 , stw:14143-1 , wd:Q7368 ;
	skos:inScheme	ccat: ;
	skos:notation	"251020" ;
	skos:note	"""Numbering a little over one billion, domestic sheep are also the most numerous species of sheep. A sheep's wool is the most widely used animal fibre, and is usually harvested by shearing. Ovine meat is called lamb when from younger animals and mutton when from older ones in Commonwealth countries, and lamb in the United States (including from adults).

Sheep husbandry is practised throughout the majority of the inhabited world. Australia, New Zealand, the southern and central South American nations, and the British Isles are most closely associated with sheep production."""@en ;
	skos:prefLabel	"Sheep"@en .

ccat:251025
	a	skos:Concept ;
	skos:broader	ccat:2510 ;
	skos:definition	"Domesticated animal in the subspecies Capra aegagrus hircus."@en ;
	skos:exactMatch	agrovoc:c_3324 , eurovoc:5252 , stw:14146-2 , wd:Q2934 ;
	skos:inScheme	ccat: ;
	skos:notation	"251025" ;
	skos:note	"""In 2011, there were more than 924 million goats living in the world, according to the UN Food and Agriculture Organization."""@en ;
	skos:prefLabel	"Goats"@en .

ccat:251030
	a	skos:Concept ;
	skos:altLabel	"Hogs"@en , "Pigs"@en ;
	skos:broader	ccat:2510 ;
	skos:definition	"Domesticated even-toed ungulate in the species Sus scrofa domesticus."@en ;
	skos:exactMatch	agrovoc:c_7555 , eurovoc:2560 , stw:14144-6 , wd:Q787 ;
	skos:inScheme	ccat: ;
	skos:notation	"251030" ;
	skos:note	"""The domestic pig's head-plus-body length ranges from 0.9 to 1.8 m (35 to 71 in), and adult pigs typically weigh between 50 and 350 kg (110 and 770 lb), with well-fed individuals often exceeding this weight range. The size and weight of hogs largely depends on their breed."""@en ;
	skos:prefLabel	"Swine"@en .

ccat:251040
	a	skos:Concept ;
	skos:broadMatch	stw:14135-0 ;
	skos:broader	ccat:2510 ;
	skos:definition	"Domesticated animal in the subspecies Gallus gallus domesticus, a subspecies of the red junglefowl."@en ;
	skos:exactMatch	agrovoc:c_1540 , wd:Q780 ;
	skos:inScheme	ccat: ;
	skos:notation	"251040" ;
	skos:note	"""Chickens are one of the most common and widespread domestic animals, with a total population of 23.7 billion as of 2018, up from more than 19 billion in 2011. There are more chickens in the world than any other bird."""@en ;
	skos:prefLabel	"Chickens"@en .

ccat:251042
	a	skos:Concept ;
	skos:broadMatch	stw:14135-0 ;
	skos:broader	ccat:2510 ;
	skos:definition	"Domesticated aninmal in the species Meleagris gallopavo domesticus."@en ;
	skos:exactMatch	agrovoc:c_8016 , wd:Q848706 ;
	skos:inScheme	ccat: ;
	skos:notation	"251042" ;
	skos:note	"""The domestic turkey is a popular form of poultry, and it is raised throughout temperate parts of the world, partially because industrialized farming has made it very cheap for the amount of meat it produces."""@en ;
	skos:prefLabel	"Turkeys"@en .

ccat:251045
	a	skos:Concept ;
	skos:altLabel	"Mallards"@en ;
	skos:broadMatch	stw:14135-0 ;
	skos:broader	ccat:2510 ;
	skos:definition	"Domesticated animal in the subspecies Anas platyrhynchos domesticus."@en ;
	skos:exactMatch	agrovoc:c_2406 , wd:Q742292 ;
	skos:inScheme	ccat: ;
	skos:notation	"251045" ;
	skos:prefLabel	"Ducks"@en .

ccat:251047
	a	skos:Concept ;
	skos:broadMatch	stw:14135-0 ;
	skos:broader	ccat:2510 ;
	skos:definition	"Domesticated animal in the species Anser anser domesticus or Anser cygnoides domesticus."@en ;
	skos:exactMatch	agrovoc:c_3208 , wd:Q255503 ;
	skos:inScheme	ccat: ;
	skos:notation	"251047" ;
	skos:note	"""Approximately 700 million geese are slaughtered each year for meat worldwide."""@en ;
	skos:prefLabel	"Geese"@en .

ccat:251048
	a	skos:Concept ;
	skos:broader	ccat:2510 ;
	skos:closeMatch	agrovoc:c_3180 ;
	skos:definition	"Domesticated bird in the subspecies Columba livia domestica."@en ;
	skos:inScheme	ccat: ;
	skos:narrowMatch	agrovoc:c_5870 , wd:Q204179 ;
	skos:notation	"251048" ;
	skos:prefLabel	"Pigeons"@en .

ccat:251049
	a	skos:Concept ;
	skos:broader	ccat:2510 ;
	skos:definition	"Other birds, gamebirds, or domestic birds bred or hunted for consumption, such as quail, ostrich, Guinea fowl, etc."@en ;
	skos:inScheme	ccat: ;
	skos:notation	"251049" ;
	skos:prefLabel	"Other Birds"@en .

ccat:251050
	a	skos:Concept ;
	skos:broader	ccat:2510 ;
	skos:definition	"Domesticated odd-toed, hoofed mammal in the species Equus ferus caballus."@en ;
	skos:exactMatch	agrovoc:c_3668 , wd:Q726 ;
	skos:inScheme	ccat: ;
	skos:notation	"251050" ;
	skos:prefLabel	"Horses"@en .

ccat:251055
	a	skos:Concept ;
	skos:altLabel	"Donkey"@en ;
	skos:broader	ccat:2510 ;
	skos:definition	"Domesticated hoofed mammal in the subspecies Equus africanus asinus"@en ;
	skos:inScheme	ccat: ;
	skos:notation	"251055" ;
	skos:prefLabel	"Asses"@en .

ccat:251058
	a	skos:Concept ;
	skos:broader	ccat:2510 ;
	skos:definition	"Domestic equine hybrid between a donkey and a horse, Equus africanus asinus x Equus ferus caballus"@en ;
	skos:inScheme	ccat: ;
	skos:notation	"251058" ;
	skos:prefLabel	"Mules"@en .

ccat:251060
	a	skos:Concept ;
	skos:broader	ccat:2510 ;
	skos:definition	"Even-toed ungulate in the genus Camelus that bears distinctive fatty deposits (humps) on its back."@en ;
	skos:inScheme	ccat: ;
	skos:notation	"251060" ;
	skos:prefLabel	"Camels"@en .

ccat:251069
	a	skos:Concept ;
	skos:broader	ccat:2510 ;
	skos:definition	"Any other animals in the family Camelidae."@en ;
	skos:inScheme	ccat: ;
	skos:notation	"251069" ;
	skos:prefLabel	"Other Camelids"@en .

ccat:251070
	a	skos:Concept ;
	skos:broader	ccat:2510 ;
	skos:definition	"Small mammals in the family Leporidae."@en ;
	skos:inScheme	ccat: ;
	skos:notation	"251070" ;
	skos:prefLabel	"Rabbits"@en .

ccat:251079
	a	skos:Concept ;
	skos:broader	ccat:2510 ;
	skos:definition	"Any other rodents of economic value."@en ;
	skos:inScheme	ccat: ;
	skos:notation	"251079" ;
	skos:prefLabel	"Other Rodents"@en .

ccat:251090
	a	skos:Concept ;
	skos:broader	ccat:2510 ;
	skos:definition	"Any other live animals."@en ;
	skos:inScheme	ccat: ;
	skos:notation	"251090" ;
	skos:prefLabel	"Other Live Animals"@en .

ccat:251095
	a	skos:Concept ;
	skos:broader	ccat:2510 ;
	skos:definition	"Any other live animals not kept for food."@en ;
	skos:inScheme	ccat: ;
	skos:notation	"251095" ;
	skos:prefLabel	"Other Non-Food Live Animals"@en .

ccat:2520
	a	skos:Concept ;
	skos:broader	ccat:20 ;
	skos:definition	"Animal fats and oils are lipids derived from animals: oils are liquid at room temperature, and fats are solid."@en ;
	skos:inScheme	ccat: ;
	skos:notation	"2520" ;
	skos:prefLabel	"Animal Oils and Fats"@en .

ccat:252010
	a	skos:Concept ;
	skos:altLabel	"Beef Tallow"@en ;
	skos:broader	ccat:2520 ;
	skos:definition	"Rendered beef fat."@en ;
	skos:inScheme	ccat: ;
	skos:notation	"252010" ;
	skos:prefLabel	"Fat of Cattle"@en .

ccat:252015
	a	skos:Concept ;
	skos:broader	ccat:2520 ;
	skos:definition	"Rendered fat of the buffalo."@en ;
	skos:inScheme	ccat: ;
	skos:notation	"252015" ;
	skos:prefLabel	"Fat of Buffalo"@en .

ccat:252020
	a	skos:Concept ;
	skos:altLabel	"Mutton Tallow"@en ;
	skos:broader	ccat:2520 ;
	skos:definition	"Rendered mutton fat."@en ;
	skos:inScheme	ccat: ;
	skos:notation	"252020" ;
	skos:prefLabel	"Fat of Sheep"@en .

ccat:252025
	a	skos:Concept ;
	skos:broader	ccat:2520 ;
	skos:definition	"Rendered fatty tissue of a goat."@en ;
	skos:inScheme	ccat: ;
	skos:notation	"252025" ;
	skos:prefLabel	"Fat of Goats"@en .

ccat:252030
	a	skos:Concept ;
	skos:altLabel	"Lard"@en ;
	skos:broader	ccat:2520 ;
	skos:definition	"Rendered fatty tissue of a pig."@en ;
	skos:inScheme	ccat: ;
	skos:notation	"252030" ;
	skos:prefLabel	"Fat of Pigs"@en .

ccat:252040
	a	skos:Concept ;
	skos:broader	ccat:2520 ;
	skos:definition	"Rendered fat of, typically, waterfowl, e.g. ducks and geese."@en ;
	skos:inScheme	ccat: ;
	skos:notation	"252040" ;
	skos:prefLabel	"Fat of Poultry"@en .

ccat:252060
	a	skos:Concept ;
	skos:broader	ccat:2520 ;
	skos:definition	"Rendered hump of a camel."@en ;
	skos:inScheme	ccat: ;
	skos:notation	"252060" ;
	skos:prefLabel	"Fat of Camels"@en .

ccat:252069
	a	skos:Concept ;
	skos:broader	ccat:2520 ;
	skos:definition	"Rendering of fatty tissue of any other member of Camelidae."@en ;
	skos:inScheme	ccat: ;
	skos:notation	"252069" ;
	skos:prefLabel	"Fat of Other Camelids"@en .

ccat:252080
	a	skos:Concept ;
	skos:broader	ccat:2520 ;
	skos:definition	"Rendered tissue of oily fish, e.g. tuna or salmon."@en ;
	skos:inScheme	ccat: ;
	skos:notation	"252080" ;
	skos:prefLabel	"Oil of Oily Fish"@en .

ccat:252090
	a	skos:Concept ;
	skos:broader	ccat:2520 ;
	skos:definition	"Rendering of fatty tissue of any other animal."@en ;
	skos:inScheme	ccat: ;
	skos:notation	"252090" ;
	skos:prefLabel	"Other Animal Fats"@en .

ccat:2530
	a	skos:Concept ;
	skos:broader	ccat:20 ;
	skos:closeMatch	agrovoc:c_4669 , eurovoc:4681 , stw:14122-2 ;
	skos:definition	"Edible products from slaughtered animals, such as meat, offal, and bones, excluding edible or inedible products used as material, e.g. skins and hides."@en ;
	skos:exactMatch	<https://www.trade-tariff.service.gov.uk/chapters/02> ;
	skos:inScheme	ccat: ;
	skos:notation	"2530" ;
	skos:prefLabel	"Food from Slaughtered Animals"@en ;
	skos:scopeNote	"Meat here refers to skeletal muscle, associated fat, and other edible tissues such as offal. Also includes animals that have not been domesticated or raised and prepared for human consumption, like game, insects, fish, seafood, and snails."@en .

ccat:253010
	a	skos:Concept ;
	skos:altLabel	"Beef"@en ;
	skos:broader	ccat:2530 ;
	skos:definition	"Meat from cattle, particularly skeletal muscle."@en ;
	skos:exactMatch	agrovoc:c_861 , eurovoc:4682 , stw:18220-3 , wd:Q192628 ;
	skos:inScheme	ccat: ;
	skos:notation	"253010" ;
	skos:note	"""Beef is the third most widely consumed meat in the world, accounting for about 25% of meat production worldwide, after pork and poultry at 38% and 30% respectively. In absolute numbers, the United States, Brazil, and the People's Republic of China are the world's three largest consumers of beef; Uruguay, however, has the highest beef and veal consumption per capita, followed by Argentina and Brazil. According to the data from OECD, the average Uruguayan ate over 42 kg (93 lb) of beef or veal in 2014, representing the highest beef/veal consumption per capita in the world. In comparison, the average American consumed only about 24 kg (53 lb) beef or veal in the same year, while African countries, such as Mozambique, Ghana, and Nigeria, consumed the least beef or veal per capita.

In 2018, the United States, Brazil, and China produced the most beef with 12.22 million tons, 9.9 million tons, and 6.46 million tons respectively. The top 3 beef exporting countries in 2019 were Australia (14.8% of total exports), the United States (13.4% of total exports), and Brazil (12.6% of total exports). Beef production is also important to the economies of Japan, Argentina, Uruguay, Canada, Paraguay, Mexico, Belarus and Nicaragua.

Beef production has a high environmental impact per gram of protein."""@en ;
	skos:prefLabel	"Meat of Cattle"@en ;
	skos:related	<https://www.trade-tariff.service.gov.uk/headings/0201> , <https://www.trade-tariff.service.gov.uk/headings/0202> .

ccat:253015
	a	skos:Concept ;
	skos:altLabel	"Buff"@en , "Red Beef"@en ;
	skos:broader	ccat:2530 ;
	skos:definition	"Meat of the water buffalo."@en ;
	skos:exactMatch	agrovoc:c_23996 , eurovoc:4685 , wd:Q23808610 ;
	skos:inScheme	ccat: ;
	skos:notation	"253015" ;
	skos:note	"""Buffalo have exceptional muscular development and thus they are considerably heavy, with some weighing more than a tonne. The main agricultural use of buffalo is to obtain milk. India has the largest number of buffalo and is the largest producer of its milk, producing nearly 57 million tonnes of it annually. This accounts for 67% of global production. Slaughtering buffalo for meat is a secondary agricultural priority.

Buffalo meat from young buffalo has a much better quality as they have a higher proportion of muscle and a lower proportion of fat as compared to other cattle meat. The highest quality buffalo meat is known as \"padwa\" in India, taken from a buffalo younger than 24 months.

India accounts for about 43% of the world buffalo meat production, with Uttar Pradesh producing the most, followed by Andhra Pradesh and Maharashtra. In the 21st century, buffalo meat production in India has been growing and has increased from 4.1 million tonnes CWE (carcass weight equivalent) in 2014 to 4.3 million tonnes CWE in 2015.

In India, during the calendar year 2014-2015, consumption estimates had been forecasted to rise from 3.1% and 3.5% to 2.1 and 2.175 million tonnes CWE respectively, according to the US Department of Agriculture."""@en ;
	skos:prefLabel	"Buffalo Meat"@en ;
	skos:related	<https://www.trade-tariff.service.gov.uk/headings/0201> , <https://www.trade-tariff.service.gov.uk/headings/0202> .

ccat:253020
	a	skos:Concept ;
	skos:altLabel	"Mutton"@en ;
	skos:broader	ccat:2530 ;
	skos:definition	"Meat of domestic sheep (Ovis aries)."@en ;
	skos:exactMatch	agrovoc:c_5015 , stw:19021-4 , wd:Q14566073 ;
	skos:inScheme	ccat: ;
	skos:notation	"253020" ;
	skos:prefLabel	"Meat of Sheep"@en ;
	skos:related	<https://www.trade-tariff.service.gov.uk/headings/0204> ;
	skos:scopeNote	"A sheep in its first year is a lamb and its meat is also lamb. A sheep in its second year and its meat are hogget. Older sheep meat is mutton. In South Asian and Caribbean cuisine, \"mutton\" often means goat meat. At various times and places, \"mutton\" or \"goat mutton\" has occasionally been used to mean goat meat."@en .

ccat:253025
	a	skos:Concept ;
	skos:broader	ccat:2530 ;
	skos:definition	"Meat of the domestic goat (Capra aegagrus hircus)."@en ;
	skos:exactMatch	agrovoc:c_15978 , wd:Q449506 ;
	skos:inScheme	ccat: ;
	skos:notation	"253025" ;
	skos:prefLabel	"Goat Meat"@en ;
	skos:related	<https://www.trade-tariff.service.gov.uk/headings/0204> ;
	skos:scopeNote	"The common name for goat meat is simply \"goat\", though meat from adult goats is referred to as chevon, while that from young goats can be called capretto (It.), cabrito (Sp.) or kid. In South Asian and Caribbean cuisine, mutton commonly means goat meat. In South Asia, where mutton curry is popular, \"mutton\" is used for both goat and lamb meat. The United States Department of Agriculture promoted the term \"chevon\", a portmanteau of chvre ('goat') and mouton ('sheep', 'mutton') in the 1920s. According to market research, consumers in the United States prefer the pseudo-French-language-derived culinary name \"chevon\". \"Cabrito\", a word of Spanish and Portuguese origin, refers specifically to the meat of a young, milk-fed goat. It is also known as chivo."@en .

ccat:253030
	a	skos:Concept ;
	skos:altLabel	"Pork"@en ;
	skos:broader	ccat:2530 ;
	skos:definition	"Meat of the domestic pig (Sus scrofa domesticus)."@en ;
	skos:exactMatch	agrovoc:c_6120 , eurovoc:4692 , stw:18219-2 , wd:Q191768 ;
	skos:inScheme	ccat: ;
	skos:notation	"253030" ;
	skos:note	"""It is the most commonly consumed meat worldwide, with evidence of pig husbandry dating back to 5000 BC.

Pork is not only the most popular meat in the Western world and in Central Europe, it is also very popular in East Asia, the non-Muslim parts of India, Southeast Asia (Indochina, Philippines, Singapore, East Timor) and in Malaysia. It is highly prized in Asian cuisines, especially in China, for its fat content and texture."""@en ;
	skos:prefLabel	"Pig Meat"@en ;
	skos:related	<https://www.trade-tariff.service.gov.uk/headings/0203> .

ccat:253040
	a	skos:Concept ;
	skos:broader	ccat:2530 ;
	skos:definition	"Meat of the domestic chicken (Gallus gallus domesticus)."@en ;
	skos:exactMatch	agrovoc:c_24000 , wd:Q864693 ;
	skos:inScheme	ccat: ;
	skos:notation	"253040" ;
	skos:note	"""The United Nations estimates there to be 19 billion chickens on Earth today, making them outnumber humans more than two to one."""@en ;
	skos:prefLabel	"Chicken Meat"@en ;
	skos:related	<https://www.trade-tariff.service.gov.uk/headings/0207> .

ccat:253042
	a	skos:Concept ;
	skos:broader	ccat:2530 ;
	skos:definition	"Meat from turkeys, typically domesticated turkeys but also wild turkeys."@en ;
	skos:exactMatch	agrovoc:c_24096 , wd:Q4200953 ;
	skos:inScheme	ccat: ;
	skos:notation	"253042" ;
	skos:note	"""It is a popular poultry dish, especially in North America, where it is traditionally consumed as part of culturally significant events such as Thanksgiving and Christmas, as well as in standard cuisine."""@en ;
	skos:prefLabel	"Turkey Meat"@en ;
	skos:related	<https://www.trade-tariff.service.gov.uk/headings/0207> .

ccat:253045
	a	skos:Concept ;
	skos:broader	ccat:2530 ;
	skos:definition	"Meat of several species of bird in the family Anatidae."@en ;
	skos:exactMatch	agrovoc:c_24021 , wd:Q542042 ;
	skos:inScheme	ccat: ;
	skos:notation	"253045" ;
	skos:note	"""Duck is particularly predominant in the Chinese cuisine, partly in the (Northeast) Indian cuisine, and in a variety of dishes around the world. Some dishes use parts of the duck as an ingredient along with other ingredients."""@en ;
	skos:prefLabel	"Duck Meat"@en ;
	skos:related	<https://www.trade-tariff.service.gov.uk/headings/0207> .

ccat:253047
	a	skos:Concept ;
	skos:broader	ccat:2530 ;
	skos:definition	"Goose is the meat of domesticated or wild geese."@en ;
	skos:exactMatch	agrovoc:c_24034 , wd:Q46976697 ;
	skos:inScheme	ccat: ;
	skos:notation	"253047" ;
	skos:note	"""Goose is used traditionally in the French, Polish, and Baltic cuisines, particularly during the Christmas season."""@en ;
	skos:prefLabel	"Goose Meat"@en ;
	skos:related	<https://www.trade-tariff.service.gov.uk/headings/0207> .

ccat:253048
	a	skos:Concept ;
	skos:altLabel	"Squab"@en ;
	skos:broader	ccat:2530 ;
	skos:definition	"Meat of domestic pigeons, or more broadly of all dove and pigeon species."@en ;
	skos:exactMatch	wd:Q7581884 ;
	skos:inScheme	ccat: ;
	skos:notation	"253048" ;
	skos:note	"""The modern squab industry uses utility pigeons. Squabs are raised until they are roughly a month old, when they reach adult size but have not yet flown, before being slaughtered."""@en ;
	skos:prefLabel	"Meat of Pigeons"@en ;
	skos:related	<https://www.trade-tariff.service.gov.uk/commodities/0208901000> , agrovoc:c_6147 .

ccat:253049
	a	skos:Concept ;
	skos:broader	ccat:2530 ;
	skos:definition	"Meat from other birds bred or hunted for consumption, such as quail, ostrich, Guinea fowl, etc."@en ;
	skos:inScheme	ccat: ;
	skos:notation	"253049" ;
	skos:prefLabel	"Meat of Other Birds"@en .

ccat:253050
	a	skos:Concept ;
	skos:broader	ccat:2530 ;
	skos:definition	"Meat from domestic horses (Equus ferus caballus)."@en ;
	skos:exactMatch	agrovoc:c_15983 , wd:Q1124327 ;
	skos:inScheme	ccat: ;
	skos:notation	"253050" ;
	skos:note	"""Horse meat forms a significant part of the culinary traditions of many countries, particularly in Europe and Asia. The eight countries that consume the most horse meat consume about 4.3 million horses a year.

Jurisdictions that allow for the slaughter of horses for food rarely have age restrictions, so many are quite young, some even as young as 16 to 24 months old. They are processed in a similar fashion to cattle, i.e., in large-scale factory slaughter houses (abattoirs) where they are stunned with a captive bolt gun and bled to death. In countries with a less industrialized food-production system, horses and other animals are slaughtered individually outdoors as needed, in or near the village where they will be consumed."""@en ;
	skos:prefLabel	"Horse Meat"@en ;
	skos:related	<https://www.trade-tariff.service.gov.uk/headings/0205> .

ccat:253055
	a	skos:Concept ;
	skos:broader	ccat:2530 ;
	skos:definition	"Meat from domestic asses (Equus africanus asinus)."@en ;
	skos:exactMatch	agrovoc:c_24021 ;
	skos:inScheme	ccat: ;
	skos:notation	"253055" ;
	skos:prefLabel	"Meat of Asses"@en ;
	skos:related	<https://www.trade-tariff.service.gov.uk/headings/0205> .

ccat:253058
	a	skos:Concept ;
	skos:broader	ccat:2530 ;
	skos:definition	"Meat from mules (Equus africanus asinus x Equus ferus caballus)."@en ;
	skos:inScheme	ccat: ;
	skos:notation	"253058" ;
	skos:prefLabel	"Meat of Mules"@en ;
	skos:related	<https://www.trade-tariff.service.gov.uk/headings/0205> .

ccat:253060
	a	skos:Concept ;
	skos:broader	ccat:2530 ;
	skos:definition	"Meat from camels (species in the genus Camelus)."@en ;
	skos:exactMatch	agrovoc:c_23998 ;
	skos:inScheme	ccat: ;
	skos:notation	"253060" ;
	skos:prefLabel	"Meat of Camels"@en ;
	skos:related	<https://www.trade-tariff.service.gov.uk/commodities/0208600000> .

ccat:253069
	a	skos:Concept ;
	skos:broader	ccat:2530 ;
	skos:definition	"Meat from any other camelids (species in the family Camelidae)."@en ;
	skos:inScheme	ccat: ;
	skos:notation	"253069" ;
	skos:prefLabel	"Meat of other Domestic Camelids"@en ;
	skos:related	<https://www.trade-tariff.service.gov.uk/commodities/0208600000> .

ccat:253070
	a	skos:Concept ;
	skos:broader	ccat:2530 ;
	skos:definition	"Meat from animals in the family Leporidae."@en ;
	skos:inScheme	ccat: ;
	skos:notation	"253070" ;
	skos:prefLabel	"Rabbit Meat"@en .

ccat:253079
	a	skos:Concept ;
	skos:broader	ccat:2530 ;
	skos:definition	"Meat from domestic animals in the order Rodentia, excluding non-domestic but indigenous animals (cf. 253540 Indigenous Meat)."@en ;
	skos:inScheme	ccat: ;
	skos:notation	"253079" ;
	skos:prefLabel	"Meat of other Domestic Rodents"@en .

ccat:253080
	a	skos:Concept ;
	dct:isReplacedBy	ccat:25501010 ;
	skos:broader	ccat:2530 ;
	skos:definition	"Saltwater fish in the tribe Thunnini that has been gutted and put on ice."@en ;
	skos:inScheme	ccat: ;
	skos:notation	"253080" ;
	skos:prefLabel	"Gutted Iced Tuna"@en .

ccat:253085
	a	skos:Concept ;
	dct:isReplacedBy	ccat:25501020 ;
	skos:broader	ccat:2530 ;
	skos:definition	"Several species in the family Salmonidae that have been gutted and put on ice."@en ;
	skos:inScheme	ccat: ;
	skos:notation	"253085" ;
	skos:prefLabel	"Gutted Iced Salmon"@en .

ccat:253089
	a	skos:Concept ;
	dct:isReplacedBy	ccat:25501090 ;
	skos:broader	ccat:2530 ;
	skos:definition	"Any other oily fish that has been gutted and put on ice."@en ;
	skos:inScheme	ccat: ;
	skos:notation	"253089" ;
	skos:prefLabel	"Other Gutted Iced Oily Fish"@en .

ccat:253090
	a	skos:Concept ;
	skos:broader	ccat:2530 ;
	skos:definition	"Meat from any other animals."@en ;
	skos:inScheme	ccat: ;
	skos:notation	"253090" ;
	skos:prefLabel	"Other Meat"@en .

ccat:253095
	a	skos:Concept ;
	skos:broader	ccat:2530 ;
	skos:definition	"Viscera (internal organs) and entrails of a butchered animal."@en ;
	skos:inScheme	ccat: ;
	skos:notation	"253095" ;
	skos:prefLabel	"Offal"@en .

ccat:2535
	a	skos:Concept ;
	skos:broader	ccat:20 ;
	skos:definition	"Fresh meat or meat that has been reduced to fragments which has had foodstuffs, seasonings or additives added to it or which has undergone processes."@en ;
	skos:inScheme	ccat: ;
	skos:notation	"2535" ;
	skos:prefLabel	"Meat Products and Meat Preparations"@en ;
	skos:scopeNote	"Meat preparations defined in EC No 853/2004"@en .

ccat:253510
	a	skos:Concept ;
	skos:broader	ccat:2535 ;
	skos:definition	"Meat that has been dehydrated, i.e. hot-air-dried or cured with salt. Freeze-dried meat is to be considered fresh."@en ;
	skos:inScheme	ccat: ;
	skos:notation	"253510" ;
	skos:prefLabel	"Dried Meat"@en .

ccat:253520
	a	skos:Concept ;
	skos:altLabel	"MBM"@en ;
	skos:broader	ccat:2535 ;
	skos:definition	"Residue of fat extraction (by rendering)."@en ;
	skos:inScheme	ccat: ;
	skos:notation	"253520" ;
	skos:prefLabel	"Meat and Bone Meal"@en .

ccat:253525
	a	skos:Concept ;
	skos:broader	ccat:2535 ;
	skos:definition	"Blood that has been dehydrated, i.e. hot-air-dried, drum dried, flash dried, or spray dried."@en ;
	skos:inScheme	ccat: ;
	skos:notation	"253525" ;
	skos:prefLabel	"Blood Meal"@en .

ccat:253540
	a	skos:Concept ;
	skos:altLabel	"Bushmeat"@en ;
	skos:broader	ccat:2535 ;
	skos:definition	"Meat or meat products or meat preparations from wildlife species that are hunted rather than grown."@en ;
	skos:inScheme	ccat: ;
	skos:notation	"253540" ;
	skos:prefLabel	"Indigenous Meat"@en .

ccat:253550
	a	skos:Concept ;
	skos:altLabel	"Organic Meat"@en ;
	skos:broader	ccat:2535 ;
	skos:definition	"Meat or meat products or meat preparations from animals that have been bred and grown under natural living conditions and feed."@en ;
	skos:inScheme	ccat: ;
	skos:notation	"253550" ;
	skos:prefLabel	"Biological Meat"@en ;
	skos:scopeNote	"Distinct from Indigenous Meat (253540) in that animals are deliberately kept for meat production."@en .

ccat:253590
	a	skos:Concept ;
	skos:broader	ccat:2535 ;
	skos:definition	"Any other meat products or meat preparations."@en ;
	skos:inScheme	ccat: ;
	skos:notation	"253590" ;
	skos:prefLabel	"Other Meat Preparations"@en .

ccat:2540
	a	skos:Concept ;
	skos:broader	ccat:20 ;
	skos:definition	"Produce sourced from animals without slaughtering them."@en ;
	skos:inScheme	ccat: ;
	skos:notation	"2540" ;
	skos:prefLabel	"Food from Live Animals"@en .

ccat:254010
	a	skos:Concept ;
	skos:broader	ccat:2540 ;
	skos:definition	"Raw cow milk with all its constituents that is not concentrated, pasteurized, sterilized or other-wise preserved, homogenized or peptonized."@en ;
	skos:inScheme	ccat: ;
	skos:notation	"254010" ;
	skos:prefLabel	"Cow Milk"@en .

ccat:25401010
	a	skos:Concept ;
	skos:broader	ccat:254010 ;
	skos:definition	"Milk in which the fat content is adjusted to a predetermined value without altering any other constituents."@en ;
	skos:inScheme	ccat: ;
	skos:notation	"25401010" ;
	skos:prefLabel	"Standardized Milk"@en .

ccat:25401011
	a	skos:Concept ;
	skos:broader	ccat:254010 ;
	skos:definition	"Milk and cream from which water has been partly removed after heat-treating and concentrating. Normally sucrose is added to give the product stability and bacteriological safety."@en ;
	skos:inScheme	ccat: ;
	skos:notation	"25401011" ;
	skos:prefLabel	"Condensed Whole Milk"@en .

ccat:25401012
	a	skos:Concept ;
	skos:broader	ccat:254010 ;
	skos:definition	"Milk and cream from which the water has been partly removed and which has been heat- treated to render it bacteriologically safe and stable."@en ;
	skos:inScheme	ccat: ;
	skos:notation	"25401012" ;
	skos:prefLabel	"Evaporated Whole Milk"@en .

ccat:25401013
	a	skos:Concept ;
	skos:broader	ccat:254010 ;
	skos:definition	"Milk and cream from which water has been completely removed by various methods. In form of powder, granules or other solid forms. May contain added sugar or other sweeteners."@en ;
	skos:inScheme	ccat: ;
	skos:notation	"25401013" ;
	skos:prefLabel	"Dry Whole Cow Milk"@en .

ccat:25401015
	a	skos:Concept ;
	skos:broader	ccat:254010 ;
	skos:definition	"That portion of milk which is rich in milk fat and is separated by skimming or centrifuging."@en ;
	skos:inScheme	ccat: ;
	skos:notation	"25401015" ;
	skos:prefLabel	"Fresh Cream"@en .

ccat:25401016
	a	skos:Concept ;
	skos:broader	ccat:254010 ;
	skos:definition	"Emulsion of milk fat and water that is obtained by churning cream. Trade data cover butter from the milk of any animal."@en ;
	skos:inScheme	ccat: ;
	skos:notation	"25401016" ;
	skos:prefLabel	"Butter of Cow Milk"@en .

ccat:25401017
	a	skos:Concept ;
	skos:broader	ccat:254010 ;
	skos:definition	"Butter from which the water has been removed. Very common in hot countries. Includes also anhydrous butterfat or butter oil."@en ;
	skos:inScheme	ccat: ;
	skos:notation	"25401017" ;
	skos:prefLabel	"Ghee from Cow Milk"@en .

ccat:25401020
	a	skos:Concept ;
	skos:broader	ccat:254010 ;
	skos:definition	"Milk from which most of the fat has been removed."@en ;
	skos:inScheme	ccat: ;
	skos:notation	"25401020" ;
	skos:prefLabel	"Skim Milk of Cows"@en .

ccat:25401021
	a	skos:Concept ;
	skos:broader	ccat:254010 ;
	skos:definition	"Same as 25401011, but applied to skim milk."@en ;
	skos:inScheme	ccat: ;
	skos:notation	"25401021" ;
	skos:prefLabel	"Condensed Skim Milk"@en .

ccat:25401022
	a	skos:Concept ;
	skos:broader	ccat:254010 ;
	skos:definition	"Same as 25401012, but applied to skim milk."@en ;
	skos:inScheme	ccat: ;
	skos:notation	"25401022" ;
	skos:prefLabel	"Evaporated Skim Milk"@en .

ccat:25401023
	a	skos:Concept ;
	skos:broader	ccat:254010 ;
	skos:definition	"Same as 25401013, but from skim milk. Normally does not exceed 1.5% fat content."@en ;
	skos:inScheme	ccat: ;
	skos:notation	"25401023" ;
	skos:prefLabel	"Dry Skim Cow Milk"@en .

ccat:25401030
	a	skos:Concept ;
	skos:broader	ccat:254010 ;
	skos:definition	"Liquid part of the milk that remains after the separation of curd in cheese making."@en ;
	skos:exactMatch	agrovoc:c_8376 , wd:Q185009 ;
	skos:inScheme	ccat: ;
	skos:notation	"25401030" ;
	skos:note	"""Its main food use is in the preparation of whey cheese, whey drinks and fermented whey drinks. The main industrial uses are in the manufacture of lactose, whey paste and dried whey."""@en ;
	skos:prefLabel	"Fresh Whey"@en .

ccat:25401031
	a	skos:Concept ;
	skos:broader	ccat:254010 ;
	skos:definition	"Pasteurised fresh whey where some of the liquid has been evaporated in a vaccum."@en ;
	skos:inScheme	ccat: ;
	skos:notation	"25401031" ;
	skos:prefLabel	"Condensed Whey"@en .

ccat:25401033
	a	skos:Concept ;
	skos:altLabel	"Whey Powder"@en ;
	skos:broader	ccat:254010 ;
	skos:definition	"Condensed whey where all water has been removed."@en ;
	skos:exactMatch	agrovoc:c_24019 , wd:Q57656307 ;
	skos:inScheme	ccat: ;
	skos:notation	"25401033" ;
	skos:prefLabel	"Dry Whey"@en .

ccat:25401040
	a	skos:Concept ;
	skos:broader	ccat:254010 ;
	skos:definition	"Curd of milk that has been coagulated and separated from whey. May include some whole milk."@en ;
	skos:inScheme	ccat: ;
	skos:notation	"25401040" ;
	skos:prefLabel	"Cheese from Whole Cow Milk"@en .

ccat:25401042
	a	skos:Concept ;
	skos:broader	ccat:254010 ;
	skos:definition	"Curd of milk that has been coagulated and separated from whey. May include some skimmed milk."@en ;
	skos:inScheme	ccat: ;
	skos:notation	"25401042" ;
	skos:prefLabel	"Cheese From Skimmed Cow Milk"@en .

ccat:25401043
	a	skos:Concept ;
	skos:broader	ccat:254010 ;
	skos:definition	"Made from fresh whey by coagulating, e.g. by heat or acid."@en ;
	skos:inScheme	ccat: ;
	skos:notation	"25401043" ;
	skos:prefLabel	"Whey Cheese"@en .

ccat:25401045
	a	skos:Concept ;
	skos:broader	ccat:254010 ;
	skos:definition	"Made from cheese and unfermented dairy ingredients mixed with emulsifiers."@en ;
	skos:inScheme	ccat: ;
	skos:notation	"25401045" ;
	skos:prefLabel	"Processed Cheese"@en .

ccat:25401050
	a	skos:Concept ;
	skos:altLabel	"Curdled Milk"@en ;
	skos:broader	ccat:254010 ;
	skos:definition	"Milk inoculated with a culture of Lactococcus lactis or Lactobacillus bulgaricus plus Leuconostoc citrovorum."@en ;
	skos:inScheme	ccat: ;
	skos:notation	"25401050" ;
	skos:note	"""As most modern butter is not made with cultured cream but uncultured sweet cream, most modern buttermilk is cultured separately."""@en ;
	skos:prefLabel	"Buttermilk"@en .

ccat:25401053
	a	skos:Concept ;
	skos:broader	ccat:254010 ;
	skos:definition	"Buttermilk where water has been removed, e.g. by spray drying or roller drying."@en ;
	skos:inScheme	ccat: ;
	skos:notation	"25401053" ;
	skos:prefLabel	"Dry Buttermilk"@en .

ccat:25401055
	a	skos:Concept ;
	skos:broader	ccat:254010 ;
	skos:definition	"Milk inoculated with yoghurt cultures, may include additives such as sugar, flavouring materials, fruit or cocoa."@en ;
	skos:inScheme	ccat: ;
	skos:notation	"25401055" ;
	skos:prefLabel	"Unconcentrated Yoghurt"@en .

ccat:25401056
	a	skos:Concept ;
	skos:broader	ccat:254010 ;
	skos:definition	"Yoghurt where the whey has been removed by straining."@en ;
	skos:inScheme	ccat: ;
	skos:notation	"25401056" ;
	skos:prefLabel	"Concentrated Yoghurt"@en .

ccat:25401060
	a	skos:Concept ;
	skos:broader	ccat:254010 ;
	skos:definition	"Main sugar constituent of milk, obtained from whey permeate."@en ;
	skos:inScheme	ccat: ;
	skos:notation	"25401060" ;
	skos:note	"Lactose makes up 2%-8% of milk, or about 5% of whey solids."@en ;
	skos:prefLabel	"Lactose"@en .

ccat:25401065
	a	skos:Concept ;
	skos:broader	ccat:254010 ;
	skos:definition	"Main protein constituent of milk, obtained from skimmed milk by precipitation (curdling) with acids or rennet."@en ;
	skos:inScheme	ccat: ;
	skos:notation	"25401065" ;
	skos:prefLabel	"Casein"@en .

ccat:25401070
	a	skos:Concept ;
	skos:broader	ccat:254010 ;
	skos:definition	"Product obtained by adding water, fat, etc. to milk powder."@en ;
	skos:inScheme	ccat: ;
	skos:notation	"25401070" ;
	skos:prefLabel	"Reconstitued Milk"@en .

ccat:25401080
	a	skos:Concept ;
	skos:broader	ccat:254010 ;
	skos:definition	"Product that is included in Item 125 on the Import Control List (ICL)."@en ;
	skos:inScheme	ccat: ;
	skos:notation	"25401080" ;
	skos:prefLabel	"Products of Natural Milk Constituents"@en ;
	skos:related	<https://www.trade-tariff.service.gov.uk/commodities/0404900000> ;
	skos:scopeNote	"E.g. infant formula"@en .

ccat:25401085
	a	skos:Concept ;
	skos:broader	ccat:254010 ;
	skos:definition	"Milk or cream base with sweeteners, eggs, etc."@en ;
	skos:inScheme	ccat: ;
	skos:notation	"25401085" ;
	skos:prefLabel	"Ice Cream and Edible Ice"@en .

ccat:25401090
	a	skos:Concept ;
	skos:broader	ccat:254010 ;
	skos:definition	"Milk products not classified elsewhere."@en ;
	skos:inScheme	ccat: ;
	skos:notation	"25401090" ;
	skos:prefLabel	"Other Milk Products"@en .

ccat:254015
	a	skos:Concept ;
	skos:broader	ccat:2540 ;
	skos:definition	"Milk from water buffalo cows."@en ;
	skos:inScheme	ccat: ;
	skos:notation	"254015" ;
	skos:note	"""India and Pakistan produce the most buffalo milk worldwide."""@en ;
	skos:prefLabel	"Buffalo Milk"@en .

ccat:254016
	a	skos:Concept ;
	skos:broader	ccat:2540 ;
	skos:definition	"Milk from ewes."@en ;
	skos:inScheme	ccat: ;
	skos:notation	"254016" ;
	skos:prefLabel	"Sheep Milk"@en .

ccat:254017
	a	skos:Concept ;
	skos:broader	ccat:2540 ;
	skos:definition	"Milk from nannies."@en ;
	skos:inScheme	ccat: ;
	skos:notation	"254017" ;
	skos:prefLabel	"Goat Milk"@en .

ccat:254018
	a	skos:Concept ;
	skos:broader	ccat:2540 ;
	skos:definition	"Milk from camel cows."@en ;
	skos:inScheme	ccat: ;
	skos:notation	"254018" ;
	skos:prefLabel	"Camel Milk"@en .

ccat:254019
	a	skos:Concept ;
	skos:broader	ccat:2540 ;
	skos:definition	"Milk from any other female mammal."@en ;
	skos:inScheme	ccat: ;
	skos:notation	"254019" ;
	skos:prefLabel	"Other Milk"@en .

ccat:254020
	a	skos:Concept ;
	skos:altLabel	"Chicken Eggs"@en ;
	skos:broadMatch	stw:14121-4 ;
	skos:broader	ccat:2540 ;
	skos:definition	"Oval reproductive body of hens used as food."@en ;
	skos:exactMatch	agrovoc:c_2502 , wd:Q15260613 ;
	skos:inScheme	ccat: ;
	skos:notation	"254020" ;
	skos:note	"""In 2017, world production of chicken eggs was 80.1 million tonnes. The largest producers were China with 31.3 million of this total, the United States with 6.3 million, India at 4.8 million, Mexico at 2.8 million, Japan at 2.6 million, and Brazil and Russia with 2.5 million each."""@en ;
	skos:prefLabel	"Hen Eggs"@en .

ccat:254022
	a	skos:Concept ;
	skos:broader	ccat:2540 ;
	skos:definition	"Oval reproductive body of ducks used as food."@en ;
	skos:inScheme	ccat: ;
	skos:notation	"254022" ;
	skos:prefLabel	"Duck Eggs"@en .

ccat:254029
	a	skos:Concept ;
	skos:broader	ccat:2540 ;
	skos:definition	"Any other bird eggs."@en ;
	skos:inScheme	ccat: ;
	skos:notation	"254029" ;
	skos:prefLabel	"Other Bird Eggs"@en .

ccat:254030
	a	skos:Concept ;
	skos:broader	ccat:2540 ;
	skos:definition	"Honey produced by bees (Apis mellifera) or by other insects."@en ;
	skos:exactMatch	agrovoc:c_3652 , eurovoc:1907 , stw:14123-0 , wd:Q10987 ;
	skos:inScheme	ccat: ;
	skos:notation	"254030" ;
	skos:prefLabel	"Honey"@en .

ccat:2550
	a	skos:Concept ;
	skos:broader	ccat:20 ;
	skos:closeMatch	agrovoc:c_550 , eurovoc:2320 , stw:12969-3 ;
	skos:definition	"Food from the controlled cultivation of aquatic organisms."@en ;
	skos:inScheme	ccat: ;
	skos:notation	"2550" ;
	skos:prefLabel	"Food from Aquaculture"@en .

ccat:255010
	a	skos:Concept ;
	skos:broader	ccat:2550 ;
	skos:definition	"Oily fish that has been gutted and put on ice."@en ;
	skos:inScheme	ccat: ;
	skos:notation	"255010" ;
	skos:prefLabel	"Gutted Iced Oily Fish"@en .

ccat:25501010
	a	skos:Concept ;
	skos:broader	ccat:255010 ;
	skos:definition	"Saltwater fish in the tribe Thunnini that has been gutted and put on ice."@en ;
	skos:inScheme	ccat: ;
	skos:notation	"25501010" ;
	skos:prefLabel	"Gutted Iced Tuna"@en .

ccat:25501020
	a	skos:Concept ;
	skos:broader	ccat:255010 ;
	skos:definition	"Several species in the family Salmonidae that have been gutted and put on ice."@en ;
	skos:inScheme	ccat: ;
	skos:notation	"25501020" ;
	skos:prefLabel	"Gutted Iced Salmon"@en .

ccat:25501090
	a	skos:Concept ;
	skos:broader	ccat:255010 ;
	skos:definition	"Any other oily fish that has been gutted and put on ice."@en ;
	skos:inScheme	ccat: ;
	skos:notation	"25501090" ;
	skos:prefLabel	"Other Gutted Iced Oily Fish"@en .

ccat:255020
	a	skos:Concept ;
	skos:broader	ccat:2550 ;
	skos:definition	"Order of Crustaceans within the class Malacostraca whose meat is considered a delicacy."@en ;
	skos:inScheme	ccat: ;
	skos:notation	"255020" ;
	skos:prefLabel	"Decapoda"@en .

ccat:25502010
	a	skos:Concept ;
	skos:broader	ccat:255020 ;
	skos:definition	"Salt water crustaceans of the family Nephropidae."@en ;
	skos:inScheme	ccat: ;
	skos:notation	"25502010" ;
	skos:prefLabel	"Lobster"@en .

ccat:25502015
	a	skos:Concept ;
	skos:broader	ccat:255020 ;
	skos:definition	"Freshwater crustaceans of the family Astacidea."@en ;
	skos:inScheme	ccat: ;
	skos:notation	"25502015" ;
	skos:prefLabel	"Crayfish"@en .

ccat:25502020
	a	skos:Concept ;
	skos:broader	ccat:255020 ;
	skos:definition	"Decapod crustaceans of the infraorder Brachyura."@en ;
	skos:inScheme	ccat: ;
	skos:notation	"25502020" ;
	skos:prefLabel	"Crab"@en .

ccat:25502030
	a	skos:Concept ;
	skos:broader	ccat:255020 ;
	skos:definition	"Decapod crustaceans of the suborder Dendrobranchiata."@en ;
	skos:inScheme	ccat: ;
	skos:notation	"25502030" ;
	skos:prefLabel	"Prawn"@en .

ccat:25502035
	a	skos:Concept ;
	skos:broader	ccat:255020 ;
	skos:definition	"Decapod crustaceans of the family Crangonidae."@en ;
	skos:inScheme	ccat: ;
	skos:notation	"25502035" ;
	skos:prefLabel	"Shrimp"@en .

ccat:30
	a	skos:Concept ;
	skos:closeMatch	agrovoc:c_92337 ;
	skos:definition	"Commodities used as inputs to manufacturing processes to produce prodcts or more complex materials."@en ;
	skos:inScheme	ccat: ;
	skos:notation	"30" ;
	skos:note	"""Materials can be classified based on their physical and chemical properties, or on their geological origin or biological function.

Raw materials can be processed in different ways to influence their properties, by purification, shaping or the introduction of other materials. New materials can be produced from raw materials by synthesis."""@en ;
	skos:prefLabel	"Materials"@en ;
	skos:related	agrovoc:c_330705 ;
	skos:topConceptOf	ccat: .

ccat:3010
	a	skos:Concept ;
	skos:broader	ccat:30 ;
	skos:definition	"Plants or plant parts that are primarily harvested for their fibre, or fibre products of vegetal origin."@en ;
	skos:exactMatch	agrovoc:c_5966 ;
	skos:inScheme	ccat: ;
	skos:notation	"3010" ;
	skos:prefLabel	"Fibres of Vegetal Origin"@en .

ccat:301010
	a	skos:Concept ;
	skos:broader	ccat:3010 ;
	skos:definition	"Soft, fluffy fibre from the boll of the plants of the genus Gossypium in the mallow family Malvaceae."@en ;
	skos:exactMatch	agrovoc:c_1926 , eurovoc:252 , stw:14055-5 , wd:Q11457 ;
	skos:inScheme	ccat: ;
	skos:notation	"301010" ;
	skos:note	"""The plant is a shrub native to tropical and subtropical regions around the world, including the Americas, Africa, Egypt and India. The greatest diversity of wild cotton species is found in Mexico, followed by Australia and Africa. Cotton was independently domesticated in the Old and New Worlds.

Current estimates for world production are about 25 million tonnes or 110 million bales annually, accounting for 2.5% of the world's arable land. India is the world's largest producer of cotton. The United States has been the largest exporter for many years. In the United States, cotton is usually measured in bales, which measure approximately 0.48 cubic meters (17 cubic feet) and weigh 226.8 kilograms (500 pounds)."""@en ;
	skos:prefLabel	"Cotton Lint"@en .

ccat:301020
	a	skos:Concept ;
	skos:broader	ccat:3010 ;
	skos:definition	"Fibre extracted from the bast beneath the surface of the stem of the flax plant."@en ;
	skos:exactMatch	agrovoc:c_2970 , eurovoc:1667 , stw:14057-1 , wd:Q47089651 ;
	skos:inScheme	ccat: ;
	skos:notation	"301020" ;
	skos:note	"""The best grades are used for fabrics such as damasks, lace, and sheeting. Coarser grades are used for the manufacturing of twine and rope, and historically, for canvas and webbing equipment."""@en ;
	skos:prefLabel	"Flax Fibre and Tow"@en .

ccat:301025
	a	skos:Concept ;
	skos:broader	ccat:3010 ;
	skos:closeMatch	agrovoc:c_2970 , eurovoc:1667 , stw:14057-1 , wd:Q47089651 ;
	skos:definition	"Retted (or unretted) stalks of the flax plant (Linum usitatissimum)."@en ;
	skos:inScheme	ccat: ;
	skos:notation	"301025" ;
	skos:prefLabel	"Flax Raw or Retted"@en .

ccat:301030
	a	skos:Concept ;
	skos:broader	ccat:3010 ;
	skos:definition	"Fibre extracted from the bast of the cultivars of Cannabis sativa."@en ;
	skos:exactMatch	agrovoc:c_3558 , eurovoc:5384 , stw:19017-2 , wd:Q13414920 ;
	skos:inScheme	ccat: ;
	skos:notation	"301030" ;
	skos:note	"""Hemp is used in a number of consumer goods, including clothing, shoes, accessories, dog collars, and home wares. For clothing, in some instances, hemp is mixed with lyocell."""@en ;
	skos:prefLabel	"Hemp Fibre and Tow"@en .

ccat:301040
	a	skos:Concept ;
	skos:broader	ccat:3010 ;
	skos:definition	"Fibre extracted from the bast of plants in the genus Corchorus, primarily Corchorus olitorius, or alternatively Corchorus capsularis."@en ;
	skos:exactMatch	agrovoc:c_4065 , eurovoc:1554 , stw:14063-6 , wd:Q107211 ;
	skos:inScheme	ccat: ;
	skos:notation	"301040" ;
	skos:note	"""Jute is one of the most affordable natural fibres, and second only to cotton in the amount produced and variety of uses. Jute is also called the \"golden fiber\" for its colour and high cash value."""@en ;
	skos:prefLabel	"Jute Fibre"@en .

ccat:301045
	a	skos:Concept ;
	skos:broader	ccat:3010 ;
	skos:definition	"Fibre that shares most of the mechanical properties and the look of jute."@en ;
	skos:inScheme	ccat: ;
	skos:notation	"301045" ;
	skos:prefLabel	"Jute-like Fibre"@en .

ccat:301048
	a	skos:Concept ;
	skos:altLabel	"Manila Hemp"@en ;
	skos:broader	ccat:3010 ;
	skos:definition	"Fibre extracted from the leaf-stems of Musa textilis."@en ;
	skos:exactMatch	agrovoc:c_4 , wd:Q1814695 ;
	skos:inScheme	ccat: ;
	skos:notation	"301048" ;
	skos:note	"""The name refers to the capital of the Philippines, one of the main producers of Manila hemp. The hatmaking straw made from Manila hemp is called tagal or tagal straw."""@en ;
	skos:prefLabel	"Abaca"@en .

ccat:301050
	a	skos:Concept ;
	skos:broader	ccat:3010 ;
	skos:definition	"Decorticated leaf stems or fibre extracted from the leaf-stems of Agave sisalana, possibly dried, brushed and baled."@en ;
	skos:exactMatch	agrovoc:c_7086 , eurovoc:4173 , wd:Q847423 ;
	skos:inScheme	ccat: ;
	skos:notation	"301050" ;
	skos:prefLabel	"Sisal"@en .

ccat:301059
	a	skos:Concept ;
	skos:broader	ccat:3010 ;
	skos:definition	"Any other fibre extracted from the leaf-stems of agaves."@en ;
	skos:inScheme	ccat: ;
	skos:notation	"301059" ;
	skos:prefLabel	"Other Agave Fibres"@en .

ccat:301060
	a	skos:Concept ;
	skos:broader	ccat:3010 ;
	skos:definition	"Fibre obtained of the seed pods of Ceiba pentandra."@en ;
	skos:exactMatch	agrovoc:c_16497 , eurovoc:1556 , wd:Q1728687 ;
	skos:inScheme	ccat: ;
	skos:notation	"301060" ;
	skos:note	"""In Spanish speaking countries the tree is commonly known as \"ceiba\". The tree is cultivated for the seed fibre, particularly in south-east Asia, and is also known as the Java cotton, Java kapok, silk-cotton or samauma.

The fibre is light, very buoyant, resilient, resistant to water, but very flammable. The process of harvesting and separating the fiber is labour-intensive and menial. It is difficult to spin, but is used as an alternative to down as filling in mattresses, pillows, upholstery, zafus, and stuffed toys such as teddy bears, and for insulation."""@en ;
	skos:prefLabel	"Kapok Fibre"@en .

ccat:301070
	a	skos:Concept ;
	skos:broader	ccat:3010 ;
	skos:definition	"Decorticated leaf stems or fibre obtained from the inner bark (phloem) of the vegetative stalks of the Ramie plant, possibly degummed."@en ;
	skos:exactMatch	agrovoc:c_6442 , wd:Q2130134 ;
	skos:inScheme	ccat: ;
	skos:notation	"301070" ;
	skos:note	"""The dry weight of harvested stem from crops ranges from 3.4 to 4.5 t/ha/a. A 4.5-ton crop yields 1,600 kg/ha/a of dry undegummed fibre. The weight loss during degumming can be up to 25%, giving a yield of degummed fibre of about 1,200 kg/ha/a."""@en ;
	skos:prefLabel	"Ramie"@en .

ccat:301080
	a	skos:Concept ;
	skos:broader	ccat:3010 ;
	skos:definition	"Fibre extracted from the outer husk of coconut."@en ;
	skos:exactMatch	agrovoc:c_1734 , wd:Q1029620 ;
	skos:inScheme	ccat: ;
	skos:notation	"301080" ;
	skos:prefLabel	"Coir"@en .

ccat:301090
	a	skos:Concept ;
	skos:broader	ccat:3010 ;
	skos:definition	"Any other fibre of vegetal origin."@en ;
	skos:inScheme	ccat: ;
	skos:notation	"301090" ;
	skos:prefLabel	"Other Crop Fibre"@en .

ccat:3015
	a	skos:Concept ;
	skos:broader	ccat:30 ;
	skos:definition	"Fibres that are produced by animals. Most notably they comprise bristles, hair, wool, and silk."@en ;
	skos:exactMatch	agrovoc:c_430 ;
	skos:inScheme	ccat: ;
	skos:notation	"3015" ;
	skos:prefLabel	"Fibres of Animal Origin"@en .

ccat:301510
	a	skos:Concept ;
	skos:broader	ccat:3015 ;
	skos:definition	"Wool straight off a sheep, i.e. unscoured."@en ;
	skos:inScheme	ccat: ;
	skos:notation	"301510" ;
	skos:prefLabel	"Greasy Wool"@en .

ccat:301515
	a	skos:Concept ;
	skos:broader	ccat:3015 ;
	skos:definition	"Wool of the shoulder and sides, less than 20 microns in diameter."@en ;
	skos:inScheme	ccat: ;
	skos:notation	"301515" ;
	skos:prefLabel	"Fine Hair"@en .

ccat:301520
	a	skos:Concept ;
	skos:broader	ccat:3015 ;
	skos:definition	"Hair of goat with diameters >30 microns."@en ;
	skos:inScheme	ccat: ;
	skos:notation	"301520" ;
	skos:prefLabel	"Coarse Goat Hair"@en .

ccat:301525
	a	skos:Concept ;
	skos:broader	ccat:3015 ;
	skos:definition	"Hair of goat with diameters <30 microns."@en ;
	skos:inScheme	ccat: ;
	skos:notation	"301525" ;
	skos:prefLabel	"Fine Goat Hair"@en .

ccat:301530
	a	skos:Concept ;
	skos:broader	ccat:3015 ;
	skos:definition	"Long hair growing on the manes and tails of horses."@en ;
	skos:inScheme	ccat: ;
	skos:notation	"301530" ;
	skos:prefLabel	"Hair of Horses"@en .

ccat:301540
	a	skos:Concept ;
	skos:broader	ccat:3015 ;
	skos:definition	"Cocoons of the silkworm (Bombyx mori)."@en ;
	skos:inScheme	ccat: ;
	skos:notation	"301540" ;
	skos:prefLabel	"Reelable Cocoons"@en .

ccat:301590
	a	skos:Concept ;
	skos:broader	ccat:3015 ;
	skos:definition	"Other hair of animal origin."@en ;
	skos:inScheme	ccat: ;
	skos:notation	"301590" ;
	skos:prefLabel	"Other Hair"@en .

ccat:3020
	a	skos:Concept ;
	skos:broader	ccat:20 ;
	skos:definition	"Oleochemicals are products derived from vegetal oils and fats, e.g. by hydrolysis, transesterification, or hydrogenation."@en ;
	skos:inScheme	ccat: ;
	skos:notation	"3020" ;
	skos:prefLabel	"Oleochemicals"@en .

ccat:302010
	a	skos:Concept ;
	skos:altLabel	"FAME"@en , "Fatty Acid Methyl Ester"@en ;
	skos:broader	ccat:3020 ;
	skos:definition	"Oleochemical derived by transesterification of fats with methanol, usually blended with petrodiesel."@en ;
	skos:inScheme	ccat: ;
	skos:notation	"302010" ;
	skos:prefLabel	"Biodiesel"@en .

ccat:302015
	a	skos:Concept ;
	skos:altLabel	"UCOME"@en , "Used Cooking Oil Methyl Ester"@en ;
	skos:broader	ccat:3020 ;
	skos:definition	"Feedstock to produce biofuel, most notably Fatty Acid Methyl Ester (FAME)."@en ;
	skos:inScheme	ccat: ;
	skos:notation	"302015" ;
	skos:prefLabel	"Used Cooking Oil"@en .

ccat:302018
	a	skos:Concept ;
	skos:altLabel	"HVO"@en ;
	skos:broader	ccat:3020 ;
	skos:definition	"Feedstock to produce biofuel, most notably Fatty Acid Methyl Ester (FAME)."@en ;
	skos:inScheme	ccat: ;
	skos:notation	"302018" ;
	skos:prefLabel	"Hydrotreated Vegetable Oil"@en .

ccat:302020
	a	skos:Concept ;
	skos:altLabel	"PLA"@en ;
	skos:broader	ccat:3020 ;
	skos:definition	"Thermoplastic polyester obtained by condensation of lactic acid, a monomer made from fermented plant starch such as from corn, cassava, sugarcane or sugar beet pulp."@en ;
	skos:inScheme	ccat: ;
	skos:notation	"302020" ;
	skos:prefLabel	"Polylactic Acid"@en .

ccat:302030
	a	skos:Concept ;
	skos:altLabel	"PA 11"@en ;
	skos:broader	ccat:3020 ;
	skos:definition	"Polyamide produced by the polymerization of 11-aminoundecanoic acid which is produced from castor beans under the trade name Rilsan."@en ;
	skos:inScheme	ccat: ;
	skos:notation	"302030" ;
	skos:prefLabel	"Polyamide 11"@en .

ccat:302040
	a	skos:Concept ;
	skos:altLabel	"Ethene"@en ;
	skos:broader	ccat:3020 ;
	skos:definition	"Simplest hydrocarbon with carbon-carbon double bonds, formula CH2=CH2."@en ;
	skos:inScheme	ccat: ;
	skos:notation	"302040" ;
	skos:note	"""Produced by steam cracking purified natural gas, naphtha, gasoil or condy."""@en ;
	skos:prefLabel	"Ethylene"@en .

ccat:302050
	a	skos:Concept ;
	skos:altLabel	"Propene"@en ;
	skos:broader	ccat:3020 ;
	skos:definition	"Unsaturated compound with one double bond, formula CH3CH=CH."@en ;
	skos:inScheme	ccat: ;
	skos:notation	"302050" ;
	skos:prefLabel	"Propylene"@en .

ccat:302060
	a	skos:Concept ;
	skos:altLabel	"Xylol"@en ;
	skos:broader	ccat:3020 ;
	skos:definition	"Mixture of organic compounds with the formula (CH3)2C6H4."@en ;
	skos:inScheme	ccat: ;
	skos:notation	"302060" ;
	skos:prefLabel	"Xylene"@en .

ccat:3030
	a	skos:Concept ;
	skos:broader	ccat:30 ;
	skos:definition	"Material derived from forestry for direct consumption or commercial use."@en ;
	skos:exactMatch	agrovoc:c_3049 , stw:14149-3 ;
	skos:inScheme	ccat: ;
	skos:notation	"3030" ;
	skos:prefLabel	"Forest Products"@en .

ccat:303010
	a	skos:Concept ;
	skos:altLabel	"Timber"@en ;
	skos:broader	ccat:3030 ;
	skos:definition	"Standing or felled trees."@en ;
	skos:exactMatch	agrovoc:c_8421 , stw:14150-4 , wd:Q287 ;
	skos:inScheme	ccat: ;
	skos:notation	"303010" ;
	skos:prefLabel	"Wood"@en .

ccat:303015
	a	skos:Concept ;
	skos:altLabel	"Lumber"@en ;
	skos:broader	ccat:3030 ;
	skos:definition	"Wood that has been processed into beams and planks."@en ;
	skos:exactMatch	agrovoc:c_6831 ;
	skos:inScheme	ccat: ;
	skos:notation	"303015" ;
	skos:note	"""80% of lumber comes from softwood, e.g. from coniferous species, including pine, fir and spruce (collectively spruce-pine-fir), cedar, and hemlock."""@en ;
	skos:prefLabel	"Sawnwood"@en ;
	skos:scopeNote	"May be supplied either rough-sawn, or surfaced on one or more of its faces."@en .

ccat:303020
	a	skos:Concept ;
	skos:altLabel	"Blockboard"@en ;
	skos:broader	ccat:3030 ;
	skos:definition	"Material manufactured from thin layers or \"plies\" of wood veneer."@en ;
	skos:inScheme	ccat: ;
	skos:notation	"303020" ;
	skos:prefLabel	"Plywood"@en .

ccat:303030
	a	skos:Concept ;
	skos:broader	ccat:3030 ;
	skos:definition	"Material made out of wood fibres."@en ;
	skos:inScheme	ccat: ;
	skos:notation	"303030" ;
	skos:prefLabel	"Fibreboard"@en .

ccat:303050
	a	skos:Concept ;
	skos:broader	ccat:3030 ;
	skos:definition	"Fuel for a pellet stove made from compacted sawdust."@en ;
	skos:inScheme	ccat: ;
	skos:notation	"303050" ;
	skos:prefLabel	"Wood Pellets"@en .

ccat:3035
	a	skos:Concept ;
	skos:broader	ccat:30 ;
	skos:definition	"Material produced by mechanically or chemically processing cellulose fibres derived from wood, rags, grasses or other vegetable sources in water."@en ;
	skos:inScheme	ccat: ;
	skos:notation	"3035" ;
	skos:prefLabel	"Paper"@en .

ccat:303510
	a	skos:Concept ;
	skos:broader	ccat:3035 ;
	skos:definition	"Material consisting mainly of wood pulp and most commonly used to print newspapers and other publications and advertising material."@en ;
	skos:inScheme	ccat: ;
	skos:notation	"303510" ;
	skos:prefLabel	"Newsprint"@en .

ccat:303520
	a	skos:Concept ;
	skos:broader	ccat:3035 ;
	skos:definition	"Material made out of natural unbleached wood fibres for the production of corrugated board."@en ;
	skos:inScheme	ccat: ;
	skos:notation	"303520" ;
	skos:prefLabel	"Containerboard"@en .

ccat:303530
	a	skos:Concept ;
	skos:broader	ccat:3035 ;
	skos:definition	"Material prepared by chemically or mechanically separating cellulose fibres from wood, fiber crops, waste paper, or rags."@en ;
	skos:inScheme	ccat: ;
	skos:notation	"303530" ;
	skos:prefLabel	"Pulp"@en .

ccat:303550
	a	skos:Concept ;
	skos:broader	ccat:3035 ;
	skos:definition	"Material made from cellulose obtained by breaking down waste paper."@en ;
	skos:inScheme	ccat: ;
	skos:notation	"303550" ;
	skos:prefLabel	"Recovered Paper"@en .

ccat:3040
	a	skos:Concept ;
	skos:broader	ccat:30 ;
	skos:definition	"Biodegradable solid or highly viscous compounds."@en ;
	skos:inScheme	ccat: ;
	skos:notation	"3040" ;
	skos:prefLabel	"Rubber and Wax"@en .

ccat:304010
	a	skos:Concept ;
	skos:broader	ccat:3040 ;
	skos:definition	"Field latex, raw caucho or caoutchouc, with minor impurities of other organic compounds, plus water."@en ;
	skos:exactMatch	agrovoc:c_6678 , stw:14151-2 , wd:Q131877 ;
	skos:inScheme	ccat: ;
	skos:notation	"304010" ;
	skos:note	"""Thailand and Indonesia are two of the leading rubber producers."""@en ;
	skos:prefLabel	"Raw Natural Rubber"@en .

ccat:304019
	a	skos:Concept ;
	skos:broader	ccat:3040 ;
	skos:definition	"Any other resin."@en ;
	skos:inScheme	ccat: ;
	skos:notation	"304019" ;
	skos:prefLabel	"Other Resins"@en .

ccat:304020
	a	skos:Concept ;
	skos:altLabel	"HA Latex"@en ;
	skos:broader	ccat:3040 ;
	skos:definition	"Centrifuged and ammoniated field latex that has been processed into latex concentrate."@en ;
	skos:inScheme	ccat: ;
	skos:notation	"304020" ;
	skos:prefLabel	"Concentrated Latex"@en .

ccat:304022
	a	skos:Concept ;
	skos:broader	ccat:3040 ;
	skos:definition	"Field latex that has been transferred into coagulation tanks"@en ;
	skos:inScheme	ccat: ;
	skos:notation	"304022" ;
	skos:prefLabel	"Coagulated Latex"@en .

ccat:304025
	a	skos:Concept ;
	skos:altLabel	"TSR"@en ;
	skos:broader	ccat:3040 ;
	skos:definition	"Naturally coagulated rubber (cup lump) that has been reduced in size, cleaned and dried, then baled and palletised for storage and shipment."@en ;
	skos:inScheme	ccat: ;
	skos:notation	"304025" ;
	skos:prefLabel	"Technically Specified Rubber"@en .

ccat:304027
	a	skos:Concept ;
	skos:altLabel	"RSS Rubber"@en ;
	skos:broader	ccat:3040 ;
	skos:definition	"Coagulated latex sheets that have been air dried or smoked in ovens."@en ;
	skos:inScheme	ccat: ;
	skos:notation	"304027" ;
	skos:prefLabel	"Ribbed Smoked Sheet Rubber"@en .

ccat:304030
	a	skos:Concept ;
	skos:broader	ccat:3040 ;
	skos:definition	"Waxy substnce of plnt origin, e.g. rice bran wax or sunflower wax."@en ;
	skos:inScheme	ccat: ;
	skos:notation	"304030" ;
	skos:prefLabel	"Vegetal Wax"@en .

ccat:304035
	a	skos:Concept ;
	skos:broader	ccat:3040 ;
	skos:definition	"Natural wax produced by honey bees of the genus Apis."@en ;
	skos:inScheme	ccat: ;
	skos:notation	"304035" ;
	skos:prefLabel	"Beeswax"@en .

ccat:3050
	a	skos:Concept ;
	skos:broader	ccat:30 ;
	skos:definition	"Compounds that do not contain a C atom. Exceptions are made for isocyanide/cyanide and their non-hydrocarbyl derivatives, thiophosgene, carbon diselenide, carbon monosulfide, carbon disulfide, carbon subsulfide, carbon monoxide, carbon trioxide, carbon suboxide, and dicarbon monoxide."@en ;
	skos:exactMatch	<http://classyfire.wishartlab.com/tax_nodes/C0000001> , agrovoc:c_3881 ;
	skos:inScheme	ccat: ;
	skos:notation	"3050" ;
	skos:prefLabel	"Inorganic Compounds"@en .

ccat:305010
	a	skos:Concept ;
	skos:altLabel	"E500"@en , "Soda Ash"@en , "Washing Soda"@en ;
	skos:broader	ccat:3050 ;
	skos:definition	"Sodium carbonate."@en ;
	skos:exactMatch	<http://classyfire.wishartlab.com/entities/CDBYLPFSWZWCQE-UHFFFAOYSA-L> ;
	skos:inScheme	ccat: ;
	skos:notation	"305010" ;
	skos:note	"""As a common alkali, it is preferred in many chemical processes because it is cheaper than sodium hydroxide and far safer to handle."""@en ;
	skos:prefLabel	"Sodium Carbonate"@en .

ccat:305015
	a	skos:Concept ;
	skos:altLabel	"Caustic Soda"@en , "Lye"@en ;
	skos:broader	ccat:3050 ;
	skos:definition	"Sodium hydroxide."@en ;
	skos:exactMatch	<https://pubchem.ncbi.nlm.nih.gov/compound/14798> ;
	skos:inScheme	ccat: ;
	skos:notation	"305015" ;
	skos:note	"""Sodium hydroxide is used in many industries: in the making of wood pulp and paper, textiles, drinking water, soaps and detergents, and as a drain opener. Worldwide production in 2004 was approximately 60 million tons, while demand was 51 million tons."""@en ;
	skos:prefLabel	"Sodium Hydroxide"@en .

ccat:305020
	a	skos:Concept ;
	skos:broader	ccat:3050 ;
	skos:definition	"Non-crystalline, often transparent amorphous solid."@en ;
	skos:inScheme	ccat: ;
	skos:notation	"305020" ;
	skos:note	"""Soda-lime glass, containing around 70% silica, accounts for around 90% of manufactured glass."""@en ;
	skos:prefLabel	"Glass"@en .

ccat:305030
	a	skos:Concept ;
	skos:broader	ccat:3050 ;
	skos:definition	"Intermetallics are metallic alloys that form ordered solid-state compounds between two or more metallic elements."@en ;
	skos:inScheme	ccat: ;
	skos:notation	"305030" ;
	skos:note	"""Intermetallics are generally hard and brittle, with good high-temperature mechanical properties. They can be classified as stoichiometric or nonstoichiometic intermetallic compounds."""@en ;
	skos:prefLabel	"Intermetallics"@en .

ccat:30503010
	a	skos:Concept ;
	skos:broader	ccat:305030 ;
	skos:definition	"Alloy of iron and silicon with a typical silicon content by weight of 15%-90%."@en ;
	skos:inScheme	ccat: ;
	skos:notation	"30503010" ;
	skos:prefLabel	"Ferrosilicon"@en .

ccat:30503020
	a	skos:Concept ;
	skos:broader	ccat:305030 ;
	skos:definition	"Alloy of manganese and silicon."@en ;
	skos:inScheme	ccat: ;
	skos:notation	"30503020" ;
	skos:prefLabel	"Manganese Silicide"@en .

ccat:3060
	a	skos:Concept ;
	skos:broader	ccat:30 ;
	skos:definition	"Compounds that contain at least one carbon atom, excluding the exceptions made for inorganic compounds."@en ;
	skos:exactMatch	<http://classyfire.wishartlab.com/tax_nodes/C0000000> , agrovoc:c_5384 ;
	skos:inScheme	ccat: ;
	skos:notation	"3060" ;
	skos:prefLabel	"Organic Compounds"@en .

ccat:306010
	a	skos:Concept ;
	skos:broader	ccat:3060 ;
	skos:definition	"Macromolecules composed of many repeating units."@en ;
	skos:exactMatch	<http://classyfire.wishartlab.com/tax_nodes/C0003297> , agrovoc:c_32041 , stw:14710-6 ;
	skos:inScheme	ccat: ;
	skos:notation	"306010" ;
	skos:prefLabel	"Polymers"@en .

ccat:30601010
	a	skos:Concept ;
	skos:altLabel	"PVC"@en ;
	skos:broader	ccat:306010 ;
	skos:definition	"Polymer made up of vinyl chloride monomers (VCM)."@en ;
	skos:exactMatch	agrovoc:c_28508 , stw:14715-3 , wd:Q146368 ;
	skos:inScheme	ccat: ;
	skos:notation	"30601010" ;
	skos:note	"""The world's third-most widely produced synthetic plastic polymer (after polyethylene and polypropylene). About 40 million tons of PVC are produced each year."""@en ;
	skos:prefLabel	"Polyvinyl Chloride"@en .

ccat:30601020
	a	skos:Concept ;
	skos:altLabel	"PE"@en ;
	skos:broader	ccat:306010 ;
	skos:definition	"Polymer made up of ethylene monomers (ethene)."@en ;
	skos:exactMatch	agrovoc:c_28510 , stw:14705-6 , wd:Q143429 ;
	skos:inScheme	ccat: ;
	skos:notation	"30601020" ;
	skos:note	"""The most common plastic in use today.

PE is usually a mixture of similar polymers of ethylene of various chain-lengths. It can be low density or high density: low density polyethylene is extruded using high pressure (1000-5000 atm) and high temperature (520 Kelvin), while high density polyethylene is extruded using low pressure (6-7 atm) and low temperature (333-343 Kelvin). Polyethylene is usually thermoplastic, however it can be modified to become thermosetting instead, for example in cross-linked polyethylene."""@en ;
	skos:prefLabel	"Polyethylene"@en .

ccat:30601025
	a	skos:Concept ;
	skos:altLabel	"PET"@en ;
	skos:broader	ccat:306010 ;
	skos:definition	"Thermoplastic polymer resin of the polyester family, formula (C10H8O4)n."@en ;
	skos:inScheme	ccat: ;
	skos:notation	"30601025" ;
	skos:prefLabel	"Polyethylene Terephthalate"@en .

ccat:30601030
	a	skos:Concept ;
	skos:altLabel	"PP"@en ;
	skos:broader	ccat:306010 ;
	skos:definition	"Polymer made up of propylene monomers (propene)."@en ;
	skos:exactMatch	agrovoc:c_24221 , stw:14711-4 , wd:Q146174 ;
	skos:inScheme	ccat: ;
	skos:notation	"30601030" ;
	skos:note	"""Bio-PP is the bio-based counterpart of polypropylene (PP).

Polypropylene is the second-most widely produced commodity plastic (after polyethylene). In 2019, the global market for polypropylene was worth $126.03 billion. Revenues are expected to exceed US$145 billion by 2019. The sales of this material are forecast to grow at a rate of 5.8% per year until 2021."""@en ;
	skos:prefLabel	"Polypropylene"@en .

ccat:30601040
	a	skos:Concept ;
	skos:altLabel	"PS"@en ;
	skos:broader	ccat:306010 ;
	skos:definition	"Polymer made up of styrene monomers, formula (C8H8)n."@en ;
	skos:exactMatch	agrovoc:c_28512 , stw:14712-2 ;
	skos:inScheme	ccat: ;
	skos:notation	"30601040" ;
	skos:note	"""Polystyrene is one of the most widely used plastics, the scale of its production being several million tonnes per year."""@en ;
	skos:prefLabel	"Polystyrene"@en .

ccat:30601050
	a	skos:Concept ;
	skos:altLabel	"SBR"@en , "Styrene-butadiene Rubber"@en ;
	skos:broader	ccat:306010 ;
	skos:definition	"Polymer made up of styrene and butadiene monomers, formula (C8H8)m(C4H6)n."@en ;
	skos:inScheme	ccat: ;
	skos:notation	"30601050" ;
	skos:note	"""Styrene-butadiene copolymer is a synthetic rubber that is highly resistant to wear, the scale of its production is about six million tonnes per year."""@en ;
	skos:prefLabel	"Styrene-butadiene copolymer"@en .

ccat:30601055
	a	skos:Concept ;
	skos:altLabel	"BR"@en , "Butadiene Rubber"@en ;
	skos:broader	ccat:306010 ;
	skos:definition	"Polymer made up of buta-1,3-diene monomers, formula (C4H6)n."@en ;
	skos:inScheme	ccat: ;
	skos:notation	"30601055" ;
	skos:note	"""Polybutadiene is a synthetic rubber that is highly resistant to wear, the scale of its production is about two million tonnes per year."""@en ;
	skos:prefLabel	"Polybutadiene"@en .

ccat:306020
	a	skos:Concept ;
	skos:broader	ccat:3060 ;
	skos:definition	"Aromatic compounds containing one or more benzene rings."@en ;
	skos:exactMatch	<http://classyfire.wishartlab.com/tax_nodes/C0002448> ;
	skos:inScheme	ccat: ;
	skos:notation	"306020" ;
	skos:prefLabel	"Benzenoids"@en .

ccat:30602010
	a	skos:Concept ;
	skos:broader	ccat:306020 ;
	skos:definition	"Compound of six carbon atoms joined in a planar ring with one hydrogen atom attached to each, formula C6H6."@en ;
	skos:inScheme	ccat: ;
	skos:notation	"30602010" ;
	skos:prefLabel	"Benzene"@en .

ccat:30602015
	a	skos:Concept ;
	skos:broader	ccat:306020 ;
	skos:definition	"Fusion of two benzene rings, formula C10H8."@en ;
	skos:inScheme	ccat: ;
	skos:notation	"30602015" ;
	skos:prefLabel	"Naphthalene"@en .

ccat:30602017
	a	skos:Concept ;
	skos:altLabel	"Ethenylbenzene"@en , "Phenylethene"@en ;
	skos:broader	ccat:306020 ;
	skos:definition	"Derivative of benzene bearing a vinyl functional group (ethylene, ethene) at one position, formula C6H5CH=CH2."@en ;
	skos:inScheme	ccat: ;
	skos:notation	"30602017" ;
	skos:prefLabel	"Styrene"@en .

ccat:30602020
	a	skos:Concept ;
	skos:altLabel	"p-Xylene"@en ;
	skos:broadMatch	<http://classyfire.wishartlab.com/tax_nodes/C0004211> ;
	skos:broader	ccat:306020 ;
	skos:definition	"Derivative of benzene bearing two methyl groups at the 1- and 4-positions.  The most valued compound in mixed xylene (302060)."@en ;
	skos:inScheme	ccat: ;
	skos:notation	"30602020" ;
	skos:prefLabel	"Paraxylene"@en .

ccat:30602030
	a	skos:Concept ;
	skos:altLabel	"PTA"@en ;
	skos:broadMatch	<http://classyfire.wishartlab.com/tax_nodes/C0001108> ;
	skos:broader	ccat:306020 ;
	skos:definition	"Derivative of benzene bearing a carboxylic acid group at the 1- and 4-positions."@en ;
	skos:inScheme	ccat: ;
	skos:notation	"30602030" ;
	skos:prefLabel	"Terephthalic Acid"@en .

ccat:306030
	a	skos:Concept ;
	skos:broader	ccat:3060 ;
	skos:definition	"Compounds that carry at least one hydroxyl functional group (bOH) bound to a saturated carbon atom."@en ;
	skos:exactMatch	<http://classyfire.wishartlab.com/tax_nodes/C0000129> ;
	skos:inScheme	ccat: ;
	skos:notation	"306030" ;
	skos:prefLabel	"Alkanols and Polyols"@en .

ccat:30603010
	a	skos:Concept ;
	skos:broader	ccat:306030 ;
	skos:definition	"Methanol or methyl alcohol."@en ;
	skos:exactMatch	agrovoc:c_12521 , eurovoc:1893 , wd:Q14982 ;
	skos:inScheme	ccat: ;
	skos:notation	"30603010" ;
	skos:prefLabel	"Methanol"@en .

ccat:30603020
	a	skos:Concept ;
	skos:broader	ccat:306030 ;
	skos:definition	"Ethanol or ethyl alcohol."@en ;
	skos:exactMatch	agrovoc:c_10677 , eurovoc:890 , wd:Q153 ;
	skos:inScheme	ccat: ;
	skos:notation	"30603020" ;
	skos:note	"""Ethanol is an alternative fuel source."""@en ;
	skos:prefLabel	"Ethanol"@en .

ccat:30603025
	a	skos:Concept ;
	skos:broader	ccat:306030 ;
	skos:definition	"Ethane-1,2-diol, formula (CH2OH)2."@en ;
	skos:inScheme	ccat: ;
	skos:notation	"30603025" ;
	skos:prefLabel	"Ethylene Glycol"@en .

ccat:30603030
	a	skos:Concept ;
	skos:broader	ccat:306030 ;
	skos:definition	"Propanol or propyl alcohol."@en ;
	skos:inScheme	ccat: ;
	skos:notation	"30603030" ;
	skos:prefLabel	"Propanol"@en .

ccat:30603040
	a	skos:Concept ;
	skos:broader	ccat:306030 ;
	skos:definition	"Butanol or butyl alcohol."@en ;
	skos:inScheme	ccat: ;
	skos:notation	"30603040" ;
	skos:prefLabel	"Butanol"@en .

ccat:3070
	a	skos:Concept ;
	skos:broader	ccat:30 ;
	skos:definition	"Substances providing nutrients to plants."@en ;
	skos:exactMatch	agrovoc:c_2867 , stw:13427-6 , wd:Q83323 ;
	skos:inScheme	ccat: ;
	skos:notation	"3070" ;
	skos:prefLabel	"Fertilizer"@en ;
	skos:scopeNote	"This includes natural as well as synthetic fertilizers. Fertilizers may be distinct from liming materials or other non-nutrient soil amendments."@en .

ccat:307010
	a	skos:Concept ;
	skos:altLabel	"Carbamide"@en ;
	skos:broader	ccat:3070 ;
	skos:definition	"Compound of two -NH2 groups joined by a carbonyl group (C=O), formula CO(NH2)2."@en ;
	skos:inScheme	ccat: ;
	skos:notation	"307010" ;
	skos:note	"""Substance used in fertilizers as a source of nitrogen (N)."""@en ;
	skos:prefLabel	"Urea"@en .

ccat:307012
	a	skos:Concept ;
	skos:broader	ccat:3070 ;
	skos:definition	"Compound of nitrogen and hydrogen, formula NH3."@en ;
	skos:inScheme	ccat: ;
	skos:notation	"307012" ;
	skos:prefLabel	"Ammonia"@en .

ccat:307013
	a	skos:Concept ;
	skos:broader	ccat:3070 ;
	skos:definition	"Compound of ammonium (NH4+) and nitrate (NO3-)."@en ;
	skos:inScheme	ccat: ;
	skos:notation	"307013" ;
	skos:prefLabel	"Ammonium Nitrate"@en .

ccat:307015
	a	skos:Concept ;
	skos:altLabel	"Urea Ammonium Nitrate"@en ;
	skos:broader	ccat:3070 ;
	skos:definition	"Solution of urea and ammonium nitrate in water."@en ;
	skos:inScheme	ccat: ;
	skos:notation	"307015" ;
	skos:prefLabel	"UAN"@en .

ccat:307020
	a	skos:Concept ;
	skos:altLabel	"Diamidophosphate"@en ;
	skos:broader	ccat:3070 ;
	skos:definition	"Ion with formula PO2(NH2)2-."@en ;
	skos:inScheme	ccat: ;
	skos:notation	"307020" ;
	skos:prefLabel	"DAP"@en .

ccat:307025
	a	skos:Concept ;
	skos:altLabel	"Monoammonium phosphate"@en ;
	skos:broader	ccat:3070 ;
	skos:definition	"Compound of ammonium (NH4+) and dihydrogen phosphate (PO2(OH)2-)."@en ;
	skos:inScheme	ccat: ;
	skos:notation	"307025" ;
	skos:prefLabel	"MAP"@en .

ccat:307030
	a	skos:Concept ;
	skos:broader	ccat:3070 ;
	skos:closeMatch	wd:Q10564271 ;
	skos:definition	"Various mined and manufactured salts that contain potassium in water-soluble form."@en ;
	skos:exactMatch	agrovoc:c_6138 , stw:14034-6 ;
	skos:inScheme	ccat: ;
	skos:notation	"307030" ;
	skos:note	"""Potash is produced worldwide in amounts exceeding 90 million tonnes (40 million tonnes K2O equivalent) per year, mostly for use in fertilizer. Various kinds of fertilizer-potash constitute the single greatest industrial use of the element potassium in the world. Potassium was first derived in 1807 by electrolysis of caustic potash (potassium hydroxide)."""@en ;
	skos:prefLabel	"Potash"@en .

ccat:3080
	a	skos:Concept ;
	skos:broader	ccat:30 ;
	skos:definition	"Substances meant to control pests."@en ;
	skos:exactMatch	<http://classyfire.wishartlab.com/tax_nodes/C0000000> , agrovoc:c_5384 ;
	skos:inScheme	ccat: ;
	skos:notation	"3080" ;
	skos:prefLabel	"Pesticide"@en ;
	skos:scopeNote	"Any chemical (such as carbamate) or biological agent (such as a virus, bacterium, or fungus) that deters, incapacitates, kills, or otherwise discourages pests. Target pests can include insects, plant pathogens, weeds, molluscs, birds, mammals, fish, nematodes (roundworms), and microbes that destroy property, cause nuisance, or spread disease, or are disease vectors."@en .

ccat:308010
	a	skos:Concept ;
	skos:broader	ccat:3080 ;
	skos:definition	"Substance to control undesired plants, also known as weeds."@en ;
	skos:inScheme	ccat: ;
	skos:notation	"308010" ;
	skos:prefLabel	"Herbicide"@en .

ccat:308020
	a	skos:Concept ;
	skos:broader	ccat:3080 ;
	skos:definition	"Substance to control insects by targeting insect eggs or larvae."@en ;
	skos:inScheme	ccat: ;
	skos:notation	"308020" ;
	skos:prefLabel	"Insecticide"@en .

ccat:308030
	a	skos:Concept ;
	skos:broader	ccat:3080 ;
	skos:definition	"Substance to control plant-parasitic nematodes."@en ;
	skos:inScheme	ccat: ;
	skos:notation	"308030" ;
	skos:prefLabel	"Nematicide"@en .

ccat:308040
	a	skos:Concept ;
	skos:broader	ccat:3080 ;
	skos:definition	"Substance to control bacteria."@en ;
	skos:inScheme	ccat: ;
	skos:notation	"308040" ;
	skos:prefLabel	"Bactericide"@en .

ccat:308050
	a	skos:Concept ;
	skos:broader	ccat:3080 ;
	skos:definition	"Substance to control parasitic fungi or their spores."@en ;
	skos:inScheme	ccat: ;
	skos:notation	"308050" ;
	skos:prefLabel	"Fungicide"@en .

ccat:308060
	a	skos:Concept ;
	skos:broader	ccat:3080 ;
	skos:definition	"Specific animal repellents, in particular molluscicides, piscicides, avicides, and rodenticides."@en ;
	skos:inScheme	ccat: ;
	skos:notation	"308060" ;
	skos:prefLabel	"Animal Repellent"@en .

ccat:40
	a	skos:Concept ;
	skos:definition	"Commoditized goods are tradables that have been made fungible by standardisation."@en ;
	skos:inScheme	ccat: ;
	skos:notation	"40" ;
	skos:prefLabel	"Commoditized"@en ;
	skos:topConceptOf	ccat: .

ccat:4010
	a	skos:Concept ;
	skos:broader	ccat:40 ;
	skos:closeMatch	wd:Q7498085 ;
	skos:definition	"Contractual arrangements for carrying cargo, voyage charter, contract of affreightment, time charter and the bareboat charter."@en ;
	skos:exactMatch	stw:13621-3 ;
	skos:inScheme	ccat: ;
	skos:notation	"4010" ;
	skos:prefLabel	"Freight"@en .

ccat:401010
	a	skos:Concept ;
	skos:broader	ccat:4010 ;
	skos:definition	"Cargo carried by tanker at a freight rate."@en ;
	skos:inScheme	ccat: ;
	skos:notation	"401010" ;
	skos:prefLabel	"Wet Freight"@en .

ccat:40101010
	a	skos:Concept ;
	skos:broader	ccat:401010 ;
	skos:definition	"Tanker for dirty loads, i.e. crude oils."@en ;
	skos:inScheme	ccat: ;
	skos:notation	"40101010" ;
	skos:prefLabel	"Dirty Freight"@en ;
	skos:scopeNote	"TDx at the Baltic Exchange"@en .

ccat:40101020
	a	skos:Concept ;
	skos:broader	ccat:401010 ;
	skos:definition	"Tanker for clean loads, i.e. refined products excluding gases."@en ;
	skos:inScheme	ccat: ;
	skos:notation	"40101020" ;
	skos:prefLabel	"Clean Freight"@en ;
	skos:scopeNote	"TCx at the Baltic Exchange"@en .

ccat:40101030
	a	skos:Concept ;
	skos:broader	ccat:401010 ;
	skos:definition	"Tanker for gas loads, i.e. liquefied natural gas or petroleum gas."@en ;
	skos:inScheme	ccat: ;
	skos:notation	"40101030" ;
	skos:prefLabel	"Gas Freight"@en ;
	skos:scopeNote	"BLNGx, BLPGx at the Baltic Exchange"@en .

ccat:401020
	a	skos:Concept ;
	skos:broader	ccat:4010 ;
	skos:definition	"Cargoes on a per container basis."@en ;
	skos:inScheme	ccat: ;
	skos:notation	"401020" ;
	skos:prefLabel	"Container Freight"@en ;
	skos:scopeNote	"FBXx at the Baltic Exchange"@en .

ccat:401025
	a	skos:Concept ;
	skos:broader	ccat:4010 ;
	skos:definition	"Bulk cargoes on a time-charter or tonne voyage basis."@en ;
	skos:inScheme	ccat: ;
	skos:notation	"401025" ;
	skos:prefLabel	"Dry Bulk Freight"@en ;
	skos:scopeNote	"Cx, Px, Sx, HSx at the Baltic Exchange"@en .

ccat:401030
	a	skos:Concept ;
	skos:broader	ccat:4010 ;
	skos:definition	"Freight shipped in an aircraft."@en ;
	skos:inScheme	ccat: ;
	skos:notation	"401030" ;
	skos:prefLabel	"Air Freight"@en .

ccat:401050
	a	skos:Concept ;
	skos:broader	ccat:4010 ;
	skos:definition	"Premium of one freight rate over another to a different location, or with different shipping agreements."@en ;
	skos:inScheme	ccat: ;
	skos:notation	"401050" ;
	skos:prefLabel	"Cargo Spread"@en .

ccat:4020
	a	skos:Concept ;
	skos:broader	ccat:40 ;
	skos:definition	"Financial instrument to reduce risk associated with adverse or unexpected weather conditions."@en ;
	skos:exactMatch	stw:29603-4 , wd:Q1759704 ;
	skos:inScheme	ccat: ;
	skos:notation	"4020" ;
	skos:prefLabel	"Weather"@en .

ccat:402010
	a	skos:Concept ;
	skos:broader	ccat:4020 ;
	skos:definition	"An aggregate of (average, trimmed mean, daily high, daily low) temperature as measured by a (set of) reference weather stations over a pre-defined time period. Sometimes capped/floored under the name heating degree days/cooling degree days, respectively."@en ;
	skos:inScheme	ccat: ;
	skos:notation	"402010" ;
	skos:prefLabel	"Temperature"@en .

ccat:402020
	a	skos:Concept ;
	skos:broader	ccat:4020 ;
	skos:definition	"Product that tracks the (average, trimmed mean, minimum, maxium, ...) rainfall in a region over a predefined time period."@en ;
	skos:inScheme	ccat: ;
	skos:notation	"402020" ;
	skos:prefLabel	"Rainfall"@en .

ccat:402030
	a	skos:Concept ;
	skos:broader	ccat:4020 ;
	skos:definition	"Product that tracks damages incurred by abnormal weather conditions or their consequences such as typhoons, hurricanes, or floods."@en ;
	skos:inScheme	ccat: ;
	skos:notation	"402030" ;
	skos:prefLabel	"Catastrophe"@en ;
	skos:scopeNote	"It is permissible to classify non-weather related catastrophes here, e.g. bush fires, earthquakes, or volcano eruptions."@en .

ccat:4030
	a	skos:Concept ;
	skos:broader	ccat:40 ;
	skos:closeMatch	agrovoc:c_1b1e0e70 , eurovoc:434843 , stw:20762-1 , wd:Q8348417 ;
	skos:definition	"Permits and allowances in writing issued by a central authority (usually a governmental body) that allow a discharge of a specific quantity of a specific pollutant over a set time period."@en ;
	skos:inScheme	ccat: ;
	skos:notation	"4030" ;
	skos:note	"""Polluters are required to hold permits in amount equal to their emissions. Polluters that want to increase their emissions must buy permits from others willing to sell them."""@en ;
	skos:prefLabel	"Emissions"@en .

ccat:403010
	a	skos:Concept ;
	skos:broader	ccat:4030 ;
	skos:definition	"Permits and allowances specifically for carbon dioxide (CO2) emission."@en ;
	skos:inScheme	ccat: ;
	skos:notation	"403010" ;
	skos:prefLabel	"CO2 permits"@en .

ccat:403020
	a	skos:Concept ;
	skos:broader	ccat:4030 ;
	skos:definition	"Permits and allowances specifically for nitrogen oxides (NOx) emissions."@en ;
	skos:inScheme	ccat: ;
	skos:notation	"403020" ;
	skos:prefLabel	"NOx permits"@en .

ccat:403030
	a	skos:Concept ;
	skos:broader	ccat:4030 ;
	skos:definition	"Permits and allowances specifically for sulfur dioxide (SO2) emission."@en ;
	skos:inScheme	ccat: ;
	skos:notation	"403030" ;
	skos:prefLabel	"SO2 permits"@en .

ccat:403040
	a	skos:Concept ;
	skos:altLabel	"GO"@en , "REC"@en ;
	skos:broader	ccat:4030 ;
	skos:closeMatch	wd:Q1478326 , wd:Q2143923 ;
	skos:definition	"Tradable, non-tangible energy commodities that represent proof that 1 megawatt-hour (MWh) of electricity was generated from an eligible renewable energy resource and was fed into the shared system of power lines which transport energy."@en ;
	skos:exactMatch	wd:Q7313092 ;
	skos:inScheme	ccat: ;
	skos:notation	"403040" ;
	skos:prefLabel	"Renewable Energy Credits/Guarantee of Origin"@en ;
	skos:scopeNote	"Tracking instruments as outlined in  <https://resource-solutions.org/wp-content/uploads/2015/07/The-Legal-Basis-for-RECs.pdf>, or following article 15 of the European Directive 2009/28/EC, or similar."@en .

ccat:403042
	a	skos:Concept ;
	skos:altLabel	"RIN"@en ;
	skos:broader	ccat:4030 ;
	skos:definition	"Tradable tracking instrument generated by the production of biofuels to verify refiner or obligated party compliance with the blending requirements of the Renewable Fuel Standard."@en ;
	skos:inScheme	ccat: ;
	skos:notation	"403042" ;
	skos:prefLabel	"Renewable Identification Number"@en .

ccat:403050
	a	skos:Concept ;
	skos:altLabel	"CER"@en , "ERU"@en ;
	skos:broader	ccat:4030 ;
	skos:definition	"Emission Reduction Unit that represents a reduction of greenhouse gases under the Joint Implementation mechanism, where it represents one tonne of CO2 equivalent reduced."@en ;
	skos:inScheme	ccat: ;
	skos:notation	"403050" ;
	skos:prefLabel	"Emission Reduction Unit/Certified Emission Reduction"@en .

ccat:4040
	a	skos:Concept ;
	skos:broader	ccat:40 ;
	skos:closeMatch	msa:2779948615 , wd:Q7973730 ;
	skos:definition	"Ownership interest in water."@en ;
	skos:inScheme	ccat: ;
	skos:notation	"4040" ;
	skos:prefLabel	"Commercial Water Rights"@en .

ccat:404010
	a	skos:Concept ;
	skos:broader	ccat:4040 ;
	skos:definition	"Entitlement to divert a river or pump water from a river or lake."@en ;
	skos:inScheme	ccat: ;
	skos:notation	"404010" ;
	skos:prefLabel	"Diversion Rights"@en .

ccat:404020
	a	skos:Concept ;
	skos:broader	ccat:4040 ;
	skos:definition	"Entitlement to pump groundwater above a certain level."@en ;
	skos:inScheme	ccat: ;
	skos:notation	"404020" ;
	skos:prefLabel	"Groundwater Rights"@en .

ccat:404030
	a	skos:Concept ;
	skos:broader	ccat:4040 ;
	skos:definition	"Entitlement to use the water in a surface storage reservoir."@en ;
	skos:inScheme	ccat: ;
	skos:notation	"404030" ;
	skos:prefLabel	"Surface Storage Reservoir Rights"@en .

ccat:404040
	a	skos:Concept ;
	skos:broader	ccat:4040 ;
	skos:definition	"Entitlement to use treated wastewater."@en ;
	skos:inScheme	ccat: ;
	skos:notation	"404040" ;
	skos:prefLabel	"Treated Wastewater Rights"@en .

ccat:4050
	a	skos:Concept ;
	skos:broader	ccat:40 ;
	skos:definition	"Levy on specific commodities, financial transactions, estates, etc. rather than being a direct imposition on individuals or corporations such income or property taxes."@en ;
	skos:inScheme	ccat: ;
	skos:notation	"4050" ;
	skos:prefLabel	"Tax and Duties"@en .

ccat:50
	a	skos:Concept ;
	skos:definition	"Product whose underlying is, generally, non-physical."@en ;
	skos:inScheme	ccat: ;
	skos:notation	"50" ;
	skos:prefLabel	"Financials"@en ;
	skos:topConceptOf	ccat: .

ccat:5010
	a	skos:Concept ;
	skos:broader	ccat:50 ;
	skos:definition	"Money is characterised by the following properties (1) a medium of exchange, (2) a unit of account, (3) a store of value, (4) a standard of deferred payment."@en ;
	skos:inScheme	ccat: ;
	skos:notation	"5010" ;
	skos:prefLabel	"Money"@en .

ccat:501010
	a	skos:Concept ;
	skos:broader	ccat:5010 ;
	skos:definition	"Currency excluding privately issued (digital) currency and notes."@en ;
	skos:exactMatch	wd:Q8142 ;
	skos:inScheme	ccat: ;
	skos:notation	"501010" ;
	skos:prefLabel	"Currency"@en .

ccat:501015
	a	skos:Concept ;
	skos:broader	ccat:5010 ;
	skos:definition	"Product that tracks the variance or volatility of currency pairs."@en ;
	skos:inScheme	ccat: ;
	skos:notation	"501015" ;
	skos:prefLabel	"Currency Variance"@en .

ccat:501020
	a	skos:Concept ;
	skos:broader	ccat:5010 ;
	skos:definition	"Digital currency including virtual currencies or cryptocurrencies."@en ;
	skos:exactMatch	wd:Q10836209 ;
	skos:inScheme	ccat: ;
	skos:notation	"501020" ;
	skos:prefLabel	"Digital Currency"@en .

ccat:501080
	a	skos:Concept ;
	skos:broader	ccat:5010 ;
	skos:definition	"Portfolio of selected currencies with a preagreed weighting."@en ;
	skos:inScheme	ccat: ;
	skos:notation	"501080" ;
	skos:prefLabel	"Currency Basket"@en .

ccat:5020
	a	skos:Concept ;
	skos:broader	ccat:50 ;
	skos:closeMatch	wd:Q3239315 ;
	skos:definition	"Tradeable debt or rate instrument that provides a return in the form of fixed periodic interest payments and/or the eventual return of principal at maturity."@en ;
	skos:inScheme	ccat: ;
	skos:notation	"5020" ;
	skos:prefLabel	"Fixed Income"@en .

ccat:502010
	a	skos:Concept ;
	skos:altLabel	"Government bonds"@en ;
	skos:broader	ccat:5020 ;
	skos:definition	"Debt security issued by a government to fund government spending."@en ;
	skos:exactMatch	<https://spec.edmcouncil.org/fibo/ontology/SEC/Debt/Bonds/SovereignBond> , wd:Q2324820 ;
	skos:inScheme	ccat: ;
	skos:notation	"502010" ;
	skos:prefLabel	"Sovereign bond"@en .

ccat:502015
	a	skos:Concept ;
	skos:broader	ccat:5020 ;
	skos:definition	"Product that tracks the variance or volatility of debt securities issued by a government."@en ;
	skos:inScheme	ccat: ;
	skos:notation	"502015" ;
	skos:prefLabel	"Sovereign bond variance"@en .

ccat:502020
	a	skos:Concept ;
	skos:broader	ccat:5020 ;
	skos:definition	"Rates with tenors of up to 12 months."@en ;
	skos:exactMatch	wd:Q102113162 ;
	skos:inScheme	ccat: ;
	skos:notation	"502020" ;
	skos:prefLabel	"STIR"@en .

ccat:502030
	a	skos:Concept ;
	skos:broader	ccat:5020 ;
	skos:definition	"Interest rate swaps, vanilla, basis, etc."@en ;
	skos:exactMatch	msa:99560960 , wd:Q205258 ;
	skos:inScheme	ccat: ;
	skos:notation	"502030" ;
	skos:prefLabel	"IRS"@en .

ccat:502032
	a	skos:Concept ;
	skos:broader	ccat:5020 ;
	skos:definition	"Forward rate agreement, one payment of an IRS."@en ;
	skos:inScheme	ccat: ;
	skos:notation	"502032" ;
	skos:prefLabel	"FRA"@en .

ccat:502035
	a	skos:Concept ;
	skos:broader	ccat:5020 ;
	skos:definition	"Overnight Index Swaps, float/float or compounded."@en ;
	skos:exactMatch	msa:99560960 , wd:Q205258 ;
	skos:inScheme	ccat: ;
	skos:notation	"502035" ;
	skos:prefLabel	"OIS"@en .

ccat:502040
	a	skos:Concept ;
	skos:broader	ccat:5020 ;
	skos:definition	"Securities that offset or are linked to a predefined inflation index, e.g. a coupon that adds realised inflation during the interest accrual period."@en ;
	skos:inScheme	ccat: ;
	skos:notation	"502040" ;
	skos:prefLabel	"Inflation-linked Security"@en .

ccat:502080
	a	skos:Concept ;
	skos:broader	ccat:5010 ;
	skos:definition	"Product that tracks the performance of a basket of fixed-income securities, e.g. a bond index."@en ;
	skos:inScheme	ccat: ;
	skos:notation	"502080" ;
	skos:prefLabel	"FI Basket"@en ;
	skos:scopeNote	"A basket of FRAs shall be classified IRS, a basket that is a strip of STIRs shall be classified as STIR."@en .

ccat:5030
	a	skos:Concept ;
	skos:broader	ccat:50 ;
	skos:definition	"Ownership of assets that may have debt and liabilities attached to them."@en ;
	skos:inScheme	ccat: ;
	skos:notation	"5030" ;
	skos:prefLabel	"Equity"@en .

ccat:503010
	a	skos:Concept ;
	skos:broader	ccat:5030 ;
	skos:definition	"Derivative products with a single stock or ETF as underlying."@en ;
	skos:inScheme	ccat: ;
	skos:notation	"503010" ;
	skos:prefLabel	"Single Stock"@en .

ccat:503020
	a	skos:Concept ;
	skos:broader	ccat:5030 ;
	skos:definition	"Product that tracks the dividend of a stock or stock index."@en ;
	skos:inScheme	ccat: ;
	skos:notation	"503020" ;
	skos:prefLabel	"Dividend"@en .

ccat:503030
	a	skos:Concept ;
	skos:broader	ccat:5030 ;
	skos:definition	"Product that tracks the variance or volatility of a stock or stock index."@en ;
	skos:inScheme	ccat: ;
	skos:notation	"503030" ;
	skos:prefLabel	"Variance"@en .

ccat:503080
	a	skos:Concept ;
	skos:broader	ccat:5030 ;
	skos:definition	"Product that tracks the performance of stock indices."@en ;
	skos:inScheme	ccat: ;
	skos:notation	"503080" ;
	skos:prefLabel	"Stock Index"@en .

ccat:5040
	a	skos:Concept ;
	skos:broader	ccat:50 ;
	skos:definition	"Property consisting of land and the buildings on it, along with its natural resources such as crops, minerals or water."@en ;
	skos:inScheme	ccat: ;
	skos:notation	"5040" ;
	skos:prefLabel	"Real Estate"@en .

ccat:504010
	a	skos:Concept ;
	skos:broader	ccat:5040 ;
	skos:definition	"Product that track the performance of a REIT."@en ;
	skos:inScheme	ccat: ;
	skos:notation	"504010" ;
	skos:prefLabel	"REIT"@en .

ccat:504020
	a	skos:Concept ;
	skos:broader	ccat:5040 ;
	skos:definition	"Product that track some quality of properties, e.g. rents or average sales prices in a particular area."@en ;
	skos:inScheme	ccat: ;
	skos:notation	"504020" ;
	skos:prefLabel	"Property Market Indicator"@en .

ccat:504080
	a	skos:Concept ;
	skos:broader	ccat:5040 ;
	skos:definition	"Derivative product with a basket of properties or REITs as underlying."@en ;
	skos:inScheme	ccat: ;
	skos:notation	"504080" ;
	skos:prefLabel	"Property Portfolio"@en .

ccat:5090
	a	skos:Concept ;
	skos:broader	ccat:50 ;
	skos:definition	"Generally non-deliverable product that cannot be classified elsewhere."@en ;
	skos:inScheme	ccat: ;
	skos:notation	"5090" ;
	skos:prefLabel	"Other Financial"@en .

ccat:509080
	a	skos:Concept ;
	skos:broader	ccat:50 ;
	skos:definition	"Non-deliverable product that tracks the performance of a basket of commodities."@en ;
	skos:inScheme	ccat: ;
	skos:notation	"509080" ;
	skos:prefLabel	"Commodity Index"@en .

ccat:509090
	a	skos:Concept ;
	skos:broader	ccat:50 ;
	skos:definition	"Product over an index that cannot be categorised elsewhere."@en ;
	skos:inScheme	ccat: ;
	skos:notation	"509090" ;
	skos:prefLabel	"Other Index"@en .

ccat:90
	a	skos:Concept ;
	skos:definition	"Ephemerals are products for the purpose of transition or testing, they might be temporary or not tradable at all."@en ;
	skos:inScheme	ccat: ;
	skos:notation	"90" ;
	skos:prefLabel	"Ephemerals"@en ;
	skos:topConceptOf	ccat: .

ccat:9080
	a	skos:Concept ;
	skos:broader	ccat:90 ;
	skos:definition	"Product that can be bought and sold without delivery or payment."@en ;
	skos:inScheme	ccat: ;
	skos:notation	"9080" ;
	skos:prefLabel	"Test"@en .

ccat:9090
	a	skos:Concept ;
	skos:broader	ccat:90 ;
	skos:definition	"Catch-all category, to be used when no other category fits but it needs to be documented that classification has been tried."@en ;
	skos:inScheme	ccat: ;
	skos:notation	"9090" ;
	skos:prefLabel	"Unclassified"@en .
