@prefix agrovoc: <http://aims.fao.org/aos/agrovoc/> .
@prefix ccat: <http://data.ga-group.nl/comcat/> .
@prefix dbr: <http://dbpedia.org/resource/> .
@prefix dct: <http://purl.org/dc/terms/> .
@prefix eurovoc: <http://eurovoc.europa.eu/> .
@prefix msa: <http://academic.microsoft.com/v2/detail/> .
@prefix owl: <http://www.w3.org/2002/07/owl#> .
@prefix rdf: <http://www.w3.org/1999/02/22-rdf-syntax-ns#> .
@prefix rdfs: <http://www.w3.org/2000/01/rdf-schema#> .
@prefix skos: <http://www.w3.org/2004/02/skos/core#> .
@prefix sm: <http://www.omg.org/techprocess/ab/SpecificationMetadata/> .
@prefix stw: <http://zbw.eu/stw/descriptor/> .
@prefix vann: <http://purl.org/vocab/vann/> .
@prefix wd: <http://www.wikidata.org/entity/> .
@prefix xsd: <http://www.w3.org/2001/XMLSchema#> .

ccat:
	a	skos:ConceptScheme ;
	dct:abstract	"""A taxonomy concerned with the collection of traded commodities for use by the global financial community. Taxons are assigned a numeric code across up to four tiers of hierarchy: the class of commodity, the category within the class, and the kind of commodity within the category, possibly extended with the sub-kind.

The list of traded commodities, be it standard listed products or products traded OTC, is constantly monitored for the purpose of regular revisions to the standard."""@en ;
	dct:creator	<https://orcid.org/0000-0002-7352-2825> ;
	dct:format	"text/turtle"^^xsd:string ;
	dct:issued	"2022-06-28T02:25:19Z"^^xsd:dateTime ;
	dct:license	<https://creativecommons.org/licenses/by/4.0/> ;
	dct:modified	"2022-06-18T12:43:00Z"^^xsd:dateTime ;
	dct:title	"comcat" ;
	skos:definition	"A commodity is an economic good or service that has full or substantial fungibility, i.e the market treats instances of the good as equivalent or nearly so with no regard to who produced them."@en ;
	skos:note	"This taxonomy (broadly) follows industry's vocabularies, such as FAO's agrovoc, various tariff systems, or the STW thesaurus. It is made by market participants who needed  a single fine-grained classification system instead of choosing between several domain-specific ones or a single coarse one."@en ;
	skos:prefLabel	"Taxonomy for traded commodities"@en ;
	sm:copyright	"Copyright (c) 2022 GA Financial Solutions GmbH" ;
	sm:fileAbbreviation	"comcat" ;
	sm:filename	"comcat.skos.ttl" ;
	vann:preferredNamespacePrefix	"ccat"^^xsd:string ;
	vann:preferredNamespaceUri	"http://data.ga-group.nl/comcat/" .

ccat:10
	a	skos:Concept ;
	skos:definition	"Hard commodities, or hards, are commodities that, generally, are mined, rather than grown."@en ;
	skos:inScheme	ccat: ;
	skos:notation	"10" ;
	skos:prefLabel	"Hards"@en ;
	skos:topConceptOf	ccat: .

ccat:1010
	a	skos:Concept ;
	skos:broader	ccat:10 ;
	skos:closeMatch	stw:18996-5 , wd:Q1239166 ;
	skos:definition	"Commodities that deal specifically with the trade and supply of energy."@en ;
	skos:inScheme	ccat: ;
	skos:notation	"1010" ;
	skos:prefLabel	"Energy"@en .

ccat:101010
	a	skos:Concept ;
	skos:broader	ccat:1010 ;
	skos:definition	"Petroleum is a naturally occurring, yellowish-black liquid found in geological formations beneath the Earth's surface. It is commonly refined into various types of fuels. Components of petroleum are separated using a technique called fractional distillation, i.e. separation of a liquid mixture into fractions differing in boiling point by means of distillation, typically using a fractionating column."@en ;
	skos:exactMatch	agrovoc:c_5747 , eurovoc:2366 , stw:14197-6 , wd:Q22656 ;
	skos:inScheme	ccat: ;
	skos:notation	"101010" ;
	skos:prefLabel	"Crude Oil"@en .

ccat:101020
	a	skos:Concept ;
	skos:broader	ccat:1010 ;
	skos:definition	"""Coal is a combustible black or brownish-black sedimentary rock, formed as rock strata called coal seams. Coal is mostly carbon with variable amounts of other elements; chiefly hydrogen, sulfur, oxygen, and nitrogen. Coal is formed when dead plant matter decays into peat and is converted into coal by the heat and pressure of deep burial over millions of years. Vast deposits of coal originate in former wetlands that covered much of the Earth's tropical land areas during the late Carboniferous (Pennsylvanian) and Permian times.
	
	Coal is primarily used as a fuel. While coal has been known and used for thousands of years, its usage was limited prior to the Industrial Revolution. With the invention of the steam engine coal consumption increased. As of 2016, coal remains an important fuel as it supplied about a quarter of the world's primary energy and two-fifths of electricity. Some iron and steel making and other industrial processes burn coal."""@en ;
	skos:exactMatch	agrovoc:c_1693 , eurovoc:5386 , stw:14200-1 , wd:Q24489 ;
	skos:inScheme	ccat: ;
	skos:notation	"101020" ;
	skos:prefLabel	"Coal"@en .

ccat:10102010
	a	skos:Concept ;
	skos:broader	ccat:101020 ;
	skos:definition	"""Anthracite, also known as hard coal, is a hard, compact variety of coal that has a submetallic luster. It has the highest carbon content, the fewest impurities, and the highest energy density of all types of coal and is the highest ranking of coals.

Anthracite is the most metamorphosed type of coal (but still represents low-grade metamorphism), in which the carbon content is between 86% and 98%. The term is applied to those varieties of coal which do not give off tarry or other hydrocarbon vapours when heated below their point of ignition. Anthracite ignites with difficulty and burns with a short, blue, and smokeless flame.

Anthracite is categorized into standard grade, which is used mainly in power generation, and high grade (HG) and ultra high grade (UHG), the principal uses of which are in the metallurgy sector. Anthracite accounts for about 1% of global coal reserves, and is mined in only a few countries around the world. China accounts for the majority of global production; other producers are Russia, Ukraine, North Korea, South Africa, Vietnam, the UK, Australia, Canada and the US. Total production in 2010 was 670 million tons."""@en ;
	skos:exactMatch	wd:Q182458 ;
	skos:inScheme	ccat: ;
	skos:notation	"10102010" ;
	skos:prefLabel	"Anthracite"@en .

ccat:10102020
	a	skos:Concept ;
	skos:broader	ccat:101020 ;
	skos:definition	"""Lignite, often referred to as brown coal, is a soft, brown, combustible, sedimentary rock formed from naturally compressed peat. It is considered the lowest rank of coal due to its relatively low heat content. It has a carbon content around 25 to 35 percent. It is mined all around the world and is used almost exclusively as a fuel for steam-electric power generation."""@en ;
	skos:exactMatch	agrovoc:c_32489 , eurovoc:1656 , stw:14194-5 , wd:Q156267 ;
	skos:inScheme	ccat: ;
	skos:notation	"10102020" ;
	skos:prefLabel	"Lignite"@en .

ccat:10102030
	a	skos:Concept ;
	skos:broader	ccat:101020 ;
	skos:definition	"""Coke is a grey, hard, and porous fuel with a high carbon content and few impurities, made by heating coal or oil in the absence of air--a destructive distillation process. It is an important industrial product, used mainly in iron ore smelting, but also as a fuel in stoves and forges when air pollution is a concern.

The unqualified term \"coke\" usually refers to the product derived from low-ash and low-sulphur bituminous coal by a process called coking. A similar product called petroleum coke, or pet coke, is obtained from crude oil in oil refineries. Coke may also be formed naturally by geologic processes."""@en ;
	skos:exactMatch	wd:Q192795 ;
	skos:inScheme	ccat: ;
	skos:notation	"10102030" ;
	skos:prefLabel	"Coke"@en .

ccat:101030
	a	skos:Concept ;
	skos:broader	ccat:1010 ;
	skos:definition	"Natural gas (also called fossil gas; sometimes just gas), is a naturally occurring hydrocarbon gas mixture consisting primarily of methane, but commonly including varying amounts of other higher alkanes, and sometimes a small percentage of carbon dioxide, nitrogen, hydrogen sulfide, or helium. It is formed when layers of decomposing plant and animal matter are exposed to intense heat and pressure under the surface of the Earth over millions of years. The energy that the plants originally obtained from the sun is stored in the form of chemical bonds in the gas. Natural gas is a fossil fuel."@en ;
	skos:exactMatch	agrovoc:c_5087 , eurovoc:1141 , stw:14196-1 , wd:Q40858 ;
	skos:inScheme	ccat: ;
	skos:notation	"101030" ;
	skos:prefLabel	"Natural Gas"@en .

ccat:101032
	a	skos:Concept ;
	skos:altLabel	"LNG"@en ;
	skos:broader	ccat:1010 ;
	skos:definition	"""Liquefied natural gas (LNG) is natural gas (predominantly methane, CH4, with some mixture of ethane, C2H6) that has been cooled down to liquid form for ease and safety of non-pressurized storage or transport. It takes up about 1/600th the volume of natural gas in the gaseous state (at standard conditions for temperature and pressure). It is odorless, colorless, non-toxic and non-corrosive. Hazards include flammability after vaporization into a gaseous state, freezing and asphyxia. The liquefaction process involves removal of certain components, such as dust, acid gases, helium, water, and heavy hydrocarbons, which could cause difficulty downstream. The natural gas is then condensed into a liquid at close to atmospheric pressure by cooling it to approximately -162 Â°C; maximum transport pressure is set at around 25 kPa (4 psi).

The gas produced from hydrocarbon deposits typically contains a wide range of hydrocarbon products, which usually includes methane (CH4), ethane (C2H6), propane (C3H8) and butane (C4H10). All these products have wide-ranging boiling points and also different heating values allowing different routes to commercialization and also different uses. The \"acidic\" elements such as hydrogen sulphide (H2S) and carbon dioxide (CO2), together with oil, mud, water, and mercury, are removed from the gas to deliver a clean sweetened stream of gas. Failure to remove such acidic molecules, mercury, and other impurities could result in damage to the equipment. Corrosion of steel pipes and amalgamization of mercury to aluminium within cryogenic heat exchangers could cause expensive damage.

The gas stream is typically separated into the Liquefied Petroleum fractions (butane and propane), which can be stored in liquid form at relatively low pressure, and the lighter ethane and methane fractions. These lighter fractions of methane and ethane are then liquefied to make up the bulk of LNG that is shipped.

Natural gas was considered to be economically unimportant wherever gas-producing oil or gas fields were distant from gas pipelines or located in offshore locations where pipelines were not viable. In the past this usually meant that natural gas produced was typically flared, especially since unlike oil no viable method for natural gas storage or transport existed other than pipelines which required the immediate use by end users of the same gas. This meant that natural gas markets were historically entirely local and any production had to be consumed within the local network.

Developments of production processes, cryogenic storage, and transportation effectively created the tools required to commercialize natural gas into a global market which now competes with other fuels. Furthermore, the development of LNG storage also introduced a reliability in networks which was previously thought impossible. Given that storage of other fuels is relatively easily secured using simple tanks, a supply for several months could be kept in storage. With the advent of large scale cryogenic storage, it was possible to create long term gas storage reserves. These reserves of liquefied gas could be deployed at a moment's notice through regasification processes and today are the main means for networks to handle local peak shaving requirements."""@en ;
	skos:exactMatch	stw:18236-2 , wd:Q358333 ;
	skos:inScheme	ccat: ;
	skos:notation	"101032" ;
	skos:prefLabel	"Liquefied Natural Gas"@en .

ccat:101035
	a	skos:Concept ;
	skos:altLabel	"LPG"@en ;
	skos:broader	ccat:1010 ;
	skos:definition	"""Liquefied petroleum gas (LPG or LP gas), is a flammable mixture of hydrocarbon gases used as fuel in heating appliances, cooking equipment, and vehicles. It is a mixture of 48% propane, 50% butane, and 2% pentane.

It is increasingly used as an aerosol propellant and a refrigerant, replacing chlorofluorocarbons in an effort to reduce damage to the ozone layer. When specifically used as a vehicle fuel it is often referred to as autogas.

Varieties of LPG bought and sold include mixes that are mostly propane (C3H8), mostly butane (C4H10), and, most commonly, mixes including both propane and butane. In the northern hemisphere winter, the mixes contain more propane, while in summer, they contain more butane. In the United States, mainly two grades of LPG are sold: commercial propane and HD-5. These specifications are published by the Gas Processors Association (GPA) and the American Society of Testing and Materials. Propane/butane blends are also listed in these specifications.

Propylene, butylenes and various other hydrocarbons are usually also present in small concentrations such as C2H6 ,CH4, and C3H8. HD-5 limits the amount of propylene that can be placed in LPG to 5% and is utilized as an autogas specification. A powerful odorant, ethanethiol, is added so that leaks can be detected easily. The internationally recognized European Standard is EN 589. In the United States, tetrahydrothiophene (thiophane) or amyl mercaptan are also approved odorants, although neither is currently being utilized.

LPG is prepared by refining petroleum or \"wet\" natural gas, and is almost entirely derived from fossil fuel sources, being manufactured during the refining of petroleum (crude oil), or extracted from petroleum or natural gas streams as they emerge from the ground. It was first produced in 1910 by Dr. Walter Snelling, and the first commercial products appeared in 1912. It currently provides about 3% of all energy consumed, and burns relatively cleanly with no soot and very few sulfur emissions. As it is a gas, it does not pose ground or water pollution hazards, but it can cause air pollution. LPG has a typical specific calorific value of 46.1 MJ/kg compared with 42.5 MJ/kg for fuel oil and 43.5 MJ/kg for premium grade petrol (gasoline). However, its energy density per volume unit of 26 MJ/L is lower than either that of petrol or fuel oil, as its relative density is lower (about 0.5-0.58 kg/L, compared to 0.71-0.77 kg/L for gasoline).

Besides using as energy carrier, the LPG is also a promising feedstock in the chemical industry for the synthesis of olefins such as ethylene, propylene, butene as well as acrylic acid.

As its boiling point is below room temperature and heat, LPG will evaporate quickly at normal temperatures and pressures and is usually supplied in pressurized steel vessels. They are typically filled to 80%-85% of their capacity to allow for thermal expansion of the contained liquid. The ratio between the volumes of the vaporized gas and the liquefied gas varies depending on composition, pressure, and temperature, but is typically around 250:1. The pressure at which LPG becomes liquid, called its vapour pressure, likewise varies depending on composition and temperature; for example, it is approximately 220 kilopascals (32 psi) for pure butane at 20 Â°C (68 Â°F), and approximately 2,200 kilopascals (320 psi) for pure propane at 55 Â°C (131 Â°F). LPG is heavier than air, unlike natural gas, and thus will flow along floors and tend to settle in low spots, such as basements. There are two main dangers to this. The first is a possible explosion if the mixture of LPG and air is within the explosive limits and there is an ignition source. The second is suffocation due to LPG displacing air, causing a decrease in oxygen concentration.

A full LPG cylinder contains 85% liquid; the ullage volume will contain vapour at a pressure that varies with temperature."""@en ;
	skos:exactMatch	wd:Q351609 ;
	skos:inScheme	ccat: ;
	skos:notation	"101035" ;
	skos:prefLabel	"Liquefied Petroleum Gas"@en .

ccat:101040
	a	skos:Concept ;
	skos:broader	ccat:1010 ;
	skos:definition	"""Petroleum products are materials derived from crude oil (petroleum) as it is processed in oil refineries. Unlike petrochemicals, which are a collection of well-defined usually pure chemical compounds, petroleum products are complex mixtures. The majority of petroleum is converted to petroleum products, which includes several classes of fuels.
	
	According to the composition of the crude oil and depending on the demands of the market, refineries can produce different shares of petroleum products. The largest share of oil products is used as \"energy carriers\", i.e. various grades of fuel oil and gasoline. These fuels include or can be blended to give gasoline, jet fuel, diesel fuel, heating oil, and heavier fuel oils. Heavier (less volatile) fractions can also be used to produce asphalt, tar, paraffin wax, lubricating and other heavy oils. Refineries also produce other chemicals, some of which are used in chemical processes to produce plastics and other useful materials. Since petroleum often contains a few percent sulfur-containing molecules, elemental sulfur is also often produced as a petroleum product. Carbon, in the form of petroleum coke, and hydrogen may also be produced as petroleum products. The hydrogen produced is often used as an intermediate product for other oil refinery processes such as hydrocracking and hydrodesulfurization."""@en ;
	skos:exactMatch	eurovoc:2772 , wd:Q1059843 ;
	skos:inScheme	ccat: ;
	skos:notation	"101040" ;
	skos:prefLabel	"Refined Products"@en ;
	skos:related	wd:Q3444730 .

ccat:10104010
	a	skos:Concept ;
	skos:broader	ccat:101040 ;
	skos:definition	"""Heating oil is any petroleum product or other oil used for heating; a fuel oil. Most commonly, it refers to low viscosity grades of fuel oil used for furnaces or boilers use for home heating and in other buildings. Home heating oil is often abbreviated as HHO.

Most heating oil products are chemically very similar to diesel fuel used as motor fuel; motor fuel is typically subject to higher fuel taxes. Many countries add fuel dyes to heating oil, allowing law enforcement to check if a driver is evading fuel taxes. Since 2002, Solvent Yellow 124 has been added as a \"Euromarker\" in the European Union; untaxed diesel is known as \"red diesel\" in the United Kingdom.

Heating oil is commonly delivered by tank truck to residential, commercial and municipal buildings and stored in above-ground storage tanks (\"ASTs\") located in the basements, garages, or outside adjacent to the building. It is sometimes stored in underground storage tanks (or \"USTs\") but less often than ASTs. ASTs are used for smaller installations due to the lower cost factor. Heating oil is less commonly used as an industrial fuel or for power generation."""@en ;
	skos:exactMatch	wd:Q912452 ;
	skos:inScheme	ccat: ;
	skos:narrowMatch	stw:14215-2 ;
	skos:notation	"10104010" ;
	skos:prefLabel	"Heating Oil"@en .

ccat:10104020
	a	skos:Concept ;
	skos:altLabel	"Petrol"@en ;
	skos:broader	ccat:101040 ;
	skos:definition	"""Gasoline, or petrol (see the etymology for naming differences), is a transparent, petroleum-derived flammable liquid that is used primarily as a fuel in most spark-ignited internal combustion engines. It consists mostly of organic compounds obtained by the fractional distillation of petroleum, enhanced with a variety of additives. On average, a 160-liter (42-U.S.-gallon) barrel of crude oil can yield up to about 72 liters (19 U.S. gallons) of gasoline after processing in an oil refinery, depending on the crude oil assay and on what other refined products are also extracted. The characteristic of a particular gasoline blend to resist igniting too early (which causes knocking and reduces efficiency in reciprocating engines) is measured by its octane rating, which is produced in several grades. Tetraethyl lead and other lead compounds, once widely used to increase octane rating, are no longer used in most areas (they are still used in aviation and auto-racing). Other chemicals are frequently added to gasoline to improve chemical stability and performance characteristics, control corrosiveness, and provide fuel system cleaning. Gasoline may contain oxygen-containing chemicals such as ethanol, MTBE, or ETBE to improve combustion.

Gasoline can enter the environment uncombusted, both as liquid and as vapor, from leakage and handling during production, transport, and delivery (e.g., from storage tanks, from spills, etc.). As an example of efforts to control such leakage, many underground storage tanks are required to have extensive measures in place to detect and prevent such leaks."""@en ;
	skos:exactMatch	agrovoc:c_5746 , eurovoc:3771 , stw:14212-1 , wd:Q39558 ;
	skos:inScheme	ccat: ;
	skos:notation	"10104020" ;
	skos:prefLabel	"Gasoline"@en .

ccat:10104030
	a	skos:Concept ;
	skos:broader	ccat:101040 ;
	skos:definition	"""Kerosene, also known as paraffin, is a combustible hydrocarbon liquid which is derived from petroleum. It is widely used as a fuel in aviation as well as households. Its name derives from Greek keros meaning \"wax\", and was registered as a trademark by Canadian geologist and inventor Abraham Gesner in 1854 before evolving into a genericized trademark. It is sometimes spelled kerosine in scientific and industrial usage. The term kerosene is common in much of Argentina, Australia, Canada, India, New Zealand, Nigeria, and the United States, while the term paraffin (or a closely related variant) is used in Chile, eastern Africa, South Africa, Norway, and in the United Kingdom. The term lamp oil, or the equivalent in the local languages, is common in the majority of Asia. Liquid paraffin (called mineral oil in the US) is a more viscous and highly refined product which is used as a laxative. Paraffin wax is a waxy solid extracted from petroleum.

Kerosene is widely used to power jet engines of aircraft (jet fuel) and some rocket engines in a highly refined form called RP-1. It is also commonly used as a cooking and lighting fuel, and for fire toys such as poi. In parts of Asia, kerosene is sometimes used as fuel for small outboard motors or even motorcycles. World total kerosene consumption for all purposes is equivalent to about 1.2 million barrels (50 million U.S. gallons; 42 million imperial gallons; 190 million liters) per day."""@en ;
	skos:exactMatch	wd:Q76904 ;
	skos:inScheme	ccat: ;
	skos:notation	"10104030" ;
	skos:prefLabel	"Kerosene"@en .

ccat:10104040
	a	skos:Concept ;
	skos:altLabel	"Petrodiesel"@en ;
	skos:broader	ccat:101040 ;
	skos:definition	"""Diesel fuel in general is any liquid fuel specifically designed for use in diesel engines, whose fuel ignition takes place, without any spark, as a result of compression of the inlet air mixture and then injection of fuel. Therefore, diesel fuel needs good compression ignition characteristics.

The most common type of diesel fuel is a specific fractional distillate of petroleum fuel oil, but alternatives that are not derived from petroleum, such as biodiesel, biomass to liquid (BTL) or gas to liquid (GTL) diesel, are increasingly being developed and adopted. To distinguish these types, petroleum-derived diesel is increasingly called petrodiesel in some academic circles.

In many countries, diesel fuel is standardised. For example, in the European Union, the standard for diesel fuel is EN 590. Diesel fuel has many colloquial names, most commonly, it is simply referred to as Diesel. In the UK, diesel fuel for on-road use is commonly abbreviated DERV, standing for diesel-engined road vehicle, which carries a tax premium over equivalent fuel for non-road use. In Australia, diesel fuel is also known as distillate, and in Indonesia, it is known as Solar, a trademarked name by the local oil company Pertamina.

Ultra-low-sulfur diesel (ULSD) is a diesel fuel with substantially lowered sulfur contents. As of 2016, almost all of the petroleum-based diesel fuel available in the UK, mainland Europe, and North America is of a ULSD type.

Before diesel fuel had been standardised, the majority of diesel engines typically ran on cheap fuel oils; these fuel oils are still used in watercraft diesel engines. Despite being specifically designed for diesel engines, diesel fuel can also be used as fuel for several non-diesel engines, for example the Akroyd engine, the Stirling engine, or boilers for steam engines."""@en ;
	skos:exactMatch	eurovoc:3772 , stw:14214-4 , wd:Q38423 ;
	skos:inScheme	ccat: ;
	skos:notation	"10104040" ;
	skos:prefLabel	"Diesel"@en .

ccat:101050
	a	skos:Concept ;
	skos:broader	ccat:1010 ;
	skos:definition	"""Electrical energy is energy derived from electric potential energy or kinetic energy. When used loosely, electrical energy refers to energy that has been converted from electric potential energy. This energy is supplied by the combination of electric current and electric potential that is delivered by an electrical circuit (e.g., provided by an electric power utility). At the point that this electric potential energy has been converted to another type of energy, it ceases to be electric potential energy. Thus, all electrical energy is potential energy before it is delivered to the end-use. Once converted from potential energy, electrical energy can always be called another type of energy (heat, light, motion, etc.).
	
	Electrical energy is usually sold by the kilowatt hour (1 kWÃÂ·h = 3.6 MJ) which is the product of the power in kilowatts multiplied by running time in hours. Electric utilities measure energy using an electricity meter, which keeps a running total of the electric energy delivered to a customer."""@en ;
	skos:exactMatch	eurovoc:747 , stw:14174-4 , wd:Q206799 ;
	skos:inScheme	ccat: ;
	skos:notation	"101050" ;
	skos:prefLabel	"Electricity"@en .

ccat:10105010
	a	skos:Concept ;
	skos:broader	ccat:101050 ;
	skos:definition	"The base load is the minimum level of demand on an electrical grid over a span of time, for example, one week. This demand can be met by unvarying power plants, dispatchable generation, or by a collection of smaller intermittent energy sources, depending on which approach has the best mix of low cost, availability and high reliability in any particular market."@en ;
	skos:exactMatch	wd:Q360897 ;
	skos:inScheme	ccat: ;
	skos:notation	"10105010" ;
	skos:prefLabel	"Base Load"@en .

ccat:10105020
	a	skos:Concept ;
	skos:broader	ccat:101050 ;
	skos:definition	"Peak demand on an electrical grid is simply the highest electrical power demand that has occurred over a specified time period (GC6nen 2008). Peak demand is typically characterized as annual, daily or seasonal and has the unit of power. Peak demand, peak load or on-peak are terms used in energy demand management describing a period in which electrical power is expected to be provided for a sustained period at a significantly higher than average supply level. Peak demand fluctuations may occur on daily, monthly, seasonal and yearly cycles. For an electric utility company, the actual point of peak demand is a single half-hour or hourly period which represents the highest point of customer consumption of electricity. At this time there is a combination of office, domestic demand and at some times of the year, the fall of darkness."@en ;
	skos:exactMatch	wd:Q3393666 ;
	skos:inScheme	ccat: ;
	skos:notation	"10105020" ;
	skos:prefLabel	"Peak Load"@en .

ccat:10105030
	a	skos:Concept ;
	skos:broader	ccat:101050 ;
	skos:definition	"Period in the load profile that shows nearly no peaks, typically the night."@en ;
	skos:inScheme	ccat: ;
	skos:notation	"10105030" ;
	skos:prefLabel	"Off-peak"@en .

ccat:10105040
	a	skos:Concept ;
	skos:broader	ccat:101050 ;
	skos:definition	"Upwards or downwards flank between off-peak and on-peak demand covered by special load following plants."@en ;
	skos:inScheme	ccat: ;
	skos:notation	"10105040" ;
	skos:prefLabel	"Shoulder"@en .

ccat:10105050
	a	skos:Concept ;
	skos:broader	ccat:101050 ;
	skos:definition	"Transmission rights entitle the holder to receive compensation for congestion charges across an energy path."@en ;
	skos:inScheme	ccat: ;
	skos:notation	"10105050" ;
	skos:prefLabel	"Transmission Rights"@en .

ccat:1020
	a	skos:Concept ;
	skos:broader	ccat:10 ;
	skos:definition	"""Precious metals are rare, naturally occurring metallic chemical element of high economic value. Chemically, the precious metals tend to be less reactive than most elements (see noble metal). They are usually ductile and have a high lustre. Historically, precious metals were important as currency but are now regarded mainly as investment and industrial commodities. Gold, silver, platinum, and palladium each have an ISO 4217 currency code.

The best known precious metals are the coinage metals, which are gold and silver. Although both have industrial uses, they are better known for their uses in art, jewelry, and coinage. Other precious metals include the platinum group metals: ruthenium, rhodium, palladium, osmium, iridium, and platinum, of which platinum is the most widely traded. The demand for precious metals is driven not only by their practical use but also by their role as investments and a store of value. Historically, precious metals have commanded much higher prices than common industrial metals."""@en ;
	skos:exactMatch	eurovoc:1886 , stw:14296-4 , wd:Q271449 ;
	skos:inScheme	ccat: ;
	skos:notation	"1020" ;
	skos:prefLabel	"Precious Metal"@en .

ccat:102010
	a	skos:Concept ;
	skos:broader	ccat:1020 ;
	skos:definition	"""Gold in its pure form is a bright, slightly reddish yellow, dense, soft, malleable, and ductile metal. It is one of the least reactive chemical elements and is solid under standard conditions. Gold often occurs in free elemental (native) form, as nuggets or grains, in rocks, in veins, and in alluvial deposits. It occurs in a solid solution series with the native element silver (as electrum) and also naturally alloyed with copper and palladium. Less commonly, it occurs in minerals as gold compounds, often with tellurium (gold tellurides).

A relatively rare element, gold is a precious metal that has been used for coinage, jewelry, and other arts throughout recorded history. In the past, a gold standard was often implemented as a monetary policy, but gold coins ceased to be minted as a circulating currency in the 1930s, and the world gold standard was abandoned for a fiat currency system after 1971.

The world consumption of new gold produced is about 50% in jewelry, 40% in investments, and 10% in industry. Gold's high malleability, ductility, resistance to corrosion and most other chemical reactions, and conductivity of electricity have led to its continued use in corrosion resistant electrical connectors in all types of computerized devices (its chief industrial use). Gold is also used in infrared shielding, colored-glass production, gold leafing, and tooth restoration. Certain gold salts are still used as anti-inflammatories in medicine. As of 2017, the world's largest gold producer by far was China with 440 tonnes per year."""@en ;
	skos:exactMatch	agrovoc:c_33067 , eurovoc:2156 , stw:14298-0 , wd:Q897 ;
	skos:inScheme	ccat: ;
	skos:notation	"102010" ;
	skos:prefLabel	"Gold"@en .

ccat:102020
	a	skos:Concept ;
	skos:broader	ccat:1020 ;
	skos:definition	"""Silver in its pure form is a soft, white, lustrous transition metal, it exhibits the highest electrical conductivity, thermal conductivity, and reflectivity of any metal. The metal is found in the Earth's crust in the pure, free elemental form (\"native silver\"), as an alloy with gold and other metals, and in minerals such as argentite and chlorargyrite. Most silver is produced as a byproduct of copper, gold, lead, and zinc refining.

Silver has long been valued as a precious metal. Silver metal is used in many bullion coins, sometimes alongside gold: while it is more abundant than gold, it is much less abundant as a native metal. Its purity is typically measured on a per-mille basis; a 94%-pure alloy is described as \"0.940 fine\". As one of the seven metals of antiquity, silver has had an enduring role in most human cultures.

Other than in currency and as an investment medium (coins and bullion), silver is used in solar panels, water filtration, jewellery, ornaments, high-value tableware and utensils (hence the term silverware), in electrical contacts and conductors, in specialized mirrors, window coatings, in catalysis of chemical reactions, as a colorant in stained glass and in specialised confectionery. Its compounds are used in photographic and X-ray film. Dilute solutions of silver nitrate and other silver compounds are used as disinfectants and microbiocides (oligodynamic effect), added to bandages and wound-dressings, catheters, and other medical instruments."""@en ;
	skos:exactMatch	agrovoc:c_7068 , eurovoc:2514 , stw:14308-2 , wd:Q1090 ;
	skos:inScheme	ccat: ;
	skos:notation	"102020" ;
	skos:prefLabel	"Silver"@en .

ccat:102030
	a	skos:Concept ;
	skos:broader	ccat:1020 ;
	skos:definition	"""Platinum in its pure form is a dense, malleable, ductile, highly unreactive, precious, silverish-white transition metal. Its name is derived from the Spanish term platino, meaning \"little silver\".

Platinum is a member of the platinum group of elements and group 10 of the periodic table of elements. It has six naturally occurring isotopes. It is one of the rarer elements in Earth's crust, with an average abundance of approximately 5 Â¼g/kg. It occurs in some nickel and copper ores along with some native deposits, mostly in South Africa, which accounts for 80% of the world production. Because of its scarcity in Earth's crust, only a few hundred tonnes are produced annually, and given its important uses, it is highly valuable and is a major precious metal commodity.

Platinum is one of the least reactive metals. It has remarkable resistance to corrosion, even at high temperatures, and is therefore considered a noble metal. Consequently, platinum is often found chemically uncombined as native platinum. Because it occurs naturally in the alluvial sands of various rivers, it was first used by pre-Columbian South American natives to produce artifacts. It was referenced in European writings as early as 16th century, but it was not until Antonio de Ulloa published a report on a new metal of Colombian origin in 1748 that it began to be investigated by scientists.

Platinum is used in catalytic converters, laboratory equipment, electrical contacts and electrodes, platinum resistance thermometers, dentistry equipment, and jewelry. Being a heavy metal, it leads to health problems upon exposure to its salts; but due to its corrosion resistance, metallic platinum has not been linked to adverse health effects. Compounds containing platinum, such as cisplatin, oxaliplatin and carboplatin, are applied in chemotherapy against certain types of cancer."""@en ;
	skos:exactMatch	agrovoc:c_33116 , eurovoc:2424 , stw:14306-6 , wd:Q880 ;
	skos:inScheme	ccat: ;
	skos:notation	"102030" ;
	skos:prefLabel	"Platinum"@en .

ccat:102040
	a	skos:Concept ;
	skos:broader	ccat:1020 ;
	skos:definition	"""Palladium in its pure form is a rare and lustrous silvery-white metal discovered in 1803 by the English chemist William Hyde Wollaston. He named it after the asteroid Pallas, which was itself named after the epithet of the Greek goddess Athena, acquired by her when she slew Pallas. Palladium, platinum, rhodium, ruthenium, iridium and osmium form a group of elements referred to as the platinum group metals (PGMs). They have similar chemical properties, but palladium has the lowest melting point and is the least dense of them.

More than half the supply of palladium and its congener platinum is used in catalytic converters, which convert as much as 90% of the harmful gases in automobile exhaust (hydrocarbons, carbon monoxide, and nitrogen dioxide) into less noxious substances (nitrogen, carbon dioxide and water vapor). Palladium is also used in electronics, dentistry, medicine, hydrogen purification, chemical applications, groundwater treatment, and jewelry. Palladium is a key component of fuel cells, which react hydrogen with oxygen to produce electricity, heat, and water.

Ore deposits of palladium and other PGMs are rare. The most extensive deposits have been found in the norite belt of the Bushveld Igneous Complex covering the Transvaal Basin in South Africa, the Stillwater Complex in Montana, United States; the Sudbury Basin and Thunder Bay District of Ontario, Canada, and the Norilsk Complex in Russia. Recycling is also a source, mostly from scrapped catalytic converters. The numerous applications and limited supply sources result in considerable investment interest."""@en ;
	skos:exactMatch	wd:Q1089 ;
	skos:inScheme	ccat: ;
	skos:notation	"102040" ;
	skos:prefLabel	"Palladium"@en .

ccat:102050
	a	skos:Concept ;
	skos:broader	ccat:1020 ;
	skos:definition	"""Iridium a is very hard, brittle, silvery-white transition metal of the platinum group, iridium is considered to be the second-densest metal (after osmium). ridium is one of the rarest elements in Earth's crust, with annual production and consumption of only three tonnes.

The most important iridium compounds in use are the salts and acids it forms with chlorine, though iridium also forms a number of organometallic compounds used in industrial catalysis, and in research. Iridium metal is employed when high corrosion resistance at high temperatures is needed, as in high-performance spark plugs, crucibles for recrystallization of semiconductors at high temperatures, and electrodes for the production of chlorine in the chloralkali process. Iridium radioisotopes are used in some radioisotope thermoelectric generators."""@en ;
	skos:exactMatch	wd:Q877 ;
	skos:inScheme	ccat: ;
	skos:notation	"102050" ;
	skos:prefLabel	"Iridium"@en .

ccat:102060
	a	skos:Concept ;
	skos:broader	ccat:1020 ;
	skos:definition	"""Rhodium is an ultra-rare, silvery-white, hard, corrosion-resistant, and chemically inert transition metal. It is a noble metal and a member of the platinum group. Rhodium is found in platinum or nickel ores together with the other members of the platinum group metals.

The element's major use (approximately 80% of world rhodium production) is as one of the catalysts in the three-way catalytic converters in automobiles. Because rhodium metal is inert against corrosion and most aggressive chemicals, and because of its rarity, rhodium is usually alloyed with platinum or palladium and applied in high-temperature and corrosion-resistive coatings. White gold is often plated with a thin rhodium layer to improve its appearance while sterling silver is often rhodium-plated for tarnish resistance. Rhodium is sometimes used to cure silicones; a two-part silicone in which one part containing a silicon hydride and the other containing a vinyl-terminated silicone are mixed. One of these liquids contains a rhodium complex.

Rhodium detectors are used in nuclear reactors to measure the neutron flux level. Other uses of rhodium include asymmetric hydrogenation used to form drug precursors and the processes for the production of acetic acid."""@en ;
	skos:exactMatch	wd:Q1087 ;
	skos:inScheme	ccat: ;
	skos:notation	"102060" ;
	skos:prefLabel	"Rhodium"@en .

ccat:102070
	a	skos:Concept ;
	skos:broader	ccat:1020 ;
	skos:definition	"""Ruthenium is a chemical element with the symbol Ru and atomic number 44. It is a rare transition metal belonging to the platinum group of the periodic table. Like the other metals of the platinum group, ruthenium is inert to most other chemicals. Russian-born scientist of Baltic-German ancestry Karl Ernst Claus discovered the element in 1844 at Kazan State University and named ruthenium in honor of Russia. Ruthenium is usually found as a minor component of platinum ores; the annual production has risen from about 19 tonnes in 2009 to some 35.5 tonnes in 2017. Most ruthenium produced is used in wear-resistant electrical contacts and thick-film resistors. A minor application for ruthenium is in platinum alloys and as a chemistry catalyst. A new application of ruthenium is as the capping layer for extreme ultraviolet photomasks. Ruthenium is generally found in ores with the other platinum group metals in the Ural Mountains and in North and South America. Small but commercially important quantities are also found in pentlandite extracted from Sudbury, Ontario and in pyroxenite deposits in South Africa."""@en ;
	skos:exactMatch	wd:Q1086 ;
	skos:inScheme	ccat: ;
	skos:notation	"102070" ;
	skos:prefLabel	"Ruthenium"@en .

ccat:1030
	a	skos:Concept ;
	skos:altLabel	"Non-ferrous Metal"@en ;
	skos:broader	ccat:10 ;
	skos:closeMatch	wd:Q428855 , wd:Q5679431 ;
	skos:definition	"A base metal is a common and inexpensive non-ferrous metal, as opposed to a precious metal."@en ;
	skos:inScheme	ccat: ;
	skos:notation	"1030" ;
	skos:prefLabel	"Base Metal"@en .

ccat:103010
	a	skos:Concept ;
	skos:broader	ccat:1030 ;
	skos:definition	"Copper is a soft, malleable, and ductile metal with very high thermal and electrical conductivity. A freshly exposed surface of pure copper has a pinkish-orange color. Copper is used as a conductor of heat and electricity, as a building material, and as a constituent of various metal alloys, such as sterling silver used in jewelry, cupronickel used to make marine hardware and coins, and constantan used in strain gauges and thermocouples for temperature measurement."@en ;
	skos:exactMatch	agrovoc:c_1868 , stw:14299-5 , wd:Q753 ;
	skos:inScheme	ccat: ;
	skos:notation	"103010" ;
	skos:prefLabel	"Copper"@en .

ccat:103020
	a	skos:Concept ;
	skos:broader	ccat:1030 ;
	skos:definition	"""Aluminium (aluminum in American and Canadian English) is a chemical element with the symbol Al and atomic number 13. It is a silvery-white, soft, non-magnetic and ductile metal in the boron group. By mass, aluminium is the most abundant metal in the Earth's crust and the third most abundant element (after oxygen and silicon). The abundance of aluminium decreases relative to other elements at greater depths into Earth's mantle and beyond. The chief ore of aluminium is bauxite. Aluminium metal is highly reactive, so native specimens are rare and limited to extreme reducing environments. Instead, it is found combined in over 270 different minerals.

Aluminium is remarkable for its low density and its ability to resist corrosion through the phenomenon of passivation. Aluminium and its alloys are vital to the aerospace industry and important in transportation and building industries, such as building facades and window frames. The oxides and sulfates are the most useful compounds of aluminium.

Despite its prevalence in the environment, no living organism is known to use aluminium salts metabolically, but aluminium is well tolerated by plants and animals. Because of these salts' abundance, the potential for a biological role for them is of continuing interest, and studies continue."""@en ;
	skos:exactMatch	agrovoc:c_317 , eurovoc:1446 , msa:513153333 , stw:14293-3 , wd:Q663 ;
	skos:inScheme	ccat: ;
	skos:notation	"103020" ;
	skos:prefLabel	"Aluminium"@en .

ccat:103025
	a	skos:Concept ;
	skos:altLabel	"NASAAC"@en ;
	skos:broader	ccat:1030 ;
	skos:definition	"Aluminium alloy conforming to the LME NA380.1 specification which is a modification of The Aluminium Association Inc. A380.1 specification (1989).  The alloy has a composition of 8.50%-9.50% Si, 3.00%-3.50% Cu, 0.80%-1.00% Fe, a maximum of 3.00% Zn, a maximum of 1.80% sludge (Fe + 2Mn + 3Cr), a maximum of 0.50% Ni, a maximum of 0.45% Mn, a maximum of 0.10% Mg, Sn, Pb, Ti, and Cr each."@en ;
	skos:inScheme	ccat: ;
	skos:notation	"103025" ;
	skos:prefLabel	"North American Special Aluminum Alloy"@en .

ccat:103030
	a	skos:Concept ;
	skos:broader	ccat:1030 ;
	skos:definition	"""Zinc is a chemical element with the symbol Zn and atomic number 30. Zinc is a slightly brittle metal at room temperature and has a blue-silvery appearance when oxidation is removed. It is the first element in group 12 of the periodic table. In some respects, zinc is chemically similar to magnesium: both elements exhibit only one normal oxidation state (+2), and the Zn2+ and Mg2+ ions are of similar size. Zinc is the 24th most abundant element in Earth's crust and has five stable isotopes. The most common zinc ore is sphalerite (zinc blende), a zinc sulfide mineral. The largest workable lodes are in Australia, Asia, and the United States. Zinc is refined by froth flotation of the ore, roasting, and final extraction using electricity (electrowinning).

Brass, an alloy of copper and zinc in various proportions, was used as early as the third millennium BC in the Aegean, Iraq, the United Arab Emirates, Kalmykia, Turkmenistan and Georgia, and the second millennium BC in West India, Uzbekistan, Iran, Syria, Iraq, and Israel/Palestine. Zinc metal was not produced on a large scale until the 12th century in India, though it was known to the ancient Romans and Greeks. The mines of Rajasthan have given definite evidence of zinc production going back to the 6th century BC. To date, the oldest evidence of pure zinc comes from Zawar, in Rajasthan, as early as the 9th century AD when a distillation process was employed to make pure zinc. Alchemists burned zinc in air to form what they called \"philosopher's wool\" or \"white snow\".

Zinc is an essential mineral, including to prenatal and postnatal development. Zinc deficiency affects about two billion people in the developing world and is associated with many diseases. In children, deficiency causes growth retardation, delayed sexual maturation, infection susceptibility, and diarrhea. Enzymes with a zinc atom in the reactive center are widespread in biochemistry, such as alcohol dehydrogenase in humans."""@en ;
	skos:exactMatch	agrovoc:c_8517 , eurovoc:4783 , stw:14309-0 , wd:Q758 ;
	skos:inScheme	ccat: ;
	skos:notation	"103030" ;
	skos:prefLabel	"Zinc"@en .

ccat:103040
	a	skos:Concept ;
	skos:broader	ccat:1030 ;
	skos:definition	"""Nickel is a chemical element with the symbol Ni and atomic number 28. It is a silvery-white lustrous metal with a slight golden tinge. Nickel belongs to the transition metals and is hard and ductile. Pure nickel, powdered to maximize the reactive surface area, shows a significant chemical activity, but larger pieces are slow to react with air under standard conditions because an oxide layer forms on the surface and prevents further corrosion (passivation). Even so, pure native nickel is found in Earth's crust only in tiny amounts, usually in ultramafic rocks, and in the interiors of larger nickel-iron meteorites that were not exposed to oxygen when outside Earth's atmosphere.

Meteoric nickel is found in combination with iron, a reflection of the origin of those elements as major end products of supernova nucleosynthesis. An iron-nickel mixture is thought to compose Earth's outer and inner cores.

Use of nickel (as a natural meteoric nickel-iron alloy) has been traced as far back as 3500 BCE. Nickel was first isolated and classified as a chemical element in 1751 by Axel Fredrik Cronstedt, who initially mistook the ore for a copper mineral, in the cobalt mines of Los, HÃÂ¤lsingland, Sweden. The element's name comes from a mischievous sprite of German miner mythology, Nickel (similar to Old Nick), who personified the fact that copper-nickel ores resisted refinement into copper. An economically important source of nickel is the iron ore limonite, which often contains 1-2% nickel. Nickel's other important ore minerals include pentlandite and a mixture of Ni-rich natural silicates known as garnierite. Major production sites include the Sudbury region in Canada (which is thought to be of meteoric origin), New Caledonia in the Pacific, and Norilsk in Russia.

Nickel is slowly oxidized by air at room temperature and is considered corrosion-resistant. Historically, it has been used for plating iron and brass, coating chemistry equipment, and manufacturing certain alloys that retain a high silvery polish, such as German silver. About 9% of world nickel production is still used for corrosion-resistant nickel plating. Nickel-plated objects sometimes provoke nickel allergy. Nickel has been widely used in coins, though its rising price has led to some replacement with cheaper metals in recent years.

Nickel is one of four elements (the others are iron, cobalt, and gadolinium) that are ferromagnetic at approximately room temperature. Alnico permanent magnets based partly on nickel are of intermediate strength between iron-based permanent magnets and rare-earth magnets. The metal is valuable in modern times chiefly in alloys; about 68% of world production is used in stainless steel. A further 10% is used for nickel-based and copper-based alloys, 7% for alloy steels, 3% in foundries, 9% in plating and 4% in other applications, including the fast-growing battery sector, including those in electric vehicles (EVs). As a compound, nickel has a number of niche chemical manufacturing uses, such as a catalyst for hydrogenation, cathodes for batteries, pigments and metal surface treatments. Nickel is an essential nutrient for some microorganisms and plants that have enzymes with nickel as an active site."""@en ;
	skos:exactMatch	agrovoc:c_5172 , eurovoc:2056 , stw:14305-1 , wd:Q744 ;
	skos:inScheme	ccat: ;
	skos:notation	"103040" ;
	skos:prefLabel	"Nickel"@en .

ccat:103050
	a	skos:Concept ;
	skos:broader	ccat:1030 ;
	skos:definition	"""Tin is a chemical element with the symbol Sn (from Latin: stannum) and atomic number 50. Tin is a silvery metal that characteristically has a faint yellow hue. Tin, like indium, is soft enough to be cut without much force. When a bar of tin is bent, the so-called \"tin cry\" can be heard as a result of twinning in tin crystals; this trait is shared by indium, cadmium, and frozen mercury. Pure tin after solidifying keeps a mirror-like appearance similar to most metals. However, in most tin alloys (such as pewter), the metal solidifies with a dull gray color. Tin is a post-transition metal in group 14 of the periodic table of elements. It is obtained chiefly from the mineral cassiterite, which contains stannic oxide, SnO2. Tin shows a chemical similarity to both of its neighbors in group 14, germanium and lead, and has two main oxidation states, +2 and the slightly more stable +4. Tin is the 49th most abundant element on Earth and has, with 10 stable isotopes, the largest number of stable isotopes in the periodic table, thanks to its magic number of protons. It has two main allotropes: at room temperature, the stable allotrope is beta-tin, a silvery-white, malleable metal, but at low temperatures, it transforms into the less dense grey alpha-tin, which has the diamond cubic structure. Metallic tin does not easily oxidize in air.

The first tin alloy used on a large scale was bronze, made of 1/8 tin and 7/8 copper, from as early as 3000 BC. After 600 BC, pure metallic tin was produced. Pewter, which is an alloy of 85-90% tin with the remainder commonly consisting of copper, antimony, and lead, was used for flatware from the Bronze Age until the 20th century. In modern times, tin is used in many alloys, most notably tin / lead soft solders, which are typically 60% or more tin, and in the manufacture of transparent, electrically conducting films of indium tin oxide in optoelectronic applications. Another large application for tin is corrosion-resistant tin plating of steel. Because of the low toxicity of inorganic tin, tin-plated steel is widely used for food packaging as tin cans. However, some organotin compounds can be almost as toxic as cyanide."""@en ;
	skos:exactMatch	agrovoc:c_7782 , eurovoc:879 , stw:14310-1 , wd:Q1096 ;
	skos:inScheme	ccat: ;
	skos:notation	"103050" ;
	skos:prefLabel	"Tin"@en .

ccat:103060
	a	skos:Concept ;
	skos:broader	ccat:1030 ;
	skos:definition	"""Lead is a chemical element with the symbol Pb (from the Latin plumbum) and atomic number 82. It is a heavy metal that is denser than most common materials. Lead is soft and malleable, and also has a relatively low melting point. When freshly cut, lead is silvery with a hint of blue; it tarnishes to a dull gray color when exposed to air. Lead has the highest atomic number of any stable element and three of its isotopes are endpoints of major nuclear decay chains of heavier elements.

Lead is a relatively unreactive post-transition metal. Its weak metallic character is illustrated by its amphoteric nature; lead and lead oxides react with acids and bases, and it tends to form covalent bonds. Compounds of lead are usually found in the +2 oxidation state rather than the +4 state common with lighter members of the carbon group. Exceptions are mostly limited to organolead compounds. Like the lighter members of the group, lead tends to bond with itself; it can form chains and polyhedral structures.

Lead is easily extracted from its ores; prehistoric people in Western Asia knew of it. Galena is a principal ore of lead which often bears silver. Interest in silver helped initiate widespread extraction and use of lead in ancient Rome. Lead production declined after the fall of Rome and did not reach comparable levels until the Industrial Revolution. In 2014, the annual global production of lead was about ten million tonnes, over half of which was from recycling. Lead's high density, low melting point, ductility and relative inertness to oxidation make it useful. These properties, combined with its relative abundance and low cost, resulted in its extensive use in construction, plumbing, batteries, bullets and shot, weights, solders, pewters, fusible alloys, white paints, leaded gasoline, and radiation shielding.

In the late 19th century, lead's toxicity was recognized, and its use has since been phased out of many applications. However, many countries still allow the sale of products that expose humans to lead, including some types of paints and bullets. Lead is a neurotoxin that accumulates in soft tissues and bones; it damages the nervous system and interferes with the function of biological enzymes, causing neurological disorders, such as brain damage and behavioral problems."""@en ;
	skos:exactMatch	agrovoc:c_4235 , eurovoc:2428 , msa:2909791279 , stw:14294-1 , wd:Q708 ;
	skos:inScheme	ccat: ;
	skos:notation	"103060" ;
	skos:prefLabel	"Lead"@en .

ccat:103070
	a	skos:Concept ;
	skos:broader	ccat:1030 ;
	skos:definition	"""Titanium is a lustrous transition metal with a silver color, low density, and high strength. Titanium is resistant to corrosion in sea water, aqua regia, and chlorine.

The element occurs within a number of mineral deposits, principally rutile and ilmenite, which are widely distributed in the Earth's crust and lithosphere; it is found in almost all living things, as well as bodies of water, rocks, and soils. The metal is extracted from its principal mineral ores by the Kroll and Hunter processes. The most common compound, titanium dioxide, is a popular photocatalyst and is used in the manufacture of white pigments. Other compounds include titanium tetrachloride (TiCl4), a component of smoke screens and catalysts; and titanium trichloride (TiCl3), which is used as a catalyst in the production of polypropylene.

Titanium can be alloyed with iron, aluminium, vanadium, and molybdenum, among other elements, to produce strong, lightweight alloys for aerospace (jet engines, missiles, and spacecraft), military, industrial processes (chemicals and petrochemicals, desalination plants, pulp, and paper), automotive, agriculture (farming), medical prostheses, orthopedic implants, dental and endodontic instruments and files, dental implants, sporting goods, jewelry, mobile phones, and other applications.

The two most useful properties of the metal are corrosion resistance and strength-to-density ratio, the highest of any metallic element. In its unalloyed condition, titanium is as strong as some steels, but less dense.

Titanium is traded almost exclusively as titanium dioxide."""@en ;
	skos:exactMatch	agrovoc:c_32704 , eurovoc:4462 , msa:506065880 , stw:18240-4 , wd:Q716 ;
	skos:inScheme	ccat: ;
	skos:notation	"103070" ;
	skos:prefLabel	"Titanium"@en .

ccat:1035
	a	skos:Concept ;
	skos:broader	ccat:10 ;
	skos:definition	"Iron and iron-related metals, or alloys that contain iron or iron-related metals, such as steel or pig iron."@en ;
	skos:exactMatch	wd:Q2380954 ;
	skos:inScheme	ccat: ;
	skos:notation	"1035" ;
	skos:prefLabel	"Ferrous Metal"@en .

ccat:103510
	a	skos:Concept ;
	skos:broader	ccat:1035 ;
	skos:definition	"""Pig iron, also known as crude iron, is an intermediate product of the iron industry in the production of steel which is obtained by smelting iron ore in a blast furnace. Pig iron has a very high carbon content, typically 3.8-4.7% along with silica and other constituents of dross, which makes it very brittle and not useful directly as a material except for limited applications.

Iron is a chemical element with symbol Fe (from Latin: ferrum) and atomic number 26. It is a metal that belongs to the first transition series and group 8 of the periodic table. It is by mass the most common element on Earth, right in front of oxygen (32.1% and 30.1%, respectively), forming much of Earth's outer and inner core. It is the fourth most common element in the Earth's crust.

In its metallic state, iron is rare in the Earth's crust, limited mainly to deposition by meteorites. Iron ores, by contrast, are among the most abundant in the Earth's crust, although extracting usable metal from them requires kilns or furnaces capable of reaching 1,500 Â°C (2,730 Â°F) or higher, about 500 Â°C (900 Â°F) higher than that required to smelt copper. Humans started to master that process in Eurasia only about 2000 BCE, and the use of iron tools and weapons began to displace copper alloys, in some regions, only around 1200 BCE. That event is considered the transition from the Bronze Age to the Iron Age. In the modern world, iron alloys, such as steel, inox, cast iron and special steels are by far the most common industrial metals, because of their mechanical properties and low cost.

Pristine and smooth pure iron surfaces are mirror-like silvery-gray. However, iron reacts readily with oxygen and water to give brown to black hydrated iron oxides, commonly known as rust. Unlike the oxides of some other metals, that form passivating layers, rust occupies more volume than the metal and thus flakes off, exposing fresh surfaces for corrosion.

The body of an adult human contains about 4 grams (0.005% body weight) of iron, mostly in hemoglobin and myoglobin. These two proteins play essential roles in vertebrate metabolism, respectively oxygen transport by blood and oxygen storage in muscles. To maintain the necessary levels, human iron metabolism requires a minimum of iron in the diet. Iron is also the metal at the active site of many important redox enzymes dealing with cellular respiration and oxidation and reduction in plants and animals."""@en ;
	skos:exactMatch	agrovoc:c_3950 , eurovoc:981 , stw:14281-3 , wd:Q901785 ;
	skos:inScheme	ccat: ;
	skos:notation	"103510" ;
	skos:prefLabel	"Pig Iron"@en .

ccat:103520
	a	skos:Concept ;
	skos:broader	ccat:1035 ;
	skos:definition	"Steel is an alloy of iron with typically a few percent of carbon to improve its strength and fracture resistance compared to iron. Many other additional elements may be present or added. Stainless steels that are corrosion and oxidation resistant need typically an additional 11% chromium. Because of its high tensile strength and low cost, steel is used in buildings, infrastructure, tools, ships, trains, cars, machines, electrical appliances, and weapons. Iron is the base metal of steel and it can take on two crystalline forms (allotropic forms): body centred cubic and face-centred cubic. These forms depend on temperature. In the body-centred cubic arrangement, there is an iron atom in the centre and eight atoms at the vertices of each cubic unit cell; in the face-centred cubic, there is one atom at the centre of each of the six faces of the cubic unit cell and eight atoms at its vertices. It is the interaction of the allotropes of iron with the alloying elements, primarily carbon, that gives steel and cast iron their range of unique properties."@en ;
	skos:exactMatch	agrovoc:c_7384 , eurovoc:5065 , stw:14285-2 , wd:Q11427 ;
	skos:inScheme	ccat: ;
	skos:notation	"103520" ;
	skos:prefLabel	"Steel"@en .

ccat:103530
	a	skos:Concept ;
	skos:broader	ccat:1035 ;
	skos:definition	"""Iron ores are rocks and minerals from which metallic iron can be economically extracted. The ores are usually rich in iron oxides and vary in color from dark grey, bright yellow, or deep purple to rusty red. The iron is usually found in the form of magnetite (Fe3O4, 72.4% Fe), hematite (Fe2O3, 69.9% Fe), goethite (FeO(OH), 62.9% Fe), limonite (FeO(OH)ÃÂ·n(H2O), 55% Fe) or siderite (FeCO3, 48.2% Fe).

Ores containing very high quantities of hematite or magnetite (greater than about 60% iron) are known as \"natural ore\" or \"direct shipping ore\", meaning they can be fed directly into iron-making blast furnaces. Iron ore is the raw material used to make pig iron, which is one of the main raw materials to make steel---98% of the mined iron ore is used to make steel. In 2011 the Financial Times has speculated that iron ore is \"more integral to the global economy than any other commodity, except perhaps oil."""@en ;
	skos:exactMatch	eurovoc:1933 , stw:14195-3 , wd:Q191552 ;
	skos:inScheme	ccat: ;
	skos:notation	"103530" ;
	skos:prefLabel	"Iron Ore"@en .

ccat:103535
	a	skos:Concept ;
	skos:broader	ccat:1035 ;
	skos:definition	"Ferrous scrap is the most recycled material in the world. The U.S. Geological Survey estimates that 65 million metric tons (143 BILLION pounds!) of iron and steel scrap was processed around the world in 2016.  Ferrous scrap comes from many consumer products like automobiles or household appliances, or from industrial structures and equipment such as buildings, railroads, trains, bridges, ships, and farming equipment."@en ;
	skos:inScheme	ccat: ;
	skos:notation	"103535" ;
	skos:prefLabel	"Ferrous Scrap"@en .

ccat:103540
	a	skos:Concept ;
	skos:broader	ccat:1035 ;
	skos:closeMatch	wd:Q102078 ;
	skos:definition	"Bauxite is a sedimentary rock with a relatively high aluminium content. It is the world's main source of aluminium and gallium. Bauxite is used as flux in blast furnaces for smelting."@en ;
	skos:inScheme	ccat: ;
	skos:notation	"103540" ;
	skos:prefLabel	"Bauxite"@en .

ccat:103550
	a	skos:Concept ;
	skos:broader	ccat:1035 ;
	skos:closeMatch	wd:Q731 ;
	skos:definition	"Often found in minerals in combination with iron."@en ;
	skos:inScheme	ccat: ;
	skos:notation	"103550" ;
	skos:prefLabel	"Manganese"@en .

ccat:103560
	a	skos:Concept ;
	skos:broader	ccat:1035 ;
	skos:closeMatch	wd:Q1053 ;
	skos:definition	"Molybdenum does not occur naturally as a free metal on Earth; it is found only in various oxidation states in minerals. The free element, a silvery metal with a gray cast, has the sixth-highest melting point of any element. It readily forms hard, stable carbides in alloys, and for this reason most of world production of the element (about 80%) is used in steel alloys, including high-strength alloys and superalloys."@en ;
	skos:inScheme	ccat: ;
	skos:notation	"103560" ;
	skos:prefLabel	"Molybdenum"@en .

ccat:103570
	a	skos:Concept ;
	skos:broader	ccat:1035 ;
	skos:closeMatch	wd:Q725 ;
	skos:definition	"Chromium is the main additive in stainless steel, to which it adds anti-corrosive properties. Chromium is also highly valued as a metal that is able to be highly polished while resisting tarnishing. Polished chromium reflects almost 70% of the visible spectrum, with almost 90% of infrared light being reflected."@en ;
	skos:inScheme	ccat: ;
	skos:notation	"103570" ;
	skos:prefLabel	"Chromium"@en .

ccat:1040
	a	skos:Concept ;
	skos:broader	ccat:10 ;
	skos:definition	"Metals that are not abundant and mostly extracted as a by-product."@en ;
	skos:inScheme	ccat: ;
	skos:notation	"1040" ;
	skos:prefLabel	"Rare Metal"@en .

ccat:104010
	a	skos:Concept ;
	skos:broader	ccat:1040 ;
	skos:definition	"""Uranium is a chemical element with the symbol U and atomic number 92. It is a silvery-grey metal in the actinide series of the periodic table. A uranium atom has 92 protons and 92 electrons, of which 6 are valence electrons. Uranium is weakly radioactive because all isotopes of uranium are unstable; the half-lives of its naturally occurring isotopes range between 159,200 years and 4.5 billion years. The most common isotopes in natural uranium are uranium-238 (which has 146 neutrons and accounts for over 99% of uranium on Earth) and uranium-235 (which has 143 neutrons). Uranium has the highest atomic weight of the primordially occurring elements. Its density is about 70% higher than that of lead, and slightly lower than that of gold or tungsten. It occurs naturally in low concentrations of a few parts per million in soil, rock and water, and is commercially extracted from uranium-bearing minerals such as uraninite.

In nature, uranium is found as uranium-238 (99.2739-99.2752%), uranium-235 (0.7198-0.7202%), and a very small amount of uranium-234 (0.0050-0.0059%). Uranium decays slowly by emitting an alpha particle. The half-life of uranium-238 is about 4.47 billion years and that of uranium-235 is 704 million years, making them useful in dating the age of the Earth.

Many contemporary uses of uranium exploit its unique nuclear properties. Uranium-235 is the only naturally occurring fissile isotope, which makes it widely used in nuclear power plants and nuclear weapons. However, because of the tiny amounts found in nature, uranium needs to undergo enrichment so that enough uranium-235 is present. Uranium-238 is fissionable by fast neutrons, and is fertile, meaning it can be transmuted to fissile plutonium-239 in a nuclear reactor. Another fissile isotope, uranium-233, can be produced from natural thorium and is studied for future industrial use in nuclear technology. Uranium-238 has a small probability for spontaneous fission or even induced fission with fast neutrons; uranium-235 and to a lesser degree uranium-233 have a much higher fission cross-section for slow neutrons. In sufficient concentration, these isotopes maintain a sustained nuclear chain reaction. This generates the heat in nuclear power reactors, and produces the fissile material for nuclear weapons. Depleted uranium (238U) is used in kinetic energy penetrators and armor plating. Uranium is used as a colorant in uranium glass, producing lemon yellow to green colors. Uranium glass fluoresces green in ultraviolet light. It was also used for tinting and shading in early photography."""@en ;
	skos:exactMatch	agrovoc:c_8084 , eurovoc:4617 , stw:14222-5 , wd:Q1098 ;
	skos:inScheme	ccat: ;
	skos:notation	"104010" ;
	skos:prefLabel	"Uranium"@en .

ccat:104020
	a	skos:Concept ;
	skos:broader	ccat:1040 ;
	skos:definition	"""Cobalt is a chemical element with the symbol Co and atomic number 27. Like nickel, cobalt is found in the Earth's crust only in chemically combined form, save for small deposits found in alloys of natural meteoric iron. The free element, produced by reductive smelting, is a hard, lustrous, silver-gray metal.

Cobalt-based blue pigments (cobalt blue) have been used since ancient times for jewelry and paints, and to impart a distinctive blue tint to glass, but the color was later thought to be due to the known metal bismuth. Miners had long used the name kobold ore (German for goblin ore) for some of the blue-pigment-producing minerals; they were so named because they were poor in known metals, and gave poisonous arsenic-containing fumes when smelted. In 1735, such ores were found to be reducible to a new metal (the first discovered since ancient times), and this was ultimately named for the kobold.

Today, some cobalt is produced specifically from one of a number of metallic-lustered ores, such as cobaltite (CoAsS). The element is, however, more usually produced as a by-product of copper and nickel mining. The copper belt in the Democratic Republic of the Congo (DRC) and Zambia yields most of the global cobalt production. World production in 2016 was 116,000 metric tons (114,000 long tons; 128,000 short tons) (according to Natural Resources Canada), and the DRC alone accounted for more than 50%.

Cobalt is primarily used in lithium-ion batteries, and in the manufacture of magnetic, wear-resistant and high-strength alloys. The compounds cobalt silicate and cobalt(II) aluminate (CoAl2O4, cobalt blue) give a distinctive deep blue color to glass, ceramics, inks, paints and varnishes. Cobalt occurs naturally as only one stable isotope, cobalt-59. Cobalt-60 is a commercially important radioisotope, used as a radioactive tracer and for the production of high-energy gamma rays.

Cobalt is the active center of a group of coenzymes called cobalamins. Vitamin B12, the best-known example of the type, is an essential vitamin for all animals. Cobalt in inorganic form is also a micronutrient for bacteria, algae, and fungi."""@en ;
	skos:exactMatch	agrovoc:c_1702 , eurovoc:6018 , wd:Q740 ;
	skos:inScheme	ccat: ;
	skos:notation	"104020" ;
	skos:prefLabel	"Cobalt"@en .

ccat:104030
	a	skos:Concept ;
	skos:broader	ccat:1040 ;
	skos:closeMatch	wd:Q568 ;
	skos:definition	"""Lithium is a soft, silvery-white alkali metal. Under standard conditions, it is the lightest metal and the lightest solid element. Like all alkali metals, lithium is highly reactive and flammable, and must be stored in mineral oil. When cut, it exhibits a metallic luster, but moist air corrodes it quickly to a dull silvery gray, then black tarnish. It never occurs freely in nature, but only in (usually ionic) compounds, such as pegmatitic minerals, which were once the main source of lithium. Due to its solubility as an ion, it is present in ocean water and is commonly obtained from brines. Lithium metal is isolated electrolytically from a mixture of lithium chloride and potassium chloride.

Lithium and its compounds have several industrial applications, including heat-resistant glass and ceramics, lithium grease lubricants, flux additives for iron, steel and aluminium production, lithium batteries, and lithium-ion batteries. These uses consume more than three-quarters of lithium production.

Lithium is present in biological systems in trace amounts; its functions are uncertain. Lithium salts have proven to be useful as a mood-stabilizing drug in the treatment of bipolar disorder in humans."""@en ;
	skos:exactMatch	agrovoc:c_4386 ;
	skos:inScheme	ccat: ;
	skos:notation	"104030" ;
	skos:prefLabel	"Lithium"@en .

ccat:104040
	a	skos:Concept ;
	skos:broader	ccat:1040 ;
	skos:closeMatch	wd:Q942 ;
	skos:definition	"Bismuth is a pentavalent post-transition metal and one of the pnictogens with chemical properties resembling its lighter group 15 siblings arsenic and antimony. Elemental bismuth may occur naturally, although its sulfide and oxide form important commercial ores. The free element is 86% as dense as lead. It is a brittle metal with a silvery white color when freshly produced, but surface oxidation can give it an iridescent tinge in numerous colours. Bismuth is the most naturally diamagnetic element, and has one of the lowest values of thermal conductivity among metals."@en ;
	skos:exactMatch	agrovoc:c_938 , eurovoc:4990 ;
	skos:inScheme	ccat: ;
	skos:notation	"104040" ;
	skos:prefLabel	"Bismuth"@en .

ccat:20
	a	skos:Concept ;
	skos:definition	"Soft commodities, or softs, are commodities that, generally, are grown, rather than mined.  Furthermore, softs in this concept scheme are primarily for consumption, i.e. distinct from Materials."@en ;
	skos:inScheme	ccat: ;
	skos:notation	"20" ;
	skos:prefLabel	"Softs"@en ;
	skos:topConceptOf	ccat: .

ccat:2010
	a	skos:Concept ;
	skos:broader	ccat:20 ;
	skos:definition	"A cereal is any grass cultivated for the edible components of its grain. The term may also refer to the resulting grain itself. Cereal grain crops are grown in greater quantities and provide more food energy worldwide than any other type of crop and are therefore staple crops. Edible grains from other plant families, such as buckwheat, quinoa and chia, are referred to as pseudocereals."@en ;
	skos:exactMatch	agrovoc:c_1474 , eurovoc:536 , wd:Q12117 ;
	skos:inScheme	ccat: ;
	skos:notation	"2010" ;
	skos:prefLabel	"Cereals"@en .

ccat:201010
	a	skos:Concept ;
	skos:altLabel	"Corn"@en ;
	skos:broader	ccat:2010 ;
	skos:closeMatch	wd:Q25618328 ;
	skos:definition	"""Maize, also known as corn (American English), is a cereal grain first domesticated by indigenous peoples in southern Mexico about 10,000 years ago. The leafy stalk of the plant produces pollen inflorescences and separate ovuliferous inflorescences called ears that yield kernels or seeds, which are fruits.

Maize has become a staple food in many parts of the world, with the total production of maize surpassing that of wheat or rice. In addition to being consumed directly by humans (often in the form of masa), maize is also used for corn ethanol, animal feed and other maize products, such as corn starch and corn syrup."""@en ;
	skos:exactMatch	agrovoc:c_12332 , stw:14093-4 ;
	skos:inScheme	ccat: ;
	skos:notation	"201010" ;
	skos:prefLabel	"Maize"@en .

ccat:201020
	a	skos:Concept ;
	skos:broader	ccat:2010 ;
	skos:closeMatch	wd:Q5090 ;
	skos:definition	"Rice is the seed of the grass species Oryza glaberrima (African rice) or Oryza sativa (Asian rice). As a cereal grain, it is the most widely consumed staple food for a large part of the world's human population, especially in Asia and Africa. It is the agricultural commodity with the third-highest worldwide production (rice, 741.5 million tonnes in 2014), after sugarcane (1.9 billion tonnes) and maize (1.0 billion tonnes)."@en ;
	skos:exactMatch	agrovoc:c_6599 , stw:14095-0 ;
	skos:inScheme	ccat: ;
	skos:notation	"201020" ;
	skos:prefLabel	"Rice"@en .

ccat:201030
	a	skos:Concept ;
	skos:broader	ccat:2010 ;
	skos:closeMatch	wd:Q15645384 ;
	skos:definition	"Wheat is a grass widely cultivated for its seed, a cereal grain which is a worldwide staple food. The many species of wheat together make up the genus Triticum; the most widely grown is common wheat (T. aestivum). The archaeological record suggests that wheat was first cultivated in the regions of the Fertile Crescent around 9600 BCE. Botanically, the wheat kernel is a type of fruit called a caryopsis."@en ;
	skos:exactMatch	agrovoc:c_8373 , stw:14098-1 ;
	skos:inScheme	ccat: ;
	skos:notation	"201030" ;
	skos:prefLabel	"Wheat"@en .

ccat:201035
	a	skos:Concept ;
	skos:broader	ccat:2010 ;
	skos:definition	"""Durum wheat, also called pasta wheat or macaroni wheat (Triticum durum or Triticum turgidum subsp. durum), is a tetraploid species of wheat. It is the second most cultivated species of wheat after common wheat, although it represents only 5% to 8% of global wheat production. It was developed by artificial selection of the domesticated emmer wheat strains formerly grown in Central Europe and the Near East around 7000 BC, which developed a naked, free-threshing form. Like emmer, durum wheat is awned (with bristles). It is the predominant wheat that grows in the Middle East.

Durum in Latin means \"hard\", and the species is the hardest of all wheats. This refers to the resistance of the grain to milling, in particular of the starchy endosperm, implying dough made from its flour is weak or \"soft\". This makes durum favorable for semolina and pasta and less practical for flour, which requires more work than with hexaploid wheats like common bread wheats. Despite its high protein content, durum is not a strong wheat in the sense of giving strength to dough through the formation of a gluten network. Durum contains 27% extractable wet gluten, about 3% higher than in common wheat (T. aestivum L.)."""@en ;
	skos:exactMatch	agrovoc:c_11456 , wd:Q618324 ;
	skos:inScheme	ccat: ;
	skos:notation	"201035" ;
	skos:prefLabel	"Durum"@en .

ccat:201040
	a	skos:Concept ;
	skos:broader	ccat:2010 ;
	skos:definition	"""Barley (Hordeum vulgare), a member of the grass family, is a major cereal grain grown in temperate climates globally. It was one of the first cultivated grains, particularly in Eurasia as early as 10,000 years ago. Barley has been used as animal fodder, as a source of fermentable material for beer and certain distilled beverages, and as a component of various health foods. It is used in soups and stews, and in barley bread of various cultures. Barley grains are commonly made into malt in a traditional and ancient method of preparation.

In 2017, barley was ranked fourth among grains in quantity produced (149 million tonnes) behind maize, rice and wheat."""@en ;
	skos:exactMatch	agrovoc:c_823 , stw:14087-6 ;
	skos:inScheme	ccat: ;
	skos:notation	"201040" ;
	skos:prefLabel	"Barley"@en .

ccat:201050
	a	skos:Concept ;
	skos:broader	ccat:2010 ;
	skos:definition	"The oat (Avena sativa), sometimes called the common oat, is a species of cereal grain grown for its seed, which is known by the same name (usually in the plural, unlike other cereals and pseudocereals). While oats are suitable for human consumption as oatmeal and oat milk, one of the most common uses is as livestock feed. Oats are associated with lower blood cholesterol when consumed regularly."@en ;
	skos:exactMatch	agrovoc:c_5287 , stw:14090-3 ;
	skos:inScheme	ccat: ;
	skos:notation	"201050" ;
	skos:prefLabel	"Oats"@en .

ccat:201060
	a	skos:Concept ;
	skos:broader	ccat:2010 ;
	skos:definition	"""Sorghum bicolor, often called Sorghum, and also known as great millet, durra, jowari/jowar, or milo, is a grass species cultivated for its grain, which is used for food for humans, animal feed, and ethanol production. Sorghum originated in Africa, and is now cultivated widely in tropical and subtropical regions. Sorghum is the world's fifth-most important cereal crop after rice, wheat, maize, and barley, with 59.34 million metric tons of annual global production in 2018. S. bicolor is typically an annual, but some cultivars are perennial. It grows in clumps that may reach over 4 m high. The grain is small, ranging from 2 to 4 mm in diameter. Sweet sorghums are sorghum cultivars that are primarily grown for forage, syrup production, and ethanol; they are taller than those grown for grain.

The leading producers of S. bicolor in 2011 were Nigeria (12.6%), India (11.2%), Mexico (11.2%), and the United States (10.0%). Sorghum grows in a wide range of temperatures, high altitudes, and toxic soils, and can recover growth after some drought. It has five features that make it one of the most drought-resistant crops:

- It has a very large root-to-leaf surface area ratio.
- In times of drought, it rolls its leaves to lessen water loss by transpiration.
- If drought continues, it goes into dormancy rather than dying.
- Its leaves are protected by a waxy cuticle.
- It uses C4 carbon fixation thus using only a third the amount of water that C3 plants require."""@en ;
	skos:exactMatch	agrovoc:c_7247 , wd:Q332062 ;
	skos:inScheme	ccat: ;
	skos:notation	"201060" ;
	skos:prefLabel	"Sorghum"@en .

ccat:201070
	a	skos:Concept ;
	skos:broader	ccat:2010 ;
	skos:definition	"""Rye (Secale cereale) is a grass grown extensively as a grain, a cover crop and a forage crop. It is a member of the wheat tribe (Triticeae) and is closely related to both wheat (Triticum) and barley (genus Hordeum). Rye grain is used for flour, bread, beer, crispbread, some whiskeys, some vodkas, and animal fodder. It can also be eaten whole, either as boiled rye berries or by being rolled, similar to rolled oats.

Rye is a cereal grain and should not be confused with ryegrass, which is used for lawns, pasture, and hay for livestock."""@en ;
	skos:exactMatch	agrovoc:c_14010 , eurovoc:4059 , stw:14096-5 , wd:Q12099 ;
	skos:inScheme	ccat: ;
	skos:notation	"201070" ;
	skos:prefLabel	"Rye"@en .

ccat:201075
	a	skos:Concept ;
	skos:broader	ccat:2010 ;
	skos:definition	"""Hybrid of wheat (female) and rye (male) first bred in laboratories during the late 19th century in Scotland and Germany. Commercially available triticale is almost always a second-generation hybrid, i.e., a cross between two kinds of primary (first-cross) triticales. As a rule, triticale combines the yield potential and grain quality of wheat with the disease and environmental tolerance (including soil conditions) of rye. Only recently has it been developed into a commercially viable crop. Depending on the cultivar, triticale can more or less resemble either of its parents. It is grown mostly for forage or fodder, although some triticale-based foods can be purchased at health food stores and can be found in some breakfast cereals.

When crossing wheat and rye, wheat is used as the female parent and rye as the male parent (pollen donor). The resulting hybrid is sterile and must be treated with colchicine to induce polyploidy and thus the ability to reproduce itself.

The primary producers of triticale are Poland, Germany, Belarus, France and Russia. In 2014, according to the Food and Agriculture Organization (FAO), 17.1 million tons were harvested in 37 countries across the world.

The triticale hybrids are all amphidiploid, which means the plant is diploid for two genomes derived from different species. In other words, triticale is an allotetraploid. In earlier years, most work was done on octoploid triticale. Different ploidy levels have been created and evaluated over time. The tetraploids showed little promise, but hexaploid triticale was successful enough to find commercial application.

The International Maize and Wheat Improvement Center triticale improvement program was intended to improve food production and nutrition in developing countries. Triticale was thought to have potential in the production of bread and other food products, such as cookies, pasta, pizza dough and breakfast cereals. The protein content is higher than that of wheat, although the glutenin fraction is less. The grain has also been stated to have higher levels of lysine than wheat. Acceptance would require the milling industry to adapt to triticale, as the milling techniques employed for wheat are unsuited to triticale. Past research indicated that triticale could be used as a feed grain and, particularly, later research found that its starch is readily digested. As a feed grain, triticale is already well established and of high economic importance. It has received attention as a potential energy crop, and research is currently being conducted on the use of the crop's biomass in bioethanol production."""@en ;
	skos:exactMatch	agrovoc:c_33914 , wd:Q380329 ;
	skos:inScheme	ccat: ;
	skos:notation	"201075" ;
	skos:prefLabel	"Triticale"@en .

ccat:201080
	a	skos:Concept ;
	skos:broader	ccat:2010 ;
	skos:definition	"Fonio is the term for two cultivated grasses, black fonio and white fonio, in the genus Digitaria that are notable crops in parts of West Africa. They are millets with small grains."@en ;
	skos:exactMatch	agrovoc:c_3b4c07e9 , wd:Q1340738 ;
	skos:inScheme	ccat: ;
	skos:notation	"201080" ;
	skos:prefLabel	"White Fonio"@en .

ccat:201090
	a	skos:Concept ;
	skos:broader	ccat:2010 ;
	skos:closeMatch	agrovoc:c_6301 , wd:Q2643145 ;
	skos:definition	"Cereals of minor economic importance."@en ;
	skos:inScheme	ccat: ;
	skos:notation	"201090" ;
	skos:prefLabel	"Other Cereals and Pseudocereals"@en .

ccat:20109010
	a	skos:Concept ;
	skos:broader	ccat:201090 ;
	skos:definition	"""Cultivated for its grain-like seeds and as a cover crop, primarily in northern regions. The name \"buckwheat\" is used for several other species, such as Fagopyrum tataricum, a domesticated food plant raised in Asia. Despite the name, buckwheat is not closely related to wheat, as it is not a grass. Instead, buckwheat is related to sorrel, knotweed, and rhubarb. Buckwheat is referred to as a pseudocereal because its seeds' culinary use is the same as cereals', owing to their composition of complex carbohydrates."""@en ;
	skos:exactMatch	agrovoc:c_9471 , eurovoc:3898 , wd:Q132734 ;
	skos:inScheme	ccat: ;
	skos:notation	"20109010" ;
	skos:prefLabel	"Buckwheat"@en .

ccat:20109020
	a	skos:Concept ;
	skos:broader	ccat:201090 ;
	skos:definition	"""A flowering plant in the amaranth family. It is a herbaceous annual plant grown as a crop primarily for its edible seeds; the seeds are rich in protein, dietary fiber, B vitamins, and dietary minerals in amounts greater than in many grains. Quinoa is not a grass, but rather a pseudocereal botanically related to spinach and amaranth (Amaranthus spp.), and originated in the Andean region of northwestern South America. It was first used to feed livestock 5.2-7.0 thousand years ago, and for human consumption-4 thousand years ago in the Lake Titicaca basin of Peru and Bolivia.

Today, almost all production in the Andean region is done by small farms and associations. Its cultivation has spread to more than 70 countries, including Kenya, India, the United States, and several European countries. As a result of increased popularity and consumption in North America, Europe, and Australasia, quinoa crop prices tripled between 2006 and 2014."""@en ;
	skos:exactMatch	agrovoc:c_13716 , wd:Q139925 ;
	skos:inScheme	ccat: ;
	skos:notation	"20109020" ;
	skos:prefLabel	"Quinoa"@en .

ccat:2020
	a	skos:Concept ;
	skos:broader	ccat:20 ;
	skos:definition	"Oil-bearing crops are plants that are grown primarily for their oil. Edible vegetable oils may be used for cooking, or as food additives. Many vegetable oils, edible and otherwise, are burned as fuel, for instance as a substitute for petroleum-based fuels. Some may be also used for cosmetics, medical purposes, wood finishing, oil painting and other industrial purposes."@en ;
	skos:inScheme	ccat: ;
	skos:notation	"2020" ;
	skos:prefLabel	"Oil-Bearing Crops and Derived Products"@en .

ccat:202010
	a	skos:Concept ;
	skos:broader	ccat:2020 ;
	skos:definition	"""The soybean or soya bean (Glycine max) is a species of legume native to East Asia, widely grown for its edible bean, which has numerous uses.

Traditional unfermented food uses of soybeans include soy milk, from which tofu and tofu skin are made. Fermented soy foods include soy sauce, fermented bean paste, natto, and tempeh. Fat-free (defatted) soybean meal is a significant and cheap source of protein for animal feeds and many packaged meals. For example, soybean products, such as textured vegetable protein (TVP), are ingredients in many meat and dairy substitutes.

Soy beans contain significant amounts of phytic acid, dietary minerals and B vitamins. Soy vegetable oil, used in food and industrial applications, is another product of processing the soybean crop. Soybean is the most important protein source for feed farm animals (that in turn yields animal protein for human consumption)."""@en ;
	skos:exactMatch	agrovoc:c_14477 , stw:14081-4 ;
	skos:inScheme	ccat: ;
	skos:notation	"202010" ;
	skos:prefLabel	"Soybeans"@en .

ccat:202020
	a	skos:Concept ;
	skos:altLabel	"Canola"@en ;
	skos:broader	ccat:2020 ;
	skos:definition	"Rapeseed (Brassica napus subsp. napus) is a bright-yellow flowering member of the family Brassicaceae (mustard or cabbage family), cultivated mainly for its oil-rich seed, which naturally contains appreciable amounts of toxic erucic acid. Canola are a group of rapeseed cultivars which were bred to have very low levels of erucic acid and are especially prized for use for human and animal food. Rapeseed is the third-largest source of vegetable oil and second-largest source of protein meal in the world."@en ;
	skos:exactMatch	agrovoc:c_25499 , eurovoc:6042 , stw:14078-0 , wd:Q177932 ;
	skos:inScheme	ccat: ;
	skos:notation	"202020" ;
	skos:prefLabel	"Rapeseed"@en .

ccat:202030
	a	skos:Concept ;
	skos:broader	ccat:2020 ;
	skos:closeMatch	agrovoc:c_5330 ;
	skos:definition	"""Species of palm commonly just called oil palm, or African oil palm, or macaw-fat. It is the principal source of palm oil. It is native to west and southwest Africa, specifically the area between Angola and The Gambia; the species name guineensis refers to the name for the area, Guinea, and not the modern country which now bears that name. The species is also now naturalised in Madagascar, Sri Lanka, Malaysia, Indonesia, Central America, Cambodia, the West Indies, and several islands in the Indian and Pacific Oceans. The closely related American oil palm Elaeis oleifera and a more distantly related palm, Attalea maripa, are also used to produce palm oil.

Human use of oil palms may date as far back as 5,000 years in West Africa; in the late 1800s, archaeologists discovered palm oil in a tomb at Abydos dating back to 3000 BCE. It is thought that Arab traders brought the oil palm to Egypt.

Oil palms can produce much more oil per unit of land area than most other oil-producing plants (about nine time more than soy, and 4.5 times more than rapeseed)."""@en ;
	skos:exactMatch	agrovoc:c_2509 , wd:Q165403 ;
	skos:inScheme	ccat: ;
	skos:notation	"202030" ;
	skos:prefLabel	"Oil Palm"@en .

ccat:202035
	a	skos:Concept ;
	skos:broader	ccat:2020 ;
	skos:definition	"""The term \"coconut\" (or the archaic \"cocoanut\") can refer to the whole coconut palm, the seed, or the fruit, which botanically is a drupe, not a nut. The name comes from the old Portuguese word coco, meaning \"head\" or \"skull\", after the three indentations on the coconut shell that resemble facial features. They are ubiquitous in coastal tropical regions and are a cultural icon of the tropics.

The inner flesh of the mature seed, as well as the coconut milk extracted from it, form a regular part of the diets of many people in the tropics and subtropics. Coconuts are distinct from other fruits because their endosperm contains a large quantity of clear liquid, called coconut water or coconut juice. Mature, ripe coconuts can be used as edible seeds, or processed for oil and plant milk from the flesh, charcoal from the hard shell, and coir from the fibrous husk. Dried coconut flesh is called copra, and the oil and milk derived from it are commonly used in cooking---frying in particular---as well as in soaps and cosmetics. The hard shells, fibrous husks and long pinnate leaves can be used as material to make a variety of products for furnishing and decoration.

Coconuts have been used by humans for thousands of years and may have spread to their present range by Pacific island settlers. The evolutionary origin of the coconut is under dispute, with theories stating that it may have evolved in Asia, South America, or on Pacific islands. Trees grow up to 30 m (100 ft) tall and can yield up to 75 fruits per year, though fewer than 30 is more typical. Plants are intolerant of cold weather and prefer copious precipitation, as well as full sunlight. Many insect pests and diseases affect the species and are a nuisance for commercial production. About 75% of the world's supply of coconuts is produced by Indonesia, the Philippines, and India combined."""@en ;
	skos:exactMatch	agrovoc:c_25470 , stw:14066-0 , wd:Q3342808 ;
	skos:inScheme	ccat: ;
	skos:notation	"202035" ;
	skos:prefLabel	"Coconuts"@en .

ccat:202040
	a	skos:Concept ;
	skos:broader	ccat:2020 ;
	skos:definition	"Cottonseed is the seed of the cotton plant. This includes seeds with the attached lint."@en ;
	skos:exactMatch	agrovoc:c_25473 , wd:Q17104079 ;
	skos:inScheme	ccat: ;
	skos:notation	"202040" ;
	skos:prefLabel	"Cottonseed"@en .

ccat:202050
	a	skos:Concept ;
	skos:broader	ccat:2020 ;
	skos:definition	"The groundnut is a legume crop grown mainly for its edible seeds. It is widely grown in the tropics and subtropics, being important to both small and large commercial producers. It is classified as both a grain legume and, due to its high oil content, an oil crop."@en ;
	skos:exactMatch	agrovoc:c_11368 , stw:14056-3 , wd:Q37383 ;
	skos:inScheme	ccat: ;
	skos:notation	"202050" ;
	skos:prefLabel	"Groundnuts"@en .

ccat:202055
	a	skos:Concept ;
	skos:altLabel	"Azuki Beans"@en ;
	skos:broader	ccat:2020 ;
	skos:definition	"""The adzuki bean is an annual vine widely cultivated throughout East Asia for its small (approximately 5 millimetres (0.20 in) long) bean. The cultivars most familiar in East Asia have a uniform red color, but there are also white, black, gray, and variously mottled varieties."""@en ;
	skos:exactMatch	agrovoc:c_8632 , wd:Q380279 ;
	skos:inScheme	ccat: ;
	skos:notation	"202055" ;
	skos:prefLabel	"Adzuki Beans"@en .

ccat:202090
	a	skos:Concept ;
	skos:broader	ccat:2020 ;
	skos:definition	"The rosids are members of a large clade (monophyletic group) of flowering plants making up more than a quarter of all angiosperms with their about 70,000 species."@en ;
	skos:inScheme	ccat: ;
	skos:notation	"202090" ;
	skos:prefLabel	"Other Rosid Seeds"@en .

ccat:20209010
	a	skos:Concept ;
	skos:altLabel	"Egusi"@en ;
	skos:broader	ccat:202090 ;
	skos:closeMatch	agrovoc:c_12487 ;
	skos:definition	"""Egusi (also known by variations including agusi,ohue,agushi) is the name for the protein-rich seeds of certain cucurbitaceous plants (squash, melon, gourd), which after being dried and ground are used as a major ingredient in West African cuisine.

Authorities disagree whether the word is used more properly for the seeds of the colocynth, those of a particular large-seeded variety of the watermelon, or generically for those of any cucurbitaceous plant. The characteristics and uses of all these seeds are broadly similar. Major egusi-growing nations include Mali, Burkina Faso, Togo, Ghana, Cote d'Ivoire, Benin, Nigeria, and Cameroon.

Species from which egusi is derived include Cucumeropsis mannii and Citrullus lanatus."""@en ;
	skos:exactMatch	wd:Q10771593 ;
	skos:inScheme	ccat: ;
	skos:notation	"20209010" ;
	skos:prefLabel	"Melonseed"@en .

ccat:20209020
	a	skos:Concept ;
	skos:broader	ccat:202090 ;
	skos:definition	"""The castor bean is a species of perennial flowering plant in the spurge family, Euphorbiaceae. It is the sole species in the monotypic genus, Ricinus, and subtribe, Ricininae. It reproduces with a mixed pollination system which favors selfing by geitonogamy but at the same time can be an out-crosser by anemophily (wind pollination) or entomophily (insect pollination).

Its seed is the castor bean, which, despite its name, is not a bean (that is, the seed of many Fabaceae). Castor is indigenous to the southeastern Mediterranean Basin, Eastern Africa, and India, but is widespread throughout tropical regions (and widely grown elsewhere as an ornamental plant).

Castor seed is the source of castor oil, which has a wide variety of uses. The seeds contain between 40% and 60% oil that is rich in triglycerides, mainly ricinolein. The seed also contains ricin, a water-soluble toxin, which is also present in lower concentrations throughout the plant."""@en ;
	skos:exactMatch	agrovoc:c_18705 , eurovoc:3724 , wd:Q64597240 ;
	skos:inScheme	ccat: ;
	skos:notation	"20209020" ;
	skos:prefLabel	"Castor Beans"@en .

ccat:20209030
	a	skos:Concept ;
	skos:broader	ccat:202090 ;
	skos:closeMatch	wd:Q2699247 ;
	skos:definition	"""The tung nut is the fruit of Vernicia fordii, usually known as the tung tree, a species of Vernicia in the spurge family native to southern China, Burma, and northern Vietnam. It is a hard, woody pear-shaped berry 4 to 6 cm long and 3 to 5 cm in diameter, containing four or five large, oily seeds. The tung nut is green initially, becoming dull brown when it is ripe in autumn. Tung oil, or China wood oil, is extracted from the nut.

Global production of the fruit rose from just over 100,000 tonnes in 1970 to almost 200,000 tonnes by 1980. Fruit yields are typically in the range of 4.5 to 5 tonnes per hectare. A number of cultivars have been selected for increased yield and small tree size, including 'Folsom', 'Cahl', 'Isabel', 'La Crosser', and 'Lampton'."""@en ;
	skos:inScheme	ccat: ;
	skos:notation	"20209030" ;
	skos:prefLabel	"Tung Nuts"@en .

ccat:20209040
	a	skos:Concept ;
	skos:broader	ccat:202090 ;
	skos:definition	"""Mustard seeds are the small round seeds of various mustard plants. The seeds are usually about 1 to 2 millimetres in diameter and may be coloured from yellowish white to black. They are an important spice in many regional foods and may come from one of three different plants: black mustard (Brassica nigra), brown Indian mustard (B. juncea), or white/yellow mustard (B. hirta/Sinapis alba).

Mustard seeds are a rich source of oil and protein. The seed has oil as high as 46-48%, and whole seed meal has 43.6% protein. Grinding and mixing the seeds with water, vinegar or other liquids creates the yellow condiment known as prepared mustard."""@en ;
	skos:exactMatch	agrovoc:c_fd07a050 , wd:Q1937700 ;
	skos:inScheme	ccat: ;
	skos:notation	"20209040" ;
	skos:prefLabel	"Mustard Seed"@en .

ccat:20209050
	a	skos:Concept ;
	skos:broader	ccat:202090 ;
	skos:definition	"""Triadica sebifera is a tree native to eastern China and Taiwan. It is commonly called Chinese tallow, Chinese tallowtree, Florida aspen, chicken tree, gray popcorn tree, or candleberry tree.

The seeds (as well as from those of Triadica cochinchinensis) are the sources of stillingia oil, a drying oil used in paints and varnishes. The fatty coat of the seeds, used for candle and soap making, is known as stillingia tallow; hence its common name. It is relevant to biodiesel production because it is the third most productive vegetable oil producing crop in the world, after algae and oil palm. The leaves are used as herbal medicine to treat boils. The plant sap and leaves are reputed to be toxic, and decaying leaves from the plant are toxic to other species of plants."""@en ;
	skos:exactMatch	wd:Q113005689 ;
	skos:inScheme	ccat: ;
	skos:notation	"20209050" ;
	skos:prefLabel	"Tallowtree Seeds"@en .

ccat:20209060
	a	skos:Concept ;
	skos:broader	ccat:202090 ;
	skos:definition	"Linseed is the seed of the flax plant. Depending on the sort they are brown or yellow in colour, taste nutty and contain about 40% oil."@en ;
	skos:exactMatch	agrovoc:c_12192 , wd:Q911332 ;
	skos:inScheme	ccat: ;
	skos:notation	"20209060" ;
	skos:prefLabel	"Linseed"@en .

ccat:20209065
	a	skos:Concept ;
	skos:broader	ccat:202090 ;
	skos:definition	"Hempseed is the seed of Cannabis sativa. Hempseed can be cold-pressed into hempseed oil and is high in unsaturated fatty acids."@en ;
	skos:exactMatch	wd:Q113005802 ;
	skos:inScheme	ccat: ;
	skos:notation	"20209065" ;
	skos:prefLabel	"Hempseed"@en .

ccat:202095
	a	skos:Concept ;
	skos:broader	ccat:2020 ;
	skos:definition	"The asterids are members of the largest group of flowering plant with more than 80,000 species, about a third of the total flowering plant species."@en ;
	skos:inScheme	ccat: ;
	skos:notation	"202095" ;
	skos:prefLabel	"Other Asterid Seeds"@en .

ccat:20209510
	a	skos:Concept ;
	skos:broader	ccat:202095 ;
	skos:definition	"""The sunflower seed is the fruit of the sunflower (Helianthus annuus). There are three types of commonly used sunflower seeds: linoleic (most common), high oleic, and sunflower oil seeds. Each variety has its own unique levels of monounsaturated, saturated, and polyunsaturated fats. The information in this article refers mainly to the linoleic variety.

For commercial purposes, sunflower seeds are usually classified by the pattern on their husks. If the husk is solid black, the seeds are called black oil sunflower seeds. The crops may be referred to as oilseed sunflower crops. These seeds are usually pressed to extract their oil. Striped sunflower seeds are primarily eaten as a snack food; as a result, they may be called confectionery sunflower seeds.

The term \"sunflower seed\" is actually a misnomer when applied to the seed in its pericarp (hull). Botanically speaking, it is a cypsela. When dehulled, the edible remainder is called the sunflower kernel or heart."""@en ;
	skos:exactMatch	agrovoc:c_25507 , wd:Q1076906 ;
	skos:inScheme	ccat: ;
	skos:notation	"20209510" ;
	skos:prefLabel	"Sunflower Seed"@en .

ccat:20209520
	a	skos:Concept ;
	skos:broader	ccat:202095 ;
	skos:definition	"""The olive, known by the botanical name Olea europaea, meaning \"European olive\", is a species of small tree in the family Oleaceae, found traditionally in the Mediterranean Basin. The species is cultivated in all the countries of the Mediterranean, as well as South America, South Africa, China, Australia, New Zealand, Mexico, and the United States. Olea europaea is the type species for the genus Olea.

The olive's fruit, also called an \"olive\", is of major agricultural importance in the Mediterranean region as the source of olive oil; it is one of the core ingredients in Mediterranean cuisine. The tree and its fruit give their name to the plant family, which also includes species such as lilacs, jasmine, Forsythia, and the true ash trees (Fraxinus).

The olive tree, Olea europaea, is an evergreen tree or shrub native to Mediterranean Europe, Asia, and Africa. It is short and squat, and rarely exceeds 8-15 m in height. 'Pisciottana', a unique variety comprising 40,000 trees found only in the area around Pisciotta in the Campania region of southern Italy, often exceeds this, with correspondingly large trunk diameters. The silvery green leaves are oblong, measuring 4-10 cm long and 1-3 cm wide. The trunk is typically gnarled and twisted.

The small, white, feathery flowers, with ten-cleft calyx and corolla, two stamens, and bifid stigma, are borne generally on the previous year's wood, in racemes springing from the axils of the leaves.

The fruit is a small drupe 1-2.5 cm long when ripe, thinner-fleshed and smaller in wild plants than in orchard cultivars. Olives are harvested in the green to purple stage. Canned black olives have often been artificially blackened (see below on processing) and may contain the chemical ferrous gluconate to improve the appearance. Olea europaea contains a seed commonly referred to in American English as a \"pit\", and in British English as a \"stone\"."""@en ;
	skos:exactMatch	agrovoc:c_12926 , wd:Q1621080 ;
	skos:inScheme	ccat: ;
	skos:notation	"20209520" ;
	skos:prefLabel	"Olives"@en .

ccat:20209530
	a	skos:Concept ;
	skos:broader	ccat:202095 ;
	skos:definition	"""Safflower seed is the seed of Carthamus tinctorius, a highly branched, herbaceous, thistle-like annual plant in the family Asteraceae. It is commercially cultivated for vegetable oil extracted from the seeds.

In 2020, global production of safflower seeds was 653,030 tonnes, led by Kazakhstan with 35% of the world total. Other significant producers were Russia and Mexico, with 28% of world production combined."""@en ;
	skos:exactMatch	agrovoc:c_25503 , wd:Q104413623 ;
	skos:inScheme	ccat: ;
	skos:notation	"20209530" ;
	skos:prefLabel	"Safflower Seed"@en .

ccat:20209535
	a	skos:Concept ;
	skos:broader	ccat:202095 ;
	skos:definition	"""Sesame seed is the seed of Sesamum indicum. Sesame seeds are small. Their sizes vary with the thousands of varieties known. Typically, the seeds are about 3 to 4 mm long by 2 mm wide and 1 mm thick.

Sesame seed is considered to be the oldest oilseed crop known to humanity. The genus has many species, and most are wild. Most wild species of the genus Sesamum are native to sub-Saharan Africa. Sesamum indicum, the cultivated type, originated in India.

Sesame seeds are protected by a capsule that bursts when the seeds are ripe. The time of this bursting, or \"dehiscence\", tends to vary, so farmers cut plants by hand and place them together in an upright position to continue ripening until all the capsules have opened.

Since sesame is a small, flat seed, it is difficult to dry it after harvest because the small seed makes the movement of air around the seed difficult. Therefore, the seeds need to be harvested as dry as possible and stored at 6% moisture or less. If the seed is too moist, it can quickly heat up and become rancid. After harvesting, the seeds are usually cleaned and hulled. In some countries, once the seeds have been hulled, they are passed through an electronic color-sorting machine that rejects any discolored seeds to ensure perfect color, because sesame seeds with consistent appearance are perceived to be of better quality by consumers, and sell for a higher price. Immature or off-sized seeds are removed and used for sesame oil production.

In 2020, world production of sesame seeds was 7 million metric tons (6,900,000 long tons; 7,700,000 short tons), led by Sudan, Myanmar, and Tanzania. The white and other lighter-coloured sesame seeds are common in Europe, the Americas, West Asia, and the Indian subcontinent. The black and darker-coloured sesame seeds are mostly produced in China and Southeast Asia. In the United States most sesame is raised by farmers under contract to Sesaco, which also supplies proprietary seed.

Japan is the world's largest sesame importer. Sesame oil, particularly from roasted seed, is an important component of Japanese cooking and traditionally the principal use of the seed. China is the second-largest importer of sesame, mostly oil-grade. China exports lower-priced food-grade sesame seeds, particularly to Southeast Asia. Other major importers are United States, Canada, Netherlands, Turkey, and France."""@en ;
	skos:exactMatch	agrovoc:c_14216 , wd:Q12000036 ;
	skos:inScheme	ccat: ;
	skos:notation	"20209535" ;
	skos:prefLabel	"Sesame Seed"@en .

ccat:20209540
	a	skos:Concept ;
	skos:altLabel	"Shea Nuts"@en ;
	skos:broader	ccat:202095 ;
	skos:definition	"""Shea nut (karite nut) is seed from Butyrospermum parkii, a tree that can get up to 300 years old. After 20 years it blooms for the first time and carries fruits, after 50 years it will carry an anual yield of about 20 kg of fruits.

Farming and processing the fruit is arduous work that is traditionally done by hand by the African women. The falling shea fruits are collected from the savanna ground. They are then separated from the pulp, cleaned, and left out in the sun to dry. After a few days the nuts are cracked open, and the kernels are removed and dried bagain before the fat extraction can begin."""@en ;
	skos:exactMatch	agrovoc:c_25505 , wd:Q104212650 ;
	skos:inScheme	ccat: ;
	skos:notation	"20209540" ;
	skos:prefLabel	"Karite Nuts"@en .

ccat:20209545
	a	skos:Concept ;
	skos:broader	ccat:202095 ;
	skos:definition	"""Kapok fruit is the fruit of Ceiba pentandra, a tropical tree of the order Malvales and the family Malvaceae, native to Mexico, Central America and the Caribbean, northern South America, and (as the variety Ceiba pentandra var guineensis) West Africa. A somewhat smaller variety was introduced to South and Southeast Asia, where it is cultivated.

The fruit is famous for its cottonlike seed fibre, known as Java cotton. Its seeds are used to press a vegetable oil. The oil has a yellow colour and a pleasant, mild odour and taste, resembling cottonseed oil. It becomes rancid quickly when exposed to air. Kapok oil is produced in India, Indonesia and Malaysia. The oil has some potential as a biofuel and in paint preparation."""@en ;
	skos:inScheme	ccat: ;
	skos:notation	"20209545" ;
	skos:prefLabel	"Kapok Fruit"@en .

ccat:202099
	a	skos:Concept ;
	skos:broader	ccat:2020 ;
	skos:definition	"Any other oil seeds"@en ;
	skos:inScheme	ccat: ;
	skos:notation	"202099" ;
	skos:prefLabel	"Other Oilseeds"@en .

ccat:20209910
	a	skos:Concept ;
	skos:broader	ccat:202099 ;
	skos:definition	"""Poppy seed is an oilseed obtained from the opium poppy (Papaver somniferum). The tiny, kidney-shaped seeds have been harvested from dried seed pods by various civilizations for thousands of years. It is still widely used in many countries, especially in Central Europe and South Asia, where it is legally grown and sold in shops. The seeds are used whole or ground into meal as an ingredient in many foods---especially in pastry and bread---and they are pressed to yield poppyseed oil."""@en ;
	skos:exactMatch	agrovoc:c_25498 , wd:Q2007388 ;
	skos:inScheme	ccat: ;
	skos:notation	"20209910" ;
	skos:prefLabel	"Poppy Seed"@en .

ccat:20209920
	a	skos:Concept ;
	skos:altLabel	"Goat Nut"@en ;
	skos:broader	ccat:202099 ;
	skos:closeMatch	wd:Q267749 ;
	skos:definition	"Jojoba, or goat nut, deer nut, pignut, wild hazel, quinine nut, coffeeberry, is the seed of Simmondsia chinensis which is native to the Southwestern United States. Jojoba is grown commercially to produce jojoba oil, a liquid wax ester extracted from its seed. Jojoba is normally harvested by hand because seeds do not all mature in the same time. Yield is around 3.5 t/ha depending on the age of the plantation."@en ;
	skos:exactMatch	agrovoc:c_11913 ;
	skos:inScheme	ccat: ;
	skos:notation	"20209920" ;
	skos:prefLabel	"Jojoba"@en .

ccat:2025
	a	skos:Concept ;
	skos:broader	ccat:20 ;
	skos:definition	"Vegetal oils or vegetal fats are extracted from seeds, or less often, from other parts of fruits. Like animal fats, vegetable fats are mixtures of triglycerides. In common usage, vegetable oil may refer exclusively to vegetable fats which are liquid at room temperature. Vegetal oils are usually edible."@en ;
	skos:exactMatch	agrovoc:c_8170 , wd:Q4739805 ;
	skos:inScheme	ccat: ;
	skos:notation	"2025" ;
	skos:prefLabel	"Vegetal Oils"@en .

ccat:202510
	a	skos:Concept ;
	skos:broader	ccat:2025 ;
	skos:definition	"Soybean oil is a vegetable oil extracted from the seeds of the soybean (Glycine max). It is one of the most widely consumed cooking oils. As a drying oil, processed soybean oil is also used as a base for printing inks (soy ink) and oil paints."@en ;
	skos:exactMatch	agrovoc:c_16508 , wd:Q926892 ;
	skos:inScheme	ccat: ;
	skos:notation	"202510" ;
	skos:prefLabel	"Oil of Soybeans"@en .

ccat:202520
	a	skos:Concept ;
	skos:broader	ccat:2025 ;
	skos:definition	"Rapeseed oil is an edible vegetable oil derived from a variety of rapeseed, that is the seed of any of several cultivars of the plant family Brassicaceae. It is a comparatively nonodoriferous oil of a yellow colour, having a specific gravity varying between 0.9/12 and 0.920. The cake left after extraction of the oil is a valuable feed ingredient for pigs. Rapeseed oil is also used as a source of biodiesel."@en ;
	skos:exactMatch	agrovoc:c_24939 ;
	skos:inScheme	ccat: ;
	skos:narrowMatch	wd:Q697248 , wd:Q98841400 ;
	skos:notation	"202520" ;
	skos:prefLabel	"Oil of Rapeseed"@en .

ccat:202530
	a	skos:Concept ;
	skos:broader	ccat:2025 ;
	skos:definition	"Palm oil is an edible vegetable oil derived from the mesocarp (reddish pulp) of the fruit of the oil palms, primarily the African oil palm Elaeis guineensis, and to a lesser extent from the American oil palm Elaeis oleifera and the maripa palm Attalea maripa."@en ;
	skos:exactMatch	agrovoc:c_5514 , stw:18077-3 , wd:Q231458 ;
	skos:inScheme	ccat: ;
	skos:notation	"202530" ;
	skos:prefLabel	"Oil of Palm"@en .

ccat:202532
	a	skos:Concept ;
	skos:broader	ccat:2025 ;
	skos:definition	"""Palm kernel oil is an edible plant oil derived from the kernel of the oil palm Elaeis guineensis. It should not be confused with the other two edible oils derived from palm fruits: palm oil, extracted from the pulp of the oil palm fruit, and coconut oil, extracted from the kernel of the coconut.

Palm kernel oil, palm oil, and coconut oil are three of the few highly saturated vegetable fats; these oils give the name to the 16-carbon saturated fatty acid palmitic acid that they contain.

Palm kernel oil, which is semi-solid at room temperature, is more saturated than palm oil and comparable to coconut oil."""@en ;
	skos:exactMatch	agrovoc:c_5515 , wd:Q1960534 ;
	skos:inScheme	ccat: ;
	skos:notation	"202532" ;
	skos:prefLabel	"Oil of Palm Kernel"@en .

ccat:202535
	a	skos:Concept ;
	skos:altLabel	"Oil of Copra"@en ;
	skos:broader	ccat:2025 ;
	skos:closeMatch	<https://www.trade-tariff.service.gov.uk/commodities/1513110000> , <https://www.trade-tariff.service.gov.uk/commodities/1513190000> ;
	skos:definition	"""Coconut oil, or copra oil, is an edible oil extracted from the kernel or meat of mature coconuts harvested from the coconut palm (Cocos nucifera). It has various applications. Because of its high saturated fat content, it is slow to oxidize and, thus, resistant to rancidification, lasting up to six months at 24 Â°C (75 Â°F) without spoiling."""@en ;
	skos:exactMatch	agrovoc:c_1714 , wd:Q216235 ;
	skos:inScheme	ccat: ;
	skos:notation	"202535" ;
	skos:prefLabel	"Oil of Coconuts"@en .

ccat:202540
	a	skos:Concept ;
	skos:broader	ccat:2025 ;
	skos:definition	"""Cottonseed oil is cooking oil from the seeds of cotton plants of various species, mainly Gossypium hirsutum and Gossypium herbaceum, that are grown for cotton fiber, animal feed, and oil.

Cotton seed has a similar structure to other oilseeds such as sunflower seed, having an oil-bearing kernel surrounded by a hard outer hull; in processing, the oil is extracted from the kernel. Cottonseed oil is used for salad oil, mayonnaise, salad dressing, and similar products because of its flavour stability."""@en ;
	skos:exactMatch	agrovoc:c_25474 , wd:Q811663 ;
	skos:inScheme	ccat: ;
	skos:notation	"202540" ;
	skos:prefLabel	"Oil of Cottonseed"@en .

ccat:202550
	a	skos:Concept ;
	skos:broader	ccat:2025 ;
	skos:definition	"Groundnut oil is a vegetal oil derived from groundnuts. The oil usually has a mild or neutral flavour. The flavour and aroma is intensified when made from roasted groundnuts. It is often used in American, Chinese, Indian, African and Southeast Asian cuisine, both for general cooking, and in the case of roasted oil, for added flavour. Peanut oil has a high smoke point (around 225 C) relative to many other cooking oils, so it is commonly used for frying foods."@en ;
	skos:exactMatch	agrovoc:c_25477 , eurovoc:1263 , wd:Q265878 ;
	skos:inScheme	ccat: ;
	skos:notation	"202550" ;
	skos:prefLabel	"Oil of Groundnuts"@en .

ccat:202590
	a	skos:Concept ;
	skos:broader	ccat:2025 ;
	skos:definition	"Oil of oil seeds of the rosid clade"@en ;
	skos:inScheme	ccat: ;
	skos:notation	"202590" ;
	skos:prefLabel	"Other Rosid Oils"@en .

ccat:20259010
	a	skos:Concept ;
	skos:broader	ccat:202590 ;
	skos:closeMatch	wd:Q3819066 ;
	skos:definition	"""Melon seed oil is extracted by pressing from the seeds of the Citrullus lanatus (watermelon). It is particularly common in West Africa, where it is also called ootanga oil. The common watermelon most likely originated almost 5,000 years ago in the Kalahari Desert of Africa where botanists have found its wild ancestors, known as the Kalahari Melon, still growing. Watermelons migrated north through Egypt, and during the Roman era they were cultivated and prized. Traditionally, the seeds are extracted from the seed casing, and dried in the sun. Once dried, the seeds are pressed to extract the oil.

Watermelon seed oil contains high amounts of unsaturated fatty acids with linoleic and oleic acids as the major acids."""@en ;
	skos:exactMatch	agrovoc:c_66bba3ad ;
	skos:inScheme	ccat: ;
	skos:notation	"20259010" ;
	skos:prefLabel	"Melon Seed Oil"@en .

ccat:20259020
	a	skos:Concept ;
	skos:broader	ccat:202590 ;
	skos:definition	"Castor oil is a vegetable oil pressed from castor beans. It is a colourless or pale yellow liquid with a distinct taste and odour. Castor oil and its derivatives are used in the manufacturing of soaps, lubricants, hydraulic and brake fluids, paints, dyes, coatings, inks, cold-resistant plastics, waxes and polishes, nylon, and perfumes."@en ;
	skos:exactMatch	agrovoc:c_25466 , wd:Q337492 ;
	skos:inScheme	ccat: ;
	skos:notation	"20259020" ;
	skos:prefLabel	"Oil of Castor Beans"@en .

ccat:20259025
	a	skos:Concept ;
	skos:broader	ccat:202590 ;
	skos:definition	"Hydrogenated castor oil is made from the oil of castor beans by hydrogenation. The process saturates the alkenes, giving a waxy lubricant."@en ;
	skos:inScheme	ccat: ;
	skos:notation	"20259025" ;
	skos:prefLabel	"Hydrogenated Castor Oil"@en .

ccat:20259030
	a	skos:Concept ;
	skos:altLabel	"China wood oil"@en ;
	skos:broader	ccat:202590 ;
	skos:definition	"""Tung oil or China wood oil is a drying oil obtained by pressing the seed from the nut of the tung tree (Vernicia fordii). The oil and its use are believed to have originated in ancient China and appear in the writings of Confucius from about 400 BC.

Tung oil hardens upon exposure to air (through polymerization), and the resulting coating is transparent and has a deep, almost wet look. Used mostly for finishing and protecting wood, after numerous coats, the finish can even look plastic-like. Related drying oils include linseed, safflower, poppy, and soybean oils."""@en ;
	skos:exactMatch	agrovoc:c_8005 , wd:Q2094522 ;
	skos:inScheme	ccat: ;
	skos:notation	"20259030" ;
	skos:prefLabel	"Oil of Tung Nuts"@en .

ccat:20259040
	a	skos:Concept ;
	skos:broader	ccat:202590 ;
	skos:definition	"""Mustard oil is oil pressed from mustard seeds and is used as cooking oil in some cultures, but sale is restricted in some countries due to high levels of erucic acid. Varieties of mustard seed also exist that are low in erucic acid.

Oil makes up about 30% of the mustard seeds. It can be produced from black mustard (Brassica nigra), brown Indian mustard (B. juncea), and white mustard (B. hirta).

Having a distinctive pungent taste, the oil is used for cooking in India, Pakistan, Nepal and Bangladesh. Its pungent flavor is due to allyl isothiocyanate, a phytochemical of plants in the mustard family, Brassicaceae (for example, cabbage, horseradish or wasabi). Mustard oil has about 60% monounsaturated fatty acids (42% erucic acid and 12% oleic acid); it has about 21% polyunsaturated fats (6% the omega-3 alpha-linolenic acid and 15% the omega-6 linoleic acid), and it has about 12% saturated fats."""@en ;
	skos:exactMatch	agrovoc:c_36137 , wd:Q910958 ;
	skos:inScheme	ccat: ;
	skos:notation	"20259040" ;
	skos:prefLabel	"Oil of Mustard Seed"@en .

ccat:20259050
	a	skos:Concept ;
	skos:altLabel	"Chinese Vegetable Tallow"@en ;
	skos:broader	ccat:202590 ;
	skos:definition	"""Stillingia tallow or Chinese vegetable tallow is a fatty substance extracted from the coat of the seeds of Triadica sebifera (Chinese tallow tree) or Triadica cochinchinensis (Mountain tallow tree). It has traditionally been used for making candles.

Stillingia tallow is essentially a mixture of triglycerides (esters of glycerol and fatty acids). The main triglycerides are glicerotriyl tripalmitate (5-30%) and 2-oleate,1,3-dipalmitate (~70%).

The \"tallow\" is edible, and has applications in confectionery. However, the risk of contamination by the seed oil, which is toxic, is a possible concern."""@en ;
	skos:exactMatch	wd:Q102347788 ;
	skos:inScheme	ccat: ;
	skos:notation	"20259050" ;
	skos:prefLabel	"Stillingia Tallow"@en .

ccat:20259052
	a	skos:Concept ;
	skos:broader	ccat:202590 ;
	skos:definition	"""Stillingia oil is an oil extracted (by solvents) from the seeds of plants of the Triadica genus such as Triadica sebifera (Chinese tallow tree) and Triadica cochinchinensis (Mountain tallow tree). It is a drying oil used in paints and varnishes, and it is believed to be toxic in China. Stillingia oil is different from stillingia tallow, a fatty substance that surround the seeds in the fruit, which is removed before extracting the oil.

Stillingia oil has a typical drying time of 4-6 hours. The seeds produce 20-30% w/w of tallow fat and 10-17% w/w of stillingia oil. It has iodine number 127, a saponification value of 206, and a thiocyanogen value of 100.7."""@en ;
	skos:exactMatch	wd:Q3142827 ;
	skos:inScheme	ccat: ;
	skos:notation	"20259052" ;
	skos:prefLabel	"Stillingia Oil"@en .

ccat:20259060
	a	skos:Concept ;
	skos:broader	ccat:202590 ;
	skos:definition	"""Linseed oil, also known as flaxseed oil or flax oil (in its edible form), is a colourless to yellowish oil obtained from the dried, ripened seeds of the flax plant (Linum usitatissimum). The oil is obtained by pressing, sometimes followed by solvent extraction.

Linseed oil is an edible oil in demand as a dietary supplement, as a source of N1-Linolenic acid, an omega-3 fatty acid. In parts of Europe, it is traditionally eaten with potatoes and quark. It is regarded as a delicacy due to its hearty taste and ability to improve the bland flavour of quark."""@en ;
	skos:exactMatch	agrovoc:c_4353 , wd:Q818405 ;
	skos:inScheme	ccat: ;
	skos:notation	"20259060" ;
	skos:prefLabel	"Oil of Linseed"@en .

ccat:20259065
	a	skos:Concept ;
	skos:broader	ccat:202590 ;
	skos:definition	"""Hempseed oil is oil obtained by pressing hemp seeds. Cold pressed, unrefined hemp oil is dark to clear light green in color, with a nutty flavor. The darker the color, the grassier the flavour.

Refined hemp seed oil is clear and colourless, with little flavour. It is primarily used in body care products. Industrial hemp seed oil is used in lubricants, paints, inks, fuel, and plastics. Hemp seed oil is used in the production of soaps, shampoos and detergents. The oil has a 3:1 ratio of omega-6 to omega-3 essential fatty acids. It may also be used as a feedstock for the large-scale production of biodiesel.

About 49% of the weight of hempseed is an edible oil that contains 76% as polyunsaturated fat, including omega-6 fatty acids such as linoleic acid (LA, 54%) and gamma-linolenic acid (GLA, 3%), and omega-3 fatty acids such as alpha-linolenic acid (ALA, 17%) and stearidonic acid (2%). Both LA and ALA are essential fatty acids. In addition, hempseed oil contains 5% to 11% monounsaturated fat and 5% to 7% saturated fat. In common with other oils and fats, hemp seed oil provides 9 kcal/g.

Compared with other culinary oils, hempseed oil is low in saturated fat and rich in polyunsaturated fat. It has a relatively low smoke point and is not suitable for frying. It is primarily used as a food oil and dietary supplement.

Hemp oil is a \"drying oil\", as it can polymerize into a solid form. Due to its polymer-forming properties, hemp oil is used on its own or blended with other oils, resins, and solvents as an impregnator and varnish in wood finishing, as a pigment binder in oil paints, and as a plasticizer and hardener in putty."""@en ;
	skos:exactMatch	wd:Q1575477 ;
	skos:inScheme	ccat: ;
	skos:notation	"20259065" ;
	skos:prefLabel	"Oil of Hempseed"@en .

ccat:202595
	a	skos:Concept ;
	skos:broader	ccat:2025 ;
	skos:definition	"Oil of oil seeds of the asterid clade"@en ;
	skos:inScheme	ccat: ;
	skos:notation	"202595" ;
	skos:prefLabel	"Other Asterid Oils"@en .

ccat:20259510
	a	skos:Concept ;
	skos:broader	ccat:202595 ;
	skos:definition	"""Sunflower oil is the non-volatile oil pressed from the seeds of sunflower (Helianthus annuus). Sunflower oil is commonly used in food as a frying oil, and in cosmetic formulations as an emollient.

Sunflower oil is primarily composed of linoleic acid, a polyunsaturated fat, and oleic acid, a monounsaturated fat. Through selective breeding and manufacturing processes, oils of differing proportions of the fatty acids are produced. The expressed oil has a neutral taste profile. The oil contains a large amount of vitamin E.

As of 2017, genome analysis and development of hybrid sunflowers to increase oil production are under development to meet greater consumer demand for sunflower oil and its commercial varieties.

Ukraine and Russia together accounted for 53% of the world's production of sunflower oil in 2018."""@en ;
	skos:exactMatch	agrovoc:c_25506 , wd:Q94787 ;
	skos:inScheme	ccat: ;
	skos:notation	"20259510" ;
	skos:prefLabel	"Oil of Sunflower"@en .

ccat:20259520
	a	skos:Concept ;
	skos:broader	ccat:202595 ;
	skos:definition	"""Olive oil is a liquid fat obtained from olives (the fruit of Olea europaea; family Oleaceae), a traditional tree crop of the Mediterranean Basin, produced by pressing whole olives and extracting the oil. It is commonly used in cooking, for frying foods or as a salad dressing. It is also used in cosmetics, pharmaceuticals, and soaps, and as a fuel for traditional oil lamps, and has additional uses in some religions. The olive is one of three core food plants in Mediterranean cuisine; the other two are wheat and grapes. Olive trees have been grown around the Mediterranean since the 8th millennium BC.

The top five producers of olive oil by volume are Spain, Italy, Tunisia, Greece and Turkey. Per capita consumption is highest in Greece, followed by Italy and Spain.

The composition of olive oil varies with the cultivar, altitude, time of harvest and extraction process. It consists mainly of oleic acid (up to 83%), with smaller amounts of other fatty acids including linoleic acid (up to 21%) and palmitic acid (up to 20%). Extra virgin olive oil is required to have no more than 0.8% free acidity and is considered to have favorable flavor characteristics."""@en ;
	skos:exactMatch	agrovoc:c_25491 , eurovoc:1264 , stw:14960-4 , wd:Q93165 ;
	skos:inScheme	ccat: ;
	skos:notation	"20259520" ;
	skos:prefLabel	"Virgin Oil of Olives"@en .

ccat:20259525
	a	skos:Concept ;
	skos:broader	ccat:202595 ;
	skos:definition	"Oil made from the olive cake left after the virgin pressing."@en ;
	skos:inScheme	ccat: ;
	skos:notation	"20259525" ;
	skos:prefLabel	"Oil of Olive Cake"@en .

ccat:20259530
	a	skos:Concept ;
	skos:broader	ccat:202595 ;
	skos:definition	"Safflower oil is made from the achenes of safflower. Cold pressing the seeds yields a cooking oil which is lower in saturated fats than olive oil. Hot pressing the seeds yields an industrial oil which is used in cosmetic products."@en ;
	skos:exactMatch	agrovoc:c_25502 , wd:Q441113 ;
	skos:inScheme	ccat: ;
	skos:notation	"20259530" ;
	skos:prefLabel	"Oil of Safflower Seed"@en .

ccat:20259535
	a	skos:Concept ;
	skos:broader	ccat:202595 ;
	skos:definition	"""Sesame oil is an edible vegetable oil derived from sesame seeds. The oil is one of the earliest-known crop-based oils. Worldwide mass modern production is limited due to the inefficient manual harvesting process required to extract the oil. Oil made from raw seeds, which may or may not be cold-pressed, is used as a cooking oil. Oil made from toasted seeds is used for its distinctive nutty aroma and taste, although it may be unsuitable for frying, which makes it taste burnt and bitter.

Industrial uses include solvents in injected drugs, as a carrier oil in cosmetics, or as a coating for stored grains to prevent weevil attacks."""@en ;
	skos:exactMatch	agrovoc:c_25504 ;
	skos:inScheme	ccat: ;
	skos:notation	"20259535" ;
	skos:prefLabel	"Oil of Sesame Seed"@en .

ccat:20259540
	a	skos:Concept ;
	skos:altLabel	"Shea Butter"@en ;
	skos:broader	ccat:202595 ;
	skos:definition	"""The butter of karite nuts, also called shea butter, is an edible fat extracted from the nut of the African shea tree (Vitellaria paradoxa). It is ivory in colour when raw and commonly dyed yellow with borututu root or palm oil.

The primary export market for shea butter is in the chocolate and confectionery industry. However, shea is also used as a cooking fat, food accompaniment and skin-care product in West Africa."""@en ;
	skos:exactMatch	agrovoc:c_37951 ;
	skos:inScheme	ccat: ;
	skos:notation	"20259540" ;
	skos:prefLabel	"Butter of Karite Nuts"@en .

ccat:20259545
	a	skos:Concept ;
	skos:broader	ccat:202595 ;
	skos:inScheme	ccat: ;
	skos:notation	"20259545" ;
	skos:prefLabel	"Oil of Kapok"@en .

ccat:202599
	a	skos:Concept ;
	skos:broader	ccat:2025 ;
	skos:inScheme	ccat: ;
	skos:notation	"202599" ;
	skos:prefLabel	"Other Vegetal Oils"@en .

ccat:20259910
	a	skos:Concept ;
	skos:broader	ccat:202599 ;
	skos:definition	"""Poppyseed oil (also poppy seed oil and poppy oil) is an edible oil from poppy seeds (specifically seeds of Papaver somniferum, the opium poppy).

Poppy seeds yield 45-50% oil. Like poppy seeds, poppyseed oil is highly palatable, high in vitamin E, and has no narcotic properties. Poppy seeds are especially high in tocopherols other than vitamin E (alpha-tocopherol). Compared to other vegetable oils, poppyseed oil has a moderate amount of phytosterols: higher than soybean oil and peanut oil, lower than safflower oil, sesame oil, wheat germ oil, corn oil, and rice bran oil. It has little or no odor and a pleasant taste, and it is less likely than some other oils to become rancid."""@en ;
	skos:exactMatch	agrovoc:c_d5fc3c98 , wd:Q1757003 ;
	skos:inScheme	ccat: ;
	skos:notation	"20259910" ;
	skos:prefLabel	"Oil of Poppy Seed"@en .

ccat:20259920
	a	skos:Concept ;
	skos:broader	ccat:202599 ;
	skos:inScheme	ccat: ;
	skos:notation	"20259920" ;
	skos:prefLabel	"Jojoba Oil"@en .

ccat:20259980
	a	skos:Concept ;
	skos:broader	ccat:202599 ;
	skos:inScheme	ccat: ;
	skos:notation	"20259980" ;
	skos:prefLabel	"Oil of Rice Bran"@en .

ccat:20259981
	a	skos:Concept ;
	skos:altLabel	"Corn Oil"@en ;
	skos:broader	ccat:202599 ;
	skos:inScheme	ccat: ;
	skos:notation	"20259981" ;
	skos:prefLabel	"Oil of Maize"@en .

ccat:2026
	a	skos:Concept ;
	skos:broader	ccat:20 ;
	skos:definition	"Vegetal cakes are made of the residue left after oil extraction. Meal is produced when the cakes are treated hydrothermally."@en ;
	skos:inScheme	ccat: ;
	skos:notation	"2026" ;
	skos:prefLabel	"Vegetal Cakes and Meals"@en .

ccat:202610
	a	skos:Concept ;
	skos:broader	ccat:2026 ;
	skos:definition	"Soybean meal is used in food and animal feeds, principally as a protein supplement, but also as a source of metabolizable energy. Typically 1 bushel (i.e. 60 lbs. or 27.2 kg) of soybeans yields 48 lbs. (21.8 kg) of soybean meal. Some, but not all, soybean meal is produced from the residue left after oil extraction. Removal of the oil, which is used mostly in food, but also for industrial oils, soaps and biodiesel, involves crushing and either pressing or solvent extraction. Some, but not all, soybean meal contains ground soybean hulls. Soybean meal is heat-treated during production, to denature the trypsin inhibitors of soybeans, which would otherwise interfere with protein digestion."@en ;
	skos:exactMatch	agrovoc:c_16043 , wd:Q364900 ;
	skos:inScheme	ccat: ;
	skos:notation	"202610" ;
	skos:prefLabel	"Cake and Meal of Soybeans"@en .

ccat:202620
	a	skos:Concept ;
	skos:broader	ccat:2026 ;
	skos:definition	"Residue of rapeseed oil extraction."@en ;
	skos:exactMatch	agrovoc:c_16027 , wd:Q113010548 ;
	skos:inScheme	ccat: ;
	skos:notation	"202620" ;
	skos:prefLabel	"Cake and Meal of Rapeseed"@en .

ccat:202630
	a	skos:Concept ;
	skos:broader	ccat:2026 ;
	skos:definition	"Residue of palm oil extraction."@en ;
	skos:inScheme	ccat: ;
	skos:notation	"202630" ;
	skos:prefLabel	"Palm Cake and Palm Meal"@en .

ccat:202632
	a	skos:Concept ;
	skos:broader	ccat:2026 ;
	skos:definition	"Palm kernel cake (PKC) is the main by-product of the palm kernel oil extraction process. It further processed into palm kernel meal (PKM) by heating up the cake and evaporating residual water. It is a highly fibrous and medium grade protein feed, hence most suited to ruminant or rabbit feeding (Pickard, 2005). Palm kernel resulting from mechanical extraction contains 5-12% oil and solvent-extracted palm kernel meal contains 0.5-3% oil (Chin, 2001)."@en ;
	skos:exactMatch	agrovoc:c_36344 , wd:Q110583134 ;
	skos:inScheme	ccat: ;
	skos:notation	"202632" ;
	skos:prefLabel	"Cake and Meal of Palm Kernel"@en .

ccat:202640
	a	skos:Concept ;
	skos:broader	ccat:2026 ;
	skos:definition	"Residue of cottonseed after oil extraction."@en ;
	skos:exactMatch	agrovoc:c_35678 , wd:Q5175773 ;
	skos:inScheme	ccat: ;
	skos:notation	"202640" ;
	skos:prefLabel	"Cake and Meal of Cottonseed"@en .

ccat:2030
	a	skos:Concept ;
	skos:broader	ccat:20 ;
	skos:definition	"""In addition to providing the source for the manufacture of sugar, SUGAR CROPS are used to produce alcohol and ethanol. In certain countries, sugar cane is eaten raw in minor quantities. It also is used in the preparation of juices and for animal feed.

There are two major sugar crops: sugar beets and sugar cane. However, sugar and syrups are also produced from the sap of certain species of maple trees, from sweet sorghum when cultivated explicitly for making syrup and from sugar palm. Sugar beets that are cultivated solely as a fodder crop and red or garden beets that are classified as vegetable crops are excluded from the FAO list of sugar crops.

Sugar cane is a perennial grass (replanted at intervals using pieces of the cane stalks) that is cultivated mainly in the tropics. Sugar beet is an annual crop that is propagated by the seeds of the flowers. It is cultivated in cooler climates than sugar cane, mainly above the 35th parallel of the Northern Hemisphere.

Both sugar beets and sugar cane have a high water content, accounting for about 75 percent of the total weight of the plants. The sugar content of sugar cane ranges from 10 to 15 percent of the total weight, while that of sugar beets is between 13 and 18 percent. The protein and fat content of both beets and cane is almost nil.

Production data on sugar beets and sugar cane relate to the harvested crop, free of soil, plant tops and leaves.

FAO lists three primary sugar crops.

Under the name SWEETENERS, FAO includes products used for sweetening that are derived from sugar crops, cereals, fruits or milk, or that are produced by insects. This category includes a wide variety of monosaccharides (glucose and fructose) and disaccharides (sucrose and saccharose). They exist either in a crystallized state as sugar, or in thick liquid form as syrups.

The traditional sources of sugar are sugar cane and sugar beets. But in recent years, ever larger quantities of cereals (mainly maize) have been used to produce sweeteners derived from starch.

OTHER DERIVED PRODUCTS. In addition to sugar, molasses is also obtained with various degrees of sugar content. The by-product obtained from the extraction of sugar is called bagasse in the case of sugar cane, and beet pulp in the case of sugar beets."""@en ;
	skos:inScheme	ccat: ;
	skos:notation	"2030" ;
	skos:prefLabel	"Sugar Crops and Sweeteners"@en .

ccat:203010
	a	skos:Concept ;
	skos:broader	ccat:2030 ;
	skos:exactMatch	agrovoc:c_7501 , wd:Q36940 ;
	skos:inScheme	ccat: ;
	skos:notation	"203010" ;
	skos:prefLabel	"Sugar Cane"@en .

ccat:20301010
	a	skos:Concept ;
	skos:broader	ccat:203010 ;
	skos:definition	"A non-refined, crystallized material derived from the juices of sugar-cane stalk and consisting either wholly or essentially of sucrose."@en ;
	skos:exactMatch	agrovoc:c_16477 , wd:Q487233 ;
	skos:inScheme	ccat: ;
	skos:notation	"20301010" ;
	skos:prefLabel	"Cane Sugar"@en .

ccat:203020
	a	skos:Concept ;
	skos:broader	ccat:2030 ;
	skos:exactMatch	agrovoc:c_7499 , wd:Q151964 ;
	skos:inScheme	ccat: ;
	skos:notation	"203020" ;
	skos:prefLabel	"Sugar Beet"@en .

ccat:20302010
	a	skos:Concept ;
	skos:broader	ccat:203020 ;
	skos:definition	"A non-refined, crystallized material derived from the juices extracted from the root of the sugar beet and consisting either wholly or essentially of sucrose."@en ;
	skos:exactMatch	agrovoc:c_16474 , wd:Q9197055 ;
	skos:inScheme	ccat: ;
	skos:notation	"20302010" ;
	skos:prefLabel	"Beet Sugar"@en .

ccat:203030
	a	skos:Concept ;
	skos:broader	ccat:2030 ;
	skos:definition	"Includes minor sugar crops of local importance. In the case of saps, production is to be expressed in liquid equivalent."@en ;
	skos:inScheme	ccat: ;
	skos:notation	"203030" ;
	skos:prefLabel	"Other Sugar Crops"@en .

ccat:203040
	a	skos:Concept ;
	skos:broader	ccat:20301010 , ccat:20302010 ;
	skos:definition	"Generally derived from sugar cane through traditional methods without centrifugation."@en ;
	skos:inScheme	ccat: ;
	skos:notation	"203040" ;
	skos:prefLabel	"Non-Centrifugal Sugar"@en .

ccat:203050
	a	skos:Concept ;
	skos:broader	ccat:20301010 , ccat:20302010 ;
	skos:definition	"Cane Sugar or Beet Sugar processed by centrifuges.  Processed further it is called Refined Sugar."@en ;
	skos:inScheme	ccat: ;
	skos:notation	"203050" ;
	skos:prefLabel	"Raw Centrifugal Sugar"@en .

ccat:20305010
	a	skos:Concept ;
	skos:broader	ccat:203050 ;
	skos:definition	"Production covers domestic production, plus or minus imports and/or exports of raw centrifugal sugar in terms of refined sugar."@en ;
	skos:inScheme	ccat: ;
	skos:notation	"20305010" ;
	skos:prefLabel	"Refined Sugar"@en .

ccat:20305020
	a	skos:Concept ;
	skos:broader	ccat:203050 ;
	skos:definition	"A by-product of the extraction or refining of beet or cane sugar or of the production of fructose from maize. Used for feed, food, industrial alcohol, alcoholic beverages and ethanol."@en ;
	skos:inScheme	ccat: ;
	skos:notation	"20305020" ;
	skos:prefLabel	"Molasses"@en .

ccat:2040
	a	skos:Concept ;
	skos:broader	ccat:20 ;
	skos:closeMatch	agrovoc:c_6651 , agrovoc:c_7998 ;
	skos:inScheme	ccat: ;
	skos:notation	"2040" ;
	skos:prefLabel	"Roots and Tubers"@en .

ccat:204010
	a	skos:Concept ;
	skos:broader	ccat:2040 ;
	skos:definition	"""The potato is a root vegetable native to the Americas, a starchy tuber of the plant Solanum tuberosum, and the plant itself is a perennial in the nightshade family, Solanaceae.

Potatoes were introduced to Europe from the Americas in the second half of the 16th century by the Spanish. Today they are a staple food in many parts of the world and an integral part of much of the world's food supply. As of 2014, potatoes were the world's fourth-largest food crop after maize (corn), wheat, and rice.

The importance of the potato as a food source and culinary ingredient varies by region and is still changing. It remains an essential crop in Europe, especially Northern and Eastern Europe, where per capita production is still the highest in the world, while the most rapid expansion in production over the past few decades has occurred in southern and eastern Asia, with China and India leading the world in overall production as of 2018."""@en ;
	skos:exactMatch	agrovoc:c_13551 , stw:14092-6 ;
	skos:inScheme	ccat: ;
	skos:notation	"204010" ;
	skos:prefLabel	"Potatoes"@en .

ccat:204015
	a	skos:Concept ;
	skos:broader	ccat:2040 ;
	skos:definition	"The sweet potato or sweetpotato (Ipomoea batatas) is a dicotyledonous plant that belongs to the bindweed or morning glory family, Convolvulaceae. Its large, starchy, sweet-tasting, tuberous roots are a root vegetable."@en ;
	skos:exactMatch	agrovoc:c_14729 ;
	skos:inScheme	ccat: ;
	skos:notation	"204015" ;
	skos:prefLabel	"Sweet Potatoes"@en .

ccat:204020
	a	skos:Concept ;
	skos:broader	ccat:2040 ;
	skos:inScheme	ccat: ;
	skos:notation	"204020" ;
	skos:prefLabel	"Yams"@en .

ccat:204030
	a	skos:Concept ;
	skos:broader	ccat:2040 ;
	skos:inScheme	ccat: ;
	skos:notation	"204030" ;
	skos:prefLabel	"Cassava"@en .

ccat:204040
	a	skos:Concept ;
	skos:broader	ccat:2040 ;
	skos:inScheme	ccat: ;
	skos:notation	"204040" ;
	skos:prefLabel	"Yautia"@en .

ccat:204050
	a	skos:Concept ;
	skos:broader	ccat:2040 ;
	skos:inScheme	ccat: ;
	skos:notation	"204050" ;
	skos:prefLabel	"Taro"@en .

ccat:204060
	a	skos:Concept ;
	skos:broader	ccat:2040 ;
	skos:inScheme	ccat: ;
	skos:notation	"204060" ;
	skos:prefLabel	"Chicory Roots"@en .

ccat:204090
	a	skos:Concept ;
	skos:broader	ccat:2040 ;
	skos:inScheme	ccat: ;
	skos:notation	"204090" ;
	skos:prefLabel	"Other Roots"@en .

ccat:2050
	a	skos:Concept ;
	skos:broader	ccat:20 ;
	skos:definition	"The ripened reproductive body of a seed plant "@en ;
	skos:exactMatch	agrovoc:c_3131 , stw:14110-2 ;
	skos:inScheme	ccat: ;
	skos:notation	"2050" ;
	skos:prefLabel	"Fruits"@en .

ccat:205010
	a	skos:Concept ;
	skos:broader	ccat:2050 ;
	skos:definition	"""The orange is the fruit of various citrus species in the family Rutaceae (see list of plants known as orange); it primarily refers to Citrus x sinensis, which is also called sweet orange, to distinguish it from the related Citrus x aurantium, referred to as bitter orange. The sweet orange reproduces asexually (apomixis through nucellar embryony); varieties of sweet orange arise through mutations.

The orange is a hybrid between pomelo (Citrus maxima) and mandarin (Citrus reticulata). The chloroplast genome, and therefore the maternal line, is that of pomelo. The sweet orange has had its full genome sequenced.

The orange originated in a region encompassing Southern China, Northeast India, and Myanmar, and the earliest mention of the sweet orange was in Chinese literature in 314 BC. As of 1987, orange trees were found to be the most cultivated fruit tree in the world. Orange trees are widely grown in tropical and subtropical climates for their sweet fruit. The fruit of the orange tree can be eaten fresh, or processed for its juice or fragrant peel. As of 2012, sweet oranges accounted for approximately 70% of citrus production.

In 2017, 73 million tonnes of oranges were grown worldwide, with Brazil producing 24% of the world total, followed by China and India."""@en ;
	skos:exactMatch	agrovoc:c_1641 , stw:14119-5 , wd:Q2574750 ;
	skos:inScheme	ccat: ;
	skos:notation	"205010" ;
	skos:prefLabel	"Oranges and Citrus Fruits"@en .

ccat:20501010
	a	skos:Concept ;
	skos:broader	ccat:205010 ;
	skos:definition	"""Citrus x sinensis, which is also called sweet orange, to distinguish it from the related Citrus x aurantium, referred to as bitter orange. The sweet orange reproduces asexually (apomixis through nucellar embryony); varieties of sweet orange arise through mutations."""@en ;
	skos:exactMatch	agrovoc:c_7550 , wd:Q13191 ;
	skos:inScheme	ccat: ;
	skos:notation	"20501010" ;
	skos:prefLabel	"Sweet Oranges"@en .

ccat:20501020
	a	skos:Concept ;
	skos:broader	ccat:205010 ;
	skos:inScheme	ccat: ;
	skos:notation	"20501020" ;
	skos:prefLabel	"Tangerines and Mandarines and Clementines and Satsumas"@en .

ccat:20501030
	a	skos:Concept ;
	skos:broader	ccat:205010 ;
	skos:exactMatch	agrovoc:c_4259 ;
	skos:inScheme	ccat: ;
	skos:notation	"20501030" ;
	skos:prefLabel	"Lemons"@en .

ccat:20501035
	a	skos:Concept ;
	skos:broader	ccat:205010 ;
	skos:exactMatch	agrovoc:c_4341 ;
	skos:inScheme	ccat: ;
	skos:notation	"20501035" ;
	skos:prefLabel	"Limes"@en .

ccat:20501040
	a	skos:Concept ;
	skos:broader	ccat:205010 ;
	skos:exactMatch	agrovoc:c_3358 ;
	skos:inScheme	ccat: ;
	skos:notation	"20501040" ;
	skos:prefLabel	"Grapefruit"@en .

ccat:20501045
	a	skos:Concept ;
	skos:broader	ccat:205010 ;
	skos:exactMatch	agrovoc:c_6367 ;
	skos:inScheme	ccat: ;
	skos:notation	"20501045" ;
	skos:prefLabel	"Pomelo"@en .

ccat:20501090
	a	skos:Concept ;
	skos:broader	ccat:205010 ;
	skos:inScheme	ccat: ;
	skos:notation	"20501090" ;
	skos:prefLabel	"Other Citrus Fruit"@en .

ccat:205020
	a	skos:Concept ;
	skos:broader	ccat:2050 ;
	skos:definition	"""Type of fruit produced by flowering plants in the subtribe Malinae of the family Rosaceae."""@en ;
	skos:exactMatch	agrovoc:c_25497 , wd:Q41274 ;
	skos:inScheme	ccat: ;
	skos:notation	"205020" ;
	skos:prefLabel	"Pome Fruits"@en .

ccat:20502010
	a	skos:Concept ;
	skos:broader	ccat:205020 ;
	skos:definition	"""An apple is an edible fruit produced by an apple tree (Malus domestica). Apple trees are cultivated worldwide and are the most widely grown species in the genus Malus. The tree originated in Central Asia, where its wild ancestor, Malus sieversii, is still found today. Apples have been grown for thousands of years in Asia and Europe and were brought to North America by European colonists. Apples have religious and mythological significance in many cultures, including Norse, Greek, and European Christian tradition.
	
	Apple trees are large if grown from seed. Generally, apple cultivars are propagated by grafting onto rootstocks, which control the size of the resulting tree. There are more than 7,500 known cultivars of apples, resulting in a range of desired characteristics. Different cultivars are bred for various tastes and use, including cooking, eating raw and cider production. Trees and fruit are prone to a number of fungal, bacterial and pest problems, which can be controlled by a number of organic and non-organic means. In 2010, the fruit's genome was sequenced as part of research on disease control and selective breeding in apple production.
	
	Worldwide production of apples in 2018 was 86 million tonnes, with China accounting for nearly half of the total."""@en ;
	skos:exactMatch	agrovoc:c_541 , stw:19014-1 , wd:Q89 ;
	skos:inScheme	ccat: ;
	skos:notation	"20502010" ;
	skos:prefLabel	"Apples"@en .

ccat:20502020
	a	skos:Concept ;
	skos:broader	ccat:205020 ;
	skos:inScheme	ccat: ;
	skos:notation	"20502020" ;
	skos:prefLabel	"Pears"@en .

ccat:20502030
	a	skos:Concept ;
	skos:broader	ccat:205020 ;
	skos:inScheme	ccat: ;
	skos:notation	"20502030" ;
	skos:prefLabel	"Quinces"@en .

ccat:20502090
	a	skos:Concept ;
	skos:broader	ccat:205020 ;
	skos:inScheme	ccat: ;
	skos:notation	"20502090" ;
	skos:prefLabel	"Other Pome Fruits"@en .

ccat:205030
	a	skos:Concept ;
	skos:altLabel	"Drupe"@en ;
	skos:broader	ccat:2050 ;
	skos:definition	"Fruits of the botanical family Rosaceae that contain a single hard seed, called a stone, pit, or pip. The term includes plums, cherries, greengages, peaches, apricots, almonds, and sloes."@en ;
	skos:exactMatch	agrovoc:c_25461 , eurovoc:1117 , wd:Q14712 ;
	skos:inScheme	ccat: ;
	skos:notation	"205030" ;
	skos:prefLabel	"Stone Fruit"@en .

ccat:20503010
	a	skos:Concept ;
	skos:broader	ccat:205030 ;
	skos:inScheme	ccat: ;
	skos:notation	"20503010" ;
	skos:prefLabel	"Cherries"@en .

ccat:20503015
	a	skos:Concept ;
	skos:broader	ccat:205030 ;
	skos:inScheme	ccat: ;
	skos:notation	"20503015" ;
	skos:prefLabel	"Sour Cherries"@en .

ccat:20503020
	a	skos:Concept ;
	skos:broader	ccat:205030 ;
	skos:inScheme	ccat: ;
	skos:notation	"20503020" ;
	skos:prefLabel	"Apricots"@en .

ccat:20503030
	a	skos:Concept ;
	skos:broader	ccat:205030 ;
	skos:inScheme	ccat: ;
	skos:notation	"20503030" ;
	skos:prefLabel	"Peaches and Nectarines"@en .

ccat:20503040
	a	skos:Concept ;
	skos:broader	ccat:205030 ;
	skos:inScheme	ccat: ;
	skos:notation	"20503040" ;
	skos:prefLabel	"Plums"@en .

ccat:20503090
	a	skos:Concept ;
	skos:broader	ccat:205030 ;
	skos:inScheme	ccat: ;
	skos:notation	"20503090" ;
	skos:prefLabel	"Other Drupes"@en .

ccat:205040
	a	skos:Concept ;
	skos:broader	ccat:2050 ;
	skos:definition	"Botanical fruit with fleshy pericarp, containing one or many seeds."@en ;
	skos:exactMatch	wd:Q13184 ;
	skos:inScheme	ccat: ;
	skos:notation	"205040" ;
	skos:prefLabel	"Berries"@en .

ccat:20504010
	a	skos:Concept ;
	skos:broader	ccat:205040 ;
	skos:inScheme	ccat: ;
	skos:notation	"20504010" ;
	skos:prefLabel	"Strawberries"@en .

ccat:20504020
	a	skos:Concept ;
	skos:broader	ccat:205040 ;
	skos:inScheme	ccat: ;
	skos:notation	"20504020" ;
	skos:prefLabel	"Raspberries"@en .

ccat:20504030
	a	skos:Concept ;
	skos:broader	ccat:205040 ;
	skos:inScheme	ccat: ;
	skos:notation	"20504030" ;
	skos:prefLabel	"Gooseberries"@en .

ccat:20504040
	a	skos:Concept ;
	skos:broader	ccat:205040 ;
	skos:inScheme	ccat: ;
	skos:notation	"20504040" ;
	skos:prefLabel	"Currants"@en .

ccat:20504050
	a	skos:Concept ;
	skos:broader	ccat:205040 ;
	skos:inScheme	ccat: ;
	skos:notation	"20504050" ;
	skos:prefLabel	"Blueberries"@en .

ccat:20504060
	a	skos:Concept ;
	skos:broader	ccat:205040 ;
	skos:inScheme	ccat: ;
	skos:notation	"20504060" ;
	skos:prefLabel	"Cranberries"@en .

ccat:20504090
	a	skos:Concept ;
	skos:broader	ccat:205040 ;
	skos:inScheme	ccat: ;
	skos:notation	"20504090" ;
	skos:prefLabel	"Other Berries"@en .

ccat:205050
	a	skos:Concept ;
	skos:broader	ccat:2050 ;
	skos:exactMatch	agrovoc:c_7974 , stw:14117-2 , wd:Q844144 ;
	skos:inScheme	ccat: ;
	skos:notation	"205050" ;
	skos:prefLabel	"Tropical Fruits"@en .

ccat:20505010
	a	skos:Concept ;
	skos:broader	ccat:205050 ;
	skos:inScheme	ccat: ;
	skos:notation	"20505010" ;
	skos:prefLabel	"Bananas"@en .

ccat:20505015
	a	skos:Concept ;
	skos:altLabel	"Cooking Bananas"@en ;
	skos:broader	ccat:205050 ;
	skos:definition	"banana cultivars in the genus Musa whose fruits are generally used in cooking"@en ;
	skos:inScheme	ccat: ;
	skos:notation	"20505015" ;
	skos:prefLabel	"Plantains"@en .

ccat:20505020
	a	skos:Concept ;
	skos:broader	ccat:205050 ;
	skos:inScheme	ccat: ;
	skos:notation	"20505020" ;
	skos:prefLabel	"Kiwi Fruit"@en .

ccat:20505030
	a	skos:Concept ;
	skos:broader	ccat:205050 ;
	skos:inScheme	ccat: ;
	skos:notation	"20505030" ;
	skos:prefLabel	"Mangoes"@en .

ccat:20505040
	a	skos:Concept ;
	skos:broader	ccat:205050 ;
	skos:definition	"Fruit of Ziziphus jujuba, freshly harvested, as well as the candied dried fruit, are often eaten as a snack, or with coffee. Smoked jujubes are consumed in Vietnam and are referred to as black jujubes. Both China and Korea produce a sweetened tea syrup containing jujube fruit in glass jars, and canned jujube tea or jujube tea in the form of teabags. To a lesser extent, jujube fruit is made into juice and jujube vinegar."@en ;
	skos:exactMatch	wd:Q3093648 ;
	skos:inScheme	ccat: ;
	skos:notation	"20505040" ;
	skos:prefLabel	"Jujube"@en .

ccat:20505050
	a	skos:Concept ;
	skos:broader	ccat:205050 ;
	skos:inScheme	ccat: ;
	skos:notation	"20505050" ;
	skos:prefLabel	"Avocados"@en .

ccat:20505060
	a	skos:Concept ;
	skos:broader	ccat:205050 ;
	skos:inScheme	ccat: ;
	skos:notation	"20505060" ;
	skos:prefLabel	"Dates"@en .

ccat:20505065
	a	skos:Concept ;
	skos:broader	ccat:205050 ;
	skos:exactMatch	agrovoc:c_10840 ;
	skos:inScheme	ccat: ;
	skos:notation	"20505065" ;
	skos:prefLabel	"Figs"@en .

ccat:20505068
	a	skos:Concept ;
	skos:broader	ccat:205050 ;
	skos:exactMatch	agrovoc:c_10840 ;
	skos:inScheme	ccat: ;
	skos:notation	"20505068" ;
	skos:prefLabel	"Jackfruit"@en .

ccat:20505070
	a	skos:Concept ;
	skos:broader	ccat:205050 ;
	skos:inScheme	ccat: ;
	skos:notation	"20505070" ;
	skos:prefLabel	"Papayas"@en .

ccat:20505080
	a	skos:Concept ;
	skos:broader	ccat:205050 ;
	skos:inScheme	ccat: ;
	skos:notation	"20505080" ;
	skos:prefLabel	"Pineapples"@en .

ccat:20505090
	a	skos:Concept ;
	skos:broader	ccat:205050 ;
	skos:inScheme	ccat: ;
	skos:notation	"20505090" ;
	skos:prefLabel	"Other Tropical Fruit"@en .

ccat:205090
	a	skos:Concept ;
	skos:broader	ccat:2050 ;
	skos:inScheme	ccat: ;
	skos:notation	"205090" ;
	skos:prefLabel	"Other Fresh Fruit"@en .

ccat:2060
	a	skos:Concept ;
	skos:broader	ccat:20 ;
	skos:definition	"A spice is a seed, fruit, root, bark, salt, or other plant substance primarily used for flavouring or colouring food. Spices are distinguished from herbs, which are the leaves, flowers, or stems of plants used for flavoring or as a garnish. Spices are sometimes used in medicine, religious rituals, cosmetics or perfume production."@en ;
	skos:exactMatch	agrovoc:c_15685 , stw:14060-5 , wd:Q42527 ;
	skos:inScheme	ccat: ;
	skos:notation	"2060" ;
	skos:prefLabel	"Spices"@en .

ccat:206010
	a	skos:Concept ;
	skos:broader	ccat:2060 ;
	skos:definition	"""Cardamom, sometimes cardamon or cardamum, is a spice made from the seeds of several plants in the genera Elettaria and Amomum in the family Zingiberaceae. Both genera are native to the Indian subcontinent and Indonesia. They are recognized by their small seed pods: triangular in cross-section and spindle-shaped, with a thin, papery outer shell and small, black seeds; Elettaria pods are light green and smaller, while Amomum pods are larger and dark brown.

Species used for cardamom are native throughout tropical and subtropical Asia. The first references to cardamom are found in Sumer, and in the Ayurvedic literatures of India. Nowadays it is also cultivated in Guatemala, Malaysia, and Tanzania. The German coffee planter Oscar Majus KlÃ¶ffer introduced Indian cardamom to cultivation in Guatemala before World War I; by 2000, that country had become the biggest producer and exporter of cardamom in the world, followed by India.

Cardamom is the world's third-most expensive spice, surpassed in price per weight only by saffron and vanilla."""@en ;
	skos:exactMatch	agrovoc:c_9620 ;
	skos:inScheme	ccat: ;
	skos:notation	"206010" ;
	skos:prefLabel	"Cardamom"@en .

ccat:206020
	a	skos:Concept ;
	skos:broader	ccat:2060 ;
	skos:definition	"""Cinnamon is a spice obtained from the inner bark of several tree species from the genus Cinnamomum. Cinnamon is used mainly as an aromatic condiment and flavouring additive in a wide variety of cuisines, sweet and savoury dishes, breakfast cereals, snackfoods, tea and traditional foods. The aroma and flavour of cinnamon derive from its essential oil and principal component, cinnamaldehyde, as well as numerous other constituents including eugenol.

Cinnamon is the name for several species of trees and the commercial spice products that some of them produce. All are members of the genus Cinnamomum in the family Lauraceae. Only a few Cinnamomum species are grown commercially for spice. Cinnamomum verum is sometimes considered to be \"true cinnamon\", but most cinnamon in international commerce is derived from the related species Cinnamomum cassia, also referred to as \"cassia\". In 2018, Indonesia and China produced 70% of the world's supply of cinnamon, Indonesia producing nearly 40% and China 30%."""@en ;
	skos:inScheme	ccat: ;
	skos:notation	"206020" ;
	skos:prefLabel	"Cinnamon"@en .

ccat:206030
	a	skos:Concept ;
	skos:broader	ccat:2060 ;
	skos:definition	"""Nutmeg is the seed or ground spice of several species of the genus Myristica. Myristica fragrans (fragrant nutmeg or true nutmeg) is a dark-leaved evergreen tree cultivated for two spices derived from its fruit: nutmeg, from its seed, and mace, from the seed covering. It is also a commercial source of an essential oil and nutmeg butter. The California nutmeg, Torreya californica, has a seed of similar appearance, but is not closely related to Myristica fragrans, and is not used as a spice. Indonesia is the main producers of nutmeg and mace.

If consumed in amounts exceeding its typical use as a spice, nutmeg powder may produce allergic reactions, cause contact dermatitis, or have psychoactive effects. Although used in traditional medicine for treating various disorders, nutmeg has no known medicinal value."""@en ;
	skos:exactMatch	agrovoc:c_23169 , wd:Q83165 ;
	skos:inScheme	ccat: ;
	skos:notation	"206030" ;
	skos:prefLabel	"Nutmeg"@en .

ccat:206035
	a	skos:Concept ;
	skos:broader	ccat:2060 ;
	skos:definition	"""Mace is the spice made from the reddish seed covering (aril) of the nutmeg seed. Its flavour is similar to nutmeg but more delicate; it is used to flavour baked goods, meat, fish, vegetables and in preserving and pickling.

In the processing of mace, the crimson-colored aril is removed from the nutmeg seed that it envelops and is flattened out and dried for 10 to 14 days. Its color changes to pale yellow, orange, or tan. Whole dry mace consists of flat pieces---smooth, horn-like, and brittle---about 40 mm (1.6 in) long."""@en ;
	skos:exactMatch	agrovoc:c_25484 , wd:Q1882876 ;
	skos:inScheme	ccat: ;
	skos:notation	"206035" ;
	skos:prefLabel	"Mace"@en .

ccat:206040
	a	skos:Concept ;
	skos:broader	ccat:2060 ;
	skos:definition	"""Ginger (Zingiber officinale) is a flowering plant whose rhizome, ginger root or ginger, is widely used as a spice and a folk medicine. It is a herbaceous perennial which grows annual pseudostems (false stems made of the rolled bases of leaves) about one meter tall bearing narrow leaf blades. The inflorescences bear flowers having pale yellow petals with purple edges, and arise directly from the rhizome on separate shoots.

Though it is grown in many areas across the globe, ginger is among the earliest recorded spices to be cultivated and exported from southwest India. India holds the seventh position in ginger export worldwide, however is the largest producer of ginger in the world. Regions in southwest and Northeast India are most suitable for ginger production due to their warm and humid climate, average rainfall and land space."""@en ;
	skos:inScheme	ccat: ;
	skos:notation	"206040" ;
	skos:prefLabel	"Ginger"@en .

ccat:206045
	a	skos:Concept ;
	skos:altLabel	"Curcuma"@en ;
	skos:broader	ccat:2060 ;
	skos:closeMatch	wd:Q42562 ;
	skos:definition	"""Turmeric is a flowering plant, Curcuma longa of the ginger family, Zingiberaceae, the roots of which are used in cooking. The plant is a perennial, rhizomatous, herbaceous plant native to the Indian subcontinent and Southeast Asia, that requires temperatures between 20 and 30 ÃÂ°C (68 and 86 ÃÂ°F) and a considerable amount of annual rainfall to thrive. Plants are gathered each year for their rhizomes, some for propagation in the following season and some for consumption.

The rhizomes are used fresh or boiled in water and dried, after which they are ground into a deep orange-yellow powder commonly used as a coloring and flavoring agent in many Asian cuisines, especially for curries, as well as for dyeing. Turmeric powder has a warm, bitter, black pepper-like flavor and earthy, mustard-like aroma.

Although long used in Ayurvedic medicine, where it is also known as haridra, there is no high-quality clinical evidence for using turmeric or its constituent, curcumin, to treat any disease, according to the US Food and Drug Administration."""@en ;
	skos:exactMatch	agrovoc:c_15048 , wd:Q20730193 ;
	skos:inScheme	ccat: ;
	skos:notation	"206045" ;
	skos:prefLabel	"Turmeric"@en .

ccat:206050
	a	skos:Concept ;
	skos:altLabel	"Jeera"@en ;
	skos:broader	ccat:2060 ;
	skos:definition	"""Cumin (Cuminum cyminum) is a flowering plant in the family Apiaceae, native to a territory including the Middle East and stretching east to India. Its seeds---each one contained within a fruit, which is dried---are used in the cuisines of many cultures in both whole and ground form. Although cumin is thought to have uses in traditional medicine, there is no high-quality evidence that it is safe or effective as a therapeutic agent."""@en ;
	skos:exactMatch	agrovoc:c_10205 , wd:Q57328174 ;
	skos:inScheme	ccat: ;
	skos:notation	"206050" ;
	skos:prefLabel	"Cumin"@en .

ccat:206055
	a	skos:Concept ;
	skos:broader	ccat:2060 ;
	skos:definition	"""Coriander is an annual herb in the family Apiaceae. It is also known as Chinese parsley, dhania or cilantro. All parts of the plant are edible, but the fresh leaves and the dried seeds (as a spice) are the parts most traditionally used in cooking.

Most people perceive the taste of coriander leaves as a tart, lemon/lime taste, but to nearly a quarter of those surveyed, the leaves taste like dish soap, linked to a gene which detects some specific aldehydes that are also used as odorant substances in many soaps and detergents."""@en ;
	skos:exactMatch	agrovoc:c_10097 , wd:Q41611 ;
	skos:inScheme	ccat: ;
	skos:notation	"206055" ;
	skos:prefLabel	"Coriander"@en .

ccat:206060
	a	skos:Concept ;
	skos:broader	ccat:2060 ;
	skos:definition	"""Vanilla is a spice derived from orchids of the genus Vanilla, primarily obtained from pods of the Mexican species, flat-leaved vanilla (V. planifolia). The word vanilla, derived from vainilla, the diminutive of the Spanish word vaina (vaina itself meaning a sheath or a pod), is translated simply as \"little pod\". Pre-Columbian Mesoamerican people cultivated the vine of the vanilla orchid, called tlÃÂ«lxochitl by the Aztecs.

Pollination is required to make the plants produce the fruit from which the vanilla spice is obtained. In 1837, Belgian botanist Charles FranÃÂ§ois Antoine Morren discovered this fact and pioneered a method of artificially pollinating the plant. The method proved financially unworkable and was not deployed commercially. In 1841, Edmond Albius, a 12-year-old slave who lived on the French island of RÃÂ©union in the Indian Ocean, discovered that the plant could be hand-pollinated. Hand-pollination allowed global cultivation of the plant. Noted French botanist and plant collector Jean Michel Claude Richard falsely claimed to have discovered the technique three or four years earlier. By the end of the 20th century, Albius was considered the true discoverer.

Three major species of vanilla currently are grown globally, all of which derive from a species originally found in Mesoamerica, including parts of modern-day Mexico. They are V. planifolia (syn. V. fragrans), grown on Madagascar, RÃÂ©union, and other tropical areas along the Indian Ocean; V. tahitensis, grown in the South Pacific; and V. pompona, found in the West Indies, Central America, and South America. The majority of the world's vanilla is the V. planifolia species, more commonly known as Bourbon vanilla (after the former name of RÃÂ©union, Ãï¿½e Bourbon) or Madagascar vanilla, which is produced in Madagascar and neighboring islands in the southwestern Indian Ocean, and in Indonesia. Madagascar's and Indonesia's cultivations produce two-thirds of the world's supply of vanilla.

Vanilla is the second-most expensive spice after saffron because growing the vanilla seed pods is labor-intensive. Nevertheless, vanilla is widely used in both commercial and domestic baking, perfume manufacture, and aromatherapy."""@en ;
	skos:exactMatch	agrovoc:c_15126 , wd:Q13241 ;
	skos:inScheme	ccat: ;
	skos:notation	"206060" ;
	skos:prefLabel	"Vanilla"@en .

ccat:206070
	a	skos:Concept ;
	skos:broader	ccat:2060 ;
	skos:definition	"""Black pepper (Piper nigrum) is a flowering vine in the family Piperaceae, cultivated for its fruit, known as a peppercorn, which is usually dried and used as a spice and seasoning. When fresh and fully mature, the fruit is about 5 mm (0.20 in) in diameter and dark red, and contains a single seed, like all drupes. Peppercorns and the ground pepper derived from them may be described simply as pepper, or more precisely as black pepper (cooked and dried unripe fruit), green pepper (dried unripe fruit), or white pepper (ripe fruit seeds).

Black pepper is native to present-day South India, and is extensively cultivated there and elsewhere in tropical regions. Producing 24% of the world total in 2019, Vietnam is the largest exporter of pepper.

Ground, dried and cooked peppercorns have been used since antiquity, both for flavour and as a traditional medicine. Black pepper is the world's most traded spice, and is one of the most common spices added to cuisines around the world. Its spiciness is due to the chemical compound piperine, which is a different kind of spicy from the capsaicin characteristic of chili peppers. It is ubiquitous in the modern world as a seasoning."""@en ;
	skos:exactMatch	agrovoc:c_25495 , wd:Q3143131 ;
	skos:inScheme	ccat: ;
	skos:notation	"206070" ;
	skos:prefLabel	"Pepper"@en .

ccat:206075
	a	skos:Concept ;
	skos:altLabel	"Allspice"@en ;
	skos:broader	ccat:2060 ;
	skos:definition	"""Allspice, also known as Jamaica pepper, myrtle pepper, pimenta, or pimento, is the dried unripe berry of Pimenta dioica, a midcanopy tree native to the Greater Antilles, southern Mexico, and Central America, now cultivated in many warm parts of the world. The name \"allspice\" was coined as early as 1621 by the English, who valued it as a spice that combined the flavours of cinnamon, nutmeg, and clove.

Allspice is the dried fruit of the Pimenta dioica plant. The fruits are picked when green and unripe and are traditionally dried in the sun. When dry they are brown and resemble large, smooth peppercorns. Fresh leaves are similar in texture to bay leaves and similarly used in cooking. Leaves and wood are often used for smoking meats where allspice is a local crop.

Care must be taken during drying to ensure that volatile oil, such as eugenol, remains in the end products."""@en ;
	skos:exactMatch	agrovoc:c_19193 , wd:Q1963621 ;
	skos:inScheme	ccat: ;
	skos:notation	"206075" ;
	skos:prefLabel	"Pimento"@en .

ccat:206090
	a	skos:Concept ;
	skos:broader	ccat:2060 ;
	skos:inScheme	ccat: ;
	skos:notation	"206090" ;
	skos:prefLabel	"Other Spices"@en .

ccat:2070
	a	skos:Concept ;
	skos:broader	ccat:20 ;
	skos:inScheme	ccat: ;
	skos:notation	"2070" ;
	skos:prefLabel	"Stimulant Crops"@en .

ccat:207010
	a	skos:Concept ;
	skos:broader	ccat:2070 ;
	skos:definition	"""A coffee bean is a seed of the Coffea plant and the source for coffee. It is the pit inside the red or purple fruit often referred to as a cherry. Just like ordinary cherries, the coffee fruit is also a so-called stone fruit. Even though the coffee beans are not technically beans, they are referred to as such because of their resemblance to true beans. The fruits -- coffee cherries or coffee berries -- most commonly contain two stones with their flat sides together. A small percentage of cherries contain a single seed, instead of the usual two. This is called a \"peaberry\". The peaberry occurs only between 10 and 15% of the time, and it is a fairly common (yet scientifically unproven) belief that they have more flavour than normal coffee beans. Like Brazil nuts (a seed) and white rice, coffee beans consist mostly of endosperm.

The two most economically important varieties of coffee plant are the Arabica and the Robusta; ~60% of the coffee produced worldwide is Arabica and ~40% is Robusta. Arabica beans consist of 0.8-1.4% caffeine and Robusta beans consist of 1.7-4% caffeine. As coffee is one of the world's most widely consumed beverages, coffee beans are a major cash crop and an important export product, accounting for over 50% of some developing nations' foreign exchange earnings."""@en ;
	skos:exactMatch	agrovoc:c_28379 ;
	skos:inScheme	ccat: ;
	skos:notation	"207010" ;
	skos:prefLabel	"Green Coffee"@en .

ccat:207020
	a	skos:Concept ;
	skos:broader	ccat:2070 ;
	skos:definition	"Seeds from the pod of the cacao tree (Theobroma cacao), native to Amazon forests. The center of the cocoa bean is called the nib, from which chocolate is made.  The cocoa bean or simply cocoa, also called cacao bean or cacao, is the dried and fully fermented seed of Theobroma cacao, from which cocoa solids (a mixture of nonfat substances) and cocoa butter (the fat) can be extracted. Cocoa beans are the basis of chocolate, and Mesoamerican foods including tejate, an indigenous Mexican drink that also includes maize. "@en ;
	skos:exactMatch	agrovoc:c_1711 ;
	skos:inScheme	ccat: ;
	skos:notation	"207020" ;
	skos:prefLabel	"Cocoa Beans"@en .

ccat:207025
	a	skos:Concept ;
	skos:broader	ccat:2070 ;
	skos:inScheme	ccat: ;
	skos:notation	"207025" ;
	skos:prefLabel	"Carobs"@en .

ccat:207030
	a	skos:Concept ;
	skos:broader	ccat:2070 ;
	skos:inScheme	ccat: ;
	skos:notation	"207030" ;
	skos:prefLabel	"Tea"@en .

ccat:207035
	a	skos:Concept ;
	skos:broader	ccat:2070 ;
	skos:inScheme	ccat: ;
	skos:notation	"207035" ;
	skos:prefLabel	"Mate"@en .

ccat:207039
	a	skos:Concept ;
	skos:broader	ccat:2070 ;
	skos:inScheme	ccat: ;
	skos:notation	"207039" ;
	skos:prefLabel	"Other Tea"@en .

ccat:207040
	a	skos:Concept ;
	skos:broader	ccat:2070 ;
	skos:inScheme	ccat: ;
	skos:notation	"207040" ;
	skos:prefLabel	"Tobacco Leaves"@en .

ccat:207050
	a	skos:Concept ;
	skos:broader	ccat:2070 ;
	skos:inScheme	ccat: ;
	skos:notation	"207050" ;
	skos:prefLabel	"Hops"@en .

ccat:207090
	a	skos:Concept ;
	skos:broader	ccat:2070 ;
	skos:inScheme	ccat: ;
	skos:notation	"207090" ;
	skos:prefLabel	"Other Stimulant Crops"@en .

ccat:2510
	a	skos:Concept ;
	skos:broader	ccat:20 ;
	skos:definition	"Domesticated animals raised in an agricultural setting to produce commodities such as food, fibre, and labour."@en ;
	skos:exactMatch	agrovoc:c_4397 , stw:14145-4 , wd:Q103459 ;
	skos:inScheme	ccat: ;
	skos:notation	"2510" ;
	skos:prefLabel	"Livestock"@en .

ccat:251010
	a	skos:Concept ;
	skos:broader	ccat:2510 ;
	skos:definition	"""Cattle, or cows (female) and bulls (male), are the most common type of large domesticated ungulates. They are a prominent modern member of the subfamily Bovinae, are the most widespread species of the genus Bos, and are most commonly classified collectively as Bos taurus.

Cattle are commonly raised as livestock for meat (beef or veal, see beef cattle), for milk (see dairy cattle), and for hides, which are used to make leather. They are used as riding animals and draft animals (oxen or bullocks, which pull carts, plows and other implements). Another product of cattle is their dung, which can be used to create manure or fuel. In some regions, such as parts of India, cattle have significant religious meaning. Cattle, mostly small breeds such as the Miniature Zebu, are also kept as pets.

Around 10,500 years ago, cattle were domesticated from as few as 80 progenitors in central Anatolia, the Levant and Western Iran. According to the FAO, there are approximately 1.5 billion cattle in the world as of 2018. In 2009, cattle became one of the first livestock animals to have a fully mapped genome."""@en ;
	skos:exactMatch	agrovoc:c_1391 , eurovoc:5034 , stw:14142-3 , wd:Q830 ;
	skos:inScheme	ccat: ;
	skos:notation	"251010" ;
	skos:prefLabel	"Cattle"@en .

ccat:251015
	a	skos:Concept ;
	skos:broader	ccat:2510 ;
	skos:definition	"""the domestic water buffalo or Asian water buffalo, is a large bovid originating in the Indian subcontinent and Southeast Asia. Today, it is also found in Europe, Australia, North America, South America and some African countries. Two extant types of water buffalo are recognized, based on morphological and behavioural criteria: the river buffalo of the Indian subcontinent and further west to the Balkans, Egypt and Italy and the swamp buffalo, found from Assam in the west through Southeast Asia to the Yangtze valley of China in the east.

The husbandry system of water buffaloes depends on the purpose for which they are bred and maintained. Most of them are kept by people who work on small farms in family units. In most rice-producing countries, they are used for threshing and for transporting the sheaves during the rice harvest. They provide power for oilseed mills, sugarcane presses, and devices for raising water. They are widely used as pack animals, and in India and Pakistan, for heavy haulage, also. Their dung is used as a fertilizer, and as a fuel when dried.

Around 26 million water buffaloes are slaughtered each year for meat worldwide. They contribute 72 million tonnes of milk and three million tonnes of meat annually to world food, much of it in areas that are prone to nutritional imbalances. In India, river buffaloes are kept mainly for milk production and for transport, whereas swamp buffaloes are kept mainly for work and a small amount of milk."""@en ;
	skos:exactMatch	agrovoc:c_25410 ;
	skos:inScheme	ccat: ;
	skos:notation	"251015" ;
	skos:prefLabel	"Buffaloes"@en .

ccat:251020
	a	skos:Concept ;
	skos:broader	ccat:2510 ;
	skos:definition	"""Sheep (Ovis aries) are quadrupedal, ruminant mammals typically kept as livestock. Like all ruminants, sheep are members of the order Artiodactyla, the even-toed ungulates. Although the name sheep applies to many species in the genus Ovis, in everyday usage it almost always refers to Ovis aries. Numbering a little over one billion, domestic sheep are also the most numerous species of sheep. An adult female is referred to as a ewe, an intact male as a ram, occasionally a tup, a castrated male as a wether, and a young sheep as a lamb.

Sheep are most likely descended from the wild mouflon of Europe and Asia, with Iran being a geographic envelope of the domestication center. One of the earliest animals to be domesticated for agricultural purposes, sheep are raised for fleeces, meat (lamb, hogget or mutton) and milk. A sheep's wool is the most widely used animal fiber, and is usually harvested by shearing. Ovine meat is called lamb when from younger animals and mutton when from older ones in Commonwealth countries, and lamb in the United States (including from adults). Sheep continue to be important for wool and meat today, and are also occasionally raised for pelts, as dairy animals, or as model organisms for science.

Sheep husbandry is practised throughout the majority of the inhabited world, and has been fundamental to many civilizations. In the modern era, Australia, New Zealand, the southern and central South American nations, and the British Isles are most closely associated with sheep production."""@en ;
	skos:exactMatch	agrovoc:c_7030 , eurovoc:2211 , stw:14143-1 , wd:Q7368 ;
	skos:inScheme	ccat: ;
	skos:notation	"251020" ;
	skos:prefLabel	"Sheep"@en .

ccat:251025
	a	skos:Concept ;
	skos:broader	ccat:2510 ;
	skos:definition	""" The domestic goat or simply goat (Capra aegagrus hircus) is a subspecies of C. aegagrus domesticated from the wild goat of Southwest Asia and Eastern Europe. The goat is a member of the animal family Bovidae and the subfamily Caprinae, meaning it is closely related to the sheep. There are over 300 distinct breeds of goat. It is one of the oldest domesticated species of animal, according to archaeological evidence that its earliest domestication occurred in Iran at 10,000 calibrated calendar years ago.
Goat-herding is an ancient tradition that is still important in places like Egypt.

Goats have been used for milk, meat, fur, and skins across much of the world. Milk from goats is often turned into goat cheese.

Female goats are referred to as does or nannies, intact males are called bucks or billies, and juvenile goats of both sexes are called kids. Castrated males are called wethers. While the words hircine and caprine both refer to anything having a goat-like quality, hircine is used most often to emphasize the distinct smell of domestic goats.

In 2011, there were more than 924 million goats living in the world, according to the UN Food and Agriculture Organization."""@en ;
	skos:exactMatch	agrovoc:c_3324 , eurovoc:5252 , stw:14146-2 , wd:Q2934 ;
	skos:inScheme	ccat: ;
	skos:notation	"251025" ;
	skos:prefLabel	"Goats"@en .

ccat:251030
	a	skos:Concept ;
	skos:altLabel	"Pigs"@en ;
	skos:broader	ccat:2510 ;
	skos:definition	"""The domestic pig (Sus scrofa domesticus or only Sus domesticus), often called swine, hog, or simply pig when there is no need to distinguish it from other pigs, is a large, domesticated, even-toed ungulate. It is variously considered a subspecies of the Eurasian boar or a distinct species. The domestic pig's head-plus-body length ranges from 0.9 to 1.8 m (35 to 71 in), and adult pigs typically weigh between 50 and 350 kg (110 and 770 lb), with well-fed individuals often exceeding this weight range. The size and weight of hogs largely depends on their breed. Compared to other artiodactyls, a pig's head is relatively long, pointed, and free of warts. Most even-toed ungulates are herbivorous, but domestic pigs are omnivores, like their wild relative.

When used as livestock, domestic pigs are farmed primarily for the consumption of their flesh, called pork. A group of pigs is called a passel, a team, or a sounder. The animal's bones, hide, and bristles are also used in products. Domestic pigs, especially miniature breeds, are kept as pets."""@en ;
	skos:exactMatch	agrovoc:c_7555 , eurovoc:2560 , stw:14144-6 , wd:Q787 ;
	skos:inScheme	ccat: ;
	skos:notation	"251030" ;
	skos:prefLabel	"Swine"@en .

ccat:251040
	a	skos:Concept ;
	skos:broadMatch	stw:14135-0 ;
	skos:broader	ccat:2510 ;
	skos:definition	"""The chicken (Gallus gallus domesticus), a subspecies of the red junglefowl, is a type of domesticated fowl, originally from Asia. Rooster or cock is a term for an adult male bird. A younger male may be called a cockerel; a male that has been castrated is a capon. The adult female bird is called a hen. \"Chicken\" was originally a term only for an immature, or at least young, bird, but thanks to its usage on restaurant menus has now become the most common term for the subspecies in general, especially in American English. In older sources common fowl or domestic fowl were typically used for this.

Originally raised for cockfighting or for special ceremonies, chickens were not kept for food until the Hellenistic period (4th-2nd centuries BCE). Humans now keep chickens primarily as a source of food (consuming both their meat and eggs) and as pets.

Chickens are one of the most common and widespread domestic animals, with a total population of 23.7 billion as of 2018, up from more than 19 billion in 2011. There are more chickens in the world than any other bird."""@en ;
	skos:exactMatch	agrovoc:c_1540 , wd:Q780 ;
	skos:inScheme	ccat: ;
	skos:notation	"251040" ;
	skos:prefLabel	"Chickens"@en .

ccat:251042
	a	skos:Concept ;
	skos:broadMatch	stw:14135-0 ;
	skos:broader	ccat:2510 ;
	skos:definition	"""The domestic turkey (Meleagris gallopavo domesticus) is a large fowl, one of the two species in the genus Meleagris and the same species as the wild turkey. Although turkey domestication was thought to have occurred in central Mesoamerica at least 2,000 years ago, recent research suggests a possible second domestication event in the southwestern United States between 200 BC and AD 500. However, all of the main domestic turkey varieties today descend from the turkey raised in central Mexico that was subsequently imported into Europe by the Spanish in the 16th century.

The domestic turkey is a popular form of poultry, and it is raised throughout temperate parts of the world, partially because industrialized farming has made it very cheap for the amount of meat it produces. Female domestic turkeys are referred to as hens, and the chicks may be called poults or turkeylings. In the United States, the males are referred to as toms, while in the United Kingdom and Ireland, males are stags.

The great majority of domestic turkeys are bred to have white feathers because their pin feathers are less visible when the carcass is dressed, although brown or bronze-feathered varieties are also raised. The fleshy protuberance atop the beak is the snood, and the one attached to the underside of the beak is known as a wattle."""@en ;
	skos:exactMatch	agrovoc:c_8016 , wd:Q848706 ;
	skos:inScheme	ccat: ;
	skos:notation	"251042" ;
	skos:prefLabel	"Turkeys"@en .

ccat:251045
	a	skos:Concept ;
	skos:broadMatch	stw:14135-0 ;
	skos:broader	ccat:2510 ;
	skos:definition	"""Ducks are farmed for their meat, eggs, and down. A minority of ducks are also kept for foie gras production. The blood of ducks slaughtered for meat is also collected in some regions and is used as an ingredient in many cultures' dishes. Their eggs are blue-green to white, depending on the breed. Many ducks are also kept for show, as pets, or for their ornamental value. Almost all varieties of domestic duck apart from the Muscovy duck (Cairina moschata) are descended from the mallard (Anas platyrhynchos).

Ducks have been farmed for thousands of years. Approximately 3 billion ducks are slaughtered each year for meat worldwide. In the Western world, they are not as popular as the chicken, because chickens have much more white lean meat and are easier to keep confined, making the total price much lower for chicken meat, whereas duck is comparatively expensive. While popular in haute cuisine, duck appears less frequently in the mass-market food industry and restaurants in the lower price range. However, ducks are more popular in China and there they are raised extensively.

Ducks can be kept free range, in cages, in barns, or in batteries. Ducks enjoy access to swimming water, but do not require it to survive. They should be fed a grain and insect diet. It is a popular misconception that ducks should be fed bread; bread has limited nutritional value and can be deadly when fed to developing ducklings. Ducks should be monitored for avian influenza, as they are especially prone to infection with the dangerous H5N1 strain.

The females of many breeds of domestic ducks are unreliable at sitting their eggs and raising their young. Exceptions include the Rouen duck and especially the Muscovy duck. It has been a custom on farms for centuries to put duck eggs under broody hens for hatching; nowadays this role is often played by an incubator. However, young ducklings rely on their mothers for a supply of preen oil to make them waterproof; a chicken hen does not make as much preen oil as a female duck, and an incubator makes none. Once the duckling grows its own feathers, it produces preen oil from the sebaceous gland near the base of its tail."""@en ;
	skos:exactMatch	agrovoc:c_2406 , wd:Q742292 ;
	skos:inScheme	ccat: ;
	skos:notation	"251045" ;
	skos:prefLabel	"Ducks"@en .

ccat:251047
	a	skos:Concept ;
	skos:broadMatch	stw:14135-0 ;
	skos:broader	ccat:2510 ;
	skos:definition	"""Domestic geese (Anser anser domesticus or Anser cygnoides domesticus, two separate species) are domesticated grey geese (either greylag geese or swan geese) that are kept by humans as poultry for their meat, eggs and down feathers since ancient times. Approximately 700 million geese are slaughtered each year for meat worldwide."""@en ;
	skos:exactMatch	agrovoc:c_3208 , wd:Q255503 ;
	skos:inScheme	ccat: ;
	skos:notation	"251047" ;
	skos:prefLabel	"Geese"@en .

ccat:251048
	a	skos:Concept ;
	skos:broader	ccat:2510 ;
	skos:closeMatch	agrovoc:c_3180 ;
	skos:definition	"""Pigeons are domesticated birds bred to be a source of meat called squab. Squabs have been used as a food in many nations for centuries. They were bred to breed and grow quickly. Other birds refers to domesticated or wild fowl bred or hunted for meat."""@en ;
	skos:inScheme	ccat: ;
	skos:narrowMatch	agrovoc:c_5870 , wd:Q204179 ;
	skos:notation	"251048" ;
	skos:prefLabel	"Pigeons"@en .

ccat:251049
	a	skos:Concept ;
	skos:broader	ccat:2510 ;
	skos:definition	"Other birds, gamebirds, or domestic birds bred or hunted for consumption, such as quail, ostrich, Guinea fowl, etc."@en ;
	skos:inScheme	ccat: ;
	skos:notation	"251049" ;
	skos:prefLabel	"Other Birds"@en .

ccat:251050
	a	skos:Concept ;
	skos:broader	ccat:2510 ;
	skos:definition	"""The horse (Equus ferus caballus) is a domesticated, odd-toed, hoofed mammal. It belongs to the taxonomic family Equidae and is one of two extant subspecies of Equus ferus.

Horses are adapted to run, allowing them to quickly escape predators, possessing an excellent sense of balance and a strong fight-or-flight response. Female horses, called mares, carry their young for approximately 11 months, and a young horse, called a foal, can stand and run shortly following birth.

Horses and humans interact in a wide variety of sport competitions and non-competitive recreational pursuits, as well as in working activities such as police work, agriculture, entertainment, and therapy. Horses were historically used in warfare, from which a wide variety of riding and driving techniques developed, using many different styles of equipment and methods of control. Many products are derived from horses, including meat, milk, hide, hair, bone, and pharmaceuticals extracted from the urine of pregnant mares."""@en ;
	skos:exactMatch	agrovoc:c_3668 , wd:Q726 ;
	skos:inScheme	ccat: ;
	skos:notation	"251050" ;
	skos:prefLabel	"Horses"@en .

ccat:251055
	a	skos:Concept ;
	skos:broader	ccat:2510 ;
	skos:inScheme	ccat: ;
	skos:notation	"251055" ;
	skos:prefLabel	"Asses"@en .

ccat:251058
	a	skos:Concept ;
	skos:broader	ccat:2510 ;
	skos:inScheme	ccat: ;
	skos:notation	"251058" ;
	skos:prefLabel	"Mules"@en .

ccat:251060
	a	skos:Concept ;
	skos:broader	ccat:2510 ;
	skos:inScheme	ccat: ;
	skos:notation	"251060" ;
	skos:prefLabel	"Camels"@en .

ccat:251069
	a	skos:Concept ;
	skos:broader	ccat:2510 ;
	skos:inScheme	ccat: ;
	skos:notation	"251069" ;
	skos:prefLabel	"Other Camelids"@en .

ccat:251070
	a	skos:Concept ;
	skos:broader	ccat:2510 ;
	skos:inScheme	ccat: ;
	skos:notation	"251070" ;
	skos:prefLabel	"Rabbits"@en .

ccat:251079
	a	skos:Concept ;
	skos:broader	ccat:2510 ;
	skos:inScheme	ccat: ;
	skos:notation	"251079" ;
	skos:prefLabel	"Other Rodents"@en .

ccat:251080
	a	skos:Concept ;
	skos:broader	ccat:2510 ;
	skos:inScheme	ccat: ;
	skos:notation	"251080" ;
	skos:prefLabel	"Game and Quarries"@en .

ccat:251090
	a	skos:Concept ;
	skos:broader	ccat:2510 ;
	skos:inScheme	ccat: ;
	skos:notation	"251090" ;
	skos:prefLabel	"Other Live Animals"@en .

ccat:251095
	a	skos:Concept ;
	skos:broader	ccat:2510 ;
	skos:inScheme	ccat: ;
	skos:notation	"251095" ;
	skos:prefLabel	"Other Non-Food Live Animals"@en .

ccat:2520
	a	skos:Concept ;
	skos:broader	ccat:20 ;
	skos:inScheme	ccat: ;
	skos:notation	"2520" ;
	skos:prefLabel	"Animal Fats"@en .

ccat:252010
	a	skos:Concept ;
	skos:broader	ccat:2520 ;
	skos:inScheme	ccat: ;
	skos:notation	"252010" ;
	skos:prefLabel	"Fat of Cattle"@en .

ccat:252015
	a	skos:Concept ;
	skos:broader	ccat:2520 ;
	skos:inScheme	ccat: ;
	skos:notation	"252015" ;
	skos:prefLabel	"Fat of Buffalo"@en .

ccat:252020
	a	skos:Concept ;
	skos:broader	ccat:2520 ;
	skos:inScheme	ccat: ;
	skos:notation	"252020" ;
	skos:prefLabel	"Fat of Sheep"@en .

ccat:252025
	a	skos:Concept ;
	skos:broader	ccat:2520 ;
	skos:inScheme	ccat: ;
	skos:notation	"252025" ;
	skos:prefLabel	"Fat of Goats"@en .

ccat:252030
	a	skos:Concept ;
	skos:broader	ccat:2520 ;
	skos:inScheme	ccat: ;
	skos:notation	"252030" ;
	skos:prefLabel	"Fat of Pigs"@en .

ccat:252040
	a	skos:Concept ;
	skos:broader	ccat:2520 ;
	skos:inScheme	ccat: ;
	skos:notation	"252040" ;
	skos:prefLabel	"Fat of Poultry"@en .

ccat:252060
	a	skos:Concept ;
	skos:broader	ccat:2520 ;
	skos:inScheme	ccat: ;
	skos:notation	"252060" ;
	skos:prefLabel	"Fat of Camels"@en .

ccat:252069
	a	skos:Concept ;
	skos:broader	ccat:2520 ;
	skos:inScheme	ccat: ;
	skos:notation	"252069" ;
	skos:prefLabel	"Fat of Other Camelids"@en .

ccat:252090
	a	skos:Concept ;
	skos:broader	ccat:2520 ;
	skos:inScheme	ccat: ;
	skos:notation	"252090" ;
	skos:prefLabel	"Other Animal Fats"@en .

ccat:2530
	a	skos:Concept ;
	skos:broader	ccat:20 ;
	skos:closeMatch	agrovoc:c_4669 , eurovoc:4681 , stw:14122-2 ;
	skos:definition	"""Edible products from slaughtered animals, such as meat, offal, and bones, excludes edible or inedible products used as material, e.g. skins and hides.

Meat is mainly composed of water, protein, and fat. It is edible raw, but is normally eaten after it has been cooked and seasoned or processed in a variety of ways. Unprocessed meat will spoil or rot within hours or days as a result of infection with and decomposition by bacteria and fungi.

Meat here refers to skeletal muscle, associated fat, and other edible tissues such as offal.  Also includes animals that have not been raised and prepared for human consumption, like game, insects, fish, seafood, and snails."""@en ;
	skos:exactMatch	<https://www.trade-tariff.service.gov.uk/chapters/02> ;
	skos:inScheme	ccat: ;
	skos:notation	"2530" ;
	skos:prefLabel	"Food from Slaughtered Animals"@en .

ccat:253010
	a	skos:Concept ;
	skos:altLabel	"Beef"@en ;
	skos:broader	ccat:2530 ;
	skos:definition	"""Beef is the culinary name for meat from cattle, particularly skeletal muscle. Humans have been eating beef since prehistoric times. Beef is a source of protein and nutrients.

Most beef can be used as is by merely cutting into certain parts, such as roasts, short ribs or steak (filet mignon, sirloin steak, rump steak, rib steak, rib eye steak, hanger steak, etc.), while other cuts are processed (corned beef or beef jerky). Trimmings, on the other hand, which are usually mixed with meat from older, leaner (therefore tougher) cattle, are ground, minced or used in sausages. The blood is used in some varieties called blood sausage. Other parts that are eaten include other muscles and offal, such as the oxtail, liver, tongue, tripe from the reticulum or rumen, glands (particularly the pancreas and thymus, referred to as sweetbread), the heart, the brain (although forbidden where there is a danger of bovine spongiform encephalopathy, BSE, commonly referred to as mad cow disease), the kidneys, and the tender testicles of the bull (known in the United States as calf fries, prairie oysters, or Rocky Mountain oysters). Some intestines are cooked and eaten as is, but are more often cleaned and used as natural sausage casings. The bones are used for making beef stock. Meat from younger cows (calves) is called veal.

Beef from steers and heifers is similar. Depending on economics, the number of heifers kept for breeding varies. The meat from older bulls, because it is usually tougher, is frequently used for mince (known as ground beef in the United States). Cattle raised for beef may be allowed to roam free on grasslands, or may be confined at some stage in pens as part of a large feeding operation called a feedlot (or concentrated animal feeding operation), where they are usually fed a ration of grain, protein, roughage and a vitamin/mineral preblend.

Beef is the third most widely consumed meat in the world, accounting for about 25% of meat production worldwide, after pork and poultry at 38% and 30% respectively. In absolute numbers, the United States, Brazil, and the People's Republic of China are the world's three largest consumers of beef; Uruguay, however, has the highest beef and veal consumption per capita, followed by Argentina and Brazil. According to the data from OECD, the average Uruguayan ate over 42 kg (93 lb) of beef or veal in 2014, representing the highest beef/veal consumption per capita in the world. In comparison, the average American consumed only about 24 kg (53 lb) beef or veal in the same year, while African countries, such as Mozambique, Ghana, and Nigeria, consumed the least beef or veal per capita.

In 2018, the United States, Brazil, and China produced the most beef with 12.22 million tons, 9.9 million tons, and 6.46 million tons respectively. The top 3 beef exporting countries in 2019 were Australia (14.8% of total exports), the United States (13.4% of total exports), and Brazil (12.6% of total exports). Beef production is also important to the economies of Japan, Argentina, Uruguay, Canada, Paraguay, Mexico, Belarus and Nicaragua.

Beef production has a high environmental impact per gram of protein."""@en ;
	skos:exactMatch	agrovoc:c_861 , eurovoc:4682 , stw:18220-3 , wd:Q192628 ;
	skos:inScheme	ccat: ;
	skos:notation	"253010" ;
	skos:prefLabel	"Meat of Cattle"@en ;
	skos:related	<https://www.trade-tariff.service.gov.uk/headings/0201> , <https://www.trade-tariff.service.gov.uk/headings/0202> .

ccat:253015
	a	skos:Concept ;
	skos:broader	ccat:2530 ;
	skos:definition	"""Buffalo meat is the meat of the water buffalo, a large bovid, raised for its milk and meat in many countries including India, Nepal, Pakistan, Bangladesh, Philippines, Bulgaria, Italy, Russia, Czech Republic, Slovakia, Australia and Egypt.

Buffalo meat is known by various names in different countries. In some places it is known as red beef, or buff in India and Nepal; in some countries it is known as carabeef, from the Spanish term and breed name carabao. Meat taken from a buffalo younger than 20 months is known as padwa in India, pado in Nepal and bansgosh in Pakistan. Buffalo calves are often referred to as buffalo broilers and brought up exclusively on milk for the purpose of being slaughtered young for meat.

Buffalo are a type of bovid, but their meat is different from beef in many respects. Buffalo meat has a lower fat content, and its fat is milky white, compared to the yellow-white fat of beef. Buffalo meat is darker in color, and buffaloes, because of their larger size, have harder bones than cows. Buffalo meat has a lower muscle pH of 5.6+-Â±0.4 whereas beef muscle has a pH of 6.4+-0.7. It also has a significantly smaller amount of collagen in its muscles, but the species does not differ significantly in the degree of intramuscular collagen cross-linking.

Buffalo have exceptional muscular development and thus they are considerably heavy, with some weighing more than a tonne. The main agricultural use of buffalo is to obtain milk. India has the largest number of buffalo and is the largest producer of its milk, producing nearly 57 million tonnes of it annually. This accounts for 67% of global production. Slaughtering buffalo for meat is a secondary agricultural priority.

Buffalo meat from young buffalo has a much better quality as they have a higher proportion of muscle and a lower proportion of fat as compared to other cattle meat. The highest quality buffalo meat is known as \"padwa\" in India, taken from a buffalo younger than 24 months.

India accounts for about 43% of the world buffalo meat production, with Uttar Pradesh producing the most, followed by Andhra Pradesh and Maharashtra. In the 21st century, buffalo meat production in India has been growing and has increased from 4.1 million tonnes CWE (carcass weight equivalent) in 2014 to 4.3 million tonnes CWE in 2015.

In India, during the calendar year 2014-2015, consumption estimates had been forecasted to rise from 3.1% and 3.5% to 2.1 and 2.175 million tonnes CWE respectively, according to the US Department of Agriculture."""@en ;
	skos:exactMatch	agrovoc:c_23996 , eurovoc:4685 , wd:Q23808610 ;
	skos:inScheme	ccat: ;
	skos:notation	"253015" ;
	skos:prefLabel	"Buffalo Meat"@en ;
	skos:related	<https://www.trade-tariff.service.gov.uk/headings/0201> , <https://www.trade-tariff.service.gov.uk/headings/0202> .

ccat:253020
	a	skos:Concept ;
	skos:altLabel	"Mutton"@en ;
	skos:broader	ccat:2530 ;
	skos:definition	"""Lamb, hogget, and mutton, generically sheep meat, are the meat of domestic sheep, Ovis aries. A sheep in its first year is a lamb and its meat is also lamb. A sheep in its second year and its meat are hogget. Older sheep meat is mutton.

In South Asian and Caribbean cuisine, \"mutton\" often means goat meat. At various times and places, \"mutton\" or \"goat mutton\" has occasionally been used to mean goat meat.

Lamb is the most expensive of the three types and in recent decades sheep meat is increasingly only retailed as \"lamb\", sometimes stretching the accepted distinctions given above. The stronger-tasting mutton is now hard to find in many areas, despite the efforts of the Mutton Renaissance Campaign in the UK. In Australia, the term prime lamb is often used to refer to lambs raised for meat. Other languages, for example French, Spanish, Italian and Arabic, make similar or even more detailed, distinctions among sheep meats by age and sometimes by sex and diet, though these languages do not always use different words to refer to the animal and its meat."""@en ;
	skos:exactMatch	agrovoc:c_5015 , stw:19021-4 , wd:Q14566073 ;
	skos:inScheme	ccat: ;
	skos:notation	"253020" ;
	skos:prefLabel	"Meat of Sheep"@en ;
	skos:related	<https://www.trade-tariff.service.gov.uk/headings/0204> .

ccat:253025
	a	skos:Concept ;
	skos:broader	ccat:2530 ;
	skos:definition	"""Goat meat or goat's meat is the meat of the domestic goat (Capra aegagrus hircus). The common name for goat meat is simply \"goat\", though meat from adult goats is referred to as chevon, while that from young goats can be called capretto (It.), cabrito (Sp.) or kid. In South Asian and Caribbean cuisine, mutton commonly means goat meat. In South Asia, where mutton curry is popular, \"mutton\" is used for both goat and lamb meat. The United States Department of Agriculture promoted the term \"chevon\", a portmanteau of chÃÂ¨vre ('goat') and mouton ('sheep', 'mutton') in the 1920s. According to market research, consumers in the United States prefer the pseudo-French-language-derived culinary name \"chevon\". \"Cabrito\", a word of Spanish and Portuguese origin, refers specifically to the meat of a young, milk-fed goat. It is also known as chivo.

Goat is both a staple and a delicacy in world's cuisines. The cuisines best known for their use of goat include African cuisine, Middle Eastern, North African, West African, Indian, Indonesian, Nepali, Bangladeshi, Pakistani, Mexican, Caribbean (Haiti), and Ecuadorian. Cabrito, or baby goat, is a very typical food of Monterrey, Nuevo Leon, Mexico; in Italy it is called capretto. Goat meat is savory and less sweet than beef but slightly sweeter than lamb. It can be prepared in a variety of ways, such as being stewed, curried, baked, grilled, barbecued, minced, canned, fried, or made into sausage. Goat jerky is also another popular variety."""@en ;
	skos:exactMatch	agrovoc:c_15978 , wd:Q449506 ;
	skos:inScheme	ccat: ;
	skos:notation	"253025" ;
	skos:prefLabel	"Goat Meat"@en ;
	skos:related	<https://www.trade-tariff.service.gov.uk/headings/0204> .

ccat:253030
	a	skos:Concept ;
	skos:altLabel	"Pork"@en ;
	skos:broader	ccat:2530 ;
	skos:definition	"""Pork is the culinary name for the meat of a domestic pig (Sus scrofa domesticus). It is the most commonly consumed meat worldwide, with evidence of pig husbandry dating back to 5000 BC.

Pork is eaten both freshly cooked and preserved. Curing extends the shelf life of the pork products. Ham, smoked pork, gammon, bacon and sausage are examples of preserved pork. Charcuterie is the branch of cooking devoted to prepared meat products, many from pork.

Pork is not only the most popular meat in the Western world and in Central Europe, it is also very popular in East Asia, the non-Muslim parts of India, Southeast Asia (Indochina, Philippines, Singapore, East Timor) and in Malaysia. It is highly prized in Asian cuisines, especially in China, for its fat content and texture.

Some religions and cultures prohibit pork consumption, notably Islam and Judaism."""@en ;
	skos:exactMatch	agrovoc:c_6120 , eurovoc:4692 , stw:18219-2 , wd:Q191768 ;
	skos:inScheme	ccat: ;
	skos:notation	"253030" ;
	skos:prefLabel	"Pig Meat"@en ;
	skos:related	<https://www.trade-tariff.service.gov.uk/headings/0203> .

ccat:253040
	a	skos:Concept ;
	skos:broader	ccat:2530 ;
	skos:definition	"""Chicken is the most common type of poultry in the world. Owing to the relative ease and low cost of raising them in comparison to animals such as cattle or hogs, chickens have become prevalent in numerous cuisines.

Chicken can be prepared in a vast range of ways, including baking, grilling, barbecuing, frying, and boiling. Since the latter half of the 20th century, prepared chicken has become a staple of fast food. Chicken is sometimes cited as being more healthful than red meat, with lower concentrations of cholesterol and saturated fat.

The poultry farming industry that accounts for chicken production takes on a range of forms across different parts of the world. In developed countries, chickens are typically subject to intensive farming methods while less-developed areas raise chickens using more traditional farming techniques. The United Nations estimates there to be 19 billion chickens on Earth today, making them outnumber humans more than two to one."""@en ;
	skos:exactMatch	agrovoc:c_24000 , wd:Q864693 ;
	skos:inScheme	ccat: ;
	skos:notation	"253040" ;
	skos:prefLabel	"Chicken Meat"@en ;
	skos:related	<https://www.trade-tariff.service.gov.uk/headings/0207> .

ccat:253042
	a	skos:Concept ;
	skos:broader	ccat:2530 ;
	skos:definition	"Turkey meat, commonly referred to as just turkey, is the meat from turkeys, typically domesticated turkeys but also wild turkeys. It is a popular poultry dish, especially in North America, where it is traditionally consumed as part of culturally significant events such as Thanksgiving and Christmas, as well as in standard cuisine."@en ;
	skos:exactMatch	agrovoc:c_24096 , wd:Q4200953 ;
	skos:inScheme	ccat: ;
	skos:notation	"253042" ;
	skos:prefLabel	"Turkey Meat"@en ;
	skos:related	<https://www.trade-tariff.service.gov.uk/headings/0207> .

ccat:253045
	a	skos:Concept ;
	skos:broader	ccat:2530 ;
	skos:definition	"""Duck or duckling is the meat of several species of bird in the family Anatidae, found in both fresh and salt water. Duck is eaten in many cuisines around the world. It is a high-fat, high-protein meat rich in iron.

Duck is particularly predominant in the Chinese cuisine, partly in the (Northeast) Indian cuisine, and in a variety of dishes around the world, most of which involve roasting for at least part of the cooking process to aid in crisping the skin. Some dishes use parts of the duck as an ingredient along with other ingredients."""@en ;
	skos:exactMatch	agrovoc:c_24021 , wd:Q542042 ;
	skos:inScheme	ccat: ;
	skos:notation	"253045" ;
	skos:prefLabel	"Duck Meat"@en ;
	skos:related	<https://www.trade-tariff.service.gov.uk/headings/0207> .

ccat:253047
	a	skos:Concept ;
	skos:broader	ccat:2530 ;
	skos:definition	"Goose is the meat of domesticated or wild geese, used traditionally in the French, Polish, and Baltic cuisines, particularly during the Christmas season."@en ;
	skos:exactMatch	agrovoc:c_24034 , wd:Q46976697 ;
	skos:inScheme	ccat: ;
	skos:notation	"253047" ;
	skos:prefLabel	"Goose Meat"@en ;
	skos:related	<https://www.trade-tariff.service.gov.uk/headings/0207> .

ccat:253048
	a	skos:Concept ;
	skos:broader	ccat:2530 ;
	skos:definition	"""Pigeon meat, sometimes called squab, refers to the meat of domestic pigeons, or more broadly of all dove and pigeon species, such as the wood pigeon, the mourning dove, the extinct-in-the-wild socorro dove, and the now extinct passenger pigeon. and their meat. More recently, squab meat comes almost entirely from domesticated pigeons. The meat of dove and pigeon gamebirds hunted primarily for sport is rarely called squab.

The practice of domesticating pigeons as livestock may have come from North Africa; historically, squabs or pigeons have been consumed in many civilizations, including ancient Egypt (still common in modern Egypt), Rome, China, (Northeast) India, and Medieval Europe. Although squab has been consumed throughout much of recorded history, it is generally regarded as exotic, not as a contemporary staple food; there are more records of its preparation for the wealthy than for the poor.

The modern squab industry uses utility pigeons. Squabs are raised until they are roughly a month old, when they reach adult size but have not yet flown, before being slaughtered."""@en ;
	skos:exactMatch	wd:Q7581884 ;
	skos:inScheme	ccat: ;
	skos:notation	"253048" ;
	skos:prefLabel	"Meat of Pigeons"@en ;
	skos:related	<https://www.trade-tariff.service.gov.uk/commodities/0208901000> , agrovoc:c_6147 .

ccat:253049
	a	skos:Concept ;
	skos:broader	ccat:2530 ;
	skos:definition	"Meat from other birds bred or hunted for consumption, such as quail, ostrich, Guinea fowl, etc."@en ;
	skos:inScheme	ccat: ;
	skos:notation	"253049" ;
	skos:prefLabel	"Meat of Other Birds"@en .

ccat:253050
	a	skos:Concept ;
	skos:broader	ccat:2530 ;
	skos:definition	"""Horse meat forms a significant part of the culinary traditions of many countries, particularly in Europe and Asia. The eight countries that consume the most horse meat consume about 4.3 million horses a year. For the majority of humanity's early existence, wild horses were hunted as a source of protein.

Horse meat has a slightly sweet taste reminiscent of beef. Many consumers allege not being able to tell the difference between beef and horse meat. Meat from younger horses tends to be lighter in color, while older horses produce richer color and flavor, as with most mammals. Horse meat can be used to replace beef, pork, mutton, venison, and any other meat in virtually any recipe. Horse meat is usually very lean. Jurisdictions that allow for the slaughter of horses for food rarely have age restrictions, so many are quite young, some even as young as 16 to 24 months old. IHDH did find that horses at the age of 6 months had lower value of moisture and protein.

In most countries where horses are slaughtered for food, they are processed in a similar fashion to cattle, i.e., in large-scale factory slaughter houses (abattoirs) where they are stunned with a captive bolt gun and bled to death. In countries with a less industrialized food-production system, horses and other animals are slaughtered individually outdoors as needed, in or near the village where they will be consumed.

As horses are relatively poor converters of grass and grain to meat compared to cattle, they are not usually bred or raised specifically for their meat. Instead, horses are slaughtered when their monetary value as riding or work animals is low, but their owners can still make money selling them for horse meat."""@en ;
	skos:exactMatch	agrovoc:c_15983 , wd:Q1124327 ;
	skos:inScheme	ccat: ;
	skos:notation	"253050" ;
	skos:prefLabel	"Horse Meat"@en ;
	skos:related	<https://www.trade-tariff.service.gov.uk/headings/0205> .

ccat:253055
	a	skos:Concept ;
	skos:broader	ccat:2530 ;
	skos:exactMatch	agrovoc:c_24021 ;
	skos:inScheme	ccat: ;
	skos:notation	"253055" ;
	skos:prefLabel	"Meat of Asses"@en ;
	skos:related	<https://www.trade-tariff.service.gov.uk/headings/0205> .

ccat:253058
	a	skos:Concept ;
	skos:broader	ccat:2530 ;
	skos:inScheme	ccat: ;
	skos:notation	"253058" ;
	skos:prefLabel	"Meat of Mules"@en ;
	skos:related	<https://www.trade-tariff.service.gov.uk/headings/0205> .

ccat:253060
	a	skos:Concept ;
	skos:broader	ccat:2530 ;
	skos:exactMatch	agrovoc:c_23998 ;
	skos:inScheme	ccat: ;
	skos:notation	"253060" ;
	skos:prefLabel	"Meat of Camels"@en ;
	skos:related	<https://www.trade-tariff.service.gov.uk/commodities/0208600000> .

ccat:253069
	a	skos:Concept ;
	skos:broader	ccat:2530 ;
	skos:inScheme	ccat: ;
	skos:notation	"253069" ;
	skos:prefLabel	"Meat of other Domestic Camelids"@en ;
	skos:related	<https://www.trade-tariff.service.gov.uk/commodities/0208600000> .

ccat:253070
	a	skos:Concept ;
	skos:broader	ccat:2530 ;
	skos:inScheme	ccat: ;
	skos:notation	"253070" ;
	skos:prefLabel	"Rabbit Meat"@en .

ccat:253074
	a	skos:Concept ;
	skos:broader	ccat:2530 ;
	skos:inScheme	ccat: ;
	skos:notation	"253074" ;
	skos:prefLabel	"Meat of other Domestic Rodents"@en .

ccat:253075
	a	skos:Concept ;
	skos:broader	ccat:2530 ;
	skos:inScheme	ccat: ;
	skos:notation	"253075" ;
	skos:prefLabel	"Game Meat"@en ;
	skos:related	<https://www.trade-tariff.service.gov.uk/commodities/0208600000> , <https://www.trade-tariff.service.gov.uk/commodities/0208906000> .

ccat:253080
	a	skos:Concept ;
	skos:broader	ccat:2530 ;
	skos:inScheme	ccat: ;
	skos:notation	"253080" ;
	skos:prefLabel	"Snails"@en .

ccat:253081
	a	skos:Concept ;
	skos:broader	ccat:2530 ;
	skos:inScheme	ccat: ;
	skos:notation	"253081" ;
	skos:prefLabel	"Insects"@en .

ccat:253082
	a	skos:Concept ;
	skos:broader	ccat:2530 ;
	skos:inScheme	ccat: ;
	skos:notation	"253082" ;
	skos:prefLabel	"Reptiles"@en ;
	skos:related	<https://www.trade-tariff.service.gov.uk/commodities/0208500000> .

ccat:253083
	a	skos:Concept ;
	skos:broader	ccat:2530 ;
	skos:definition	"Whales, dolphins, porpoises, manatees, dugongs."@en ;
	skos:inScheme	ccat: ;
	skos:notation	"253083" ;
	skos:prefLabel	"Mammals of the sea"@en ;
	skos:related	<https://www.trade-tariff.service.gov.uk/commodities/0208400000> .

ccat:253084
	a	skos:Concept ;
	skos:broader	ccat:2530 ;
	skos:inScheme	ccat: ;
	skos:notation	"253084" ;
	skos:prefLabel	"Seals, Sea Lions, Walruses"@en ;
	skos:related	<https://www.trade-tariff.service.gov.uk/commodities/0208400000> .

ccat:253085
	a	skos:Concept ;
	skos:broader	ccat:2530 ;
	skos:inScheme	ccat: ;
	skos:notation	"253085" ;
	skos:prefLabel	"Frogs' Legs"@en ;
	skos:related	<https://www.trade-tariff.service.gov.uk/commodities/0208907000> .

ccat:253090
	a	skos:Concept ;
	skos:broader	ccat:2530 ;
	skos:inScheme	ccat: ;
	skos:notation	"253090" ;
	skos:prefLabel	"Other Meat"@en ;
	skos:related	<https://www.trade-tariff.service.gov.uk/commodities/0208909800> .

ccat:253095
	a	skos:Concept ;
	skos:broader	ccat:2530 ;
	skos:inScheme	ccat: ;
	skos:notation	"253095" ;
	skos:prefLabel	"Other Offals"@en .

ccat:2535
	a	skos:Concept ;
	skos:broader	ccat:20 ;
	skos:inScheme	ccat: ;
	skos:notation	"2535" ;
	skos:prefLabel	"Meat Products and Meat Preparations"@en .

ccat:253510
	a	skos:Concept ;
	skos:broader	ccat:2535 ;
	skos:inScheme	ccat: ;
	skos:notation	"253510" ;
	skos:prefLabel	"Dried Meat"@en .

ccat:253520
	a	skos:Concept ;
	skos:broader	ccat:2535 ;
	skos:inScheme	ccat: ;
	skos:notation	"253520" ;
	skos:prefLabel	"Meat Meal"@en .

ccat:253525
	a	skos:Concept ;
	skos:broader	ccat:2535 ;
	skos:inScheme	ccat: ;
	skos:notation	"253525" ;
	skos:prefLabel	"Blood Meal"@en .

ccat:253530
	a	skos:Concept ;
	skos:broader	ccat:2535 ;
	skos:inScheme	ccat: ;
	skos:notation	"253530" ;
	skos:prefLabel	"Lard Stearine and Lard Oil"@en .

ccat:253535
	a	skos:Concept ;
	skos:broader	ccat:2535 ;
	skos:inScheme	ccat: ;
	skos:notation	"253535" ;
	skos:prefLabel	"Tallow"@en .

ccat:253540
	a	skos:Concept ;
	skos:broader	ccat:2535 ;
	skos:inScheme	ccat: ;
	skos:notation	"253540" ;
	skos:prefLabel	"Indigenous Meat"@en .

ccat:253550
	a	skos:Concept ;
	skos:broader	ccat:2535 ;
	skos:inScheme	ccat: ;
	skos:notation	"253550" ;
	skos:prefLabel	"Biological Meat"@en .

ccat:253590
	a	skos:Concept ;
	skos:broader	ccat:2535 ;
	skos:inScheme	ccat: ;
	skos:notation	"253590" ;
	skos:prefLabel	"Other Prepared Meat"@en .

ccat:253592
	a	skos:Concept ;
	skos:broader	ccat:2535 ;
	skos:inScheme	ccat: ;
	skos:notation	"253592" ;
	skos:prefLabel	"Other Fat Preparations"@en .

ccat:253595
	a	skos:Concept ;
	skos:broader	ccat:2535 ;
	skos:inScheme	ccat: ;
	skos:notation	"253595" ;
	skos:prefLabel	"Other Food Preparations"@en .

ccat:2540
	a	skos:Concept ;
	skos:broader	ccat:20 ;
	skos:inScheme	ccat: ;
	skos:notation	"2540" ;
	skos:prefLabel	"Food from Live Animals"@en .

ccat:254010
	a	skos:Concept ;
	skos:broader	ccat:2540 ;
	skos:definition	"Production data refer to raw milk containing all its constituents. Trade data normally cover milk from any animal, and refer to milk that is not concentrated, pasteurized, sterilized or other-wise preserved, homogenized or peptonized."@en ;
	skos:inScheme	ccat: ;
	skos:notation	"254010" ;
	skos:prefLabel	"Cow Milk"@en .

ccat:25401010
	a	skos:Concept ;
	skos:broader	ccat:254010 ;
	skos:definition	"Milk in which the fat content is adjusted to a predetermined value without altering any other constituents."@en ;
	skos:inScheme	ccat: ;
	skos:notation	"25401010" ;
	skos:prefLabel	"Standardized Milk"@en .

ccat:25401011
	a	skos:Concept ;
	skos:broader	ccat:254010 ;
	skos:definition	"Milk and cream from which water has been partly removed after heat-treating and concentrating. Normally sucrose is added to give the product stability and bacteriological safety."@en ;
	skos:inScheme	ccat: ;
	skos:notation	"25401011" ;
	skos:prefLabel	"Condensed Whole Milk"@en .

ccat:25401012
	a	skos:Concept ;
	skos:broader	ccat:254010 ;
	skos:definition	"Milk and cream from which the water has been partly removed and which has been heat- treated to render it bacteriologically safe and stable."@en ;
	skos:inScheme	ccat: ;
	skos:notation	"25401012" ;
	skos:prefLabel	"Evaporated Whole Milk"@en .

ccat:25401013
	a	skos:Concept ;
	skos:broader	ccat:254010 ;
	skos:definition	"Milk and cream from which water has been completely removed by various methods. In form of powder, granules or other solid forms. May contain added sugar or other sweeteners."@en ;
	skos:inScheme	ccat: ;
	skos:notation	"25401013" ;
	skos:prefLabel	"Dry Whole Cow Milk"@en .

ccat:25401015
	a	skos:Concept ;
	skos:broader	ccat:254010 ;
	skos:definition	"That portion of milk which is rich in milk fat and is separated by skimming or centrifuging."@en ;
	skos:inScheme	ccat: ;
	skos:notation	"25401015" ;
	skos:prefLabel	"Fresh Cream"@en .

ccat:25401016
	a	skos:Concept ;
	skos:broader	ccat:254010 ;
	skos:definition	"Emulsion of milk fat and water that is obtained by churning cream. Trade data cover butter from the milk of any animal."@en ;
	skos:inScheme	ccat: ;
	skos:notation	"25401016" ;
	skos:prefLabel	"Butter of Cow Milk"@en .

ccat:25401017
	a	skos:Concept ;
	skos:broader	ccat:254010 ;
	skos:definition	"Butter from which the water has been removed. Very common in hot countries. Includes also anhydrous butterfat or butter oil."@en ;
	skos:inScheme	ccat: ;
	skos:notation	"25401017" ;
	skos:prefLabel	"Ghee from Cow Milk"@en .

ccat:25401020
	a	skos:Concept ;
	skos:broader	ccat:254010 ;
	skos:definition	"Milk from which most of the fat has been removed."@en ;
	skos:inScheme	ccat: ;
	skos:notation	"25401020" ;
	skos:prefLabel	"Skim Milk of Cows"@en .

ccat:25401021
	a	skos:Concept ;
	skos:broader	ccat:254010 ;
	skos:definition	"Same as 0889, but applied to skim milk."@en ;
	skos:inScheme	ccat: ;
	skos:notation	"25401021" ;
	skos:prefLabel	"Condensed Skim Milk"@en .

ccat:25401022
	a	skos:Concept ;
	skos:broader	ccat:254010 ;
	skos:definition	"Same as 0894, but applied to skim milk."@en ;
	skos:inScheme	ccat: ;
	skos:notation	"25401022" ;
	skos:prefLabel	"Evaporated Skim Milk"@en .

ccat:25401023
	a	skos:Concept ;
	skos:broader	ccat:254010 ;
	skos:definition	"Same as 0897, but from skim milk. Normally does not exceed 1.5% fat content."@en ;
	skos:inScheme	ccat: ;
	skos:notation	"25401023" ;
	skos:prefLabel	"Dry Skim Cow Milk"@en .

ccat:25401030
	a	skos:Concept ;
	skos:broader	ccat:254010 ;
	skos:definition	"The liquid part of the milk that remains after the separation of curd in cheese making. Its main food use is in the preparation of whey cheese, whey drinks and fermented whey drinks. The main industrial uses are in the manufacture of lactose, whey paste and dried whey."@en ;
	skos:exactMatch	agrovoc:c_8376 , wd:Q185009 ;
	skos:inScheme	ccat: ;
	skos:notation	"25401030" ;
	skos:prefLabel	"Fresh Whey"@en .

ccat:25401031
	a	skos:Concept ;
	skos:broader	ccat:254010 ;
	skos:definition	"Condensed whey is pasteurised fresh whey where some of the liquid has been evaporated in a vaccum forming a paste that can then be dried to produce dry whey."@en ;
	skos:inScheme	ccat: ;
	skos:notation	"25401031" ;
	skos:prefLabel	"Condensed Whey"@en .

ccat:25401033
	a	skos:Concept ;
	skos:broader	ccat:254010 ;
	skos:definition	"Dry whey, or whey powder, is produced by removing all water from condensed whey."@en ;
	skos:exactMatch	agrovoc:c_24019 , wd:Q57656307 ;
	skos:inScheme	ccat: ;
	skos:notation	"25401033" ;
	skos:prefLabel	"Dry Whey"@en .

ccat:25401040
	a	skos:Concept ;
	skos:broader	ccat:254010 ;
	skos:definition	"Curd of milk that has been coagulated and separated from whey. May include some skimmed milk."@en ;
	skos:inScheme	ccat: ;
	skos:notation	"25401040" ;
	skos:prefLabel	"Cheese from Whole Cow Milk"@en .

ccat:25401042
	a	skos:Concept ;
	skos:broader	ccat:254010 ;
	skos:definition	"May include some whole milk."@en ;
	skos:inScheme	ccat: ;
	skos:notation	"25401042" ;
	skos:prefLabel	"Cheese From Skimmed Cow Milk"@en .

ccat:25401043
	a	skos:Concept ;
	skos:broader	ccat:254010 ;
	skos:inScheme	ccat: ;
	skos:notation	"25401043" ;
	skos:prefLabel	"Whey Cheese"@en .

ccat:25401045
	a	skos:Concept ;
	skos:broader	ccat:254010 ;
	skos:inScheme	ccat: ;
	skos:notation	"25401045" ;
	skos:prefLabel	"Processed Cheese"@en .

ccat:25401050
	a	skos:Concept ;
	skos:broader	ccat:254010 ;
	skos:definition	"Buttermilk is a fermented dairy drink. Traditionally, it was the liquid left behind after churning butter out of cultured cream; however, most modern buttermilk is cultured."@en ;
	skos:inScheme	ccat: ;
	skos:notation	"25401050" ;
	skos:prefLabel	"Buttermilk, Curdled Milk, Acidifie"@en .

ccat:25401053
	a	skos:Concept ;
	skos:broader	ccat:254010 ;
	skos:inScheme	ccat: ;
	skos:notation	"25401053" ;
	skos:prefLabel	"Dry Buttermilk"@en .

ccat:25401055
	a	skos:Concept ;
	skos:broader	ccat:254010 ;
	skos:definition	"A fermented milk food. May include additives such as sugar, flavouring materials, fruit or cocoa."@en ;
	skos:inScheme	ccat: ;
	skos:notation	"25401055" ;
	skos:prefLabel	"Unconcentrated Yoghurt"@en .

ccat:25401056
	a	skos:Concept ;
	skos:broader	ccat:254010 ;
	skos:definition	"A fermented milk food. May include additives such as sugar, flavouring materials, fruit or cocoa."@en ;
	skos:inScheme	ccat: ;
	skos:notation	"25401056" ;
	skos:prefLabel	"Concentrated Yoghurt"@en .

ccat:25401060
	a	skos:Concept ;
	skos:broader	ccat:254010 ;
	skos:inScheme	ccat: ;
	skos:notation	"25401060" ;
	skos:prefLabel	"Lactose"@en .

ccat:25401065
	a	skos:Concept ;
	skos:broader	ccat:254010 ;
	skos:definition	"The main protein constituent of milk. Casein is obtained from skimmed milk by precipitation (curdling) with acids or rennet."@en ;
	skos:inScheme	ccat: ;
	skos:notation	"25401065" ;
	skos:prefLabel	"Casein"@en .

ccat:25401070
	a	skos:Concept ;
	skos:broader	ccat:254010 ;
	skos:definition	"Obtained by adding water, fat, etc. to milk powder."@en ;
	skos:inScheme	ccat: ;
	skos:notation	"25401070" ;
	skos:prefLabel	"Reconstitued Milk"@en .

ccat:25401080
	a	skos:Concept ;
	skos:broader	ccat:254010 ;
	skos:inScheme	ccat: ;
	skos:notation	"25401080" ;
	skos:prefLabel	"Products of Natural Milk Constituents"@en .

ccat:25401085
	a	skos:Concept ;
	skos:broader	ccat:254010 ;
	skos:definition	"A product with a milk or cream base to which sweeteners, eggs, etc. have been added."@en ;
	skos:inScheme	ccat: ;
	skos:notation	"25401085" ;
	skos:prefLabel	"Ice Cream and Edible Ice"@en .

ccat:254015
	a	skos:Concept ;
	skos:broader	ccat:2540 ;
	skos:inScheme	ccat: ;
	skos:notation	"254015" ;
	skos:prefLabel	"Buffalo Milk"@en .

ccat:254016
	a	skos:Concept ;
	skos:broader	ccat:2540 ;
	skos:inScheme	ccat: ;
	skos:notation	"254016" ;
	skos:prefLabel	"Sheep Milk"@en .

ccat:254017
	a	skos:Concept ;
	skos:broader	ccat:2540 ;
	skos:inScheme	ccat: ;
	skos:notation	"254017" ;
	skos:prefLabel	"Goat Milk"@en .

ccat:254018
	a	skos:Concept ;
	skos:broader	ccat:2540 ;
	skos:inScheme	ccat: ;
	skos:notation	"254018" ;
	skos:prefLabel	"Camel Milk"@en .

ccat:254019
	a	skos:Concept ;
	skos:broader	ccat:2540 ;
	skos:inScheme	ccat: ;
	skos:notation	"254019" ;
	skos:prefLabel	"Other Milk"@en .

ccat:254020
	a	skos:Concept ;
	skos:altLabel	"Chicken Eggs"@en ;
	skos:broadMatch	stw:14121-4 ;
	skos:broader	ccat:2540 ;
	skos:definition	"Oval reproductive body of a fowl (especially a hen) used as food. Chicken eggs are widely used in many types of dishes, both sweet and savory, including many baked goods."@en ;
	skos:exactMatch	agrovoc:c_2502 , wd:Q15260613 ;
	skos:inScheme	ccat: ;
	skos:notation	"254020" ;
	skos:prefLabel	"Hen Eggs"@en .

ccat:254029
	a	skos:Concept ;
	skos:broader	ccat:2540 ;
	skos:inScheme	ccat: ;
	skos:notation	"254029" ;
	skos:prefLabel	"Other Eggs"@en .

ccat:254030
	a	skos:Concept ;
	skos:broader	ccat:2540 ;
	skos:definition	"Honey produced by bees (Apis mellifera) or by other insects."@en ;
	skos:exactMatch	agrovoc:c_3652 , eurovoc:1907 , stw:14123-0 , wd:Q10987 ;
	skos:inScheme	ccat: ;
	skos:notation	"254030" ;
	skos:prefLabel	"Honey"@en .

ccat:30
	a	skos:Concept ;
	skos:closeMatch	agrovoc:c_92337 ;
	skos:definition	"""Commodities used as inputs to manufacturing processes to produce prodcts or more complex materials. Materials can be classified based on their physical and chemical properties, or on their geological origin or biological function.

Raw materials can be processed in different ways to influence their properties, by purification, shaping or the introduction of other materials. New materials can be produced from raw materials by synthesis."""@en ;
	skos:inScheme	ccat: ;
	skos:notation	"30" ;
	skos:prefLabel	"Materials"@en ;
	skos:related	agrovoc:c_330705 ;
	skos:topConceptOf	ccat: .

ccat:3010
	a	skos:Concept ;
	skos:broader	ccat:30 ;
	skos:definition	"Plants or plant parts that are primarily harvested for their fibre, or fibre products of vegetal origin."@en ;
	skos:exactMatch	agrovoc:c_5966 ;
	skos:inScheme	ccat: ;
	skos:notation	"3010" ;
	skos:prefLabel	"Fibres of Vegetal Origin"@en .

ccat:301010
	a	skos:Concept ;
	skos:broader	ccat:3010 ;
	skos:definition	"""Cotton is a soft, fluffy staple fibre that grows in a boll, or protective case, around the seeds of the cotton plants of the genus Gossypium in the mallow family Malvaceae. The fibre is almost pure cellulose. Under natural conditions, the cotton bolls will increase the dispersal of the seeds.

The plant is a shrub native to tropical and subtropical regions around the world, including the Americas, Africa, Egypt and India. The greatest diversity of wild cotton species is found in Mexico, followed by Australia and Africa. Cotton was independently domesticated in the Old and New Worlds.

The fibre is most often spun into yarn or thread and used to make a soft, breathable textile. The use of cotton for fabric is known to date to prehistoric times; fragments of cotton fabric dated to the fifth millennium BC have been found in the Indus Valley Civilization, as well as fabric remnants dated back to 6000 BC in Peru. Although cultivated since antiquity, it was the invention of the cotton gin that lowered the cost of production that led to its widespread use, and it is the most widely used natural fibre cloth in clothing today.

Current estimates for world production are about 25 million tonnes or 110 million bales annually, accounting for 2.5% of the world's arable land. India is the world's largest producer of cotton. The United States has been the largest exporter for many years. In the United States, cotton is usually measured in bales, which measure approximately 0.48 cubic meters (17 cubic feet) and weigh 226.8 kilograms (500 pounds)."""@en ;
	skos:exactMatch	agrovoc:c_1926 , eurovoc:252 , stw:14055-5 , wd:Q11457 ;
	skos:inScheme	ccat: ;
	skos:notation	"301010" ;
	skos:prefLabel	"Cotton Lint"@en .

ccat:301020
	a	skos:Concept ;
	skos:broader	ccat:3010 ;
	skos:definition	"""Flax, also known as common flax or linseed, is a flowering plant, Linum usitatissimum, in the family Linaceae. It is cultivated as a food and fiber crop in regions of the world with temperate climate. Textiles made from flax are known in Western countries as linen, and are traditionally used for bed sheets, underclothes, and table linen. Its oil is known as linseed oil. In addition to referring to the plant itself, the word \"flax\" may refer to the unspun fibers of the flax plant.

Flax fiber is extracted from the bast beneath the surface of the stem of the flax plant. Flax fiber is soft, lustrous, and flexible; bundles of fiber have the appearance of blonde hair, hence the description \"flaxen\" hair. It is stronger than cotton fiber, but less elastic.
A flax field in bloom in North Dakota

The use of flax fibers dates back tens of thousands of years; linen, a refined textile made from flax fibers, was worn widely by Sumerian priests more than 4,000 years ago. Industrial-scale flax fiber processing existed in antiquity. A Bronze Age factory dedicated to flax processing was discovered in Euonymeia, Greece.

The best grades are used for fabrics such as damasks, lace, and sheeting. Coarser grades are used for the manufacturing of twine and rope, and historically, for canvas and webbing equipment. Flax fiber is a raw material used in the high-quality paper industry for the use of printed banknotes, laboratory paper (blotting and filter), rolling paper for cigarettes, and tea bags.

Flax mills for spinning flaxen yarn were invented by John Kendrew and Thomas Porthouse of Darlington, England, in 1787. New methods of processing flax have led to renewed interest in the use of flax as an industrial fiber."""@en ;
	skos:exactMatch	agrovoc:c_2970 , eurovoc:1667 , stw:14057-1 , wd:Q47089651 ;
	skos:inScheme	ccat: ;
	skos:notation	"301020" ;
	skos:prefLabel	"Flax Fibre and Tow"@en .

ccat:301025
	a	skos:Concept ;
	skos:broader	ccat:3010 ;
	skos:closeMatch	agrovoc:c_2970 , eurovoc:1667 , stw:14057-1 , wd:Q47089651 ;
	skos:definition	"""Flax, also known as common flax or linseed, is a flowering plant, Linum usitatissimum, in the family Linaceae. It is cultivated as a food and fiber crop in regions of the world with temperate climate. Textiles made from flax are known in Western countries as linen, and are traditionally used for bed sheets, underclothes, and table linen. Its oil is known as linseed oil. In addition to referring to the plant itself, the word \"flax\" may refer to the unspun fibers of the flax plant.

Flax fiber is extracted from the bast beneath the surface of the stem of the flax plant. Flax fiber is soft, lustrous, and flexible; bundles of fiber have the appearance of blonde hair, hence the description \"flaxen\" hair. It is stronger than cotton fiber, but less elastic.
A flax field in bloom in North Dakota

The use of flax fibers dates back tens of thousands of years; linen, a refined textile made from flax fibers, was worn widely by Sumerian priests more than 4,000 years ago. Industrial-scale flax fiber processing existed in antiquity. A Bronze Age factory dedicated to flax processing was discovered in Euonymeia, Greece.

The best grades are used for fabrics such as damasks, lace, and sheeting. Coarser grades are used for the manufacturing of twine and rope, and historically, for canvas and webbing equipment. Flax fiber is a raw material used in the high-quality paper industry for the use of printed banknotes, laboratory paper (blotting and filter), rolling paper for cigarettes, and tea bags.

Flax mills for spinning flaxen yarn were invented by John Kendrew and Thomas Porthouse of Darlington, England, in 1787. New methods of processing flax have led to renewed interest in the use of flax as an industrial fiber."""@en ;
	skos:inScheme	ccat: ;
	skos:notation	"301025" ;
	skos:prefLabel	"Flax Raw or Retted"@en .

ccat:301030
	a	skos:Concept ;
	skos:broader	ccat:3010 ;
	skos:definition	"""Hemp fiber has been used extensively throughout history, with production climaxing soon after being introduced to the New World. For centuries, items ranging from rope, to fabrics, to industrial materials were made from hemp fiber. Hemp was also commonly used to make sail canvas. The word \"canvas\" is derived from the word cannabis. Pure hemp has a texture similar to linen. Because of its versatility for use in a variety of products, today hemp is used in a number of consumer goods, including clothing, shoes, accessories, dog collars, and home wares. For clothing, in some instances, hemp is mixed with lyocell."""@en ;
	skos:exactMatch	agrovoc:c_3558 , eurovoc:5384 , stw:19017-2 , wd:Q13414920 ;
	skos:inScheme	ccat: ;
	skos:notation	"301030" ;
	skos:prefLabel	"Hemp Fibre and Tow"@en .

ccat:301040
	a	skos:Concept ;
	skos:broader	ccat:3010 ;
	skos:definition	"""Jute is a long, soft, shiny bast fiber that can be spun into coarse, strong threads. It is produced from flowering plants in the genus Corchorus, which is in the mallow family Malvaceae. The primary source of the fiber is Corchorus olitorius, but it is considered inferior to Corchorus capsularis. \"Jute\" is the name of the plant or fiber used to make burlap, hessian or gunny cloth.

Jute is one of the most affordable natural fibers, and second only to cotton in the amount produced and variety of uses. Jute fibers are composed primarily of the plant materials cellulose and lignin. It falls into the bast fiber category (fiber collected from bast, the phloem of the plant, sometimes called the \"skin\") along with kenaf, industrial hemp, flax (linen), ramie, etc. The industrial term for jute fiber is raw jute. The fibers are off-white to brown, and 1-4 metres long. Jute is also called the \"golden fiber\" for its color and high cash value."""@en ;
	skos:exactMatch	agrovoc:c_4065 , eurovoc:1554 , stw:14063-6 , wd:Q107211 ;
	skos:inScheme	ccat: ;
	skos:notation	"301040" ;
	skos:prefLabel	"Jute Fibre"@en .

ccat:301045
	a	skos:Concept ;
	skos:broader	ccat:3010 ;
	skos:inScheme	ccat: ;
	skos:notation	"301045" ;
	skos:prefLabel	"Jute-like Fibre"@en .

ccat:301048
	a	skos:Concept ;
	skos:altLabel	"Manila Hemp"@en ;
	skos:broader	ccat:3010 ;
	skos:definition	"""Manila hemp, also known as abacÃÂ¡, is a type of buff-colored fiber obtained from Musa textilis (a relative of edible bananas), which is likewise called Manila hemp as well as abacÃÂ¡. It is mostly used for pulping for a range of uses, including speciality papers. It was once used mainly to make Manila rope, but this is now of minor importance. AbacÃÂ¡ is an exceptionally strong fibre, nowadays used for special papers like teabag tissue. It is also very expensive, priced several times higher than woodpulp. Manila envelopes and Manila paper take their name from this fibre.

It is not actually hemp, but named so because hemp was long a major source of fibre, and other fibres were sometimes named after it. The name refers to the capital of the Philippines, one of the main producers of Manila hemp. The hatmaking straw made from Manila hemp is called tagal or tagal straw."""@en ;
	skos:exactMatch	agrovoc:c_4 , wd:Q1814695 ;
	skos:inScheme	ccat: ;
	skos:notation	"301048" ;
	skos:prefLabel	"Abaca"@en .

ccat:301050
	a	skos:Concept ;
	skos:broader	ccat:3010 ;
	skos:definition	"""Sisal with the botanical name Agave sisalana, is a species of flowering plant native to southern Mexico but widely cultivated and naturalized in many other countries. It yields a stiff fibre used in making rope and various other products. The term sisal may refer either to the plant's common name or the fibre, depending on the context. It is sometimes referred to as \"sisal hemp\", because for centuries hemp was a major source for fibre, and other fibre sources were named after it.

Fibre is extracted by a process known as decortication, where leaves are crushed, beaten, and brushed away by a rotating wheel set with blunt knives, so that only fibres remain. Alternatively, in East Africa, where production is typically on large estates, the leaves are transported to a central decortication plant, where water is used to wash away the waste parts of the leaf.

The fibre is then dried, brushed and baled for export. Proper drying is important as fibre quality depends largely on moisture content. Artificial drying has been found to result in generally better grades of fibre than sun drying, but is not always feasible in the less industrialised countries where sisal is produced. In the drier climate of north-east Brazil, sisal is mainly grown by smallholders and the fibre is extracted by teams using portable raspadors which do not use water.

Fibre is subsequently cleaned by brushing. Dry fibres are machine combed and sorted into various grades, largely on the basis of the previous in-field separation of leaves into size groups.

Traditionally, sisal has been the leading material for agricultural twine (binder twine and baler twine) because of its strength, durability, ability to stretch, affinity for certain dyestuffs, and resistance to deterioration in saltwater. The importance of this traditional use is diminishing with competition from polypropylene and the development of other haymaking techniques, while new higher-valued sisal products have been developed.

Apart from ropes, twines, and general cordage, sisal is used in low-cost and specialty paper, dartboards, buffing cloth, filters, geotextiles, mattresses, carpets, handicrafts, wire rope cores, and macramÃÂ©. Sisal has been utilized as an environmentally friendly strengthening agent to replace asbestos and fibreglass in composite materials in various uses including the automobile industry. The lower-grade fibre is processed by the paper industry because of its high content of cellulose and hemicelluloses. The medium-grade fibre is used in the cordage industry for making ropes, baler and binder twine. Ropes and twines are widely employed for marine, agricultural, and general industrial use. The higher-grade fibre after treatment is converted into yarns and used by the carpet industry."""@en ;
	skos:exactMatch	agrovoc:c_7086 , eurovoc:4173 , wd:Q847423 ;
	skos:inScheme	ccat: ;
	skos:notation	"301050" ;
	skos:prefLabel	"Sisal"@en .

ccat:301059
	a	skos:Concept ;
	skos:broader	ccat:3010 ;
	skos:inScheme	ccat: ;
	skos:notation	"301059" ;
	skos:prefLabel	"Other Agave Fibres"@en .

ccat:301060
	a	skos:Concept ;
	skos:broader	ccat:3010 ;
	skos:definition	"""Ceiba pentandra is a tropical tree of the order Malvales and the family Malvaceae (previously separated in the family Bombacaceae), native to Mexico, Central America and the Caribbean, northern South America, and (as the variety C. pentandra var guineensis) to West Africa. A somewhat smaller variety is cultivated in southern and southeast Asia. Kapok is a name used in English speaking countries for both the tree and the cotton-like fluff obtained from its seed pods. In Spanish speaking countries the tree is commonly known as \"ceiba\". The tree is cultivated for the seed fibre, particularly in south-east Asia, and is also known as the Java cotton, Java kapok, silk-cotton or samauma.

The fibre is light, very buoyant, resilient, resistant to water, but very flammable. The process of harvesting and separating the fiber is labour-intensive and menial. It is difficult to spin, but is used as an alternative to down as filling in mattresses, pillows, upholstery, zafus, and stuffed toys such as teddy bears, and for insulation. It was previously much used in life jackets and similar devices until synthetic materials largely replaced the fiber. The seeds produce an oil that is used locally in soap and can be used as fertilizer."""@en ;
	skos:exactMatch	agrovoc:c_16497 , eurovoc:1556 , wd:Q1728687 ;
	skos:inScheme	ccat: ;
	skos:notation	"301060" ;
	skos:prefLabel	"Kapok Fibre"@en .

ccat:301070
	a	skos:Concept ;
	skos:broader	ccat:3010 ;
	skos:definition	"""Ramie is one of the oldest fiber crops, having been used for at least 6,000 years, and is principally used for fabric production. It is a bast fiber, and the fiber used for textiles comes from the inner bark (phloem) of the vegetative stalks and not the woody stem or outer bark. Ramie is normally harvested two to three times a year, but under good growing conditions can be harvested up to six times per year. Unlike other bast crops, ramie requires chemical processing to de-gum the fiber.

When the plant begins flowering, or just before, it signals both a decline in growth and the plant being at its maximum fibre content, and is harvested. Stems are harvested by cutting just above the lateral roots or by bending the stem. This enables the core to be broken and the cortex can be stripped from the plant in situ.

After harvesting, stems are decorticated while the plants are fresh. If this is not done while the plants are still fresh, the plants dry out and the bark will be difficult to remove. The bark ribbon is then dried as quickly as possible, preventing bacteria and fungi from attacking it.

The dry weight of harvested stem from crops ranges from 3.4 to 4.5 t/ha/year. A 4.5-ton crop yields 1,600 kg/ha/year of dry undegummed fiber. The weight loss during degumming can be up to 25%, giving a yield of degummed fiber of about 1,200 kg/ha/year.

The fiber extraction occurs in three stages. First, the cortex (bark) is removed; this can be done manually or by machine. This process is called decortication. Second, the cortex is scraped to remove most of the outer bark, the parenchyma in the bast layer and some of the gums and pectins. Third, the residual cortex material is washed, dried, and degummed to extract the spinnable fiber."""@en ;
	skos:exactMatch	agrovoc:c_6442 , wd:Q2130134 ;
	skos:inScheme	ccat: ;
	skos:notation	"301070" ;
	skos:prefLabel	"Ramie"@en .

ccat:301080
	a	skos:Concept ;
	skos:broader	ccat:3010 ;
	skos:definition	"""Coir, or coconut fibre, is a natural fibre extracted from the outer husk of coconut and used in products such as floor mats, doormats, brushes and mattresses. Coir is the fibrous material found between the hard, internal shell and the outer coat of a coconut. Other uses of brown coir (made from ripe coconut) are in upholstery padding, sacking and horticulture. White coir, harvested from unripe coconuts, is used for making finer brushes, string, rope and fishing nets. It has the advantage of not sinking, so can be used in long lengths in deep water without the added weight dragging down boats and buoys."""@en ;
	skos:exactMatch	agrovoc:c_1734 , wd:Q1029620 ;
	skos:inScheme	ccat: ;
	skos:notation	"301080" ;
	skos:prefLabel	"Coir"@en .

ccat:301090
	a	skos:Concept ;
	skos:broader	ccat:3010 ;
	skos:inScheme	ccat: ;
	skos:notation	"301090" ;
	skos:prefLabel	"Other Fibre Crops"@en .

ccat:3020
	a	skos:Concept ;
	skos:broader	ccat:30 ;
	skos:definition	"Animal fibres are fibres that are produced by animals. Most notably they comprise bristles, hair, wool, and silk."@en ;
	skos:exactMatch	agrovoc:c_430 ;
	skos:inScheme	ccat: ;
	skos:notation	"3020" ;
	skos:prefLabel	"Fibres of Animal Origin"@en .

ccat:302010
	a	skos:Concept ;
	skos:broader	ccat:3020 ;
	skos:inScheme	ccat: ;
	skos:notation	"302010" ;
	skos:prefLabel	"Greasy Wool"@en .

ccat:302015
	a	skos:Concept ;
	skos:broader	ccat:3020 ;
	skos:inScheme	ccat: ;
	skos:notation	"302015" ;
	skos:prefLabel	"Fine Hair"@en .

ccat:302020
	a	skos:Concept ;
	skos:broader	ccat:3020 ;
	skos:inScheme	ccat: ;
	skos:notation	"302020" ;
	skos:prefLabel	"Coarse Goat Hair"@en .

ccat:302025
	a	skos:Concept ;
	skos:broader	ccat:3020 ;
	skos:inScheme	ccat: ;
	skos:notation	"302025" ;
	skos:prefLabel	"Fine Goat Hair"@en .

ccat:302030
	a	skos:Concept ;
	skos:broader	ccat:3020 ;
	skos:inScheme	ccat: ;
	skos:notation	"302030" ;
	skos:prefLabel	"Hair of Horses"@en .

ccat:302040
	a	skos:Concept ;
	skos:broader	ccat:3020 ;
	skos:inScheme	ccat: ;
	skos:notation	"302040" ;
	skos:prefLabel	"Reelable Cocoons"@en .

ccat:302090
	a	skos:Concept ;
	skos:broader	ccat:3020 ;
	skos:inScheme	ccat: ;
	skos:notation	"302090" ;
	skos:prefLabel	"Other Coarse Hair"@en .

ccat:3030
	a	skos:Concept ;
	skos:broader	ccat:30 ;
	skos:exactMatch	agrovoc:c_3049 , stw:14149-3 ;
	skos:inScheme	ccat: ;
	skos:notation	"3030" ;
	skos:prefLabel	"Forest Products"@en .

ccat:303010
	a	skos:Concept ;
	skos:altLabel	"Timber"@en ;
	skos:broader	ccat:3030 ;
	skos:definition	"The hard fibrous lignified substance under the bark of trees."@en ;
	skos:exactMatch	agrovoc:c_8421 , stw:14150-4 , wd:Q287 ;
	skos:inScheme	ccat: ;
	skos:notation	"303010" ;
	skos:prefLabel	"Wood"@en .

ccat:303015
	a	skos:Concept ;
	skos:altLabel	"Lumber"@en ;
	skos:broader	ccat:3030 ;
	skos:definition	"""Lumber, also known as timber, is a type of wood that has been processed into beams and planks, a stage in the process of wood production. Lumber is mainly used for structural purposes but has many other uses as well.

There are two main types of lumber. It may be supplied either rough-sawn, or surfaced on one or more of its faces. Besides pulpwood, rough lumber is the raw material for furniture-making and other items requiring additional cutting and shaping. It is available in many species, usually hardwoods; but it is also readily available in softwoods, such as white pine and red pine, because of their low cost.

Finished lumber is supplied in standard sizes, mostly for the construction industry---primarily softwood, from coniferous species, including pine, fir and spruce (collectively spruce-pine-fir), cedar, and hemlock, but also some hardwood, for high-grade flooring. It is more commonly made from softwood than hardwoods, and 80% of lumber comes from softwood."""@en ;
	skos:exactMatch	agrovoc:c_6831 ;
	skos:inScheme	ccat: ;
	skos:notation	"303015" ;
	skos:prefLabel	"Sawnwood"@en .

ccat:3035
	a	skos:Concept ;
	skos:broader	ccat:30 ;
	skos:inScheme	ccat: ;
	skos:notation	"3035" ;
	skos:prefLabel	"Paper"@en .

ccat:303510
	a	skos:Concept ;
	skos:broader	ccat:3035 ;
	skos:inScheme	ccat: ;
	skos:notation	"303510" ;
	skos:prefLabel	"Newsprint"@en .

ccat:303520
	a	skos:Concept ;
	skos:broader	ccat:3035 ;
	skos:inScheme	ccat: ;
	skos:notation	"303520" ;
	skos:prefLabel	"Containerboard"@en .

ccat:303530
	a	skos:Concept ;
	skos:broader	ccat:3035 ;
	skos:inScheme	ccat: ;
	skos:notation	"303530" ;
	skos:prefLabel	"Pulp"@en .

ccat:303550
	a	skos:Concept ;
	skos:broader	ccat:3035 ;
	skos:inScheme	ccat: ;
	skos:notation	"303550" ;
	skos:prefLabel	"Recovered Paper"@en .

ccat:3040
	a	skos:Concept ;
	skos:broader	ccat:30 ;
	skos:inScheme	ccat: ;
	skos:notation	"3040" ;
	skos:prefLabel	"Rubber and Wax"@en .

ccat:304010
	a	skos:Concept ;
	skos:broader	ccat:3040 ;
	skos:definition	"""Natural rubber, also called India rubber, latex, Amazonian rubber, caucho or caoutchouc, as initially produced, consists of polymers of the organic compound isoprene, with minor impurities of other organic compounds, plus water. Thailand and Indonesia are two of the leading rubber producers. Types of polyisoprene that are used as natural rubbers are classified as elastomers.

Currently, rubber is harvested mainly in the form of the latex from the rubber tree or others. The latex is a sticky, milky colloid drawn off by making incisions in the bark and collecting the fluid in vessels in a process called \"tapping\". The latex then is refined into rubber that is ready for commercial processing. In major areas, latex is allowed to coagulate in the collection cup. The coagulated lumps are collected and processed into dry forms for sale.

Natural rubber is used extensively in many applications and products, either alone or in combination with other materials. In most of its useful forms, it has a large stretch ratio and high resilience, and is extremely waterproof."""@en ;
	skos:exactMatch	agrovoc:c_6678 , stw:14151-2 , wd:Q131877 ;
	skos:inScheme	ccat: ;
	skos:notation	"304010" ;
	skos:prefLabel	"Natural Rubber"@en .

ccat:304015
	a	skos:Concept ;
	skos:broader	ccat:3040 ;
	skos:inScheme	ccat: ;
	skos:notation	"304015" ;
	skos:prefLabel	"Natural Gums"@en .

ccat:304016
	a	skos:Concept ;
	skos:broader	ccat:3040 ;
	skos:inScheme	ccat: ;
	skos:notation	"304016" ;
	skos:prefLabel	"Arabic Gum"@en .

ccat:304019
	a	skos:Concept ;
	skos:broader	ccat:3040 ;
	skos:inScheme	ccat: ;
	skos:notation	"304019" ;
	skos:prefLabel	"Other Resins"@en .

ccat:304030
	a	skos:Concept ;
	skos:broader	ccat:3040 ;
	skos:inScheme	ccat: ;
	skos:notation	"304030" ;
	skos:prefLabel	"Vegetable Waxes"@en .

ccat:304035
	a	skos:Concept ;
	skos:broader	ccat:3040 ;
	skos:inScheme	ccat: ;
	skos:notation	"304035" ;
	skos:prefLabel	"Beeswax"@en .

ccat:3050
	a	skos:Concept ;
	skos:broader	ccat:30 ;
	skos:definition	"Compounds that do not contain a C atom. Exceptions are made for isocyanide/cyanide and their non-hydrocarbyl derivatives, thiophosgene, carbon diselenide, carbon monosulfide, carbon disulfide, carbon subsulfide, carbon monoxide, carbon trioxide, carbon suboxide, and dicarbon monoxide."@en ;
	skos:exactMatch	<http://classyfire.wishartlab.com/tax_nodes/C0000001> , agrovoc:c_3881 ;
	skos:inScheme	ccat: ;
	skos:notation	"3050" ;
	skos:prefLabel	"Inorganic Compounds"@en .

ccat:305010
	a	skos:Concept ;
	skos:altLabel	"Soda Ash"@en , "Washing Soda"@en ;
	skos:broader	ccat:3050 ;
	skos:definition	"Sodium carbonate is a food additive (E500) used as an acidity regulator, anticaking agent, raising agent, and stabilizer. Sodium carbonate is also used as a relatively strong base in various fields. As a common alkali, it is preferred in many chemical processes because it is cheaper than sodium hydroxide and far safer to handle."@en ;
	skos:exactMatch	<http://classyfire.wishartlab.com/entities/CDBYLPFSWZWCQE-UHFFFAOYSA-L> ;
	skos:inScheme	ccat: ;
	skos:notation	"305010" ;
	skos:prefLabel	"Sodium Carbonate"@en .

ccat:3060
	a	skos:Concept ;
	skos:broader	ccat:30 ;
	skos:definition	"Compounds that contain at least one carbon atom, excluding isocyanide/cyanide and their non-hydrocarbyl derivatives, thiophosgene, carbon diselenide, carbon monosulfide, carbon disulfide, carbon subsulfide, carbon monoxide, carbon dioxide, Carbon suboxide, and dicarbon monoxide."@en ;
	skos:exactMatch	<http://classyfire.wishartlab.com/tax_nodes/C0000000> , agrovoc:c_5384 ;
	skos:inScheme	ccat: ;
	skos:notation	"3060" ;
	skos:prefLabel	"Organic Compounds"@en .

ccat:306010
	a	skos:Concept ;
	skos:broader	ccat:3060 ;
	skos:definition	"Organic compounds, generally large molecules or macromolecules, which are composed of many repeating units."@en ;
	skos:exactMatch	<http://classyfire.wishartlab.com/tax_nodes/C0003297> , agrovoc:c_32041 , stw:14710-6 ;
	skos:inScheme	ccat: ;
	skos:notation	"306010" ;
	skos:prefLabel	"Polymers"@en .

ccat:30601010
	a	skos:Concept ;
	skos:broader	ccat:306010 ;
	skos:definition	"""Polyvinyl chloride (colloquial: polyvinyl, vinyl; abbreviated: PVC) is the world's third-most widely produced synthetic plastic polymer (after polyethylene and polypropylene). About 40 million tons of PVC are produced each year.

PVC comes in two basic forms: rigid (sometimes abbreviated as RPVC) and flexible. The rigid form of PVC is used in construction for pipe and in profile applications such as doors and windows. It is also used in making bottles, non-food packaging, food-covering sheets, and cards (such as bank or membership cards). It can be made softer and more flexible by the addition of plasticizers, the most widely used being phthalates. In this form, it is also used in plumbing, electrical cable insulation, imitation leather, flooring, signage, phonograph records, inflatable products, and many applications where it replaces rubber. With cotton or linen, it is used in the production of canvas.

Pure polyvinyl chloride is a white, brittle solid. It is insoluble in alcohol but slightly soluble in tetrahydrofuran."""@en ;
	skos:exactMatch	agrovoc:c_28508 , stw:14715-3 , wd:Q146368 ;
	skos:inScheme	ccat: ;
	skos:notation	"30601010" ;
	skos:prefLabel	"Polyvinyl Chloride"@en .

ccat:30601020
	a	skos:Concept ;
	skos:broader	ccat:306010 ;
	skos:definition	"""Polyethylene or polythene (abbreviated PE; IUPAC name polyethene or poly(methylene)) is the most common plastic in use today. It is a linear, man-made, addition, homo-polymer, primarily used for packaging (plastic bags, plastic films, geomembranes, containers including bottles, etc.). As of 2017, over 100 million tonnes of polyethylene resins are being produced annually, accounting for 34% of the total plastics market.

Many kinds of polyethylene are known, with most having the chemical formula (C2H4)n. PE is usually a mixture of similar polymers of ethylene, with various values of n. It can be low density or high density: low density polyethylene is extruded using high pressure (1000-5000 atm) and high temperature (520 Kelvin), while high density polyethylene is extruded using low pressure (6-7 atm) and low temperature (333-343 Kelvin). Polyethylene is usually thermoplastic, however it can be modified to become thermosetting instead, for example in cross-linked polyethylene."""@en ;
	skos:exactMatch	agrovoc:c_28510 , stw:14705-6 , wd:Q143429 ;
	skos:inScheme	ccat: ;
	skos:notation	"30601020" ;
	skos:prefLabel	"Polyethylene"@en .

ccat:30601030
	a	skos:Concept ;
	skos:broader	ccat:306010 ;
	skos:definition	"""Polypropylene (PP), also known as polypropene, is a thermoplastic polymer used in a wide variety of applications. It is produced via chain-growth polymerization from the monomer propylene.

Polypropylene belongs to the group of polyolefins and is partially crystalline and non-polar. Its properties are similar to polyethylene, but it is slightly harder and more heat resistant. It is a white, mechanically rugged material and has a high chemical resistance.

Bio-PP is the bio-based counterpart of polypropylene (PP).

Polypropylene is the second-most widely produced commodity plastic (after polyethylene). In 2019, the global market for polypropylene was worth $126.03 billion. Revenues are expected to exceed US$145 billion by 2019. The sales of this material are forecast to grow at a rate of 5.8% per year until 2021."""@en ;
	skos:exactMatch	agrovoc:c_24221 , stw:14711-4 , wd:Q146174 ;
	skos:inScheme	ccat: ;
	skos:notation	"30601030" ;
	skos:prefLabel	"Polypropylene"@en .

ccat:30601040
	a	skos:Concept ;
	skos:broader	ccat:306010 ;
	skos:definition	"""Polystyrene (PS) is a synthetic aromatic hydrocarbon polymer made from the monomer known as styrene. Polystyrene can be solid or foamed. General-purpose polystyrene is clear, hard, and rather brittle. It is an inexpensive resin per unit weight. It is a rather poor barrier to oxygen and water vapour and has a relatively low melting point. Polystyrene is one of the most widely used plastics, the scale of its production being several million tonnes per year. Polystyrene can be naturally transparent, but can be coloured with colourants. Uses include protective packaging (such as packing peanuts and in the jewel cases used for storage of optical discs such as CDs and occasionally DVDs), containers, lids, bottles, trays, tumblers, disposable cutlery and in the making of models.

As a thermoplastic polymer, polystyrene is in a solid (glassy) state at room temperature but flows if heated above about 100 Â°C, its glass transition temperature. It becomes rigid again when cooled. This temperature behaviour is exploited for extrusion (as in Styrofoam) and also for molding and vacuum forming, since it can be cast into molds with fine detail."""@en ;
	skos:exactMatch	agrovoc:c_28512 , stw:14712-2 ;
	skos:inScheme	ccat: ;
	skos:notation	"30601040" ;
	skos:prefLabel	"Polystyrene"@en .

ccat:306020
	a	skos:Concept ;
	skos:broader	ccat:3060 ;
	skos:definition	"Aromatic compounds containing one or more benzene rings."@en ;
	skos:exactMatch	<http://classyfire.wishartlab.com/tax_nodes/C0002448> ;
	skos:inScheme	ccat: ;
	skos:notation	"306020" ;
	skos:prefLabel	"Benzenoids"@en .

ccat:30602010
	a	skos:Concept ;
	skos:broadMatch	<http://classyfire.wishartlab.com/tax_nodes/C0004211> ;
	skos:broader	ccat:306020 ;
	skos:definition	"Aromatic compounds that contain a p-xylene moiety, which is a monocyclic benzene carrying exactly two methyl groups at the 1- and 4-positions."@en ;
	skos:inScheme	ccat: ;
	skos:notation	"30602010" ;
	skos:prefLabel	"Paraxylene"@en .

ccat:30602020
	a	skos:Concept ;
	skos:broadMatch	<http://classyfire.wishartlab.com/tax_nodes/C0001108> ;
	skos:broader	ccat:306020 ;
	skos:definition	"Compounds containing a benzene ring bearing a carboxylic acid group at ring carbon atoms 1 and 4."@en ;
	skos:inScheme	ccat: ;
	skos:notation	"30602020" ;
	skos:prefLabel	"Terephthalic Acid"@en .

ccat:306030
	a	skos:Concept ;
	skos:broader	ccat:3060 ;
	skos:exactMatch	<http://classyfire.wishartlab.com/tax_nodes/C0000129> ;
	skos:inScheme	ccat: ;
	skos:notation	"306030" ;
	skos:prefLabel	"Alkanols and Polyols" .

ccat:30603010
	a	skos:Concept ;
	skos:broader	ccat:306030 ;
	skos:definition	"Methanol, also known as methyl alcohol amongst other names, is a chemical with the formula CH3OH (a methyl group linked to a hydroxyl group, often abbreviated MeOH). It is a light, volatile, colourless, flammable liquid with a distinctive alcoholic odour similar to that of ethanol. A polar solvent, methanol acquired the name wood alcohol because it was once produced chiefly by the destructive distillation of wood. Today, methanol is mainly produced industrially by hydrogenation of carbon monoxide."@en ;
	skos:exactMatch	agrovoc:c_12521 , eurovoc:1893 , wd:Q14982 ;
	skos:inScheme	ccat: ;
	skos:notation	"30603010" ;
	skos:prefLabel	"Methanol"@en .

ccat:30603020
	a	skos:Concept ;
	skos:broader	ccat:306030 ;
	skos:definition	"""Ethanol (also called ethyl alcohol, grain alcohol, drinking alcohol, or simply alcohol) is an organic chemical compound. Ethanol is a volatile, flammable, colorless liquid with a slight characteristic odor. It is a psychoactive substance, recreational drug, and the active ingredient in alcoholic drinks.  Ethanol is naturally produced by the fermentation of sugars by yeasts or via petrochemical processes such as ethylene hydration. It has medical applications as an antiseptic and disinfectant. It is used as a chemical solvent and in the synthesis of organic compounds. Ethanol is an alternative fuel source. """@en ;
	skos:exactMatch	agrovoc:c_10677 , eurovoc:890 , wd:Q153 ;
	skos:inScheme	ccat: ;
	skos:notation	"30603020" ;
	skos:prefLabel	"Ethanol"@en .

ccat:3070
	a	skos:Concept ;
	skos:broader	ccat:30 ;
	skos:definition	"""Substances that are used to provide nutrients to plants, usually via application to the soil, but also to foliage or through water in rice systems, fertigation, hydroponics or aquaculture operations.

Fertilizers may be distinct from liming materials or other non-nutrient soil amendments. Many sources of fertilizer exist, both natural and industrially produced. For most modern agricultural practices, fertilization focuses on three main macro nutrients: Nitrogen (N), Phosphorus (P), and Potassium (K) with occasional addition of supplements like rock dust for micronutrients. Farmers apply these fertilizers in a variety of ways: through dry or pelletized or liquid application processes, using large agricultural equipment or hand-tool methods.

Historically fertilization came from natural or organic sources: compost, animal manure, human manure, harvested minerals, crop rotations and byproducts of human-nature industries (i.e. fish processing waste, or bloodmeal from animal slaughter). However, starting in the 19th century, after innovations in plant nutrition, an agricultural industry developed around synthetically created fertilizers. This transition was important in transforming the global food system, allowing for larger-scale industrial agriculture with large crop yields. In particular nitrogen-fixing chemical processes such as the Haber process at the beginning of the 20th century, amplified by production capacity created during World War II led to a boom in using nitrogen fertilizers. In the later half of the 20th century, increased use of nitrogen fertilizers (800% increase between 1961 and 2019) have been a crucial component of the increased productivity of conventional food systems (more than 30% per capita) as part of the so called \"Green Revolution\".

Synthetic fertilizer used in agriculture has wide-reaching environmental consequences. According to the IPCC Special Report on Climate Change and Land, production of these fertilizers and associated land use practices are key drivers of global warming. The use of fertilizer has also led to a number of direct environmental consequences: agricultural runoff which leads to downstream effects like ocean dead zones and waterway contamination, soil microbiome degradation, and accumulation of toxins in ecosystems. Additionally, use of synthetic fertilizers can have significant indirect environmental impacts as well: for example, the environmental impacts of fracking for natural gas used in the Haber process, the agricultural boom is partially responsible for the rapid growth in human population and large-scale industrial agricultural practices are associated with habitat destruction, pressure on biodiversity and agricultural soil loss.

In order to mitigate environmental and food security concerns, the international community has included food systems in Sustainable Development Goal 2 which focuses on creating a climate-friendly and sustainable food production system. Most policy and regulatory approaches to address these issues focus on pivoting agricultural practices towards sustainable or regenerative agricultural practices that use less synthetic fertilizers, better soil management (i.e. no-till agriculture) and use more organic fertilizers."""@en ;
	skos:exactMatch	agrovoc:c_2867 , stw:13427-6 , wd:Q83323 ;
	skos:inScheme	ccat: ;
	skos:notation	"3070" ;
	skos:prefLabel	"Fertilizer"@en .

ccat:307010
	a	skos:Concept ;
	skos:broader	ccat:3070 ;
	skos:inScheme	ccat: ;
	skos:notation	"307010" ;
	skos:prefLabel	"Urea"@en .

ccat:307012
	a	skos:Concept ;
	skos:broader	ccat:3070 ;
	skos:inScheme	ccat: ;
	skos:notation	"307012" ;
	skos:prefLabel	"Ammonia"@en .

ccat:307015
	a	skos:Concept ;
	skos:altLabel	"Urea Ammonium Nitrate"@en ;
	skos:broader	ccat:3070 ;
	skos:inScheme	ccat: ;
	skos:notation	"307015" ;
	skos:prefLabel	"UAN"@en .

ccat:307020
	a	skos:Concept ;
	skos:altLabel	"Diamidophosphate"@en ;
	skos:broader	ccat:3070 ;
	skos:inScheme	ccat: ;
	skos:notation	"307020" ;
	skos:prefLabel	"DAP"@en .

ccat:307025
	a	skos:Concept ;
	skos:altLabel	"Monoammonium phosphate"@en ;
	skos:broader	ccat:3070 ;
	skos:inScheme	ccat: ;
	skos:notation	"307025" ;
	skos:prefLabel	"MAP"@en .

ccat:307030
	a	skos:Concept ;
	skos:broader	ccat:3070 ;
	skos:closeMatch	wd:Q10564271 ;
	skos:definition	"""Potash includes various mined and manufactured salts that contain potassium in water-soluble form. The name derives from pot ash, which refers to plant ashes or wood ash soaked in water in a pot, which was the primary means of manufacturing the product before the Industrial Era. The word \"potassium\" is derived from \"potash\".

Potash is produced worldwide in amounts exceeding 90 million tonnes (40 million tonnes K2O equivalent) per year, mostly for use in fertilizer. Various kinds of fertilizer-potash constitute the single greatest industrial use of the element potassium in the world. Potassium was first derived in 1807 by electrolysis of caustic potash (potassium hydroxide)."""@en ;
	skos:exactMatch	agrovoc:c_6138 , stw:14034-6 ;
	skos:inScheme	ccat: ;
	skos:notation	"307030" ;
	skos:prefLabel	"Potash"@en .

ccat:3080
	a	skos:Concept ;
	skos:broader	ccat:30 ;
	skos:definition	"""Substances that are meant to control pests. The term pesticide includes all of the following: herbicide, insecticides (which may include insect growth regulators, termiticides, etc.), nematicide, molluscicide, piscicide, avicide, rodenticide, bactericide, insect repellent, animal repellent, antimicrobial, and fungicide. Most pesticides are intended to serve as plant protection products (also known as crop protection products), which in general, protect plants from weeds, fungi, or insects. As an example - The fungus Alternaria is used to combat the Aquatic weed, Salvinia.

In general, a pesticide is a chemical (such as carbamate) or biological agent (such as a virus, bacterium, or fungus) that deters, incapacitates, kills, or otherwise discourages pests. Target pests can include insects, plant pathogens, weeds, molluscs, birds, mammals, fish, nematodes (roundworms), and microbes that destroy property, cause nuisance, or spread disease, or are disease vectors. Along with these benefits, pesticides also have drawbacks, such as potential toxicity to humans and other species."""@en ;
	skos:exactMatch	<http://classyfire.wishartlab.com/tax_nodes/C0000000> , agrovoc:c_5384 ;
	skos:inScheme	ccat: ;
	skos:notation	"3080" ;
	skos:prefLabel	"Pesticide"@en .

ccat:308010
	a	skos:Concept ;
	skos:broader	ccat:3080 ;
	skos:inScheme	ccat: ;
	skos:notation	"308010" ;
	skos:prefLabel	"Herbicide"@en .

ccat:308020
	a	skos:Concept ;
	skos:broader	ccat:3080 ;
	skos:inScheme	ccat: ;
	skos:notation	"308020" ;
	skos:prefLabel	"Insecticide"@en .

ccat:308030
	a	skos:Concept ;
	skos:broader	ccat:3080 ;
	skos:inScheme	ccat: ;
	skos:notation	"308030" ;
	skos:prefLabel	"Nematicide"@en .

ccat:308040
	a	skos:Concept ;
	skos:broader	ccat:3080 ;
	skos:inScheme	ccat: ;
	skos:notation	"308040" ;
	skos:prefLabel	"Bactericide"@en .

ccat:308050
	a	skos:Concept ;
	skos:broader	ccat:3080 ;
	skos:inScheme	ccat: ;
	skos:notation	"308050" ;
	skos:prefLabel	"Fungicide"@en .

ccat:308060
	a	skos:Concept ;
	skos:broader	ccat:3080 ;
	skos:definition	"Specific animal repellents, in particular molluscicides, piscicides, avicides, and rodenticides."@en ;
	skos:inScheme	ccat: ;
	skos:notation	"308060" ;
	skos:prefLabel	"Animal Repellent"@en .

ccat:40
	a	skos:Concept ;
	skos:definition	"Commoditized goods are tradables that have been made fungible by standardisation."@en ;
	skos:inScheme	ccat: ;
	skos:notation	"40" ;
	skos:prefLabel	"Commoditized"@en ;
	skos:topConceptOf	ccat: .

ccat:4010
	a	skos:Concept ;
	skos:broader	ccat:40 ;
	skos:closeMatch	wd:Q7498085 ;
	skos:definition	"The freight market consists of shipowners, charterers and brokers. They use four types of contractual arrangements: the voyage charter, the contract of affreightment, the time charter and the bareboat charter. Shipowners contract to carry cargo for an agreed price per tonne while the charter market hires out ships for a certain period. A charter is legally agreed upon in a charter-party in which the terms of the deal are clearly set out."@en ;
	skos:exactMatch	stw:13621-3 ;
	skos:inScheme	ccat: ;
	skos:notation	"4010" ;
	skos:prefLabel	"Freight"@en .

ccat:401010
	a	skos:Concept ;
	skos:broader	ccat:4010 ;
	skos:inScheme	ccat: ;
	skos:notation	"401010" ;
	skos:prefLabel	"Wet Freight"@en .

ccat:401020
	a	skos:Concept ;
	skos:broader	ccat:4010 ;
	skos:inScheme	ccat: ;
	skos:notation	"401020" ;
	skos:prefLabel	"Container Freight"@en .

ccat:401025
	a	skos:Concept ;
	skos:broader	ccat:4010 ;
	skos:inScheme	ccat: ;
	skos:notation	"401025" ;
	skos:prefLabel	"Dry Bulk Freight"@en .

ccat:401030
	a	skos:Concept ;
	skos:broader	ccat:4010 ;
	skos:inScheme	ccat: ;
	skos:notation	"401030" ;
	skos:prefLabel	"Air Freight"@en .

ccat:4020
	a	skos:Concept ;
	skos:broader	ccat:40 ;
	skos:definition	"Financial instrument to reduce risk associated with adverse or unexpected weather conditions."@en ;
	skos:exactMatch	stw:29603-4 , wd:Q1759704 ;
	skos:inScheme	ccat: ;
	skos:notation	"4020" ;
	skos:prefLabel	"Weather"@en .

ccat:402010
	a	skos:Concept ;
	skos:broader	ccat:4020 ;
	skos:definition	"Difference of daily high/low temperature as measured by a (set of) reference weather stations to a reference temperature, then aggregated to give degree days over the observation period.  Sometimes capped/floored as heating degree days/cooling degree days so that only temperatures below/above reference are taken into account which avoids aggregating signed differences."@en ;
	skos:inScheme	ccat: ;
	skos:notation	"402010" ;
	skos:prefLabel	"Temperature"@en .

ccat:402020
	a	skos:Concept ;
	skos:broader	ccat:4020 ;
	skos:inScheme	ccat: ;
	skos:notation	"402020" ;
	skos:prefLabel	"Rainfall"@en .

ccat:4030
	a	skos:Concept ;
	skos:broader	ccat:40 ;
	skos:closeMatch	agrovoc:c_1b1e0e70 , eurovoc:434843 , stw:20762-1 , wd:Q8348417 ;
	skos:definition	"""Permits and allowances in writing. A central authority (usually a governmental body) allocates or sells a limited number of permits that allow a discharge of a specific quantity of a specific pollutant over a set time period. Polluters are required to hold permits in amount equal to their emissions. Polluters that want to increase their emissions must buy permits from others willing to sell them."""@en ;
	skos:inScheme	ccat: ;
	skos:notation	"4030" ;
	skos:prefLabel	"Emissions"@en .

ccat:403010
	a	skos:Concept ;
	skos:broader	ccat:4030 ;
	skos:definition	"""Permits and allowances specifically for carbon dioxide (CO2) emission."""@en ;
	skos:inScheme	ccat: ;
	skos:notation	"403010" ;
	skos:prefLabel	"CO2 permits"@en .

ccat:403020
	a	skos:Concept ;
	skos:broader	ccat:4030 ;
	skos:definition	"""Permits and allowances specifically for nitrogen oxides (NOx) emissions."""@en ;
	skos:inScheme	ccat: ;
	skos:notation	"403020" ;
	skos:prefLabel	"NOx permits"@en .

ccat:403030
	a	skos:Concept ;
	skos:broader	ccat:4030 ;
	skos:definition	"""Permits and allowances specifically for sulfur dioxide (SO2) emission."""@en ;
	skos:inScheme	ccat: ;
	skos:notation	"403030" ;
	skos:prefLabel	"SO2 permits"@en .

ccat:403040
	a	skos:Concept ;
	skos:altLabel	"GO"@en , "REC"@en ;
	skos:broader	ccat:4030 ;
	skos:closeMatch	wd:Q1478326 , wd:Q2143923 ;
	skos:definition	"Renewable Energy Certificates (RECs), also known as Green tags, Renewable Energy Credits, Renewable Electricity Certificates, or Tradable Renewable Certificates (TRCs), are tradable, non-tangible energy commodities in the United States that represent proof that 1 megawatt-hour (MWh) of electricity was generated from an eligible renewable energy resource (renewable electricity) and was fed into the shared system of power lines which transport energy. Similarly Guarantees of Origin (GO) is a tracking instrument defined in article 15 of the European Directive 2009/28/EC. A GO labels electricity from renewable sources to provide information to electricity customers on the source of their energy. Guarantees of origin are the only precisely defined instruments evidencing the origin of electricity generated from renewable energy sources."@en ;
	skos:exactMatch	wd:Q7313092 ;
	skos:inScheme	ccat: ;
	skos:notation	"403040" ;
	skos:prefLabel	"Renewable Energy Credits/Guarantee of Origin"@en .

ccat:4040
	a	skos:Concept ;
	skos:broader	ccat:40 ;
	skos:closeMatch	msa:2779948615 , wd:Q7973730 ;
	skos:definition	"Water market transactions involve the sale or lease of a wide range of ownership interests in water. A water right entitles the owner to divert or pump water from rivers, streams, and groundwater basins. Water rights are the most commonly traded category of ownership interest. Other commonly traded entitlements include shares in groundwater banks, surface reservoir storage rights, and entitlements to treated wastewater."@en ;
	skos:inScheme	ccat: ;
	skos:notation	"4040" ;
	skos:prefLabel	"Commercial Water Rights"@en .

ccat:50
	a	skos:Concept ;
	skos:definition	"Financials are tradables made up of one or a basket of financial instruments."@en ;
	skos:inScheme	ccat: ;
	skos:notation	"50" ;
	skos:prefLabel	"Financials"@en ;
	skos:topConceptOf	ccat: .

ccat:5010
	a	skos:Concept ;
	skos:broader	ccat:50 ;
	skos:closeMatch	wd:Q66076 ;
	skos:definition	"The foreign exchange market (Forex, FX, or currency market) is a global decentralized or over-the-counter (OTC) market for the trading of currencies."@en ;
	skos:inScheme	ccat: ;
	skos:notation	"5010" ;
	skos:prefLabel	"Currency"@en .

ccat:5020
	a	skos:Concept ;
	skos:broader	ccat:50 ;
	skos:closeMatch	wd:Q3239315 ;
	skos:definition	"A tradeable debt instrument that provides a return in the form of fixed periodic interest payments and the eventual return of principal at maturity."@en ;
	skos:inScheme	ccat: ;
	skos:notation	"5020" ;
	skos:prefLabel	"Fixed Income"@en .

ccat:502010
	a	skos:Concept ;
	skos:altLabel	"Government bonds"@en ;
	skos:broader	ccat:5020 ;
	skos:definition	"Debt security issued by a government to fund government spending."@en ;
	skos:exactMatch	<https://spec.edmcouncil.org/fibo/ontology/SEC/Debt/Bonds/SovereignBond> , wd:Q2324820 ;
	skos:inScheme	ccat: ;
	skos:notation	"502010" ;
	skos:prefLabel	"Sovereign bonds"@en .

ccat:502020
	a	skos:Concept ;
	skos:broader	ccat:5020 ;
	skos:definition	"Rates with tenors of up to 12 months"@en ;
	skos:exactMatch	wd:Q102113162 ;
	skos:inScheme	ccat: ;
	skos:notation	"502020" ;
	skos:prefLabel	"STIR"@en .

ccat:502030
	a	skos:Concept ;
	skos:broader	ccat:5020 ;
	skos:definition	"Interest rate swaps, vanilla, basis, etc."@en ;
	skos:exactMatch	msa:99560960 , wd:Q205258 ;
	skos:inScheme	ccat: ;
	skos:notation	"502030" ;
	skos:prefLabel	"IRS"@en .

ccat:502040
	a	skos:Concept ;
	skos:broader	ccat:5020 ;
	skos:definition	"Securities that offset or are linked to a predefined inflation index, e.g. a coupon that adds realised inflation during the interest accrual period."@en ;
	skos:inScheme	ccat: ;
	skos:notation	"502040" ;
	skos:prefLabel	"Inflation-linked Security"@en .

ccat:5030
	a	skos:Concept ;
	skos:broader	ccat:50 ;
	skos:closeMatch	wd:Q2272475 ;
	skos:definition	"A statistical measure of change in a representative group of individual data points. These data may be derived from any number of sources, including company performance, prices, productivity, and employment. Excluded are indices made up of probes from different measurements of or surveys about a unique subject, or time aggegrates thereof, like the Platts Dated Brent spot price average, or the Los Angeles Seasonal Strip Rainfall index. Those are to be categorised under their respective concept. "@en ;
	skos:inScheme	ccat: ;
	skos:notation	"5030" ;
	skos:prefLabel	"Index"@en .

ccat:503010
	a	skos:Concept ;
	skos:broader	ccat:5030 ;
	skos:definition	"An index that measures the value of a basket of soft or hard commodities."@en ;
	skos:inScheme	ccat: ;
	skos:notation	"503010" ;
	skos:prefLabel	"Commodity Index"@en .

ccat:503020
	a	skos:Concept ;
	skos:broader	ccat:5030 ;
	skos:definition	"""An index that measures a stock market, or a subset of the stock market, that helps investors compare current price levels with past prices to calculate market performance. It is computed from the prices of selected stocks (typically a weighted arithmetic mean).

Two of the primary criteria of an index are that it is investable and transparent: The method of its construction are specified. Investors can invest in a stock market index by buying an index fund, which are structured as either a mutual fund or an exchange-traded fund, and \"track\" an index. The difference between an index fund's performance and the index, if any, is called tracking error. For a list of major stock market indices, see List of stock market indices."""@en ;
	skos:exactMatch	wd:Q223371 ;
	skos:inScheme	ccat: ;
	skos:notation	"503020" ;
	skos:prefLabel	"Equity Index"@en .

ccat:503030
	a	skos:Concept ;
	skos:broader	ccat:5030 ;
	skos:closeMatch	wd:Q1284784 ;
	skos:definition	"An index that measures the performance of a basket of fixed-income securities."@en ;
	skos:inScheme	ccat: ;
	skos:notation	"503030" ;
	skos:prefLabel	"Fixed Income Index"@en .

ccat:503090
	a	skos:Concept ;
	skos:broader	ccat:5030 ;
	skos:definition	"An index that isn't categorised elsewhere."@en ;
	skos:inScheme	ccat: ;
	skos:notation	"503090" ;
	skos:prefLabel	"Other Index"@en .
